@prefix : <http://www.semanticweb.org/annag/ontologies/2024/1/ontoHorses#> .
@prefix owl: <http://www.w3.org/2002/07/owl#> .
@prefix rdf: <http://www.w3.org/1999/02/22-rdf-syntax-ns#> .
@prefix xml: <http://www.w3.org/XML/1998/namespace> .
@prefix xsd: <http://www.w3.org/2001/XMLSchema#> .
@prefix rdfs: <http://www.w3.org/2000/01/rdf-schema#> .
@prefix ontoHorse: <http://www.semanticweb.org/annag/ontologies/2024/1/ontoHorses/> .
@base <http://www.semanticweb.org/annag/ontologies/2024/1/ontoHorses#> .

<http://www.semanticweb.org/annag/ontologies/2024/1/ontoHorses> rdf:type owl:Ontology ;
                                                                 owl:imports <http://www.ontologydesignpatterns.org/cp/owl/list.owl> ,
                                                                             <http://www.ontologydesignpatterns.org/cp/owl/partof.owl> ,
                                                                             <http://www.ontologydesignpatterns.org/cp/owl/price.owl> ;
                                                                 <http://purl.org/dc/elements/1.1/creator> "Annalisa Sabatelli" ;
                                                                 <http://purl.org/dc/elements/1.1/date> "2024-03-01T09:00:00"^^xsd:dateTime ;
                                                                 <http://purl.org/dc/elements/1.1/description> "Ontological representation of breeds, uses and main characteristics of horses and their sales announcements aimed at helping the user in purchasing a horse."@en ,
                                                                                                               "Rappresentazione ontologica di razze, impieghi e caratteristiche principali dei cavalli e annunci di vendita finalizzata ad aiutare l'utente nell'acquisto di un cavallo."@it ;
                                                                 <http://purl.org/dc/elements/1.1/title> "OntoHorses"@en ;
                                                                 ontoHorse:vann:preferredNamesspacePrefix "http://www.semanticweb.org/annag/ontologies/2024/1/ontoHorses"@it ,
                                                                                                          "ontohorse"@en ;
                                                                 rdfs:label "Ontologia sulle principali razze di cavallo europee"@it ,
                                                                            "Ontology on the main European horse breeds"@en .

#################################################################
#    Annotation properties
#################################################################

###  http://purl.org/dc/elements/1.1/creator
<http://purl.org/dc/elements/1.1/creator> rdf:type owl:AnnotationProperty .


###  http://purl.org/dc/elements/1.1/date
<http://purl.org/dc/elements/1.1/date> rdf:type owl:AnnotationProperty .


###  http://purl.org/dc/elements/1.1/description
<http://purl.org/dc/elements/1.1/description> rdf:type owl:AnnotationProperty .


###  http://purl.org/dc/elements/1.1/title
<http://purl.org/dc/elements/1.1/title> rdf:type owl:AnnotationProperty .


###  http://schema.org/image
<http://schema.org/image> rdf:type owl:AnnotationProperty .


###  http://www.ontologydesignpatterns.org/cp/owl/bag.owl#hasItem
<http://www.ontologydesignpatterns.org/cp/owl/bag.owl#hasItem> rdf:type owl:AnnotationProperty .


###  http://www.ontologydesignpatterns.org/cp/owl/sequence.owl#precedes
<http://www.ontologydesignpatterns.org/cp/owl/sequence.owl#precedes> rdf:type owl:AnnotationProperty .


###  http://www.semanticweb.org/annag/ontologies/2024/1/ontoHorses/vann:preferredNamespaceUri
ontoHorse:vann:preferredNamespaceUri rdf:type owl:AnnotationProperty .


###  http://www.semanticweb.org/annag/ontologies/2024/1/ontoHorses/vann:preferredNamesspacePrefix
ontoHorse:vann:preferredNamesspacePrefix rdf:type owl:AnnotationProperty .


###  http://www.w3.org/2004/02/skos/core#exactMatch
<http://www.w3.org/2004/02/skos/core#exactMatch> rdf:type owl:AnnotationProperty .


###  http://www.w3.org/2004/02/skos/core#prefLabel
<http://www.w3.org/2004/02/skos/core#prefLabel> rdf:type owl:AnnotationProperty .


#################################################################
#    Object Properties
#################################################################

###  http://www.ontologydesignpatterns.org/cp/owl/partof.owl#hasPart
<http://www.ontologydesignpatterns.org/cp/owl/partof.owl#hasPart> rdfs:domain ontoHorse:AreaGeografica ;
                                                                  rdfs:range ontoHorse:AreaGeografica .


###  http://www.ontologydesignpatterns.org/cp/owl/partof.owl#isPartOf
<http://www.ontologydesignpatterns.org/cp/owl/partof.owl#isPartOf> rdfs:domain ontoHorse:AreaGeografica ;
                                                                   rdfs:range ontoHorse:AreaGeografica .


###  http://www.ontologydesignpatterns.org/cp/owl/price.owl#hasPrice
<http://www.ontologydesignpatterns.org/cp/owl/price.owl#hasPrice> rdfs:domain ontoHorse:Cavallo .


###  http://www.semanticweb.org/annag/ontologies/2024/1/ontoHorses#haIndole
:haIndole rdf:type owl:ObjectProperty ,
                   owl:FunctionalProperty ;
          rdfs:domain ontoHorse:RazzaCavallo ;
          rdfs:range :Indole ;
          rdfs:comment "Property that expresses the temperament of a horse breed"@en ,
                       "Proprietà che esprime il temperamento di una razza di cavallo"@it ;
          rdfs:label "ha indole"@it ,
                     "has temperament"@en .


###  http://www.semanticweb.org/annag/ontologies/2024/1/ontoHorses#haNazionalità
:haNazionalità rdf:type owl:ObjectProperty ;
               rdfs:domain ontoHorse:RazzaCavallo ;
               rdfs:range ontoHorse:AreaGeografica ;
               owl:propertyChainAxiom ( ontoHorse:haRegioneDiOrigine
                                        <http://www.ontologydesignpatterns.org/cp/owl/partof.owl#isPartOf>
                                      ) ;
               rdfs:comment "Property that expresses the nation of origin of a horse breed"@en ,
                            "Proprietà che esprime la nazionalità di una razza di cavallo"@it ;
               rdfs:label "has nationality"@en ,
                          "ha nazionalità" .


###  http://www.semanticweb.org/annag/ontologies/2024/1/ontoHorses#puòEssereImpiegataIn
:puòEssereImpiegataIn rdf:type owl:ObjectProperty ;
                      rdfs:domain ontoHorse:RazzaCavallo ;
                      rdfs:range ontoHorse:Impiego ;
                      rdfs:comment "Property that expresses the possible uses of a breed in work or sport"@en ,
                                   "Proprietà che esprime i possibili impieghi di una razza nel lavoro o nello sport"@it ;
                      rdfs:label "can be used in"@en ,
                                 "può essere impiegata in"@it .


###  http://www.semanticweb.org/annag/ontologies/2024/1/ontoHorses/adattoAlConseguimentoDi
ontoHorse:adattoAlConseguimentoDi rdf:type owl:ObjectProperty ;
                                  rdfs:domain ontoHorse:Cavallo ;
                                  rdfs:range ontoHorse:Patente ;
                                  owl:propertyChainAxiom ( ontoHorse:gareggiaNelleCategorieDiSalto
                                                           ontoHorse:permetteIlConseguimentoDi
                                                         ) ;
                                  rdfs:comment "Property that expresses the relationship between the horse's sporting performance and the riding licences it allows to achieve"@en ,
                                               "Proprietà che esprime la relazione tra le prestazioni sportive del cavallo e le autorizzazioni a montare che permette di conseguire"@it ;
                                  rdfs:label "suitable for achieving"@en ,
                                             "adatto al conseguimento di" .


###  http://www.semanticweb.org/annag/ontologies/2024/1/ontoHorses/consegue
ontoHorse:consegue rdf:type owl:ObjectProperty ;
                   owl:inverseOf ontoHorse:vieneConseguitoDa ;
                   rdfs:domain ontoHorse:Cavaliere ;
                   rdfs:range ontoHorse:Patente ;
                   rdfs:comment "Property that expresses the relationship between the rider's experience and the riding licences he can achieve"@en ,
                                "Proprietà che esprime la relazione tra l'esperienza del cavaliere e l'<utorizzazioni a montare che può conseguire"@it ;
                   rdfs:label "achieve"@en ,
                              "consegue"@it .


###  http://www.semanticweb.org/annag/ontologies/2024/1/ontoHorses/gareggiaNelleCategorieDiSalto
ontoHorse:gareggiaNelleCategorieDiSalto rdf:type owl:ObjectProperty ;
                                        rdfs:domain ontoHorse:Cavallo ;
                                        rdfs:range ontoHorse:CategorieDiSalto ;
                                        rdfs:comment "Property that expresses the categories of  jumping competitions in which the horse usually participates."@en ,
                                                     "Proprietà che esprime le categorie di gare di salto ad ostacoli alle quali il cavallo di solito partecipa."@it ;
                                        rdfs:label "gareggia nelle categorie di salto ostacoli"@it ,
                                                   "take part to jumping categories"@en .


###  http://www.semanticweb.org/annag/ontologies/2024/1/ontoHorses/haRazza
ontoHorse:haRazza rdf:type owl:ObjectProperty ,
                           owl:FunctionalProperty ;
                  rdfs:domain ontoHorse:Cavallo ;
                  rdfs:range ontoHorse:RazzaCavallo ;
                  rdfs:comment "Property that expresses the breed of a horse"@en ,
                               "Proprietà che esprime la razza di un cavallo"@it ;
                  rdfs:label "ha razza"@it ,
                             "has breed"@en .


###  http://www.semanticweb.org/annag/ontologies/2024/1/ontoHorses/haRegioneDiOrigine
ontoHorse:haRegioneDiOrigine rdf:type owl:ObjectProperty ;
                             rdfs:domain ontoHorse:RazzaCavallo ;
                             rdfs:range ontoHorse:AreaGeografica ;
                             rdfs:comment "Property that expresses the territory of origin of a horse breed"@en ,
                                          "Proprietà che esprime il territorio di origine di una razza di cavallo"@it ;
                             rdfs:label "ha Regione di origine"@it ,
                                        "has region of origin"@en .


###  http://www.semanticweb.org/annag/ontologies/2024/1/ontoHorses/permetteIlConseguimentoDi
ontoHorse:permetteIlConseguimentoDi rdf:type owl:ObjectProperty ;
                                    rdfs:domain ontoHorse:CategorieDiSalto ;
                                    rdfs:range ontoHorse:Patente ;
                                    rdfs:comment "Property that expresses the relationship between the jumping categories in which a rider competes and the riding licences he can obtain. In particular, the C80 allows the obtaining of the patent; the C115 allows the achievement of the 1st degree and the C135 the 2nd degree,"@en ,
                                                 "Proprietà che esprime la relazione tra le categorie di salto ad ostacoli in cui un cavaliera gareggia e le autorizzazioni a montare che può conseguire. In particolare la C80 permette il conseguimento del brevetto; la C115 permette il conseguimento del 1° grado e la C135 del 2° grado"@it ;
                                    rdfs:label "allows the achievement of"@en ,
                                               "permette il conseguiimento di"@it .


###  http://www.semanticweb.org/annag/ontologies/2024/1/ontoHorses/vieneConseguitoDa
ontoHorse:vieneConseguitoDa rdf:type owl:ObjectProperty ;
                            rdfs:domain ontoHorse:Patente ;
                            rdfs:range ontoHorse:Cavaliere ;
                            rdfs:comment "Inverse property of \"achieve\""@en ,
                                         "Proprietà inversa di \"consegue\""@it ;
                            rdfs:label "is achieved by"@en ,
                                       "viene conseguito da"@it .


###  http://www.semanticweb.org/annag/ontologies/2024/1/ontoHorses/vieneUtilizzatoPer
ontoHorse:vieneUtilizzatoPer rdf:type owl:ObjectProperty ;
                             rdfs:domain ontoHorse:Cavallo ;
                             rdfs:range ontoHorse:Impiego ;
                             rdfs:comment "Property that expresses the use made of a horse in work or sporting activities."@en ,
                                          "Proprietà che esprime l'utilizzo che viene fatto di un cavallo in attività lavorative o sportive."@it ;
                             rdfs:label "is used for"@en ,
                                        "viene utilizzato per"@it .


###  http://www.semanticweb.org/annag/ontologies/2024/1/ontoHorses/èAdattoPer
ontoHorse:èAdattoPer rdf:type owl:ObjectProperty ;
                     rdfs:domain ontoHorse:Cavallo ;
                     rdfs:range ontoHorse:Cavaliere ;
                     owl:propertyChainAxiom ( ontoHorse:adattoAlConseguimentoDi
                                              ontoHorse:vieneConseguitoDa
                                            ) ;
                     rdfs:comment "Property that expresses the suitability of a horse for the sporting abilities of a rider. Generally horses that are used in very high jumping categories are not suitable for inexperienced riders."@en ,
                                  "Proprietà che esprime l'adeguatezza di un cavallo alle capacità sportive di un cavaliere. Generalmente cavalli che vengono utilizzati in categorie di salto molto alte non sono idonei a cavalieri poco esperti."@it ;
                     rdfs:label "is suitable for"@en ,
                                "è adatto per"@it .


#################################################################
#    Data properties
#################################################################

###  http://www.semanticweb.org/annag/ontologies/2024/1/ontoHorses#annoDiNascita
:annoDiNascita rdf:type owl:DatatypeProperty ,
                        owl:FunctionalProperty ;
               rdfs:domain ontoHorse:Cavallo ;
               rdfs:range xsd:nonNegativeInteger ;
               rdfs:comment "Anno di nascita del cavallo in vendita"@it ,
                            "Year of birth of the horse for sale"@en ;
               rdfs:label "anno di nascita"@it ,
                          "year of birth"@en .


###  http://www.semanticweb.org/annag/ontologies/2024/1/ontoHorses#contattoProprietario
:contattoProprietario rdf:type owl:DatatypeProperty ;
                      rdfs:domain ontoHorse:Cavallo ;
                      rdfs:range xsd:string ;
                      rdfs:comment "Numero telefonico  per contattare il proprietario del cavallo in vendita"@it ,
                                   "Telephone number to contact the owner of the horse for sale"@en ;
                      rdfs:label "contatto telefonico del proprietario"@it ,
                                 "owner's telephone number"@en .


###  http://www.semanticweb.org/annag/ontologies/2024/1/ontoHorses#haProprietario
:haProprietario rdf:type owl:DatatypeProperty ;
                rdfs:domain ontoHorse:Cavallo ;
                rdfs:range xsd:string ;
                rdfs:comment "Name of the current owner of the horse for sale"@en ,
                             "Nome dell'attuale proprietario del cavallo in vendita"@it ;
                rdfs:label "ha proprietario"@it ,
                           "has owner"@en .


###  http://www.semanticweb.org/annag/ontologies/2024/1/ontoHorses#nomeCavallo
:nomeCavallo rdf:type owl:DatatypeProperty ,
                      owl:FunctionalProperty ;
             rdfs:domain ontoHorse:Cavallo ;
             rdfs:range xsd:string ;
             rdfs:comment "Horse name for sale"@en ,
                          "Nome del cavallo in vendita"@it ;
             rdfs:label "horse name"@en ,
                        "nome del cavallo"@it .


###  http://www.semanticweb.org/annag/ontologies/2024/1/ontoHorses#provinciaDiScuderizzazione
:provinciaDiScuderizzazione rdf:type owl:DatatypeProperty ,
                                     owl:FunctionalProperty ;
                            rdfs:domain ontoHorse:Cavallo ;
                            rdfs:range xsd:string ;
                            rdfs:comment "Province in which the horse for sale is stabled"@en ,
                                         "Provincia in cui il cavallo in vendita è scuderizzato"@it ;
                            rdfs:label "province of horse stable"@en ,
                                       "provincia di scuderizzazione"@it .


###  http://www.semanticweb.org/annag/ontologies/2024/1/ontoHorses#regioneDiScuderizzazione
:regioneDiScuderizzazione rdf:type owl:DatatypeProperty ,
                                   owl:FunctionalProperty ;
                          rdfs:domain ontoHorse:Cavallo ;
                          rdfs:range xsd:string ;
                          rdfs:comment "Region in which the horse for sale is stabled"@en ,
                                       "Regione in cui il cavallo in vendita è scuderizzato"@it ;
                          rdfs:label "region of horse stable"@en ,
                                     "regione di scuderizzazione"@it .


###  http://www.semanticweb.org/annag/ontologies/2024/1/ontoHorses/altezzaAlGarrese_cm
ontoHorse:altezzaAlGarrese_cm rdf:type owl:DatatypeProperty ,
                                       owl:FunctionalProperty ;
                              rdfs:domain ontoHorse:Cavallo ;
                              rdfs:range xsd:nonNegativeInteger ;
                              <http://schema.org/image> <https://www.kramer.it/$WS/kraemer-pferdesport/websale8_shop-kraemer-pferdesport/benutzer/templates/ws-customer/Serviceseiten/images/content/blankets_ita.jpg> ;
                              rdfs:comment "L'altezza di un animale quadrupede si misura al garrese che è il punto più alto del dorso e si trova tra il collo e il tronco nella zona di incontro tra collo e scapole"@it ,
                                           "The height of a quadruped animal is measured at the withers which is the highest point of the back and is located between the neck and the trunk in the area where the neck and shoulder blades meet"@en ;
                              rdfs:label "altezza al garrese [cm]"@it ,
                                         "height at the withers [cm]"@en .


###  http://www.semanticweb.org/annag/ontologies/2024/1/ontoHorses/altezzaMaxDiSalto_cm
ontoHorse:altezzaMaxDiSalto_cm rdf:type owl:DatatypeProperty ,
                                        owl:FunctionalProperty ;
                               rdfs:domain ontoHorse:Cavallo ;
                               rdfs:range xsd:nonNegativeInteger ;
                               rdfs:comment "Altezza massima di salto ostacoli registrata in una competizione ufficiale FISE"@it ,
                                            "Maximum jumping height recorded in an official FISE competition"@en ;
                               rdfs:label "Maximum jumping height [cm]"@en ,
                                          "altezza massima di salto ostacoli [cm]"@it .


###  http://www.semanticweb.org/annag/ontologies/2024/1/ontoHorses/altezzaMediaAlGarrese_cm
ontoHorse:altezzaMediaAlGarrese_cm rdf:type owl:DatatypeProperty ,
                                            owl:FunctionalProperty ;
                                   rdfs:domain ontoHorse:RazzaCavallo ;
                                   rdfs:range xsd:nonNegativeInteger ;
                                   rdfs:comment "Average height at the withers of a horse breed"@en ,
                                                "Valore medio dell'altezza al garrese di una razza di cavallo"@it ;
                                   rdfs:label "Average height at the withers  [cm]"@en ,
                                              "altezza media al garrese [cm]"@it .


###  http://www.semanticweb.org/annag/ontologies/2024/1/ontoHorses/categorieDiDressage
ontoHorse:categorieDiDressage rdf:type owl:DatatypeProperty ;
                              rdfs:domain ontoHorse:Cavallo ;
                              rdfs:range [ rdf:type rdfs:Datatype ;
                                           owl:oneOf [ rdf:type rdf:List ;
                                                       rdf:first "D" ;
                                                       rdf:rest [ rdf:type rdf:List ;
                                                                  rdf:first "E" ;
                                                                  rdf:rest [ rdf:type rdf:List ;
                                                                             rdf:first "F" ;
                                                                             rdf:rest [ rdf:type rdf:List ;
                                                                                        rdf:first "M" ;
                                                                                        rdf:rest rdf:nil
                                                                                      ]
                                                                           ]
                                                                ]
                                                     ]
                                         ] ;
                              rdfs:comment "A Dressage competition is defined by a category that indicates its difficulty. In particular: E (elementary), F (easy), M (medium), D (difficult)"@en ,
                                           "Una competizione di Dressage è definita da una categoria che ne indica la difficolta. In particolare: E (elementare), F (facile), M (media), D (difficile)"@it ;
                              rdfs:label "Dressage competition categories"@en ,
                                         "categorie di Dressage"@it .


###  http://www.semanticweb.org/annag/ontologies/2024/1/ontoHorses/età
ontoHorse:età rdf:type owl:DatatypeProperty ,
                       owl:FunctionalProperty ;
              rdfs:domain ontoHorse:Cavallo ;
              rdfs:range xsd:nonNegativeInteger ;
              rdfs:comment "age of horse for sale"@en ,
                           "età del cavallo in vendita"@it ;
              rdfs:label "age"@en ,
                         "età"@it .


###  http://www.semanticweb.org/annag/ontologies/2024/1/ontoHorses/haColoreMantello
ontoHorse:haColoreMantello rdf:type owl:DatatypeProperty ;
                           rdfs:domain ontoHorse:RazzaCavallo ;
                           rdfs:range [ rdf:type rdfs:Datatype ;
                                        owl:oneOf [ rdf:type rdf:List ;
                                                    rdf:first "apaloosa" ;
                                                    rdf:rest [ rdf:type rdf:List ;
                                                               rdf:first "baio" ;
                                                               rdf:rest [ rdf:type rdf:List ;
                                                                          rdf:first "crema" ;
                                                                          rdf:rest [ rdf:type rdf:List ;
                                                                                     rdf:first "falbo" ;
                                                                                     rdf:rest [ rdf:type rdf:List ;
                                                                                                rdf:first "grigio" ;
                                                                                                rdf:rest [ rdf:type rdf:List ;
                                                                                                           rdf:first "isabella" ;
                                                                                                           rdf:rest [ rdf:type rdf:List ;
                                                                                                                      rdf:first "mantello coniugato" ;
                                                                                                                      rdf:rest [ rdf:type rdf:List ;
                                                                                                                                 rdf:first "morello" ;
                                                                                                                                 rdf:rest [ rdf:type rdf:List ;
                                                                                                                                            rdf:first "palomino" ;
                                                                                                                                            rdf:rest [ rdf:type rdf:List ;
                                                                                                                                                       rdf:first "pezzato" ;
                                                                                                                                                       rdf:rest [ rdf:type rdf:List ;
                                                                                                                                                                  rdf:first "roano" ;
                                                                                                                                                                  rdf:rest [ rdf:type rdf:List ;
                                                                                                                                                                             rdf:first "sauro" ;
                                                                                                                                                                             rdf:rest [ rdf:type rdf:List ;
                                                                                                                                                                                        rdf:first "sorcino" ;
                                                                                                                                                                                        rdf:rest [ rdf:type rdf:List ;
                                                                                                                                                                                                   rdf:first "ubero" ;
                                                                                                                                                                                                   rdf:rest rdf:nil
                                                                                                                                                                                                 ]
                                                                                                                                                                                      ]
                                                                                                                                                                           ]
                                                                                                                                                                ]
                                                                                                                                                     ]
                                                                                                                                          ]
                                                                                                                               ]
                                                                                                                    ]
                                                                                                         ]
                                                                                              ]
                                                                                   ]
                                                                        ]
                                                             ]
                                                  ]
                                      ] ;
                           rdfs:comment "Insieme dei colori del mantello ammessi per una razza di cavallo"@it ,
                                        "Set of coat colors allowed for a horse breed"@en ;
                           rdfs:label "admittet coat colors"@en ,
                                      "ha colori mantello ammessi"@it .


###  http://www.semanticweb.org/annag/ontologies/2024/1/ontoHorses/haSesso
ontoHorse:haSesso rdf:type owl:DatatypeProperty ,
                           owl:FunctionalProperty ;
                  rdfs:domain ontoHorse:Cavallo ;
                  rdfs:range [ rdf:type rdfs:Datatype ;
                               owl:oneOf [ rdf:type rdf:List ;
                                           rdf:first "castrone" ;
                                           rdf:rest [ rdf:type rdf:List ;
                                                      rdf:first "femmina" ;
                                                      rdf:rest [ rdf:type rdf:List ;
                                                                 rdf:first "maschio" ;
                                                                 rdf:rest rdf:nil
                                                               ]
                                                    ]
                                         ]
                             ] ;
                  rdfs:comment "Horse sex for sale"@en ,
                               "Sesso del cavallo in vendita" ;
                  rdfs:label "ha sesso"@it ,
                             "has sex"@en .


###  http://www.semanticweb.org/annag/ontologies/2024/1/ontoHorses/pesoMedio_Kg
ontoHorse:pesoMedio_Kg rdf:type owl:DatatypeProperty ,
                                owl:FunctionalProperty ;
                       rdfs:domain ontoHorse:RazzaCavallo ;
                       rdfs:range xsd:nonNegativeInteger ;
                       rdfs:comment "Average mass value of a specific horse breed"@en ,
                                    "Valore medio della massa di una specifica razza di cavallo"@it ;
                       rdfs:label "medium weight [Kg]"@en ,
                                  "peso medio [Kg]"@it .


#################################################################
#    Classes
#################################################################

###  http://dbpedia.org/ontology/HorseRider
<http://dbpedia.org/ontology/HorseRider> rdf:type owl:Class ;
                                         owl:equivalentClass ontoHorse:Cavaliere ;
                                         rdfs:subClassOf ontoHorse:Persona .


###  http://dbpedia.org/ontology/horse
<http://dbpedia.org/ontology/horse> rdf:type owl:Class ;
                                    owl:equivalentClass ontoHorse:Cavallo .


###  http://dbpedia.org/ontology/horseRidingDiscipline
<http://dbpedia.org/ontology/horseRidingDiscipline> rdf:type owl:Class ;
                                                    owl:equivalentClass ontoHorse:Sella ;
                                                    rdfs:subClassOf ontoHorse:Impiego .


###  http://schema.org/Place
<http://schema.org/Place> rdf:type owl:Class ;
                          owl:equivalentClass ontoHorse:AreaGeografica .


###  http://www.ontologydesignpatterns.org/cp/owl/collectionentity.owl#Collection
<http://www.ontologydesignpatterns.org/cp/owl/collectionentity.owl#Collection> owl:equivalentClass ontoHorse:CatalogoAutorizzazioniAMontareFise .


###  http://www.semanticweb.org/annag/ontologies/2024/1/ontoHorses#AltaScuola
:AltaScuola rdf:type owl:Class ;
            rdfs:subClassOf ontoHorse:SportEquestre .


###  http://www.semanticweb.org/annag/ontologies/2024/1/ontoHorses#CavalloDaEquiturismo
:CavalloDaEquiturismo rdf:type owl:Class ;
                      owl:equivalentClass [ rdf:type owl:Restriction ;
                                            owl:onProperty ontoHorse:vieneUtilizzatoPer ;
                                            owl:hasValue :Equiturismo
                                          ] ;
                      rdfs:subClassOf :CavalloDaSella ;
                      rdfs:comment "Cavallo utilizzato per equiturismo"@it ,
                                   "Horse used for equestrian tourism"@en ;
                      rdfs:label "Cavallo da equiturismo"@it ,
                                 "Equestrian tourism horse"@en .


###  http://www.semanticweb.org/annag/ontologies/2024/1/ontoHorses#CavalloDaLavoro
:CavalloDaLavoro rdf:type owl:Class ;
                 owl:equivalentClass [ rdf:type owl:Restriction ;
                                       owl:onProperty ontoHorse:vieneUtilizzatoPer ;
                                       owl:minQualifiedCardinality "1"^^xsd:nonNegativeInteger ;
                                       owl:onClass ontoHorse:Lavoro
                                     ] ;
                 rdfs:subClassOf ontoHorse:Cavallo ;
                 rdfs:comment "Cavallo impiegato nel lavoro agricolo o nel traino carrozze e/o carichi"@it ,
                              "Horse used in agricultural work or in pulling carriages and/or loads"@en ;
                 rdfs:label "Cavallo da lavoro"@it ,
                            "Work horse"@en .


###  http://www.semanticweb.org/annag/ontologies/2024/1/ontoHorses#CavalloDaSella
:CavalloDaSella rdf:type owl:Class ;
                owl:equivalentClass [ rdf:type owl:Restriction ;
                                      owl:onProperty ontoHorse:vieneUtilizzatoPer ;
                                      owl:someValuesFrom ontoHorse:Sella
                                    ] ;
                rdfs:subClassOf ontoHorse:Cavallo ;
                rdfs:comment "Cavallo che ha attitudine alla sella"@it ,
                             "Horse suitable for the saddle"@en ;
                rdfs:label "Cavallo da sella"@it ,
                           "Riding horse"@en .


###  http://www.semanticweb.org/annag/ontologies/2024/1/ontoHorses#CavalloDaTiroAgricolo
:CavalloDaTiroAgricolo rdf:type owl:Class ;
                       owl:equivalentClass [ rdf:type owl:Restriction ;
                                             owl:onProperty ontoHorse:vieneUtilizzatoPer ;
                                             owl:hasValue :TiroAgricolo
                                           ] ;
                       rdfs:subClassOf :CavalloDaLavoro ;
                       rdfs:comment "Cavallo utilizzato nei lavori agricoli"@it ,
                                    "Horse used in agricultural work"@en ;
                       rdfs:label "Agricultural wor horse"@en ,
                                  "Cavallo da tiro agricolo"@it .


###  http://www.semanticweb.org/annag/ontologies/2024/1/ontoHorses#CavalloDaTrainoCarrozze
:CavalloDaTrainoCarrozze rdf:type owl:Class ;
                         owl:equivalentClass [ rdf:type owl:Restriction ;
                                               owl:onProperty ontoHorse:vieneUtilizzatoPer ;
                                               owl:hasValue :TrainoCarrozze
                                             ] ;
                         rdfs:subClassOf :CavalloDaLavoro ;
                         rdfs:comment "Cavallo utilizzato per il traino di carrozze merci o passeggeri"@it ,
                                      "Horse used for pulling freight or passenger carriages"@en ;
                         rdfs:label "Cavallo da traino carrozze"@it ,
                                    "Horse for pulling carriages"@en .


###  http://www.semanticweb.org/annag/ontologies/2024/1/ontoHorses#CrossCountry
:CrossCountry rdf:type owl:Class ;
              rdfs:subClassOf ontoHorse:SportEquestre .


###  http://www.semanticweb.org/annag/ontologies/2024/1/ontoHorses#Dressage
:Dressage rdf:type owl:Class ;
          rdfs:subClassOf ontoHorse:SportEquestre .


###  http://www.semanticweb.org/annag/ontologies/2024/1/ontoHorses#Endurance
:Endurance rdf:type owl:Class ;
           rdfs:subClassOf ontoHorse:SportEquestre .


###  http://www.semanticweb.org/annag/ontologies/2024/1/ontoHorses#Equiturismo
:Equiturismo rdf:type owl:Class ;
             rdfs:subClassOf ontoHorse:Sella .


###  http://www.semanticweb.org/annag/ontologies/2024/1/ontoHorses#Eventing
:Eventing rdf:type owl:Class ;
          rdfs:subClassOf ontoHorse:SportEquestre .


###  http://www.semanticweb.org/annag/ontologies/2024/1/ontoHorses#Indole
:Indole rdf:type owl:Class ;
        owl:equivalentClass [ rdf:type owl:Class ;
                              owl:oneOf ( :sangueCaldo
                                          :sangueFreddo
                                          :sangueMisto
                                        )
                            ] ;
        rdfs:comment "L'indole o temperamento è uno dei classici parametri di classificazione dei cavalli"@it ,
                     "The nature or temperament is one of the classic classification parameters of horses"@en ;
        rdfs:label "Indole"@it ,
                   "Nature"@en .


###  http://www.semanticweb.org/annag/ontologies/2024/1/ontoHorses#RazzaBelga
:RazzaBelga rdf:type owl:Class ;
            owl:equivalentClass [ rdf:type owl:Restriction ;
                                  owl:onProperty :haNazionalità ;
                                  owl:hasValue :Belgio
                                ] ;
            rdfs:subClassOf :RazzaEuropea ;
            rdfs:comment "Horse breed originated from Belgium"@en ,
                         "Razza di cavallo originaria del Belgio"@it ;
            rdfs:label "Belgian horse breed"@en ,
                       "Razza belga"@it .


###  http://www.semanticweb.org/annag/ontologies/2024/1/ontoHorses#RazzaBrachimorfa
:RazzaBrachimorfa rdf:type owl:Class ;
                  rdfs:subClassOf ontoHorse:RazzaCavallo ;
                  rdfs:comment "Horse breed more inclined to the development of musculature, with a wide chest, powerful, massive and not very long shapes."@en ,
                               "Razza di cavallo  più propenso allo sviluppo di muscolatura, con un torace ampio, forme potenti, massicce e non molto lungo."@it ;
                  rdfs:label "Brachymorphic horse breed"@en ,
                             "Razza brachimorfa"@it .


###  http://www.semanticweb.org/annag/ontologies/2024/1/ontoHorses#RazzaDaAttacchi
:RazzaDaAttacchi rdf:type owl:Class ;
                 owl:equivalentClass [ rdf:type owl:Restriction ;
                                       owl:onProperty :puòEssereImpiegataIn ;
                                       owl:hasValue :TrainoCarrozze
                                     ] ;
                 rdfs:subClassOf ontoHorse:RazzaDaLavoro ;
                 rdfs:comment "Horse breed used for pulling carriages"@en ,
                              "Razza di cavallo utilizzata per il traino carrozze"@it ;
                 rdfs:label "Horse breed pulling carriages"@en ,
                            "Razza da attacchi"@it .


###  http://www.semanticweb.org/annag/ontologies/2024/1/ontoHorses#RazzaDaCrossCountry
:RazzaDaCrossCountry rdf:type owl:Class ;
                     owl:equivalentClass [ rdf:type owl:Restriction ;
                                           owl:onProperty :puòEssereImpiegataIn ;
                                           owl:hasValue :CrossCountry
                                         ] ;
                     rdfs:subClassOf :RazzaSportiva ;
                     rdfs:comment "Razza di cavallo che può essere utilizzata nella disciplina di sport equestre del cross-country"@it ;
                     rdfs:label "Cross-country horse breed"@en ,
                                "Horse breed that can be used in the equestrian sport discipline of cross-country"@en ,
                                "Razza da cross-country"@it .


###  http://www.semanticweb.org/annag/ontologies/2024/1/ontoHorses#RazzaDaEquiturismo
:RazzaDaEquiturismo rdf:type owl:Class ;
                    owl:equivalentClass [ rdf:type owl:Restriction ;
                                          owl:onProperty :puòEssereImpiegataIn ;
                                          owl:hasValue :Equiturismo
                                        ] ;
                    rdfs:subClassOf :RazzaDaSella ;
                    rdfs:comment "Horse breed that can be used for equestrian tourism (or trekking)"@en ,
                                 "Razza di cavallo che può essere utilizzata per il turismo equestre (o trekking)"@it ;
                    rdfs:label "Equestrian tourism horse breed"@en ,
                               "Razza da equiturismo"@it .


###  http://www.semanticweb.org/annag/ontologies/2024/1/ontoHorses#RazzaDaEventing
:RazzaDaEventing rdf:type owl:Class ;
                 owl:equivalentClass [ rdf:type owl:Restriction ;
                                       owl:onProperty :puòEssereImpiegataIn ;
                                       owl:hasValue :Eventing
                                     ] ;
                 rdfs:subClassOf :RazzaSportiva ;
                 rdfs:comment "Horse breed that can be used in the equestrian sport discipline of eventing"@en ,
                              "Razza di cavallo che può essere utilizzata nella disciplina di sport equestre dell'eventing"@it ;
                 rdfs:label "Eventing horse breed"@en ,
                            "Razza da eventing"@it .


###  http://www.semanticweb.org/annag/ontologies/2024/1/ontoHorses#RazzaDaSella
:RazzaDaSella rdf:type owl:Class ;
              owl:equivalentClass [ rdf:type owl:Restriction ;
                                    owl:onProperty :puòEssereImpiegataIn ;
                                    owl:someValuesFrom ontoHorse:Sella
                                  ] ;
              rdfs:subClassOf ontoHorse:RazzaCavallo ;
              rdfs:comment "Horse breed suitable for the saddle"@en ,
                           "Razza di cavallo che ha attitudine alla sella"@it ;
              rdfs:label "Razza da sella"@it ,
                         "Riding horse breed"@en .


###  http://www.semanticweb.org/annag/ontologies/2024/1/ontoHorses#RazzaDaTiroAgricolo
:RazzaDaTiroAgricolo rdf:type owl:Class ;
                     owl:equivalentClass [ rdf:type owl:Restriction ;
                                           owl:onProperty :puòEssereImpiegataIn ;
                                           owl:hasValue :TiroAgricolo
                                         ] ;
                     rdfs:subClassOf ontoHorse:RazzaDaLavoro ;
                     rdfs:comment "Horse breed used for agricultural work"@en ,
                                  "Razza di cavallo utilizzata nelle attività agricole"@it ;
                     rdfs:label "Horse breed for agricultural work"@en ,
                                "Razza da tiro agricolo"@it .


###  http://www.semanticweb.org/annag/ontologies/2024/1/ontoHorses#RazzaDanese
:RazzaDanese rdf:type owl:Class ;
             owl:equivalentClass [ rdf:type owl:Restriction ;
                                   owl:onProperty :haNazionalità ;
                                   owl:hasValue :Danimarca
                                 ] ;
             rdfs:subClassOf :RazzaEuropea ;
             rdfs:comment "Horse breed originated from Denmark"@en ,
                          "Razza di cavallo originaria della Danimarca"@it ;
             rdfs:label "Danish horse breed"@en ,
                        "Razza danese"@it .


###  http://www.semanticweb.org/annag/ontologies/2024/1/ontoHorses#RazzaEndurance
:RazzaEndurance rdf:type owl:Class ;
                owl:equivalentClass [ rdf:type owl:Restriction ;
                                      owl:onProperty :puòEssereImpiegataIn ;
                                      owl:hasValue :Endurance
                                    ] ;
                rdfs:subClassOf :RazzaSportiva ;
                rdfs:comment "Horse breed that can be used in the equestrian sport discipline of endurance"@en ,
                             "Razza di cavallo che può essere utilizzata nella disciplina di sport equestre dell'endurance"@it ;
                rdfs:label "Endurance horse breed"@en ,
                           "Razza da endurance"@it .


###  http://www.semanticweb.org/annag/ontologies/2024/1/ontoHorses#RazzaEuropea
:RazzaEuropea rdf:type owl:Class ;
              rdfs:subClassOf ontoHorse:RazzaCavallo ;
              rdfs:comment "Horse breed originating from Europe"@en ,
                           "Razza di cavallo originaria dell'Europa"@it ;
              rdfs:label "European horse breed"@en ,
                         "Razza europea"@it .


###  http://www.semanticweb.org/annag/ontologies/2024/1/ontoHorses#RazzaFrancese
:RazzaFrancese rdf:type owl:Class ;
               owl:equivalentClass [ rdf:type owl:Restriction ;
                                     owl:onProperty :haNazionalità ;
                                     owl:hasValue ontoHorse:Francia
                                   ] ;
               rdfs:subClassOf :RazzaEuropea ;
               rdfs:comment "Horse breed originated from France"@en ,
                            "Razza di cavallo originaria della Francia"@it ;
               rdfs:label "French horse breed"@en ,
                          "Razza francese"@it .


###  http://www.semanticweb.org/annag/ontologies/2024/1/ontoHorses#RazzaInglese
:RazzaInglese rdf:type owl:Class ;
              owl:equivalentClass [ rdf:type owl:Restriction ;
                                    owl:onProperty :haNazionalità ;
                                    owl:hasValue :RegnoUnito
                                  ] ;
              rdfs:subClassOf :RazzaEuropea ;
              rdfs:comment "Horse breed originated from United Kingdom"@en ,
                           "Razza di cavallo originaria del Regno Unito"@it ;
              rdfs:label "English horse breed"@en ,
                         "Razza inglese"@it .


###  http://www.semanticweb.org/annag/ontologies/2024/1/ontoHorses#RazzaMesoBrachimorfa
:RazzaMesoBrachimorfa rdf:type owl:Class ;
                      rdfs:subClassOf ontoHorse:RazzaCavallo ;
                      rdfs:comment "Horse breed between draft horses and riding horses."@en ,
                                   "Razza di cavallo a metà strada tra i cavalli da tiro e i cavalli da sella."@it ;
                      rdfs:label "Meso-brachimorphyc horse breed"@en ,
                                 "Razza meso-brachimorfa"@it .


###  http://www.semanticweb.org/annag/ontologies/2024/1/ontoHorses#RazzaMesoDolicomorfa
:RazzaMesoDolicomorfa rdf:type owl:Class ;
                      rdfs:subClassOf ontoHorse:RazzaCavallo ;
                      rdfs:comment "Powerful horse breed, strong but at the same time agile and noble in bearing."@en ,
                                   "Razza di cavallo potente, forte ma contemporaneamente agile e nobile nel portamento."@it ;
                      rdfs:label "Meso-dolicomorphic horse breed"@en ,
                                 "Razza meso-dolicomorfa"@it .


###  http://www.semanticweb.org/annag/ontologies/2024/1/ontoHorses#RazzaOlandese
:RazzaOlandese rdf:type owl:Class ;
               owl:equivalentClass [ rdf:type owl:Restriction ;
                                     owl:onProperty :haNazionalità ;
                                     owl:hasValue :PaesiBassi
                                   ] ;
               rdfs:subClassOf :RazzaEuropea ;
               rdfs:comment "Horse breed originated from Holland"@en ,
                            "Razza di cavallo originaria dei Paesi Bassi"@it ;
               rdfs:label "Dutch horse breed"@en ,
                          "Razza olandese"@it .


###  http://www.semanticweb.org/annag/ontologies/2024/1/ontoHorses#RazzaPortoghese
:RazzaPortoghese rdf:type owl:Class ;
                 owl:equivalentClass [ rdf:type owl:Restriction ;
                                       owl:onProperty :haNazionalità ;
                                       owl:hasValue :Portogallo
                                     ] ;
                 rdfs:subClassOf :RazzaEuropea ;
                 rdfs:comment "Horse breed originated from Portugal"@en ,
                              "Razza di cavallo originaria del Portogallo"@it ;
                 rdfs:label "Portoguese horse breed"@en ,
                            "Razza portoghese"@it .


###  http://www.semanticweb.org/annag/ontologies/2024/1/ontoHorses#RazzaSportiva
:RazzaSportiva rdf:type owl:Class ;
               owl:equivalentClass [ rdf:type owl:Restriction ;
                                     owl:onProperty :puòEssereImpiegataIn ;
                                     owl:minQualifiedCardinality "1"^^xsd:nonNegativeInteger ;
                                     owl:onClass ontoHorse:SportEquestre
                                   ] ;
               rdfs:subClassOf :RazzaDaSella ;
               rdfs:comment "Horse breed that can be used in equestrian sports"@en ,
                            "Razza di cavallo che può essere utilizzata negli sport equestri"@it ;
               rdfs:label "Razza sportiva"@it ,
                          "Sport horse breed"@en .


###  http://www.semanticweb.org/annag/ontologies/2024/1/ontoHorses#RazzeDolicomorfa
:RazzeDolicomorfa rdf:type owl:Class ;
                  rdfs:subClassOf ontoHorse:RazzaCavallo ;
                  rdfs:comment "Horse breed more suitable for fast and long gaits than for tests of strength: it has a deep chest, elongated lines and joints with very open angles. The figure is agile, light and slender."@en ,
                               "Razza di cavallo più idoneo alle andature veloci e allungate che alle prove di forza: ha torace profondo, linee allungate e articolazioni con angoli molto aperti. La figura è agile, leggera e slanciata."@it ;
                  rdfs:label "Dolicomorphic horse breed"@en ,
                             "Razza dolicomorfa"@it .


###  http://www.semanticweb.org/annag/ontologies/2024/1/ontoHorses#RazzeMesomorfa
:RazzeMesomorfa rdf:type owl:Class ;
                rdfs:subClassOf ontoHorse:RazzaCavallo ;
                rdfs:comment "Horse breed with a much lighter physical structure than the brachymorph, but still powerful and compact."@en ,
                             "Razza di cavallo con una struttura fisica molto più leggera rispetto al brachimorfo, ma comunque potente e compatta."@it ;
                rdfs:label "Mesomorphic horse breed"@en ,
                           "Razza mesomorfa"@it .


###  http://www.semanticweb.org/annag/ontologies/2024/1/ontoHorses#SaltoAdOstacoli
:SaltoAdOstacoli rdf:type owl:Class ;
                 rdfs:subClassOf ontoHorse:SportEquestre .


###  http://www.semanticweb.org/annag/ontologies/2024/1/ontoHorses#TiroAgricolo
:TiroAgricolo rdf:type owl:Class ;
              rdfs:subClassOf ontoHorse:Lavoro .


###  http://www.semanticweb.org/annag/ontologies/2024/1/ontoHorses#TrainoCarrozze
:TrainoCarrozze rdf:type owl:Class ;
                rdfs:subClassOf ontoHorse:Lavoro .


###  http://www.semanticweb.org/annag/ontologies/2024/1/ontoHorses/AreaGeografica
ontoHorse:AreaGeografica rdf:type owl:Class .


###  http://www.semanticweb.org/annag/ontologies/2024/1/ontoHorses/CatalogoAutorizzazioniAMontareFise
ontoHorse:CatalogoAutorizzazioniAMontareFise rdf:type owl:Class ;
                                             rdfs:comment "Catalog of horse riding licences defined by Federazione Italiana Sport Equestri"@en ,
                                                          "Catalogo di tutte le autorizzazioni a montare previste dalla Federazione Italiana Sport Equestri"@it ;
                                             rdfs:label "Catalog of horse riding licences FISE"@en ,
                                                        "Catalogo autorizzazioni a montare FISE"@it .


###  http://www.semanticweb.org/annag/ontologies/2024/1/ontoHorses/CategorieDiSalto
ontoHorse:CategorieDiSalto rdf:type owl:Class ;
                           owl:equivalentClass [ rdf:type owl:Class ;
                                                 owl:oneOf ( ontoHorse:C100
                                                             ontoHorse:C105
                                                             ontoHorse:C110
                                                             ontoHorse:C115
                                                             ontoHorse:C120
                                                             ontoHorse:C125
                                                             ontoHorse:C130
                                                             ontoHorse:C135
                                                             ontoHorse:C80
                                                             ontoHorse:C90
                                                           )
                                               ] ;
                           rdfs:subClassOf :SaltoAdOstacoli .


###  http://www.semanticweb.org/annag/ontologies/2024/1/ontoHorses/Cavaliere
ontoHorse:Cavaliere rdf:type owl:Class ;
                    owl:equivalentClass [ rdf:type owl:Class ;
                                          owl:oneOf ( ontoHorse:CavaliereEsperto
                                                      ontoHorse:CavaliereIntermedio
                                                      ontoHorse:CavaliereMoltoEsperto
                                                      ontoHorse:CavalierePrincipiante
                                                    )
                                        ] ;
                    rdfs:subClassOf ontoHorse:Persona .


###  http://www.semanticweb.org/annag/ontologies/2024/1/ontoHorses/Cavallo
ontoHorse:Cavallo rdf:type owl:Class ;
                  owl:equivalentClass [ rdf:type owl:Restriction ;
                                        owl:onProperty ontoHorse:haRazza ;
                                        owl:someValuesFrom ontoHorse:RazzaCavallo
                                      ] ,
                                      [ rdf:type owl:Restriction ;
                                        owl:onProperty ontoHorse:età ;
                                        owl:someValuesFrom xsd:integer
                                      ] ,
                                      [ rdf:type owl:Restriction ;
                                        owl:onProperty ontoHorse:haSesso ;
                                        owl:someValuesFrom xsd:string
                                      ] .


###  http://www.semanticweb.org/annag/ontologies/2024/1/ontoHorses/CavalloASangueCaldo
ontoHorse:CavalloASangueCaldo rdf:type owl:Class ;
                              owl:equivalentClass [ owl:intersectionOf ( ontoHorse:Cavallo
                                                                         [ rdf:type owl:Restriction ;
                                                                           owl:onProperty ontoHorse:haRazza ;
                                                                           owl:someValuesFrom ontoHorse:RazzaASangueCaldo
                                                                         ]
                                                                       ) ;
                                                    rdf:type owl:Class
                                                  ] ;
                              rdfs:subClassOf ontoHorse:Cavallo ;
                              rdfs:comment "Cavallo la cui razza è a sangue caldo"@it ,
                                           "Horse whose breed is warm-blooded"@en ;
                              rdfs:label "Cavallo a sangue caldo"@it ,
                                         "Warm blooded horse"@en .


###  http://www.semanticweb.org/annag/ontologies/2024/1/ontoHorses/CavalloASangueFreddo
ontoHorse:CavalloASangueFreddo rdf:type owl:Class ;
                               owl:equivalentClass [ owl:intersectionOf ( ontoHorse:Cavallo
                                                                          [ rdf:type owl:Restriction ;
                                                                            owl:onProperty ontoHorse:haRazza ;
                                                                            owl:someValuesFrom ontoHorse:RazzaASangueFreddo
                                                                          ]
                                                                        ) ;
                                                     rdf:type owl:Class
                                                   ] ;
                               rdfs:subClassOf ontoHorse:Cavallo ;
                               rdfs:comment "Cavallo la cui razza è a sangue freddo"@it ,
                                            "Horse whose breed is cold-blooded"@en ;
                               rdfs:label "Cavallo a sangue freddo"@it ,
                                          "Cold-blooded horse"@en .


###  http://www.semanticweb.org/annag/ontologies/2024/1/ontoHorses/CavalloASangueMisto
ontoHorse:CavalloASangueMisto rdf:type owl:Class ;
                              owl:equivalentClass [ owl:intersectionOf ( ontoHorse:Cavallo
                                                                         [ rdf:type owl:Restriction ;
                                                                           owl:onProperty ontoHorse:haRazza ;
                                                                           owl:someValuesFrom ontoHorse:RazzaASangueMisto
                                                                         ]
                                                                       ) ;
                                                    rdf:type owl:Class
                                                  ] ;
                              rdfs:subClassOf ontoHorse:Cavallo ;
                              rdfs:comment "Cavallo la cui razza è a sangue misto"@it ,
                                           "Horse whose breed is mixed blood"@en ;
                              rdfs:label "Cavallo a sangue misto"@it ,
                                         "Mixed-blooded horse"@en .


###  http://www.semanticweb.org/annag/ontologies/2024/1/ontoHorses/CavalloAdulto
ontoHorse:CavalloAdulto rdf:type owl:Class ;
                        owl:equivalentClass [ rdf:type owl:Restriction ;
                                              owl:onProperty ontoHorse:età ;
                                              owl:someValuesFrom [ rdf:type rdfs:Datatype ;
                                                                   owl:onDatatype xsd:integer ;
                                                                   owl:withRestrictions ( [ xsd:minExclusive 6
                                                                                          ]
                                                                                          [ xsd:maxInclusive 18
                                                                                          ]
                                                                                        )
                                                                 ]
                                            ] ;
                        rdfs:subClassOf ontoHorse:Cavallo ;
                        rdfs:comment "Cavallo con età superiore ai 6 anni"@it ,
                                     "Horse over 6 years old"@en ;
                        rdfs:label "Adult horse"@en ,
                                   "Cavallo adulto"@it .


###  http://www.semanticweb.org/annag/ontologies/2024/1/ontoHorses/CavalloAnziano
ontoHorse:CavalloAnziano rdf:type owl:Class ;
                         owl:equivalentClass [ rdf:type owl:Restriction ;
                                               owl:onProperty ontoHorse:età ;
                                               owl:someValuesFrom [ rdf:type rdfs:Datatype ;
                                                                    owl:onDatatype xsd:integer ;
                                                                    owl:withRestrictions ( [ xsd:minExclusive 18
                                                                                           ]
                                                                                         )
                                                                  ]
                                             ] ;
                         rdfs:subClassOf ontoHorse:Cavallo ;
                         rdfs:comment "Cavallo con età superiore o uguale ai 18 anni"@it ,
                                      "Horse aged 18 years or older"@en ;
                         rdfs:label "Cavallo anziano"@it ,
                                    "Old horse"@en .


###  http://www.semanticweb.org/annag/ontologies/2024/1/ontoHorses/CavalloCastrone
ontoHorse:CavalloCastrone rdf:type owl:Class ;
                          owl:equivalentClass [ rdf:type owl:Restriction ;
                                                owl:onProperty ontoHorse:haSesso ;
                                                owl:hasValue "castrone"
                                              ] ;
                          rdfs:subClassOf ontoHorse:Cavallo ;
                          rdfs:comment "Castrated male horse of any age"@en ,
                                       "Cavallo maschio castrato di qualsiasi età"@it ;
                          rdfs:label "Cavallo castrone"@it ,
                                     "Gelding horse"@en .


###  http://www.semanticweb.org/annag/ontologies/2024/1/ontoHorses/CavalloFemmina
ontoHorse:CavalloFemmina rdf:type owl:Class ;
                         owl:equivalentClass [ rdf:type owl:Restriction ;
                                               owl:onProperty ontoHorse:haSesso ;
                                               owl:hasValue "femmina"
                                             ] ;
                         rdfs:subClassOf ontoHorse:Cavallo ;
                         rdfs:comment "Cavallo il cui sesso è femmina"@it ,
                                      "Horse whose sex is female"@en ;
                         rdfs:label "Cavallo femmina"@it ,
                                    "Female horse"@en .


###  http://www.semanticweb.org/annag/ontologies/2024/1/ontoHorses/CavalloMaschio
ontoHorse:CavalloMaschio rdf:type owl:Class ;
                         owl:equivalentClass [ rdf:type owl:Restriction ;
                                               owl:onProperty ontoHorse:haSesso ;
                                               owl:hasValue "maschio"
                                             ] ;
                         rdfs:subClassOf ontoHorse:Cavallo ;
                         rdfs:comment "Cavallo il cui sesso è maschio e non è castrato"@it ,
                                      "Horse whose sex is male and is not castrated"@en ;
                         rdfs:label "Cavallo maschio"@it ,
                                    "Male horse"@en .


###  http://www.semanticweb.org/annag/ontologies/2024/1/ontoHorses/CavalloPerAltaScuola
ontoHorse:CavalloPerAltaScuola rdf:type owl:Class ;
                               owl:equivalentClass [ rdf:type owl:Restriction ;
                                                     owl:onProperty ontoHorse:vieneUtilizzatoPer ;
                                                     owl:hasValue :AltaScuola
                                                   ] ;
                               rdfs:subClassOf ontoHorse:CavalloSportivo ;
                               rdfs:comment "Cavallo utilizzato nella disciplina sportiva equestre dell'Alta Scuola"@it ,
                                            "Horse used in the equestrian sport of Spanish riding school"@en ;
                               rdfs:label "Cavallo per Alta Scuola"@it ,
                                          "Spanish riding school horse"@en .


###  http://www.semanticweb.org/annag/ontologies/2024/1/ontoHorses/CavalloPerCrossCountry
ontoHorse:CavalloPerCrossCountry rdf:type owl:Class ;
                                 owl:equivalentClass [ rdf:type owl:Restriction ;
                                                       owl:onProperty ontoHorse:vieneUtilizzatoPer ;
                                                       owl:hasValue :CrossCountry
                                                     ] ;
                                 rdfs:subClassOf ontoHorse:CavalloSportivo ;
                                 rdfs:comment "Cavallo usato nella disciplina sportiva equestre del cross-country"@it ,
                                              "Horse used in the equestrian sport discipline of cross-country"@en ;
                                 rdfs:label "Cavallo per cross-country"@it ,
                                            "Cross-country horse"@en .


###  http://www.semanticweb.org/annag/ontologies/2024/1/ontoHorses/CavalloPerDressage
ontoHorse:CavalloPerDressage rdf:type owl:Class ;
                             owl:equivalentClass [ rdf:type owl:Class ;
                                                   owl:unionOf ( [ rdf:type owl:Restriction ;
                                                                   owl:onProperty ontoHorse:vieneUtilizzatoPer ;
                                                                   owl:hasValue :Dressage
                                                                 ]
                                                                 [ rdf:type owl:Restriction ;
                                                                   owl:onProperty ontoHorse:categorieDiDressage ;
                                                                   owl:someValuesFrom xsd:string
                                                                 ]
                                                               )
                                                 ] ;
                             rdfs:subClassOf ontoHorse:CavalloSportivo ;
                             rdfs:comment "Cavallo utilizzato nella disciplina sportiva equestre del dressage"@it ,
                                          "Horse used in the equestrian sport discipline of dressage"@en ;
                             rdfs:label "Cavallo per Dressage"@it ,
                                        "Dressage horse"@en .


###  http://www.semanticweb.org/annag/ontologies/2024/1/ontoHorses/CavalloPerEndurance
ontoHorse:CavalloPerEndurance rdf:type owl:Class ;
                              owl:equivalentClass [ rdf:type owl:Restriction ;
                                                    owl:onProperty ontoHorse:vieneUtilizzatoPer ;
                                                    owl:hasValue :Endurance
                                                  ] ;
                              rdfs:subClassOf ontoHorse:CavalloSportivo ;
                              rdfs:comment "Cavallo utilizzato nella disciplina sportiva equestre dell'endurance"@it ,
                                           "Horse used in the equestrian sport discipline of endurance"@en ;
                              rdfs:label "Cavallo per Endurance"@it ,
                                         "Endurance horse"@en .


###  http://www.semanticweb.org/annag/ontologies/2024/1/ontoHorses/CavalloPerEventing
ontoHorse:CavalloPerEventing rdf:type owl:Class ;
                             owl:equivalentClass [ rdf:type owl:Restriction ;
                                                   owl:onProperty ontoHorse:vieneUtilizzatoPer ;
                                                   owl:hasValue :Eventing
                                                 ] ;
                             rdfs:subClassOf ontoHorse:CavalloSportivo ;
                             rdfs:comment "Cavallo utilizzato nella disciplina sportiva equestre dell'eventing"@it ,
                                          "Horse used in the equestrian sport discipline of eventing"@en ;
                             rdfs:label "Cavallo per Eventing"@it ,
                                        "Eventing horse"@en .


###  http://www.semanticweb.org/annag/ontologies/2024/1/ontoHorses/CavalloPerSaltoOstacoli
ontoHorse:CavalloPerSaltoOstacoli rdf:type owl:Class ;
                                  owl:equivalentClass [ rdf:type owl:Class ;
                                                        owl:unionOf ( [ rdf:type owl:Restriction ;
                                                                        owl:onProperty ontoHorse:gareggiaNelleCategorieDiSalto ;
                                                                        owl:someValuesFrom ontoHorse:CategorieDiSalto
                                                                      ]
                                                                      [ rdf:type owl:Restriction ;
                                                                        owl:onProperty ontoHorse:vieneUtilizzatoPer ;
                                                                        owl:hasValue :SaltoAdOstacoli
                                                                      ]
                                                                      [ rdf:type owl:Restriction ;
                                                                        owl:onProperty ontoHorse:altezzaMaxDiSalto_cm ;
                                                                        owl:someValuesFrom xsd:nonNegativeInteger
                                                                      ]
                                                                    )
                                                      ] ;
                                  rdfs:subClassOf ontoHorse:CavalloSportivo ;
                                  rdfs:comment "Cavallo utilizzato nella disciplina sportiva equestre del salto ostacoli"@it ,
                                               "Horse used in the equestrian sport discipline of jumping"@en ;
                                  rdfs:label "Cavallo per salto ostacoli"@it ,
                                             "Jumping horse"@en .


###  http://www.semanticweb.org/annag/ontologies/2024/1/ontoHorses/CavalloSportivo
ontoHorse:CavalloSportivo rdf:type owl:Class ;
                          owl:equivalentClass [ rdf:type owl:Restriction ;
                                                owl:onProperty ontoHorse:vieneUtilizzatoPer ;
                                                owl:minQualifiedCardinality "1"^^xsd:nonNegativeInteger ;
                                                owl:onClass ontoHorse:SportEquestre
                                              ] ;
                          rdfs:subClassOf :CavalloDaSella ;
                          rdfs:comment "Cavallo utilizzato nello sport equestre"@it ,
                                       "Horse used in some equestrian sports"@en ;
                          rdfs:label "Cavallo sportivo"@it ,
                                     "Sport horse"@en .


###  http://www.semanticweb.org/annag/ontologies/2024/1/ontoHorses/Impiego
ontoHorse:Impiego rdf:type owl:Class ;
                  rdfs:comment "I possibili impieghi del cavallo"@it ,
                               "The possible uses of the horse"@en ;
                  rdfs:label "Impiego"@it ,
                             "Use"@en .


###  http://www.semanticweb.org/annag/ontologies/2024/1/ontoHorses/Lavoro
ontoHorse:Lavoro rdf:type owl:Class ;
                 rdfs:subClassOf ontoHorse:Impiego ;
                 rdfs:comment "Impiego del cavallo in attività lavorative"@it ,
                              "Use of the horse in work activities"@en ;
                 rdfs:label "Lavoro"@it ,
                            "Work"@en .


###  http://www.semanticweb.org/annag/ontologies/2024/1/ontoHorses/Patente
ontoHorse:Patente rdf:type owl:Class ;
                  rdfs:subClassOf <http://www.ontologydesignpatterns.org/cp/owl/list.owl#ListItem> .


###  http://www.semanticweb.org/annag/ontologies/2024/1/ontoHorses/Persona
ontoHorse:Persona rdf:type owl:Class ;
                  owl:equivalentClass <http://xmlns.com/foaf/0.1/person> .


###  http://www.semanticweb.org/annag/ontologies/2024/1/ontoHorses/Puledro
ontoHorse:Puledro rdf:type owl:Class ;
                  owl:equivalentClass [ rdf:type owl:Restriction ;
                                        owl:onProperty ontoHorse:età ;
                                        owl:someValuesFrom [ rdf:type rdfs:Datatype ;
                                                             owl:onDatatype xsd:integer ;
                                                             owl:withRestrictions ( [ xsd:maxInclusive 6
                                                                                    ]
                                                                                  )
                                                           ]
                                      ] ;
                  rdfs:subClassOf ontoHorse:Cavallo ;
                  rdfs:comment "Cavallo di età inferiore ai 6 anni"@it ,
                               "Horse under 6 years of age"@en ;
                  rdfs:label "Foal"@en ,
                             "Puledro"@it .


###  http://www.semanticweb.org/annag/ontologies/2024/1/ontoHorses/RazzaASangueCaldo
ontoHorse:RazzaASangueCaldo rdf:type owl:Class ;
                            owl:equivalentClass [ rdf:type owl:Restriction ;
                                                  owl:onProperty :haIndole ;
                                                  owl:hasValue :sangueCaldo
                                                ] ;
                            rdfs:subClassOf ontoHorse:RazzaCavallo ;
                            rdfs:comment "Horse breed with warm-blooded temperament"@en ,
                                         "Razza di cavallo con temperamento a sangue caldo"@it ;
                            rdfs:label "Razza di cavallo a sangue caldo"@it ,
                                       "warm-blooded horse breed"@en .


###  http://www.semanticweb.org/annag/ontologies/2024/1/ontoHorses/RazzaASangueFreddo
ontoHorse:RazzaASangueFreddo rdf:type owl:Class ;
                             owl:equivalentClass [ rdf:type owl:Restriction ;
                                                   owl:onProperty :haIndole ;
                                                   owl:hasValue :sangueFreddo
                                                 ] ;
                             rdfs:subClassOf ontoHorse:RazzaCavallo ;
                             rdfs:comment "Horse breed with cold-blooded temperament"@en ,
                                          "Razza di cavallo con temperamento a sangue freddo"@it ;
                             rdfs:label "Cold-blooded horse breed"@en ,
                                        "Razza di cavallo a sangue freddo"@it .


###  http://www.semanticweb.org/annag/ontologies/2024/1/ontoHorses/RazzaASangueMisto
ontoHorse:RazzaASangueMisto rdf:type owl:Class ;
                            owl:equivalentClass [ rdf:type owl:Restriction ;
                                                  owl:onProperty :haIndole ;
                                                  owl:hasValue :sangueMisto
                                                ] ;
                            rdfs:subClassOf ontoHorse:RazzaCavallo ;
                            rdfs:comment "Horse breed with mixed-blooded temperament"@en ,
                                         "Razza di cavallo con temperamento a sangue misto"@it ;
                            rdfs:label "Mixed-blooded horse breed"@en ,
                                       "Razza di cavallo a sangue misto"@it .


###  http://www.semanticweb.org/annag/ontologies/2024/1/ontoHorses/RazzaCavallo
ontoHorse:RazzaCavallo rdf:type owl:Class ;
                       owl:equivalentClass [ rdf:type owl:Restriction ;
                                             owl:onProperty ontoHorse:haRegioneDiOrigine ;
                                             owl:someValuesFrom ontoHorse:AreaGeografica
                                           ] ,
                                           [ rdf:type owl:Restriction ;
                                             owl:onProperty :puòEssereImpiegataIn ;
                                             owl:minQualifiedCardinality "1"^^xsd:nonNegativeInteger ;
                                             owl:onClass ontoHorse:Impiego
                                           ] .


###  http://www.semanticweb.org/annag/ontologies/2024/1/ontoHorses/RazzaDaAltaScuola
ontoHorse:RazzaDaAltaScuola rdf:type owl:Class ;
                            owl:equivalentClass [ rdf:type owl:Restriction ;
                                                  owl:onProperty :puòEssereImpiegataIn ;
                                                  owl:hasValue :AltaScuola
                                                ] ;
                            rdfs:subClassOf :RazzaSportiva ;
                            rdfs:comment "Horse breed that can be used in the equestrian sport discipline of Spanish riding school"@en ,
                                         "Razza di cavallo che può essere utilizzata nella disciplina di sport equestre dell'Alta Scuola"@it ;
                            rdfs:label "Razza da Alta Scuola"@it ,
                                       "Spanish riding school horse breed"@en .


###  http://www.semanticweb.org/annag/ontologies/2024/1/ontoHorses/RazzaDaDressage
ontoHorse:RazzaDaDressage rdf:type owl:Class ;
                          owl:equivalentClass [ rdf:type owl:Restriction ;
                                                owl:onProperty :puòEssereImpiegataIn ;
                                                owl:hasValue :Dressage
                                              ] ;
                          rdfs:subClassOf :RazzaSportiva ;
                          rdfs:comment "Horse breed that can be used in the equestrian sport discipline of Dressage"@en ,
                                       "Razza di cavallo che può essere utilizzata nella disciplina di sport equestre del Dressage"@it ;
                          rdfs:label "Dressage horse breed"@en ,
                                     "Razza da dressage"@it .


###  http://www.semanticweb.org/annag/ontologies/2024/1/ontoHorses/RazzaDaLavoro
ontoHorse:RazzaDaLavoro rdf:type owl:Class ;
                        owl:equivalentClass [ rdf:type owl:Restriction ;
                                              owl:onProperty :puòEssereImpiegataIn ;
                                              owl:minQualifiedCardinality "1"^^xsd:nonNegativeInteger ;
                                              owl:onClass ontoHorse:Lavoro
                                            ] ;
                        rdfs:subClassOf ontoHorse:RazzaCavallo ;
                        rdfs:comment "Breed of horse used in agricultural work or for pulling carriages"@en ,
                                     "Razza di cavallo impiegata in attività lavorative agricole o di traino carrozze"@it ;
                        rdfs:label "Horse breed for work"@en ,
                                   "Razza da lavoro"@it .


###  http://www.semanticweb.org/annag/ontologies/2024/1/ontoHorses/RazzaDaSaltoOstacoli
ontoHorse:RazzaDaSaltoOstacoli rdf:type owl:Class ;
                               owl:equivalentClass [ rdf:type owl:Restriction ;
                                                     owl:onProperty :puòEssereImpiegataIn ;
                                                     owl:hasValue :SaltoAdOstacoli
                                                   ] ;
                               rdfs:subClassOf :RazzaSportiva ;
                               rdfs:comment "Horse breed that can be used in the equestrian sport discipline of jumping"@en ,
                                            "Razza di cavallo che può essere utilizzata nella disciplina di sport equestre del salto ostacoli"@it ;
                               rdfs:label "Jumping horse breed"@en ,
                                          "Razza da salto ostacoli"@it .


###  http://www.semanticweb.org/annag/ontologies/2024/1/ontoHorses/RazzaItaliana
ontoHorse:RazzaItaliana rdf:type owl:Class ;
                        owl:equivalentClass [ rdf:type owl:Restriction ;
                                              owl:onProperty :haNazionalità ;
                                              owl:hasValue ontoHorse:Italia
                                            ] ;
                        rdfs:subClassOf :RazzaEuropea ;
                        rdfs:comment "Horse breed originated from Italy"@en ,
                                     "Razza di cavallo originaria dell'Italia"@it ;
                        rdfs:label "Italian horse breed"@en ,
                                   "Razza italiana"@it .


###  http://www.semanticweb.org/annag/ontologies/2024/1/ontoHorses/RazzaSpagnola
ontoHorse:RazzaSpagnola rdf:type owl:Class ;
                        owl:equivalentClass [ rdf:type owl:Restriction ;
                                              owl:onProperty :haNazionalità ;
                                              owl:hasValue ontoHorse:Spagna
                                            ] ;
                        rdfs:subClassOf :RazzaEuropea ;
                        rdfs:comment "Horse breed originated from Spain"@en ,
                                     "Razza di cavallo originaria della Spagna"@it ;
                        rdfs:label "Razza spagnola"@it ,
                                   "Spanish horse breed"@en .


###  http://www.semanticweb.org/annag/ontologies/2024/1/ontoHorses/Sella
ontoHorse:Sella rdf:type owl:Class ;
                rdfs:subClassOf ontoHorse:Impiego ;
                rdfs:comment "Impiego del cavallo che ha attitudine alla sella per turismo o sport"@it ,
                             "Use of the horse that is suited to the saddle for tourism or sport"@en ;
                rdfs:label "Saddle"@en ,
                           "Sella"@it .


###  http://www.semanticweb.org/annag/ontologies/2024/1/ontoHorses/SportEquestre
ontoHorse:SportEquestre rdf:type owl:Class ;
                        rdfs:subClassOf ontoHorse:Sella ;
                        rdfs:comment "Insieme degli sport che prevedono la monta di un cavallo"@it ,
                                     "Set of sports that involve riding a horse"@en ;
                        rdfs:label "Equestrian sport"@en ,
                                   "Sport equestre"@it .


###  http://xmlns.com/foaf/0.1/person
<http://xmlns.com/foaf/0.1/person> rdf:type owl:Class .


#################################################################
#    Individuals
#################################################################

###  http://www.semanticweb.org/annag/ontologies/2024/1/ontoHorses#AltaScuola
:AltaScuola rdf:type owl:NamedIndividual ,
                     ontoHorse:SportEquestre .


###  http://www.semanticweb.org/annag/ontologies/2024/1/ontoHorses#AngloAraboFrancese
:AngloAraboFrancese rdf:type owl:NamedIndividual ,
                             :RazzeDolicomorfa ,
                             ontoHorse:RazzaCavallo ;
                    :haIndole :sangueCaldo ;
                    :puòEssereImpiegataIn :CrossCountry ,
                                          :Endurance ,
                                          :Eventing ,
                                          :SaltoAdOstacoli ;
                    ontoHorse:haRegioneDiOrigine ontoHorse:Normandia ;
                    ontoHorse:altezzaMediaAlGarrese_cm 161 ;
                    ontoHorse:haColoreMantello "baio" ,
                                               "grigio" ,
                                               "morello" ,
                                               "sauro" ;
                    ontoHorse:pesoMedio_Kg 475 ;
                    <http://schema.org/image> <https://upload.wikimedia.org/wikipedia/commons/thumb/8/87/Anglo-arabe-portrait02.JPG/220px-Anglo-arabe-portrait02.JPG> ;
                    rdfs:comment "L'anglo-arabo francese  è un cavallo sportivo di tipo dolicomorfo che ha caratteristiche intermedie tra il cavallo Arabo ed il Purosangue inglese."@it ,
                                 "The French Anglo-Arab is a dolichomorphic sport horse that has intermediate characteristics between the Arabian horse and the English Thoroughbred."@en ;
                    <http://www.w3.org/2004/02/skos/core#exactMatch> "https://www.wikidata.org/wiki/Q7029480"^^xsd:anyURI ;
                    <http://www.w3.org/2004/02/skos/core#prefLabel> "Anglo-Arabo francese"@it ,
                                                                    "French Anglo-Arab"@en .


###  http://www.semanticweb.org/annag/ontologies/2024/1/ontoHorses#Appenninico
:Appenninico rdf:type owl:NamedIndividual ,
                      :RazzeMesomorfa ,
                      ontoHorse:RazzaCavallo ;
             :haIndole :sangueFreddo ;
             :puòEssereImpiegataIn :Equiturismo ,
                                   :TrainoCarrozze ;
             ontoHorse:haRegioneDiOrigine :AppenninoTosco-Emiliano ;
             ontoHorse:altezzaMediaAlGarrese_cm 155 ;
             ontoHorse:haColoreMantello "baio" ,
                                        "sauro" ;
             ontoHorse:pesoMedio_Kg 575 ;
             <http://schema.org/image> <https://www.agraria.org/equini/appenninico.jpg> ;
             rdfs:comment "L'Appenninico è una razza di cavallo rustico e adattabile originario dall'Appenino tosco-emiliano."@it ,
                          "The Appenninico is a rustic and adaptable horse breed originating from the Tuscan-Emilian Apennines."@en ;
             <http://www.w3.org/2004/02/skos/core#exactMatch> "https://www.wikidata.org/wiki/Q3620866"^^xsd:anyURI ;
             <http://www.w3.org/2004/02/skos/core#prefLabel> "Appenninico"@en ,
                                                             "Appenninico"@it .


###  http://www.semanticweb.org/annag/ontologies/2024/1/ontoHorses#AppenninoTosco-Emiliano
:AppenninoTosco-Emiliano rdf:type owl:NamedIndividual ,
                                  ontoHorse:AreaGeografica ;
                         <http://www.ontologydesignpatterns.org/cp/owl/partof.owl#isPartOf> ontoHorse:Italia ;
                         rdfs:comment "It is a subdivision of the Apennine chain, in particular a stretch of the northern Apennines, which affects the border and adjacent areas of Tuscany and Emilia-Romagna"@en ,
                                      "Si tratta di una suddivisione della catena degli Appennini, in particolare un tratto dell'Appennino settentrionale, che interessa il confine e le aree adiacenti di Toscana e Emilia-Romagna"@it ;
                         rdfs:label "Appenino Tosco-Emiliano"@it ,
                                    "Tuscan-Emilian Apennines"@en .


###  http://www.semanticweb.org/annag/ontologies/2024/1/ontoHorses#Ard
:Ard rdf:type owl:NamedIndividual ,
              :RazzeDolicomorfa ,
              ontoHorse:RazzaCavallo ;
     :haIndole :sangueCaldo ;
     :puòEssereImpiegataIn :Dressage ,
                           :Equiturismo ;
     ontoHorse:haRegioneDiOrigine ontoHorse:Andalusia ;
     ontoHorse:altezzaMediaAlGarrese_cm 160 ;
     ontoHorse:haColoreMantello "baio" ,
                                "grigio" ,
                                "sauro" ;
     ontoHorse:pesoMedio_Kg 500 ;
     <http://schema.org/image> <https://www.ideegreen.it/wp-content/uploads/2020/10/cavallo-anglo-arabo-spagnolo.jpg> ;
     rdfs:comment "L'anglo-arabo spagnolo è un cavallo maneggevole, agile nei movimenti, progenitore dell'Andaluso"@it ,
                  "The Spanish Anglo-Arab is a manageable horse, agile in movement, progenitor of the Andalusian"@en ;
     rdfs:label "Anglo-Arabic Spanish"@en ;
     <http://www.w3.org/2004/02/skos/core#exactMatch> "https://www.wikidata.org/wiki/Q3617386"^^xsd:anyURI ;
     <http://www.w3.org/2004/02/skos/core#prefLabel> "Anglo-Arabo spagnolo"@it .


###  http://www.semanticweb.org/annag/ontologies/2024/1/ontoHorses#Ardenne
:Ardenne rdf:type owl:NamedIndividual ,
                  ontoHorse:AreaGeografica ;
         <http://www.ontologydesignpatterns.org/cp/owl/partof.owl#isPartOf> :Belgio ;
         rdfs:comment "Le Ardenne sono una regione collinare coperta da foreste, che si trova principalmente in Belgio e Lussemburgo e Francia"@it ,
                      "The Ardennes is a hilly, forested region, found mainly in Belgium and Luxembourg and France"@en ;
         rdfs:label "Ardenne"@it ,
                    "Ardennes"@en .


###  http://www.semanticweb.org/annag/ontologies/2024/1/ontoHorses#Ardennese
:Ardennese rdf:type owl:NamedIndividual ,
                    :RazzaBrachimorfa ,
                    ontoHorse:RazzaCavallo ;
           :haIndole :sangueFreddo ;
           :puòEssereImpiegataIn :TrainoCarrozze ;
           ontoHorse:haRegioneDiOrigine :Ardenne ;
           ontoHorse:altezzaMediaAlGarrese_cm 160 ;
           ontoHorse:haColoreMantello "baio" ,
                                      "isabella" ,
                                      "roano" ,
                                      "sauro" ,
                                      "ubero" ;
           ontoHorse:pesoMedio_Kg 800 ;
           <http://schema.org/image> <https://upload.wikimedia.org/wikipedia/commons/thumb/4/41/Ardenner.jpg/240px-Ardenner.jpg> ;
           rdfs:comment "L'Ardennese è  una razza di cavallo brachimorfo adatto al tiro pesante E' un antico cavallo noto ai tempi di Giulio Cesare"@it ,
                        "The Ardennese is a brachymorphic horse breed suitable for heavy shooting. It is an ancient horse known at the time of Julius Caesar"@en ;
           <http://www.w3.org/2004/02/skos/core#exactMatch> "https://www.wikidata.org/wiki/Q638976"^^xsd:anyURI ;
           <http://www.w3.org/2004/02/skos/core#prefLabel> "Ardennes Horse"@en ,
                                                           "Ardennese"@it .


###  http://www.semanticweb.org/annag/ontologies/2024/1/ontoHorses#BelgaDaTiro
:BelgaDaTiro rdf:type owl:NamedIndividual ,
                      :RazzaBrachimorfa ,
                      ontoHorse:RazzaCavallo ;
             :haIndole :sangueFreddo ;
             :puòEssereImpiegataIn :TiroAgricolo ,
                                   :TrainoCarrozze ;
             ontoHorse:haRegioneDiOrigine :Ardenne ;
             ontoHorse:altezzaMediaAlGarrese_cm 160 ;
             ontoHorse:haColoreMantello "baio" ,
                                        "roano" ,
                                        "sauro" ;
             ontoHorse:pesoMedio_Kg 750 ;
             <http://schema.org/image> <https://upload.wikimedia.org/wikipedia/commons/thumb/7/77/Belgisk_hest-2.jpg/240px-Belgisk_hest-2.jpg> ;
             rdfs:comment "Il Belga da tiro è una razza di cavallo originaria del Belgio: è un cavallo massiccio, uno dei più grandi, usato per il traino di oggetti sin dall'antichità"@it ,
                          "The Belgian draft horse is a breed of horse originating from Belgium: it is a massive horse, one of the largest, used for pulling objects since ancient times"@en ;
             rdfs:label "Belgian Draught"@en ;
             <http://www.w3.org/2004/02/skos/core#exactMatch> "https://www.wikidata.org/wiki/Q896476"^^xsd:anyURI ;
             <http://www.w3.org/2004/02/skos/core#prefLabel> "Belga Da Tiro"@it .


###  http://www.semanticweb.org/annag/ontologies/2024/1/ontoHorses#Belgio
:Belgio rdf:type owl:NamedIndividual ,
                 ontoHorse:AreaGeografica ;
        <http://schema.org/image> <https://upload.wikimedia.org/wikipedia/commons/thumb/6/65/Flag_of_Belgium.svg/188px-Flag_of_Belgium.svg.png> ;
        rdfs:comment "Belgium, officially the Kingdom of Belgium, is a country in Northwestern Europe."@en ,
                     "Il Belgio, ufficialmente Regno del Belgio, è uno Stato federale retto da una monarchia parlamentare  situato nell'Europa occidentale."@it ;
        rdfs:label "Belgio"@it ,
                   "Belgium"@en .


###  http://www.semanticweb.org/annag/ontologies/2024/1/ontoHorses#Boulonnais
:Boulonnais rdf:type owl:NamedIndividual ,
                     :RazzaBrachimorfa ,
                     ontoHorse:RazzaCavallo ;
            :haIndole :sangueFreddo ;
            :puòEssereImpiegataIn :TiroAgricolo ;
            ontoHorse:haRegioneDiOrigine :RegioneBoullonnais ;
            ontoHorse:altezzaMediaAlGarrese_cm 163 ;
            ontoHorse:haColoreMantello "baio" ,
                                       "grigio" ,
                                       "morello" ,
                                       "roano" ,
                                       "sauro" ;
            ontoHorse:pesoMedio_Kg 800 ;
            <http://schema.org/image> <https://upload.wikimedia.org/wikipedia/commons/thumb/4/47/T%C3%AAte_jument_boulonnaise_2.jpg/260px-T%C3%AAte_jument_boulonnaise_2.jpg> ;
            rdfs:comment "The Boulonnais is a breed of draft horse, nicknamed \"thoroughbred line horse\" or \"colossus of white marble\", native to the Boulogne-sur-Mer region of northern France."@en ,
                         "Il Boulonnais è una razza di cavallo da tiro, soprannominato \"cavallo purosangue line\" o \"colosso di marmo bianco\", originario della regione di Boulogne-sur-Mer nel nord della Francia." ;
            <http://www.w3.org/2004/02/skos/core#exactMatch> ""^^xsd:anyURI ;
            <http://www.w3.org/2004/02/skos/core#prefLabel> "Boulonnais"@en ,
                                                            "Boulonnais"@it .


###  http://www.semanticweb.org/annag/ontologies/2024/1/ontoHorses#Bretagna
:Bretagna rdf:type owl:NamedIndividual ,
                   ontoHorse:AreaGeografica ;
          <http://www.ontologydesignpatterns.org/cp/owl/partof.owl#isPartOf> ontoHorse:Francia ;
          <http://schema.org/image> <https://upload.wikimedia.org/wikipedia/commons/thumb/4/4b/Brittany_in_France_2016.svg/260px-Brittany_in_France_2016.svg.png> ;
          rdfs:comment "Brittany is a historical and administrative region of France that forms a vast promontory towards the English Channel and the Atlantic Ocean"@en ,
                       "La Bretagna  è una regione storica e amministrativa della Francia che forma un vasto promontorio verso la Manica e l'Oceano Atlantico"@it ;
          rdfs:label "Bretagna"@it ,
                     "Brittany"@en .


###  http://www.semanticweb.org/annag/ontologies/2024/1/ontoHorses#Bretone
:Bretone rdf:type owl:NamedIndividual ,
                  :RazzaBrachimorfa ,
                  ontoHorse:RazzaCavallo ;
         :puòEssereImpiegataIn :TiroAgricolo ,
                               :TrainoCarrozze ;
         ontoHorse:haRegioneDiOrigine :Bretagna ;
         ontoHorse:altezzaMediaAlGarrese_cm 155 ;
         ontoHorse:haColoreMantello "sauro" ;
         ontoHorse:pesoMedio_Kg 800 ;
         <http://schema.org/image> <https://upload.wikimedia.org/wikipedia/commons/thumb/f/fa/Breton_%C3%A9talon_SDA2012.JPG/220px-Breton_%C3%A9talon_SDA2012.JPG> ;
         rdfs:comment "Il  Bretone è una razza di cavallo da tiro pesante, originario della Francia, un tempo utilizzato specialmente nei lavori agricoli"@it ,
                      "The Breton is a breed of heavy draft horse, originally from France, once used especially in agricultural work"@en ;
         <http://www.w3.org/2004/02/skos/core#exactMatch> "https://www.wikidata.org/wiki/Q514553"^^xsd:anyURI ;
         <http://www.w3.org/2004/02/skos/core#prefLabel> "Bretone"@it ,
                                                         "Breton Horse" .


###  http://www.semanticweb.org/annag/ontologies/2024/1/ontoHorses#CastoneFrancese
:CastoneFrancese rdf:type owl:NamedIndividual ,
                          ontoHorse:Cavallo ;
                 <http://www.ontologydesignpatterns.org/cp/owl/price.owl#hasPrice> <http://www.semanticweb.org/annag/ontologies/2024/1/ontoHorses#18000Euro> ;
                 ontoHorse:gareggiaNelleCategorieDiSalto ontoHorse:C110 ,
                                                         ontoHorse:C125 ;
                 ontoHorse:haRazza :SellaFrancese ;
                 ontoHorse:vieneUtilizzatoPer :SaltoAdOstacoli ;
                 :annoDiNascita "2016"^^xsd:nonNegativeInteger ;
                 :contattoProprietario "345-234599" ;
                 :haProprietario "Gianluca Camoletto" ;
                 :nomeCavallo "Elton" ;
                 :provinciaDiScuderizzazione "Alessandria" ;
                 :regioneDiScuderizzazione "Piemonte" ;
                 ontoHorse:altezzaAlGarrese_cm "167"^^xsd:nonNegativeInteger ;
                 ontoHorse:età "8"^^xsd:nonNegativeInteger ;
                 ontoHorse:haSesso "castrone" ;
                 rdfs:comment "Esemplare di castrone francese in vendita"@it ,
                              "French gelding horse for sale"@en ;
                 rdfs:label "Castrone Francese"@it ,
                            "French gelding horse"@en .


###  http://www.semanticweb.org/annag/ontologies/2024/1/ontoHorses#CastroneAngloAraboFrancese
:CastroneAngloAraboFrancese rdf:type owl:NamedIndividual ,
                                     ontoHorse:Cavallo ;
                            <http://www.ontologydesignpatterns.org/cp/owl/price.owl#hasPrice> <http://www.semanticweb.org/annag/ontologies/2024/1/ontoHorses#15000Euro> ;
                            ontoHorse:haRazza :AngloAraboFrancese ;
                            ontoHorse:vieneUtilizzatoPer :CrossCountry ;
                            ontoHorse:èAdattoPer ontoHorse:CavaliereIntermedio ;
                            :annoDiNascita "2009"^^xsd:nonNegativeInteger ;
                            :contattoProprietario "345-456734" ;
                            :haProprietario "Giorgia Neri" ;
                            :nomeCavallo "Filè" ;
                            :provinciaDiScuderizzazione "Bergamo" ;
                            :regioneDiScuderizzazione "Lombardia" ;
                            ontoHorse:altezzaAlGarrese_cm "158"^^xsd:nonNegativeInteger ;
                            ontoHorse:età "15"^^xsd:nonNegativeInteger ;
                            ontoHorse:haSesso "castrone" ;
                            rdfs:comment "Esemplare di cavallo castrone anglo-arabo francese in vendita"@it ,
                                         "French Anglo-Arab gelding horse for sale"@en ;
                            rdfs:label "Castrone anglo-arabo francese"@it ,
                                       "French Anglo-Arabic gelding"@en .


###  http://www.semanticweb.org/annag/ontologies/2024/1/ontoHorses#CavalloDelloJutland
:CavalloDelloJutland rdf:type owl:NamedIndividual ,
                              :RazzaBrachimorfa ,
                              ontoHorse:RazzaCavallo ;
                     :haIndole :sangueFreddo ;
                     :puòEssereImpiegataIn :TiroAgricolo ;
                     ontoHorse:haRegioneDiOrigine :Jutland ;
                     ontoHorse:altezzaMediaAlGarrese_cm 160 ;
                     ontoHorse:haColoreMantello "baio" ,
                                                "grigio" ,
                                                "roano" ,
                                                "sauro" ;
                     ontoHorse:pesoMedio_Kg 725 ;
                     <http://schema.org/image> <https://upload.wikimedia.org/wikipedia/commons/thumb/4/49/Jydske_heste_vorup_enge.jpg/240px-Jydske_heste_vorup_enge.jpg> ;
                     rdfs:comment "Il cavallo dello Jutland è un cavallo da tiro pesante, di razza danese, il cui nome deriva dalla penisola dello Jutland, in cui viene allevato dal XII secolo"@it ,
                                  "The Jutland horse is a heavy draft horse, of Danish breed, whose name derives from the Jutland peninsula, where it has been bred since the 12th century"@en ;
                     <http://www.w3.org/2004/02/skos/core#exactMatch> "https://www.wikidata.org/wiki/Q1684175"^^xsd:anyURI ;
                     <http://www.w3.org/2004/02/skos/core#prefLabel> "Cavallo dello Jutland"@it ,
                                                                     "Jutland Horse"@en .


###  http://www.semanticweb.org/annag/ontologies/2024/1/ontoHorses#Clydesdale
:Clydesdale rdf:type owl:NamedIndividual ,
                     :RazzaBrachimorfa ,
                     ontoHorse:RazzaCavallo ;
            :haIndole :sangueFreddo ;
            :puòEssereImpiegataIn :TiroAgricolo ;
            ontoHorse:haRegioneDiOrigine :Scozia ;
            ontoHorse:altezzaMediaAlGarrese_cm 168 ;
            ontoHorse:haColoreMantello "baio" ,
                                       "grigio" ,
                                       "morello" ,
                                       "roano" ,
                                       "sauro" ;
            ontoHorse:pesoMedio_Kg 850 ;
            <http://schema.org/image> <https://upload.wikimedia.org/wikipedia/commons/thumb/0/07/I_feel_pretty._Oh_so_pretty..jpg/220px-I_feel_pretty._Oh_so_pretty..jpg> ;
            rdfs:comment "Il Clydesdale è una razza di cavalli da tiro pesante lentoil cui nome deriva dalle fattorie presenti nella contea di Clydesdale, situata in Scozia."@it ,
                         "The Clydesdale is a breed of slow heavy draft horse whose name derives from the farms present in the county of Clydesdale, located in Scotland"@en ;
            <http://www.w3.org/2004/02/skos/core#exactMatch> "https://www.wikidata.org/wiki/Q844058"^^xsd:anyURI ;
            <http://www.w3.org/2004/02/skos/core#prefLabel> "Clydesdale"@it ,
                                                            "Clydesdale Horse"@en .


###  http://www.semanticweb.org/annag/ontologies/2024/1/ontoHorses#CrossCountry
:CrossCountry rdf:type owl:NamedIndividual ,
                       ontoHorse:SportEquestre .


###  http://www.semanticweb.org/annag/ontologies/2024/1/ontoHorses#Danimarca
:Danimarca rdf:type owl:NamedIndividual ,
                    ontoHorse:AreaGeografica ;
           <http://schema.org/image> <https://upload.wikimedia.org/wikipedia/commons/thumb/9/9c/Flag_of_Denmark.svg/1280px-Flag_of_Denmark.svg.png> ;
           rdfs:comment "Denmark, officially the Kingdom of Denmark, is a member state of the European Union and the smallest and southernmost state in Scandinavia."@en ,
                        "La Danimarca, ufficialmente Regno di Danimarca , è uno Stato membro dell'Unione europea e lo Stato più piccolo e più meridionale della Scandinavia."@it ;
           rdfs:label "Danimarca"@it ,
                      "Denmark"@en .


###  http://www.semanticweb.org/annag/ontologies/2024/1/ontoHorses#Dressage
:Dressage rdf:type owl:NamedIndividual ,
                   ontoHorse:SportEquestre .


###  http://www.semanticweb.org/annag/ontologies/2024/1/ontoHorses#Endurance
:Endurance rdf:type owl:NamedIndividual ,
                    ontoHorse:SportEquestre .


###  http://www.semanticweb.org/annag/ontologies/2024/1/ontoHorses#Equiturismo
:Equiturismo rdf:type owl:NamedIndividual ,
                      :Equiturismo .


###  http://www.semanticweb.org/annag/ontologies/2024/1/ontoHorses#Eventing
:Eventing rdf:type owl:NamedIndividual ,
                   ontoHorse:SportEquestre .


###  http://www.semanticweb.org/annag/ontologies/2024/1/ontoHorses#FemminaBretone
:FemminaBretone rdf:type owl:NamedIndividual ,
                         ontoHorse:Cavallo ;
                <http://www.ontologydesignpatterns.org/cp/owl/price.owl#hasPrice> <http://www.semanticweb.org/annag/ontologies/2024/1/ontoHorses#2500Euro> ;
                ontoHorse:haRazza :Bretone ;
                ontoHorse:vieneUtilizzatoPer :TiroAgricolo ;
                ontoHorse:èAdattoPer ontoHorse:CavalierePrincipiante ;
                :annoDiNascita "2006"^^xsd:nonNegativeInteger ;
                :contattoProprietario "345-2343222" ;
                :haProprietario "Salvatore Bianchi" ;
                :nomeCavallo "Carmen" ;
                :provinciaDiScuderizzazione "Potenza" ;
                :regioneDiScuderizzazione "Basilicata" ;
                ontoHorse:altezzaAlGarrese_cm "150"^^xsd:nonNegativeInteger ;
                ontoHorse:età "18"^^xsd:nonNegativeInteger ;
                ontoHorse:haSesso "femmina" ;
                rdfs:comment "Esemplare di femmina bretone in vendita"@it ,
                             "Female breton horse for sale"@en ;
                rdfs:label "Female breton horse"@en ,
                           "Femmina bretone"@it .


###  http://www.semanticweb.org/annag/ontologies/2024/1/ontoHorses#FemminaMaremmano
:FemminaMaremmano rdf:type owl:NamedIndividual ,
                           ontoHorse:Cavallo ;
                  <http://www.ontologydesignpatterns.org/cp/owl/price.owl#hasPrice> <http://www.semanticweb.org/annag/ontologies/2024/1/ontoHorses#5000Euro> ;
                  ontoHorse:haRazza :Maremmano ;
                  ontoHorse:vieneUtilizzatoPer :Equiturismo ,
                                               :TrainoCarrozze ;
                  ontoHorse:èAdattoPer ontoHorse:CavalierePrincipiante ;
                  :annoDiNascita "2004"^^xsd:nonNegativeInteger ;
                  :contattoProprietario "321-3334567" ;
                  :haProprietario "Giovanni Forte" ;
                  :nomeCavallo "Penelope" ;
                  :provinciaDiScuderizzazione "Grosseto" ;
                  :regioneDiScuderizzazione "Toscana" ;
                  ontoHorse:altezzaAlGarrese_cm "162"^^xsd:nonNegativeInteger ;
                  ontoHorse:età "20"^^xsd:nonNegativeInteger ;
                  ontoHorse:haSesso "femmina" ;
                  rdfs:comment "Esemplare di femmina maremmano in vendita"@it ,
                               "Female maremmano horse for sale"@en ;
                  rdfs:label "Female maremmano horse"@en ,
                             "Femmina maremmano"@it .


###  http://www.semanticweb.org/annag/ontologies/2024/1/ontoHorses#FemminaMurgese
:FemminaMurgese rdf:type owl:NamedIndividual ,
                         ontoHorse:Cavallo ;
                <http://www.ontologydesignpatterns.org/cp/owl/price.owl#hasPrice> <http://www.semanticweb.org/annag/ontologies/2024/1/ontoHorses#4800Euro> ;
                ontoHorse:gareggiaNelleCategorieDiSalto ontoHorse:C80 ;
                ontoHorse:haRazza :Murgese ;
                ontoHorse:vieneUtilizzatoPer :Dressage ,
                                             :Equiturismo ,
                                             :SaltoAdOstacoli ;
                :annoDiNascita "2020"^^xsd:nonNegativeInteger ;
                :contattoProprietario "345-678956" ;
                :haProprietario "Paolo Grassi" ;
                :nomeCavallo "Queen" ;
                :provinciaDiScuderizzazione "Taranto" ;
                :regioneDiScuderizzazione "Puglia" ;
                ontoHorse:altezzaAlGarrese_cm "158"^^xsd:nonNegativeInteger ;
                ontoHorse:categorieDiDressage "E" ;
                ontoHorse:età "4"^^xsd:nonNegativeInteger ;
                ontoHorse:haSesso "femmina" ;
                rdfs:comment "Esemplare di femmina murgese in vendita"@it ,
                             "Female murgese horse for sale"@en ;
                rdfs:label "Female murgese"@en ,
                           "Femmina murgese"@it .


###  http://www.semanticweb.org/annag/ontologies/2024/1/ontoHorses#Frisia
:Frisia rdf:type owl:NamedIndividual ,
                 ontoHorse:AreaGeografica ;
        <http://www.ontologydesignpatterns.org/cp/owl/partof.owl#isPartOf> :PaesiBassi ;
        rdfs:comment "Friesland is a province of the Netherlands"@en ,
                     "La Frisia è una provincia dei Paesi Bassi"@it ;
        rdfs:label "Friesland"@en ,
                   "Frisia"@it .


###  http://www.semanticweb.org/annag/ontologies/2024/1/ontoHorses#Frisone
:Frisone rdf:type owl:NamedIndividual ,
                  :RazzaMesoBrachimorfa ,
                  ontoHorse:RazzaCavallo ;
         :haIndole :sangueFreddo ;
         :puòEssereImpiegataIn :Dressage ,
                               :TrainoCarrozze ;
         ontoHorse:haRegioneDiOrigine :Frisia ;
         ontoHorse:altezzaMediaAlGarrese_cm 160 ;
         ontoHorse:haColoreMantello "morello" ;
         ontoHorse:pesoMedio_Kg 525 ;
         <http://schema.org/image> <https://upload.wikimedia.org/wikipedia/commons/thumb/7/7c/Friese.jpg/220px-Friese.jpg> ;
         rdfs:comment "Il Frisone occidentale è originario della Frisia ed è una razza di cavallo robusto, possente e infaticabile, utilizzato in passato, soprattutto durante il Medioevo, come cavallo da guerra. Oggi è particolarmente apprezzato nel dressage e negli attacchi."@it ,
                      "The West Friesian originates from Friesland and is a robust, powerful and tireless breed of horse, used in the past, especially during the Middle Ages, as a war horse. Today it is particularly appreciated in dressage and driving."@en ;
         <http://www.w3.org/2004/02/skos/core#exactMatch> "https://www.wikidata.org/wiki/Q388952" ;
         <http://www.w3.org/2004/02/skos/core#prefLabel> "Friesian horse"@en ,
                                                         "Frisone"@it .


###  http://www.semanticweb.org/annag/ontologies/2024/1/ontoHorses#Hannover
:Hannover rdf:type owl:NamedIndividual ,
                   :RazzeMesomorfa ,
                   ontoHorse:RazzaCavallo ;
          :haIndole :sangueCaldo ;
          :puòEssereImpiegataIn :Dressage ,
                                :SaltoAdOstacoli ;
          ontoHorse:haRegioneDiOrigine :RegioneHannover ;
          ontoHorse:altezzaMediaAlGarrese_cm 168 ;
          ontoHorse:haColoreMantello "baio" ,
                                     "grigio" ,
                                     "morello" ,
                                     "sauro" ;
          ontoHorse:pesoMedio_Kg 575 ;
          <http://schema.org/image> <https://upload.wikimedia.org/wikipedia/commons/thumb/c/cc/RCMP_Farm_Hannoverian2.jpg/240px-RCMP_Farm_Hannoverian2.jpg> ;
          rdfs:comment "L' Hannover è una razza di cavallo a sangue caldo, originaria della Germania, più precisamente della regione di Hannover"@it ,
                       "The Hanoverian is a breed of warm-blooded horse, originating from Germany, more precisely from the Hanover region"@en ;
          <http://www.w3.org/2004/02/skos/core#exactMatch> "https://www.wikidata.org/wiki/Q1501738"^^xsd:anyURI ;
          <http://www.w3.org/2004/02/skos/core#prefLabel> "Hannover"@it ,
                                                          "Hanoverian horse"@en .


###  http://www.semanticweb.org/annag/ontologies/2024/1/ontoHorses#Holstein
:Holstein rdf:type owl:NamedIndividual ,
                   :RazzeMesomorfa ,
                   ontoHorse:RazzaCavallo ;
          :haIndole :sangueMisto ;
          :puòEssereImpiegataIn :Dressage ,
                                :SaltoAdOstacoli ;
          ontoHorse:haRegioneDiOrigine :Schleswig-Holstein ;
          ontoHorse:altezzaMediaAlGarrese_cm 168 ;
          ontoHorse:haColoreMantello "baio" ,
                                     "grigio" ,
                                     "morello" ,
                                     "sauro" ;
          ontoHorse:pesoMedio_Kg 575 ;
          <http://schema.org/image> <https://upload.wikimedia.org/wikipedia/commons/thumb/e/ea/Holstein_cavallo.jpg/192px-Holstein_cavallo.jpg> ;
          rdfs:comment "L'Holstein è una razza che nasce dall'idea di incrociare il cavallo agricolo tedesco nativo della regione Schleswing-Holstein con i purosangue per creare all'inizio un cavallo da tiro leggero e successivamente un cavallo da sella adatto alle attività sportive"@it ,
                       "The Holstein is a breed that was born from the idea of crossing the German agricultural horse native to the Schleswing-Holstein region with thoroughbreds to initially create a light draft horse and subsequently a saddle horse suitable for sporting activities"@en ;
          <http://www.w3.org/2004/02/skos/core#exactMatch> "https://www.wikidata.org/wiki/Q571149"^^xsd:anyURI ;
          <http://www.w3.org/2004/02/skos/core#prefLabel> "Holstein"@it ,
                                                          "Holsteiner"@en .


###  http://www.semanticweb.org/annag/ontologies/2024/1/ontoHorses#IrishSportHorse
:IrishSportHorse rdf:type owl:NamedIndividual ,
                          :RazzeMesomorfa ,
                          ontoHorse:RazzaCavallo ;
                 :haIndole :sangueCaldo ;
                 :haNazionalità ontoHorse:Irlanda ;
                 :puòEssereImpiegataIn :Dressage ,
                                       :Eventing ,
                                       :SaltoAdOstacoli ;
                 ontoHorse:altezzaMediaAlGarrese_cm 163 ;
                 ontoHorse:haColoreMantello "baio" ,
                                            "crema" ,
                                            "grigio" ,
                                            "morello" ,
                                            "sauro" ;
                 ontoHorse:pesoMedio_Kg 600 ;
                 <http://schema.org/image> <https://upload.wikimedia.org/wikipedia/commons/thumb/e/ea/Irish_Sport_Horse_foal_and_mare.jpg/220px-Irish_Sport_Horse_foal_and_mare.jpg> ;
                 rdfs:comment "L'Irish Sport Horse (ISH), o Irish Hunter, è una razza irlandese di cavalli sportivi a sangue caldo, utilizzata principalmente per dressage, completo e salto ostacoli"@it ,
                              "The Irish Sport Horse (ISH), or Irish Hunter, is an Irish breed of warmblood sport horse, used primarily for dressage, eventing, and show jumping"@en ;
                 <http://www.w3.org/2004/02/skos/core#exactMatch> "https://www.wikidata.org/wiki/Q1665430"^^xsd:anyURI ;
                 <http://www.w3.org/2004/02/skos/core#prefLabel> "Irish Sport Horse"@en ,
                                                                 "Irish Sport Horse"@it .


###  http://www.semanticweb.org/annag/ontologies/2024/1/ontoHorses#Jutland
:Jutland rdf:type owl:NamedIndividual ,
                  ontoHorse:AreaGeografica ;
         <http://www.ontologydesignpatterns.org/cp/owl/partof.owl#isPartOf> :Danimarca ;
         rdfs:comment "Jutland is a peninsula in northern Europe divided between Germany, to the south, and Denmark, of which it constitutes the peninsular part."@en ,
                      "Lo Jutland è una penisola del nord Europa divisa tra Germania, a sud, e Danimarca, di cui costituisce la parte peninsulare."@it ;
         rdfs:label "Jutland"@en ,
                    "Jutland"@it .


###  http://www.semanticweb.org/annag/ontologies/2024/1/ontoHorses#Lipizzano
:Lipizzano rdf:type owl:NamedIndividual ,
                    :RazzaMesoDolicomorfa ,
                    ontoHorse:RazzaCavallo ;
           :haIndole :sangueMisto ;
           :puòEssereImpiegataIn :AltaScuola ,
                                 :Dressage ,
                                 :TiroAgricolo ;
           ontoHorse:haRegioneDiOrigine :TrentinoAltoAdige ;
           ontoHorse:altezzaMediaAlGarrese_cm 155 ;
           ontoHorse:haColoreMantello "baio" ,
                                      "grigio" ,
                                      "morello" ,
                                      "roano" ;
           ontoHorse:pesoMedio_Kg 520 ;
           <http://schema.org/image> <https://upload.wikimedia.org/wikipedia/commons/thumb/c/cb/Favory_Pallavicina.jpg/330px-Favory_Pallavicina.jpg> ;
           rdfs:comment "Il Lipizzano è una razza di cavallo che deve il suo nome alla città di Lipizza e originariamente  fu usato per trainare le carrozze dei monarchi e nell'esercito"@it ,
                        "The Lipizzan is a breed of horse that owes its name to the city of Lipica and was originally used to pull the carriages of monarchs and in the army"@en ;
           <http://www.w3.org/2004/02/skos/core#exactMatch> "https://www.wikidata.org/wiki/Q217671"^^xsd:anyURI ;
           <http://www.w3.org/2004/02/skos/core#prefLabel> "Lipizzan"@en ,
                                                           "Lipizzano"@it .


###  http://www.semanticweb.org/annag/ontologies/2024/1/ontoHorses#Lusitano
:Lusitano rdf:type owl:NamedIndividual ,
                   :RazzaMesoDolicomorfa ,
                   ontoHorse:RazzaCavallo ;
          :haIndole :sangueCaldo ;
          :haNazionalità :Portogallo ;
          :puòEssereImpiegataIn :AltaScuola ,
                                :Dressage ;
          ontoHorse:altezzaMediaAlGarrese_cm 157 ;
          ontoHorse:haColoreMantello "baio" ,
                                     "crema" ,
                                     "grigio" ,
                                     "isabella" ,
                                     "palomino" ,
                                     "sauro" ;
          ontoHorse:pesoMedio_Kg 525 ;
          <http://schema.org/image> <https://upload.wikimedia.org/wikipedia/commons/thumb/0/00/Beja_lusitano.JPG/220px-Beja_lusitano.JPG> ;
          rdfs:comment "Il Lusitano deriva il suo nome dalla Lusitania, attuale Portogallo ed è il cavallo simbolo di questa nazione. Di origine antica, il Lusitano originariamente era allevato per essere utilizzato in guerra e nelle corride"@it ,
                       "The Lusitano derives its name from Lusitania, now Portugal and is the symbolic horse of this nation. Of ancient origin, the Lusitano was originally bred for use in war and bullfights"@en ;
          <http://www.w3.org/2004/02/skos/core#exactMatch> "https://www.wikidata.org/wiki/Q937595"^^xsd:anyURI ;
          <http://www.w3.org/2004/02/skos/core#prefLabel> "Lusitano"@en ,
                                                          "Lusitano"@it .


###  http://www.semanticweb.org/annag/ontologies/2024/1/ontoHorses#Maremma
:Maremma rdf:type owl:NamedIndividual ,
                  ontoHorse:AreaGeografica ;
         <http://www.ontologydesignpatterns.org/cp/owl/partof.owl#isPartOf> ontoHorse:Italia ;
         rdfs:comment "La Maremma  è una vasta regione geografica compresa fra Toscana e Lazio, di circa 5000 km², che si affaccia sul Mar Tirreno e sul Mar Ligure."@it ,
                      "Maremma is a vast geographical region between Tuscany and Lazio, of approximately 5000 km², which overlooks the Tyrrhenian Sea and the Ligurian Sea."@en ;
         rdfs:label "Maremma"@en ,
                    "Maremma"@it .


###  http://www.semanticweb.org/annag/ontologies/2024/1/ontoHorses#Maremmano
:Maremmano rdf:type owl:NamedIndividual ,
                    :RazzaMesoDolicomorfa ,
                    ontoHorse:RazzaCavallo ;
           :haIndole :sangueFreddo ;
           :puòEssereImpiegataIn :Equiturismo ;
           ontoHorse:haRegioneDiOrigine :Maremma ;
           ontoHorse:altezzaMediaAlGarrese_cm 165 ;
           ontoHorse:haColoreMantello "baio" ,
                                      "morello" ;
           ontoHorse:pesoMedio_Kg 500 ;
           <http://schema.org/image> <https://www.politicheagricole.it/flex/images/d/7/5/D.1bb62598304e4dec51c6/maremmano_large.jpg> ;
           rdfs:comment "Il cavallo di razza Maremmano è una razza equina italiana i cui primi esemplari sembra risalgano ai tempi degli Etruschi"@it ,
                        "The Maremmano Horse is an Italian horse breed whose first specimens seem to date back to Etruscan times"@en ;
           <http://www.w3.org/2004/02/skos/core#exactMatch> "https://www.wikidata.org/wiki/Q1894708"^^xsd:anyURI ;
           <http://www.w3.org/2004/02/skos/core#prefLabel> "Maremmano"@en ,
                                                           "Maremmano"@it .


###  http://www.semanticweb.org/annag/ontologies/2024/1/ontoHorses#MaschioOlandese
:MaschioOlandese rdf:type owl:NamedIndividual ,
                          ontoHorse:Cavallo ;
                 <http://www.ontologydesignpatterns.org/cp/owl/price.owl#hasPrice> <http://www.semanticweb.org/annag/ontologies/2024/1/ontoHorses#35000Euro> ;
                 ontoHorse:gareggiaNelleCategorieDiSalto ontoHorse:C135 ;
                 ontoHorse:haRazza :OlandeseASangueCaldo ;
                 ontoHorse:vieneUtilizzatoPer :SaltoAdOstacoli ;
                 :annoDiNascita "2012"^^xsd:nonNegativeInteger ;
                 :haProprietario "Federico Pellegrini" ;
                 :nomeCavallo "Mufasa" ;
                 :provinciaDiScuderizzazione "Roma" ;
                 :regioneDiScuderizzazione "Lazio" ;
                 ontoHorse:altezzaAlGarrese_cm "170"^^xsd:nonNegativeInteger ;
                 ontoHorse:altezzaMaxDiSalto_cm "135"^^xsd:nonNegativeInteger ;
                 ontoHorse:età "12"^^xsd:nonNegativeInteger ;
                 ontoHorse:haSesso "maschio" ;
                 rdfs:comment "Dutch male horse for sale"@en ,
                              "Esemplare di cavallo maschio olandese in vendita"@it ;
                 rdfs:label "Dutch male"@en ,
                            "Maschio olandese"@it .


###  http://www.semanticweb.org/annag/ontologies/2024/1/ontoHorses#MaschioPuroSangueInglese
:MaschioPuroSangueInglese rdf:type owl:NamedIndividual ,
                                   ontoHorse:Cavallo ;
                          <http://www.ontologydesignpatterns.org/cp/owl/price.owl#hasPrice> <http://www.semanticweb.org/annag/ontologies/2024/1/ontoHorses#20000Euro> ;
                          ontoHorse:haRazza :PuroSangueInglese ;
                          ontoHorse:vieneUtilizzatoPer :Endurance ;
                          ontoHorse:èAdattoPer ontoHorse:CavaliereMoltoEsperto ;
                          :annoDiNascita "2014"^^xsd:nonNegativeInteger ;
                          :contattoProprietario "325-435677" ;
                          :haProprietario "Francesco Nisi" ;
                          :nomeCavallo "Fulmine" ;
                          :provinciaDiScuderizzazione "Milano" ;
                          :regioneDiScuderizzazione "Lombardia" ;
                          ontoHorse:altezzaAlGarrese_cm "161"^^xsd:nonNegativeInteger ;
                          ontoHorse:età "10"^^xsd:nonNegativeInteger ;
                          ontoHorse:haSesso "maschio" ;
                          rdfs:comment "Esemplare di purosangue inglese in vendita"@it ,
                                       "Thoroughbred male horse for sale"@en ;
                          rdfs:label "Maschio purosangue inglese"@it ,
                                     "Thoroughbred male"@en .


###  http://www.semanticweb.org/annag/ontologies/2024/1/ontoHorses#MaschioTedesco
:MaschioTedesco rdf:type owl:NamedIndividual ,
                         ontoHorse:Cavallo ;
                <http://www.ontologydesignpatterns.org/cp/owl/price.owl#hasPrice> <http://www.semanticweb.org/annag/ontologies/2024/1/ontoHorses#15000Euro> ;
                ontoHorse:gareggiaNelleCategorieDiSalto ontoHorse:C115 ;
                ontoHorse:haRazza :Holstein ;
                ontoHorse:vieneUtilizzatoPer :CrossCountry ,
                                             :SaltoAdOstacoli ;
                :annoDiNascita "2008"^^xsd:nonNegativeInteger ;
                :contattoProprietario "324-234565" ;
                :haProprietario "Federico Neri" ;
                :nomeCavallo "Duenas" ;
                :provinciaDiScuderizzazione "Perugia" ;
                :regioneDiScuderizzazione "Umbria" ;
                ontoHorse:altezzaAlGarrese_cm "168"^^xsd:nonNegativeInteger ;
                ontoHorse:altezzaMaxDiSalto_cm "120"^^xsd:nonNegativeInteger ;
                ontoHorse:età "16"^^xsd:nonNegativeInteger ;
                ontoHorse:haSesso "maschio" ;
                rdfs:comment "Esemplare di maschio tedesco in vendita"@it ,
                             "German male horse for sale"@en ;
                rdfs:label "German male"@en ,
                           "Maschio tedesco"@it .


###  http://www.semanticweb.org/annag/ontologies/2024/1/ontoHorses#Murgese
:Murgese rdf:type owl:NamedIndividual ,
                  :RazzeMesomorfa ,
                  ontoHorse:RazzaCavallo ;
         :haIndole :sangueCaldo ;
         :puòEssereImpiegataIn :Dressage ,
                               :TrainoCarrozze ;
         ontoHorse:haRegioneDiOrigine ontoHorse:Murge ;
         ontoHorse:altezzaMediaAlGarrese_cm 162 ;
         ontoHorse:haColoreMantello "morello" ;
         ontoHorse:pesoMedio_Kg 500 ;
         <http://schema.org/image> <https://www.animali.net/wp-content/uploads/2015/09/Il_Murgese.jpg> ;
         rdfs:comment "Il Murgese è una razza equina italiana che è originaria delle Murge, una regione geografica della Puglia e Basilicata, da cui ne deriva il nome"@it ,
                      "The Murgese is an Italian horse breed that originates from the Murge, a geographical region of Puglia and Basilicata, from which its name derives"@en ;
         <http://www.w3.org/2004/02/skos/core#exactMatch> "https://www.wikidata.org/wiki/Q1953691"^^xsd:anyURI ;
         <http://www.w3.org/2004/02/skos/core#prefLabel> "Murgese"@en ,
                                                         "Murgese"@it .


###  http://www.semanticweb.org/annag/ontologies/2024/1/ontoHorses#OlandeseASangueCaldo
:OlandeseASangueCaldo rdf:type owl:NamedIndividual ,
                               :RazzaMesoDolicomorfa ,
                               ontoHorse:RazzaCavallo ;
                      :haIndole :sangueCaldo ;
                      :haNazionalità :PaesiBassi ;
                      :puòEssereImpiegataIn :Dressage ,
                                            :SaltoAdOstacoli ;
                      ontoHorse:altezzaMediaAlGarrese_cm 165 ;
                      ontoHorse:haColoreMantello "baio" ,
                                                 "grigio" ,
                                                 "morello" ,
                                                 "pezzato" ,
                                                 "sauro" ;
                      ontoHorse:pesoMedio_Kg 550 ;
                      <http://schema.org/image> <https://upload.wikimedia.org/wikipedia/commons/thumb/e/e3/Michael_Whitaker_and_Tackeray%2C_CSIO_Rome_2009.jpg/240px-Michael_Whitaker_and_Tackeray%2C_CSIO_Rome_2009.jpg> ;
                      rdfs:comment "L'Olandese a sangue caldo è una razza equina moderna di origini olandesi utilizzata per sport sebbene originariamente nasca come cavallo da tiro"@it ,
                                   "The Dutch Warmblood is a modern equine breed of Dutch origins used for sport although it was originally born as a draft horse"@en ;
                      <http://www.w3.org/2004/02/skos/core#exactMatch> "https://www.wikidata.org/wiki/Q1468737"^^xsd:anyURI ;
                      <http://www.w3.org/2004/02/skos/core#prefLabel> "Dutch Warmblood"@en ,
                                                                      "Olandese a sangue caldo"@it .


###  http://www.semanticweb.org/annag/ontologies/2024/1/ontoHorses#Oldemburghese
:Oldemburghese rdf:type owl:NamedIndividual ,
                        :RazzeMesomorfa ,
                        ontoHorse:RazzaCavallo ;
               :haIndole :sangueCaldo ;
               :haNazionalità ontoHorse:Germania ;
               :puòEssereImpiegataIn :Dressage ,
                                     :SaltoAdOstacoli ;
               ontoHorse:altezzaMediaAlGarrese_cm 170 ;
               ontoHorse:haColoreMantello "baio" ,
                                          "grigio" ,
                                          "morello" ,
                                          "sauro" ;
               ontoHorse:pesoMedio_Kg 525 ;
               <http://schema.org/image> <https://upload.wikimedia.org/wikipedia/commons/thumb/7/72/Bess2.jpg/240px-Bess2.jpg> ;
               rdfs:comment "L'Oldemburghese è una razza di cavallo originaria della Germania. Molto tranquillo ma energico, è il più grosso dei cavalli a sangue caldo tedeschi."@it ,
                            "The Oldenburger is a horse breed originating from Germany. Very calm but energetic, it is the largest of the German warmblood horses."@en ;
               <http://www.w3.org/2004/02/skos/core#exactMatch> "https://www.wikidata.org/wiki/Q166777"^^xsd:anyURI ;
               <http://www.w3.org/2004/02/skos/core#prefLabel> "Oldemburghese"@it ,
                                                               "Oldenburg Horse"@en .


###  http://www.semanticweb.org/annag/ontologies/2024/1/ontoHorses#PaesiBassi
:PaesiBassi rdf:type owl:NamedIndividual ,
                     ontoHorse:AreaGeografica ;
            <http://schema.org/image> <https://upload.wikimedia.org/wikipedia/commons/thumb/2/20/Flag_of_the_Netherlands.svg/1280px-Flag_of_the_Netherlands.svg.png> ;
            rdfs:comment "I Paesi Bassi sono una delle quattro nazioni costitutive del Regno dei Paesi Bassi; si trovano principalmente in Europa ma comprendono anche i cosiddetti Paesi Bassi caraibici. Il nome Paesi Bassi è un riferimento alla sua bassa elevazione e alla sua topografia piatta, con solo il 50% circa del suo territorio che supera 1 metro sopra il livello del mare e quasi il 26% che scende sotto il livello del mare."@it ,
                         "The Netherlands is one of the four constituent nations of the Kingdom of the Netherlands; they are found mainly in Europe but also include the so-called Caribbean Netherlands. The name Netherlands is a reference to its low elevation and flat topography, with only about 50% of its territory exceeding 1 meter above sea level and almost 26% falling below sea level."@en ;
            rdfs:label "Netherlands"@en ,
                       "Paesi Bassi"@it .


###  http://www.semanticweb.org/annag/ontologies/2024/1/ontoHorses#Perche
:Perche rdf:type owl:NamedIndividual ,
                 ontoHorse:AreaGeografica ;
        <http://www.ontologydesignpatterns.org/cp/owl/partof.owl#isPartOf> ontoHorse:Francia ;
        rdfs:comment "La contea del Perche è un territorio storico della Francia che costituisce una delle antiche province francesi."@it ,
                     "The county of Perche is a historical territory of France which constitutes one of the ancient French provinces."@en ;
        rdfs:label "Contea del Perche"@it ,
                   "Perche"@en .


###  http://www.semanticweb.org/annag/ontologies/2024/1/ontoHorses#Percheron
:Percheron rdf:type owl:NamedIndividual ,
                    :RazzaBrachimorfa ,
                    ontoHorse:RazzaCavallo ;
           :haIndole :sangueFreddo ;
           :puòEssereImpiegataIn :TiroAgricolo ,
                                 :TrainoCarrozze ;
           ontoHorse:haRegioneDiOrigine :Perche ;
           ontoHorse:altezzaMediaAlGarrese_cm 165 ;
           ontoHorse:haColoreMantello "grigio" ,
                                      "morello" ;
           ontoHorse:pesoMedio_Kg 800 ;
           <http://schema.org/image> <https://upload.wikimedia.org/wikipedia/commons/thumb/c/c1/Percheron_3_stehend_rechts.jpg/240px-Percheron_3_stehend_rechts.jpg> ;
           rdfs:comment "The Percheron is a French horse breed, originating from the province of Perche, in northern France, from which the breed takes its name. The Percheron is probably the best known and most widespread heavy breed in the world for agriculture and as a carriage horse"@en ,
                        "ll Percheron è una razza equina francese, originaria della provincia della Perche, nel nord della Francia, da cui prende nome la razza. Il Percheron è probabilmente la razza pesante più conosciuta e più diffusa del mondo per l’agricoltura e come cavallo da carrozza"@it ;
           <http://www.w3.org/2004/02/skos/core#exactMatch> "https://www.wikidata.org/wiki/Q1232528"^^xsd:anyURI ;
           <http://www.w3.org/2004/02/skos/core#prefLabel> "Percheron"@en ,
                                                           "Percheron"@it .


###  http://www.semanticweb.org/annag/ontologies/2024/1/ontoHorses#Portogallo
:Portogallo rdf:type owl:NamedIndividual ,
                     ontoHorse:AreaGeografica ;
            <http://schema.org/image> <https://upload.wikimedia.org/wikipedia/commons/thumb/5/5c/Flag_of_Portugal.svg/1280px-Flag_of_Portugal.svg.png> ;
            rdfs:comment "Il Portogallo è uno Stato membro dell'Unione europea ed è collocato nella posizione più occidentale fra tutti gli Stati dell'Europa continentale."@it ,
                         "Portugal is a member state of the European Union and is located in the most western position among all the states of continental Europe."@en ;
            rdfs:label "Portogallo"@it .


###  http://www.semanticweb.org/annag/ontologies/2024/1/ontoHorses#PuroSangueInglese
:PuroSangueInglese rdf:type owl:NamedIndividual ,
                            :RazzeDolicomorfa ,
                            ontoHorse:RazzaCavallo ;
                   :haIndole :sangueCaldo ;
                   :haNazionalità :RegnoUnito ;
                   :puòEssereImpiegataIn :SaltoAdOstacoli ;
                   ontoHorse:altezzaMediaAlGarrese_cm 160 ;
                   ontoHorse:haColoreMantello "baio" ,
                                              "grigio" ,
                                              "morello" ,
                                              "roano" ,
                                              "sauro" ;
                   ontoHorse:pesoMedio_Kg 425 ;
                   <http://schema.org/image> <https://www.animali.net/wp-content/uploads/2012/12/puro-sangue-inglese.jpg> ;
                   rdfs:comment "Il purosangue inglese è una razza equina originaria della Gran Bretagna e i  cavalli di tale razza sono ben noti per la loro agilità e velocità"@it ,
                                "The English Thoroughbred is a horse breed native to Great Britain and horses of this breed are well known for their agility and speed"@en ;
                   <http://www.w3.org/2004/02/skos/core#exactMatch> "https://www.wikidata.org/wiki/Q210826"^^xsd:anyURI ;
                   <http://www.w3.org/2004/02/skos/core#prefLabel> "Purosangue inglese"@it ,
                                                                   "Thoroughbred"@en .


###  http://www.semanticweb.org/annag/ontologies/2024/1/ontoHorses#RegioneBoullonnais
:RegioneBoullonnais rdf:type owl:NamedIndividual ,
                             ontoHorse:AreaGeografica ;
                    <http://www.ontologydesignpatterns.org/cp/owl/partof.owl#isPartOf> ontoHorse:Francia ;
                    rdfs:comment "Boulonnais is a natural coastal region in France, located on the English Channel coast in the Pas-de-Calais department."@en ,
                                 "Il Boulonnais è una regione naturale costiera francese, situata sul litorale della Manica nel dipartimento del Passo di Calais."@it ;
                    rdfs:label "Boulonnais"@en ,
                               "Boulonnais"@it .


###  http://www.semanticweb.org/annag/ontologies/2024/1/ontoHorses#RegioneHannover
:RegioneHannover rdf:type owl:NamedIndividual ,
                          ontoHorse:AreaGeografica ;
                 <http://www.ontologydesignpatterns.org/cp/owl/partof.owl#isPartOf> ontoHorse:Germania ;
                 rdfs:comment "Hannover is a city in north-central Germany, capital of the federal state of Lower Saxony"@en ,
                              "Hannover è una città della Germania centro-settentrionale, capitale dello stato federato della Bassa Sassonia"@it ;
                 rdfs:label "Hannover"@it ,
                            "Hanover"@en .


###  http://www.semanticweb.org/annag/ontologies/2024/1/ontoHorses#RegnoUnito
:RegnoUnito rdf:type owl:NamedIndividual ,
                     ontoHorse:AreaGeografica ;
            <http://schema.org/image> <https://upload.wikimedia.org/wikipedia/commons/thumb/a/a5/Flag_of_the_United_Kingdom_%281-2%29.svg/1920px-Flag_of_the_United_Kingdom_%281-2%29.svg.png> ;
            rdfs:comment "The United Kingdom, officially the United Kingdom of Great Britain and Northern Ireland, is an island country in Western Europe"@en ,
                         "ll Regno Unito, ufficialmente Regno Unito di Gran Bretagna e Irlanda del Nord è uno Stato insulare dell'Europa occidentale"@it ;
            rdfs:label "Regno Unito"@it ,
                       "United Kingdom"@en .


###  http://www.semanticweb.org/annag/ontologies/2024/1/ontoHorses#SaltoAdOstacoli
:SaltoAdOstacoli rdf:type owl:NamedIndividual ,
                          ontoHorse:SportEquestre .


###  http://www.semanticweb.org/annag/ontologies/2024/1/ontoHorses#Schleswig-Holstein
:Schleswig-Holstein rdf:type owl:NamedIndividual ,
                             ontoHorse:AreaGeografica ;
                    <http://www.ontologydesignpatterns.org/cp/owl/partof.owl#isPartOf> ontoHorse:Germania ;
                    rdfs:comment "Lo Schleswig-Holstein è uno dei sedici Stati federati della Germania, geograficamente il più settentrionale."@it ,
                                 "Schleswig-Holstein is one of the sixteen federal states of Germany, geographically the northernmost."@en ;
                    rdfs:label "Schleswig-Holstein"@en ,
                               "Schleswig-Holstein"@it .


###  http://www.semanticweb.org/annag/ontologies/2024/1/ontoHorses#Scozia
:Scozia rdf:type owl:NamedIndividual ,
                 ontoHorse:AreaGeografica ;
        <http://www.ontologydesignpatterns.org/cp/owl/partof.owl#isPartOf> :RegnoUnito ;
        rdfs:comment "La Scozia è una nazione costitutiva del Regno Unito che è posta all'estremità settentrionale dell'isola di Gran Bretagna e ne occupa più di un terzo della superficie"@it ,
                     "Scotland is a constituent nation of the United Kingdom which is located at the northern tip of the island of Great Britain and occupies more than a third of its surface"@en ;
        rdfs:label "Scotland"@en ,
                   "Scozia"@it .


###  http://www.semanticweb.org/annag/ontologies/2024/1/ontoHorses#SellaFrancese
:SellaFrancese rdf:type owl:NamedIndividual ,
                        :RazzaMesoDolicomorfa ,
                        ontoHorse:RazzaCavallo ;
               :haIndole :sangueCaldo ;
               :puòEssereImpiegataIn :Equiturismo ,
                                     :SaltoAdOstacoli ;
               ontoHorse:haRegioneDiOrigine ontoHorse:Normandia ;
               ontoHorse:altezzaMediaAlGarrese_cm 165 ;
               ontoHorse:haColoreMantello "baio" ,
                                          "grigio" ,
                                          "morello" ,
                                          "sauro" ;
               ontoHorse:pesoMedio_Kg 525 ;
               <http://schema.org/image> <https://upload.wikimedia.org/wikipedia/commons/thumb/5/5a/Cheval_selle.JPG/240px-Cheval_selle.JPG> ;
               rdfs:comment "Il Selle francese è una razza popolare di cavallo da sella di origine francese, utilizzato specialmente nelle gare di salto ostacoli e nel concorso completo"@it ,
                            "The French Selle is a popular breed of saddle horse of French origin, used especially in show jumping and eventing"@en ;
               <http://www.w3.org/2004/02/skos/core#exactMatch> "https://www.wikidata.org/wiki/Q1070901"^^xsd:anyURI ;
               <http://www.w3.org/2004/02/skos/core#prefLabel> "Sella Francese"@it ,
                                                               "Selle Français"@en .


###  http://www.semanticweb.org/annag/ontologies/2024/1/ontoHorses#TiroAgricolo
:TiroAgricolo rdf:type owl:NamedIndividual ,
                       ontoHorse:Lavoro ;
              owl:differentFrom :TrainoCarrozze .


###  http://www.semanticweb.org/annag/ontologies/2024/1/ontoHorses#TrainoCarrozze
:TrainoCarrozze rdf:type owl:NamedIndividual ,
                         ontoHorse:Lavoro .


###  http://www.semanticweb.org/annag/ontologies/2024/1/ontoHorses#Trakehner
:Trakehner rdf:type owl:NamedIndividual ,
                    :RazzaMesoDolicomorfa ,
                    ontoHorse:RazzaCavallo ;
           :haIndole :sangueMisto ;
           :haNazionalità ontoHorse:Germania ;
           :puòEssereImpiegataIn :Dressage ,
                                 :SaltoAdOstacoli ;
           ontoHorse:altezzaMediaAlGarrese_cm 165 ;
           ontoHorse:haColoreMantello "baio" ,
                                      "crema" ,
                                      "grigio" ,
                                      "morello" ,
                                      "palomino" ,
                                      "roano" ,
                                      "sauro" ;
           ontoHorse:pesoMedio_Kg 500 ;
           <http://schema.org/image> <https://upload.wikimedia.org/wikipedia/commons/thumb/8/8b/Trakehner_Horse.jpg/240px-Trakehner_Horse.jpg> ;
           rdfs:comment "Il Trakehner è una razza di cavallo da sella e tiro leggero più allevati e amati al mondo, attualmente utilizzato negli sport equestri"@it ,
                        "The Trakehner is a breed of riding and light draft horse most bred and loved in the world, currently used in equestrian sports"@en ;
           <http://www.w3.org/2004/02/skos/core#exactMatch> "https://www.wikidata.org/wiki/Q843585"^^xsd:anyURI ;
           <http://www.w3.org/2004/02/skos/core#prefLabel> "Trakehner"@en ,
                                                           "Trakehner"@it .


###  http://www.semanticweb.org/annag/ontologies/2024/1/ontoHorses#TrentinoAltoAdige
:TrentinoAltoAdige rdf:type owl:NamedIndividual ,
                            ontoHorse:AreaGeografica ;
                   <http://www.ontologydesignpatterns.org/cp/owl/partof.owl#isPartOf> ontoHorse:Italia ;
                   rdfs:comment "Il Trentino-Alto Adige  è una regione italiana a statuto speciale dell'Italia Nord-orientale con capoluogo Trento."@it ,
                                "Trentino-Alto Adige is an Italian region with a special statute in north-eastern Italy with Trento as its capital."@en ;
                   rdfs:label "Trentino-Alto Adige"@en ,
                              "Trentino-Alto Adige"@it .


###  http://www.semanticweb.org/annag/ontologies/2024/1/ontoHorses#Vestfalia
:Vestfalia rdf:type owl:NamedIndividual ,
                    ontoHorse:AreaGeografica ;
           <http://www.ontologydesignpatterns.org/cp/owl/partof.owl#isPartOf> ontoHorse:Germania ;
           rdfs:comment "La Vestfalia è una regione della Germania, inclusa nei land della Renania Settentrionale-Vestfalia e Bassa Sassonia."@it ,
                        "Westphalia is a region of Germany, included in the states of North Rhine-Westphalia and Lower Saxony."@en ;
           rdfs:label "Vestfalia"@it ,
                      "Westphalia"@en .


###  http://www.semanticweb.org/annag/ontologies/2024/1/ontoHorses#Westfalen
:Westfalen rdf:type owl:NamedIndividual ,
                    :RazzeMesomorfa ,
                    ontoHorse:RazzaCavallo ;
           :haIndole :sangueCaldo ;
           :puòEssereImpiegataIn :Dressage ,
                                 :SaltoAdOstacoli ;
           ontoHorse:haRegioneDiOrigine :Vestfalia ;
           ontoHorse:altezzaMediaAlGarrese_cm 165 ;
           ontoHorse:haColoreMantello "baio" ,
                                      "morello" ,
                                      "sauro" ;
           ontoHorse:pesoMedio_Kg 500 ;
           <http://schema.org/image> <https://upload.wikimedia.org/wikipedia/commons/thumb/9/9a/Avenger_-_Westphalian_horse.jpg/240px-Avenger_-_Westphalian_horse.jpg> ;
           rdfs:comment "Il Westfalen è  un’atletica e forte razza di cavalli tedesca da sport che ha ottenuto eccellenti risultati nel concorso di salto nel dressage."@it ,
                        "The Westfalen is an athletic and strong German sport horse breed that has achieved excellent results in dressage jumping competition."@en ;
           <http://www.w3.org/2004/02/skos/core#exactMatch> "https://www.wikidata.org/wiki/Q195395"^^xsd:anyURI ;
           <http://www.w3.org/2004/02/skos/core#prefLabel> "Westfalen"@it ,
                                                           "Westphalian horse"@en .


###  http://www.semanticweb.org/annag/ontologies/2024/1/ontoHorses#sangueCaldo
:sangueCaldo rdf:type owl:NamedIndividual ,
                      :Indole ;
             rdfs:comment "E' una categoria di razze di cavalli, classificate sulla base del temperamento, generalmente molto reattive adatte all'impiego nelle attività sportive equestri"@it ,
                          "It is a category of horses, classified on the basis of temperament, generally suitable for use in equestrian sporting activities"@en ;
             rdfs:label "sangue caldo"@it ,
                        "warm blooded horses"@en .


###  http://www.semanticweb.org/annag/ontologies/2024/1/ontoHorses#sangueFreddo
:sangueFreddo rdf:type owl:NamedIndividual ,
                       :Indole ;
              rdfs:comment "E' una categoria di razze di cavalli, classificate sulla base del temperamento, che derivano da linee di sangue di razze di cavalli da lavoro. Sono razze di cavalli molto docili e tranquilli. Necessitano maggiore impegno nell’addestramento e sollecitazioni nel lavoro."@it ,
                           "It is a category of horses, classified on the basis of temperament, which derive from bloodlines of working horses. They are very docile and calm horses. They require greater commitment to training and stress at work."@en ;
              rdfs:label "cold blood"@en ,
                         "sangue freddo"@it .


###  http://www.semanticweb.org/annag/ontologies/2024/1/ontoHorses#sangueMisto
:sangueMisto rdf:type owl:NamedIndividual ,
                      :Indole ;
             rdfs:comment "E' una categoria di razze di cavalli, classificate sulla base del temperamento, che presentano caratteristiche ibride tra le razze a sangue caldo e quelle a sangue freddo"@it ,
                          "It is a category of horse breeds, classified on the basis of temperament, which present hybrid characteristics between warm-blooded and cold-blooded breeds."@en ;
             rdfs:label "mixed blood"@en ,
                        "sangue misto"@it .


###  http://www.semanticweb.org/annag/ontologies/2024/1/ontoHorses#12000Euro
<http://www.semanticweb.org/annag/ontologies/2024/1/ontoHorses#12000Euro> rdf:type owl:NamedIndividual ,
                                                                                   <http://www.ontologydesignpatterns.org/cp/owl/price.owl#Price> ;
                                                                          <http://www.ontologydesignpatterns.org/cp/owl/price.owl#hasCurrency> ontoHorse:Euro ;
                                                                          <http://www.ontologydesignpatterns.org/cp/owl/price.owl#hasValue> "12000.0"^^xsd:float ;
                                                                          rdfs:comment "12000 Euro"@it ;
                                                                          rdfs:label "12000 Euro"@it .


###  http://www.semanticweb.org/annag/ontologies/2024/1/ontoHorses#15000Euro
<http://www.semanticweb.org/annag/ontologies/2024/1/ontoHorses#15000Euro> rdf:type owl:NamedIndividual ,
                                                                                   <http://www.ontologydesignpatterns.org/cp/owl/price.owl#Price> ;
                                                                          <http://www.ontologydesignpatterns.org/cp/owl/price.owl#hasCurrency> ontoHorse:Euro ;
                                                                          <http://www.ontologydesignpatterns.org/cp/owl/price.owl#hasValue> "15000.0"^^xsd:float ;
                                                                          rdfs:comment "15000 Euro"@it ;
                                                                          rdfs:label "15000 Euro"@it .


###  http://www.semanticweb.org/annag/ontologies/2024/1/ontoHorses#18000Euro
<http://www.semanticweb.org/annag/ontologies/2024/1/ontoHorses#18000Euro> rdf:type owl:NamedIndividual ,
                                                                                   <http://www.ontologydesignpatterns.org/cp/owl/price.owl#Price> ;
                                                                          <http://www.ontologydesignpatterns.org/cp/owl/price.owl#hasCurrency> ontoHorse:Euro ;
                                                                          <http://www.ontologydesignpatterns.org/cp/owl/price.owl#hasValue> "18000.0"^^xsd:float ;
                                                                          rdfs:comment "18000 Euro"@it ;
                                                                          rdfs:label "18000 Euro"@it .


###  http://www.semanticweb.org/annag/ontologies/2024/1/ontoHorses#20000Euro
<http://www.semanticweb.org/annag/ontologies/2024/1/ontoHorses#20000Euro> rdf:type owl:NamedIndividual ,
                                                                                   <http://www.ontologydesignpatterns.org/cp/owl/price.owl#Price> ;
                                                                          <http://www.ontologydesignpatterns.org/cp/owl/price.owl#hasCurrency> ontoHorse:Euro ;
                                                                          <http://www.ontologydesignpatterns.org/cp/owl/price.owl#hasValue> "20000.0"^^xsd:float ;
                                                                          rdfs:comment "20000 Euro"@it ;
                                                                          rdfs:label "20000 Euro"@it .


###  http://www.semanticweb.org/annag/ontologies/2024/1/ontoHorses#2500Euro
<http://www.semanticweb.org/annag/ontologies/2024/1/ontoHorses#2500Euro> rdf:type owl:NamedIndividual ,
                                                                                  <http://www.ontologydesignpatterns.org/cp/owl/price.owl#Price> ;
                                                                         <http://www.ontologydesignpatterns.org/cp/owl/price.owl#hasCurrency> ontoHorse:Euro ;
                                                                         <http://www.ontologydesignpatterns.org/cp/owl/price.owl#hasValue> "2500.0"^^xsd:float ;
                                                                         rdfs:comment "2500 Euro"@it ;
                                                                         rdfs:label "2500 Euro"@it .


###  http://www.semanticweb.org/annag/ontologies/2024/1/ontoHorses#35000Euro
<http://www.semanticweb.org/annag/ontologies/2024/1/ontoHorses#35000Euro> rdf:type owl:NamedIndividual ,
                                                                                   <http://www.ontologydesignpatterns.org/cp/owl/price.owl#Price> ;
                                                                          <http://www.ontologydesignpatterns.org/cp/owl/price.owl#hasCurrency> ontoHorse:Euro ;
                                                                          <http://www.ontologydesignpatterns.org/cp/owl/price.owl#hasValue> "35000.0"^^xsd:float ;
                                                                          rdfs:comment "35000 Euro"@it ;
                                                                          rdfs:label "35000 Euro"@it .


###  http://www.semanticweb.org/annag/ontologies/2024/1/ontoHorses#4800Euro
<http://www.semanticweb.org/annag/ontologies/2024/1/ontoHorses#4800Euro> rdf:type owl:NamedIndividual ,
                                                                                  <http://www.ontologydesignpatterns.org/cp/owl/price.owl#Price> ;
                                                                         <http://www.ontologydesignpatterns.org/cp/owl/price.owl#hasCurrency> ontoHorse:Euro ;
                                                                         <http://www.ontologydesignpatterns.org/cp/owl/price.owl#hasValue> "4800.0"^^xsd:float ;
                                                                         rdfs:comment "4800 Euro"@it ;
                                                                         rdfs:label "4800 Euro"@it .


###  http://www.semanticweb.org/annag/ontologies/2024/1/ontoHorses#5000Euro
<http://www.semanticweb.org/annag/ontologies/2024/1/ontoHorses#5000Euro> rdf:type owl:NamedIndividual ,
                                                                                  <http://www.ontologydesignpatterns.org/cp/owl/price.owl#Price> ;
                                                                         <http://www.ontologydesignpatterns.org/cp/owl/price.owl#hasCurrency> ontoHorse:Euro ;
                                                                         <http://www.ontologydesignpatterns.org/cp/owl/price.owl#hasValue> "5000.0"^^xsd:float ;
                                                                         rdfs:comment "5000 Euro"@it ;
                                                                         rdfs:label "5000 Euro"@it .


###  http://www.semanticweb.org/annag/ontologies/2024/1/ontoHorses#7000Euro
<http://www.semanticweb.org/annag/ontologies/2024/1/ontoHorses#7000Euro> rdf:type owl:NamedIndividual ,
                                                                                  <http://www.ontologydesignpatterns.org/cp/owl/price.owl#Price> ;
                                                                         <http://www.ontologydesignpatterns.org/cp/owl/price.owl#hasCurrency> ontoHorse:Euro ;
                                                                         <http://www.ontologydesignpatterns.org/cp/owl/price.owl#hasValue> "7000.0"^^xsd:float ;
                                                                         rdfs:comment "7000 Euro"@it ;
                                                                         rdfs:label "7000 Euro"@it .


###  http://www.semanticweb.org/annag/ontologies/2024/1/ontoHorses/Andalusia
ontoHorse:Andalusia rdf:type owl:NamedIndividual ,
                             ontoHorse:AreaGeografica ;
                    <http://www.ontologydesignpatterns.org/cp/owl/partof.owl#isPartOf> ontoHorse:Spagna ;
                    <http://schema.org/image> <https://upload.wikimedia.org/wikipedia/commons/thumb/2/2e/Andalucia_in_Spain_%28plus_Canarias%29.svg/260px-Andalucia_in_Spain_%28plus_Canarias%29.svg.png> ;
                    rdfs:comment "Andalusia is one of the seventeen autonomous communities of Spain and has Seville as its capital"@en ,
                                 "L'Andalusìa  è una delle diciassette comunità autonome della Spagna ed ha Siviglia come capoluogo"@it ;
                    rdfs:label "Andalusia"@en ,
                               "Andalusia"@it .


###  http://www.semanticweb.org/annag/ontologies/2024/1/ontoHorses/Andaluso
ontoHorse:Andaluso rdf:type owl:NamedIndividual ,
                            :RazzeMesomorfa ,
                            ontoHorse:RazzaCavallo ;
                   :haIndole :sangueCaldo ;
                   :puòEssereImpiegataIn :AltaScuola ,
                                         :Dressage ;
                   ontoHorse:haRegioneDiOrigine ontoHorse:Andalusia ;
                   ontoHorse:altezzaMediaAlGarrese_cm 160 ;
                   ontoHorse:haColoreMantello "baio" ,
                                              "grigio" ,
                                              "roano" ;
                   ontoHorse:pesoMedio_Kg 470 ;
                   <http://schema.org/image> <https://upload.wikimedia.org/wikipedia/commons/1/10/Fotografo-caballos-pura-raza.jpg> ;
                   rdfs:comment "Mesomorphic Spanish horse breed with a noble and elegant bearing"@en ,
                                "Razza di cavallo Spagnola mesomorfa dal portamento nobile ed elegante"@it ;
                   <http://www.w3.org/2004/02/skos/core#exactMatch> "https://www.wikidata.org/wiki/Q489798"^^xsd:anyURI ;
                   <http://www.w3.org/2004/02/skos/core#prefLabel> "Andalusian Horse"@en ,
                                                                   "Andaluso"@it .


###  http://www.semanticweb.org/annag/ontologies/2024/1/ontoHorses/C100
ontoHorse:C100 rdf:type owl:NamedIndividual ;
               ontoHorse:permetteIlConseguimentoDi ontoHorse:brevetto ;
               rdfs:comment "Categoria di salto ad ostacoli in cui l'altezza degli ostacoli lungo il percorso di gara non è mai superiore ai 100 cm"@it ,
                            "Show jumping category in which the height of the obstacles along the competition course is never higher than 100 cm"@en ;
               rdfs:label "C100"@en ,
                          "C100"@it .


###  http://www.semanticweb.org/annag/ontologies/2024/1/ontoHorses/C105
ontoHorse:C105 rdf:type owl:NamedIndividual ;
               ontoHorse:permetteIlConseguimentoDi ontoHorse:brevetto ;
               rdfs:comment "Categoria di salto ad ostacoli in cui l'altezza degli ostacoli lungo il percorso di gara non è mai superiore ai 105 cm"@it ,
                            "Show jumping category in which the height of the obstacles along the competition course is never higher than 105 cm"@en ;
               rdfs:label "C105"@en ,
                          "C105"@it .


###  http://www.semanticweb.org/annag/ontologies/2024/1/ontoHorses/C110
ontoHorse:C110 rdf:type owl:NamedIndividual ;
               ontoHorse:permetteIlConseguimentoDi ontoHorse:brevetto ;
               rdfs:comment "Categoria di salto ad ostacoli in cui l'altezza degli ostacoli lungo il percorso di gara non è mai superiore ai 110 cm"@it ,
                            "Show jumping category in which the height of the obstacles along the competition course is never higher than 110 cm"@en ;
               rdfs:label "C110"@en ,
                          "C110"@it .


###  http://www.semanticweb.org/annag/ontologies/2024/1/ontoHorses/C115
ontoHorse:C115 rdf:type owl:NamedIndividual ;
               ontoHorse:permetteIlConseguimentoDi ontoHorse:brevetto ,
                                                   ontoHorse:primoGrado ;
               rdfs:comment "Categoria di salto ad ostacoli in cui l'altezza degli ostacoli lungo il percorso di gara non è mai superiore ai 115 cm"@it ,
                            "Show jumping category in which the height of the obstacles along the competition course is never higher than 115 cm"@en ;
               rdfs:label "C115"@en ,
                          "C115"@it .


###  http://www.semanticweb.org/annag/ontologies/2024/1/ontoHorses/C120
ontoHorse:C120 rdf:type owl:NamedIndividual ;
               ontoHorse:permetteIlConseguimentoDi ontoHorse:primoGrado ;
               rdfs:comment "Categoria di salto ad ostacoli in cui l'altezza degli ostacoli lungo il percorso di gara non è mai superiore ai 120 cm"@it ,
                            "Show jumping category in which the height of the obstacles along the competition course is never higher than 120 cm"@en ;
               rdfs:label "C120"@en ,
                          "C120"@it .


###  http://www.semanticweb.org/annag/ontologies/2024/1/ontoHorses/C125
ontoHorse:C125 rdf:type owl:NamedIndividual ;
               ontoHorse:permetteIlConseguimentoDi ontoHorse:primoGrado ;
               rdfs:comment "Categoria di salto ad ostacoli in cui l'altezza degli ostacoli lungo il percorso di gara non è mai superiore ai 125 cm"@it ,
                            "Show jumping category in which the height of the obstacles along the competition course is never higher than 125 cm"@en ;
               rdfs:label "C125"@en ,
                          "C125"@it .


###  http://www.semanticweb.org/annag/ontologies/2024/1/ontoHorses/C130
ontoHorse:C130 rdf:type owl:NamedIndividual ;
               ontoHorse:permetteIlConseguimentoDi ontoHorse:primoGrado ;
               rdfs:comment "Categoria di salto ad ostacoli in cui l'altezza degli ostacoli lungo il percorso di gara non è mai superiore ai 130 cm"@it ,
                            "Show jumping category in which the height of the obstacles along the competition course is never higher than 130 cm"@en ;
               rdfs:label "C130"@en ,
                          "C130"@it .


###  http://www.semanticweb.org/annag/ontologies/2024/1/ontoHorses/C135
ontoHorse:C135 rdf:type owl:NamedIndividual ;
               ontoHorse:permetteIlConseguimentoDi ontoHorse:primoGrado ,
                                                   ontoHorse:secondoGrado ;
               rdfs:comment "Categoria di salto ad ostacoli in cui l'altezza degli ostacoli lungo il percorso di gara non è mai superiore ai 135 cm"@it ,
                            "Show jumping category in which the height of the obstacles along the competition course is never higher than 135 cm"@en ;
               rdfs:label "C135"@en ,
                          "C135"@it .


###  http://www.semanticweb.org/annag/ontologies/2024/1/ontoHorses/C80
ontoHorse:C80 rdf:type owl:NamedIndividual ;
              ontoHorse:permetteIlConseguimentoDi ontoHorse:brevetto ;
              rdfs:comment "Categoria di salto ad ostacoli in cui l'altezza degli ostacoli lungo il percorso di gara non è mai superiore ai 80 cm"@it ,
                           "Show jumping category in which the height of the obstacles along the competition course is never higher than 80 cm"@en ;
              rdfs:label "C80"@en ,
                         "C80"@it .


###  http://www.semanticweb.org/annag/ontologies/2024/1/ontoHorses/C90
ontoHorse:C90 rdf:type owl:NamedIndividual ;
              ontoHorse:permetteIlConseguimentoDi ontoHorse:brevetto ;
              rdfs:comment "Categoria di salto ad ostacoli in cui l'altezza degli ostacoli lungo il percorso di gara non è mai superiore ai 90 cm"@it ,
                           "Show jumping category in which the height of the obstacles along the competition course is never higher than 90 cm"@en ;
              rdfs:label "C90"@en ,
                         "C90"@it .


###  http://www.semanticweb.org/annag/ontologies/2024/1/ontoHorses/CastroneItaliano
ontoHorse:CastroneItaliano rdf:type owl:NamedIndividual ,
                                    ontoHorse:Cavallo ;
                           <http://www.ontologydesignpatterns.org/cp/owl/price.owl#hasPrice> <http://www.semanticweb.org/annag/ontologies/2024/1/ontoHorses#12000Euro> ;
                           ontoHorse:gareggiaNelleCategorieDiSalto ontoHorse:C100 ,
                                                                   ontoHorse:C80 ;
                           ontoHorse:haRazza ontoHorse:SellaItaliano ;
                           :annoDiNascita 2013 ;
                           :contattoProprietario "333-345628" ;
                           :haProprietario "Elisabetta Lanza" ;
                           :nomeCavallo "Dracon's Breaker" ;
                           :provinciaDiScuderizzazione "Torino" ;
                           :regioneDiScuderizzazione "Piemonte" ;
                           ontoHorse:altezzaAlGarrese_cm 160 ;
                           ontoHorse:altezzaMaxDiSalto_cm "125"^^xsd:nonNegativeInteger ;
                           ontoHorse:età "11"^^xsd:nonNegativeInteger ;
                           ontoHorse:haSesso "castrone" ;
                           rdfs:comment "Esemplare di cavallo castrone italiano in vendita"@it ,
                                        "Italian gelding horse for sale"@en ;
                           rdfs:label "Castrone italiano"@it ,
                                      "Italian Gelding horse"@en .


###  http://www.semanticweb.org/annag/ontologies/2024/1/ontoHorses/CavaliereEsperto
ontoHorse:CavaliereEsperto rdf:type owl:NamedIndividual ;
                           rdfs:comment "Cavaliere la cui abilità di di salto ostacoli è superiore alla categoria C115 ma inferiore alla categoria C130"@it ,
                                        "Horse rider whose jumping ability is above category C115 but below category C130"@en ;
                           rdfs:label "Cavaliere esperto"@it ,
                                      "Expert horse rider"@en .


###  http://www.semanticweb.org/annag/ontologies/2024/1/ontoHorses/CavaliereIntermedio
ontoHorse:CavaliereIntermedio rdf:type owl:NamedIndividual ;
                              rdfs:comment "Cavaliere la cui abilità di di salto ostacoli è inferiore alla categoria C115"@it ,
                                           "Horse rider whose jumping ability is below category C115"@en ;
                              rdfs:label "Cavaliere intermedio"@it ,
                                         "Intermediate horse rider"@en .


###  http://www.semanticweb.org/annag/ontologies/2024/1/ontoHorses/CavaliereMoltoEsperto
ontoHorse:CavaliereMoltoEsperto rdf:type owl:NamedIndividual ;
                                rdfs:comment "Cavaliere la cui abilità di di salto ostacoli è uguale o superiore alla categoria C135"@it ,
                                             "Horse rider whose show jumping ability is equal to or greater than category C135"@en ;
                                rdfs:label "Cavaliere molto esperto"@it ,
                                           "Very experienced horse rider"@en .


###  http://www.semanticweb.org/annag/ontologies/2024/1/ontoHorses/CavalierePrincipiante
ontoHorse:CavalierePrincipiante rdf:type owl:NamedIndividual ;
                                rdfs:comment "Cavaliere la cui abilità di di salto ostacoli è inferiore alla categoria C80"@it ,
                                             "Horse rider whose jumping ability is below category C80"@en ;
                                rdfs:label "Beginner horse rider"@en ,
                                           "Cavaliere principiante"@it .


###  http://www.semanticweb.org/annag/ontologies/2024/1/ontoHorses/Euro
ontoHorse:Euro rdf:type owl:NamedIndividual ,
                        <http://www.ontologydesignpatterns.org/cp/owl/price.owl#Currency> ;
               rdfs:comment "European Currency"@en ,
                            "Moneta europea"@it ;
               rdfs:label "Euro"@en ,
                          "Euro"@it .


###  http://www.semanticweb.org/annag/ontologies/2024/1/ontoHorses/Francia
ontoHorse:Francia rdf:type owl:NamedIndividual ,
                           ontoHorse:AreaGeografica ;
                  <http://www.ontologydesignpatterns.org/cp/owl/partof.owl#hasPart> ontoHorse:Normandia ;
                  <http://schema.org/image> <https://upload.wikimedia.org/wikipedia/commons/thumb/9/93/Flag_of_France_%281794%E2%80%931815%2C_1830%E2%80%931974%29.svg/1280px-Flag_of_France_%281794%E2%80%931815%2C_1830%E2%80%931974%29.svg.png> ;
                  rdfs:comment "France, officially the French Republic, is a state located in Western Europe and Southern Europe, but which also has territories spread across multiple oceans and other continents."@en ,
                               "La Francia,  ufficialmente Repubblica francese, è uno Stato situato nell'Europa occidentale e nell'Europa meridionale, ma che possiede ugualmente territori disseminati su più oceani e altri continenti."@it ;
                  rdfs:label "France"@en ,
                             "Francia"@it .


###  http://www.semanticweb.org/annag/ontologies/2024/1/ontoHorses/Germania
ontoHorse:Germania rdf:type owl:NamedIndividual ,
                            ontoHorse:AreaGeografica ;
                   <http://schema.org/image> <https://upload.wikimedia.org/wikipedia/en/thumb/b/ba/Flag_of_Germany.svg/1920px-Flag_of_Germany.svg.png> ;
                   rdfs:comment "Germany, officially the Federal Republic of Germany, is a member state of the European Union located in central-western Europe."@en ,
                                "La Germania, ufficialmente Repubblica Federale di Germania, è uno Stato membro dell'Unione europea situato nell'Europa centro-occidentale."@it ;
                   rdfs:label "Germania"@it ,
                              "Germany"@en .


###  http://www.semanticweb.org/annag/ontologies/2024/1/ontoHorses/Irlanda
ontoHorse:Irlanda rdf:type owl:NamedIndividual ,
                           ontoHorse:AreaGeografica ;
                  <http://schema.org/image> <https://upload.wikimedia.org/wikipedia/commons/thumb/4/45/Flag_of_Ireland.svg/1920px-Flag_of_Ireland.svg.png> ;
                  rdfs:comment "Ireland, officially the Republic of Ireland, is a member country of the European Union."@en ,
                               "L'Irlanda, ufficialmente Repubblica d'Irlanda, è un Paese membro dell'Unione europea."@it ;
                  rdfs:label "Irlanda"@it ,
                             "Republic of Ireland"@en .


###  http://www.semanticweb.org/annag/ontologies/2024/1/ontoHorses/Italia
ontoHorse:Italia rdf:type owl:NamedIndividual ,
                          ontoHorse:AreaGeografica ;
                 <http://schema.org/image> <https://upload.wikimedia.org/wikipedia/commons/thumb/0/03/Flag_of_Italy.svg/1280px-Flag_of_Italy.svg.png> ;
                 rdfs:comment "Italy, officially the Italian Republic, is a member state of the European Union, located in southern and western Europe, whose territory largely coincides with the geographical region of the same name."@en ,
                              "L'Italia, ufficialmente Repubblica Italiana, è uno Stato membro dell'Unione europea, situato nell'Europa meridionale e occidentale, il cui territorio coincide in gran parte con l'omonima regione geografica."@it ;
                 rdfs:label "Italia"@it ,
                            "Italy"@en .


###  http://www.semanticweb.org/annag/ontologies/2024/1/ontoHorses/MaschioAndaluso
ontoHorse:MaschioAndaluso rdf:type owl:NamedIndividual ,
                                   ontoHorse:Cavallo ;
                          <http://www.ontologydesignpatterns.org/cp/owl/price.owl#hasPrice> <http://www.semanticweb.org/annag/ontologies/2024/1/ontoHorses#7000Euro> ;
                          ontoHorse:haRazza ontoHorse:Andaluso ;
                          ontoHorse:vieneUtilizzatoPer :AltaScuola ;
                          ontoHorse:èAdattoPer ontoHorse:CavaliereIntermedio ;
                          :annoDiNascita "2020"^^xsd:nonNegativeInteger ;
                          :contattoProprietario "345-324241" ;
                          :haProprietario "Mario Rossi" ;
                          :nomeCavallo "Fuser" ;
                          :provinciaDiScuderizzazione "Siracusa" ;
                          :regioneDiScuderizzazione "Sicilia" ;
                          ontoHorse:altezzaAlGarrese_cm 165 ;
                          ontoHorse:categorieDiDressage "E" ;
                          ontoHorse:età "4"^^xsd:nonNegativeInteger ;
                          ontoHorse:haSesso "maschio" ;
                          rdfs:comment "Esemplare di cavallo maschio andaluso in vendita"@it ,
                                       "Male Andalusian horse for sale"@en ;
                          rdfs:label "Andalusian male"@en ,
                                     "Maschio andaluso"@it .


###  http://www.semanticweb.org/annag/ontologies/2024/1/ontoHorses/Murge
ontoHorse:Murge rdf:type owl:NamedIndividual ;
                <http://www.ontologydesignpatterns.org/cp/owl/partof.owl#isPartOf> ontoHorse:Italia ;
                <http://schema.org/image> <https://upload.wikimedia.org/wikipedia/commons/thumb/0/0a/Murge.jpg/1280px-Murge.jpg> ;
                rdfs:comment "Le Murge sono una subregione appulo-lucana piuttosto estesa, corrispondente a un altopiano carsico di origine tettonica e di forma quadrangolare situato tra la Puglia centrale e la Basilicata nord-orientale. Il territorio dell'altopiano fa parte prevalentemente della città metropolitana di Bari e della provincia di Barletta-Andria-Trani e si estende a occidente fin nella provincia di Matera, in Basilicata; inoltre si prolunga verso sud nelle province di Taranto (Murge tarantine) e marginalmente Brindisi."@it ,
                             "The Murge are a rather large Appulo-Lucanian subregion, corresponding to a karst plateau of tectonic origin and quadrangular in shape located between central Puglia and north-eastern Basilicata. The territory of the plateau is mainly part of the metropolitan city of Bari and the province of Barletta-Andria-Trani and extends westwards to the province of Matera, in Basilicata; it also extends southwards into the provinces of Taranto (Murge tarantine) and marginally Brindisi."@en ;
                rdfs:label "Murge"@en ,
                           "Murge"@it .


###  http://www.semanticweb.org/annag/ontologies/2024/1/ontoHorses/Normandia
ontoHorse:Normandia rdf:type owl:NamedIndividual ,
                             ontoHorse:AreaGeografica ;
                    rdfs:comment "La Normandia è una regione storica ed amministrativa della Francia."@it ,
                                 "Normandy is a historical and administrative region of France."@en ;
                    rdfs:label "Normandia"@it ,
                               "Normandy"@en .


###  http://www.semanticweb.org/annag/ontologies/2024/1/ontoHorses/SellaItaliano
ontoHorse:SellaItaliano rdf:type owl:NamedIndividual ,
                                 :RazzaMesoDolicomorfa ,
                                 ontoHorse:RazzaCavallo ;
                        :haIndole :sangueCaldo ;
                        :haNazionalità ontoHorse:Italia ;
                        :puòEssereImpiegataIn :Dressage ,
                                              :SaltoAdOstacoli ;
                        ontoHorse:altezzaMediaAlGarrese_cm 160 ;
                        ontoHorse:haColoreMantello "baio" ,
                                                   "morello" ,
                                                   "sauro" ;
                        ontoHorse:pesoMedio_Kg 500 ;
                        <http://schema.org/image> <https://www.dothorse.it/wp-content/uploads/2014/07/sella-ita.jpg> ;
                        rdfs:comment "Il sella italiano è una razza equina derivante prevalentemente da incroci del purosangue inglese, arabo, anglo-arabo. E' un cavallo dall'aspetto elegante e nobile con la robustezza tipica del purosangue inglese e la grande affidabilità delle razze italiche."@it ,
                                     "The Italian saddle is a horse breed deriving mainly from crosses of the English, Arabian and Anglo-Arab thoroughbreds. It is a horse with an elegant and noble appearance with the typical robustness of the English thoroughbred and the great reliability of the Italian breeds."@en ;
                        <http://www.w3.org/2004/02/skos/core#exactMatch> "https://www.wikidata.org/wiki/Q428039"^^xsd:anyURI ;
                        <http://www.w3.org/2004/02/skos/core#prefLabel> "Sella Italiano"@en ,
                                                                        "Sella Italiano"@it .


###  http://www.semanticweb.org/annag/ontologies/2024/1/ontoHorses/Spagna
ontoHorse:Spagna rdf:type owl:NamedIndividual ,
                          ontoHorse:AreaGeografica ;
                 <http://schema.org/image> <https://upload.wikimedia.org/wikipedia/commons/thumb/9/9a/Flag_of_Spain.svg/1280px-Flag_of_Spain.svg.png> ;
                 rdfs:comment "La Spagna è uno Stato sovrano, membro dell'Unione europea dal 1986 e si trova all'estremità occidentale dell'Europa occupando buona parte della superficie della penisola iberica."@it ,
                              "Spain is a sovereign state, member of the European Union since 1986 and is located at the western end of Europe, occupying a large part of the surface of the Iberian peninsula."@en ;
                 rdfs:label "Spagna"@it ,
                            "Spain"@en .


###  http://www.semanticweb.org/annag/ontologies/2024/1/ontoHorses/brevetto
ontoHorse:brevetto rdf:type owl:NamedIndividual ,
                            ontoHorse:Patente ;
                   ontoHorse:vieneConseguitoDa ontoHorse:CavalierePrincipiante ;
                   <http://www.ontologydesignpatterns.org/cp/owl/sequence.owl#precedes> ontoHorse:primoGrado ;
                   rdfs:comment "Authorizes the practice of competitive equestrian sports based on the specific specialty of the license acquired by the rider. Thebrevetto authorizes participation in show jumping competitions of category C80 or higher"@en ,
                                "Autorizza all’esercizio della pratica sportiva agonistica degli sport equestri in funzione della specifica specialità del brevetto acquisito dal cavaliere. Il brevetto autorizza a partecipare a gare di salto ad ostacoli di categoria C80 o superiore"@it ;
                   rdfs:label "brevetto"@en ,
                              "brevetto"@it .


###  http://www.semanticweb.org/annag/ontologies/2024/1/ontoHorses/patenteAgonistica
ontoHorse:patenteAgonistica rdf:type owl:NamedIndividual ,
                                     <http://www.ontologydesignpatterns.org/cp/owl/list.owl#List> ;
                            <http://www.ontologydesignpatterns.org/cp/owl/bag.owl#hasItem> ontoHorse:brevetto ,
                                                                                           ontoHorse:primoGrado ,
                                                                                           ontoHorse:secondoGrado ;
                            rdfs:comment "License that enables the practice of competitive sports"@en ,
                                         "Patente che abilita all'esercizio della pratica sportiva agonistica"@it ;
                            rdfs:label "Competitive license"@en ,
                                       "Patente agonistica"@it .


###  http://www.semanticweb.org/annag/ontologies/2024/1/ontoHorses/patenteLudicaA
ontoHorse:patenteLudicaA rdf:type owl:NamedIndividual ,
                                  ontoHorse:Patente ;
                         ontoHorse:vieneConseguitoDa ontoHorse:CavalierePrincipiante ;
                         rdfs:comment "Authorizes the practice of recreational and training equestrian sports in any discipline."@en ,
                                      "Autorizza all’esercizio della pratica sportiva ludico-addestrativa degli sport equestri in qualsiasi disciplina."@it ;
                         rdfs:label "Patente ludica A"@en ,
                                    "Patente ludica A"@it .


###  http://www.semanticweb.org/annag/ontologies/2024/1/ontoHorses/patenteNonAgonistica
ontoHorse:patenteNonAgonistica rdf:type owl:NamedIndividual ,
                                        <http://www.ontologydesignpatterns.org/cp/owl/list.owl#List> ;
                               <http://www.ontologydesignpatterns.org/cp/owl/bag.owl#hasItem> ontoHorse:patenteLudicaA ;
                               <http://www.ontologydesignpatterns.org/cp/owl/sequence.owl#precedes> ontoHorse:patenteAgonistica ;
                               rdfs:comment "Authorizes the practice of recreational and training equestrian sports and social integration activities through sport"@en ,
                                            "Autorizza all'esercizio della pratica sportiva equestre ludico-addestrativa e alle attività di integrazione sociale attraverso lo sport"@it ;
                               rdfs:label "Not competitive licence"@en ,
                                          "Patente non agonistica"@it .


###  http://www.semanticweb.org/annag/ontologies/2024/1/ontoHorses/primoGrado
ontoHorse:primoGrado rdf:type owl:NamedIndividual ,
                              ontoHorse:Patente ;
                     ontoHorse:vieneConseguitoDa ontoHorse:CavaliereEsperto ,
                                                 ontoHorse:CavaliereIntermedio ;
                     <http://www.ontologydesignpatterns.org/cp/owl/sequence.owl#precedes> ontoHorse:secondoGrado ;
                     rdfs:comment "Authorizes the practice of competitive equestrian sports based on the specific specialty of the license acquired by the rider. The 1° grado authorizes participation in show jumping competitions of category C115 or higher"@en ,
                                  "Autorizza all’esercizio della pratica sportiva agonistica degli sport equestri in funzione della specifica specialità del brevetto acquisito dal cavaliere. Il 1° grado autorizza a partecipare a gare di salto ad ostacoli di categoria C115 o superiore"@it ;
                     rdfs:label "1° grado"@en ,
                                "1° grado"@it .


###  http://www.semanticweb.org/annag/ontologies/2024/1/ontoHorses/secondoGrado
ontoHorse:secondoGrado rdf:type owl:NamedIndividual ,
                                ontoHorse:Patente ;
                       ontoHorse:vieneConseguitoDa ontoHorse:CavaliereMoltoEsperto ;
                       rdfs:comment "Authorizes the practice of competitive equestrian sports based on the specific specialty of the license acquired by the rider. The 2° grado authorizes participation in show jumping competitions of category C135 or higher"@en ,
                                    "Autorizza all’esercizio della pratica sportiva agonistica degli sport equestri in funzione della specifica specialità del brevetto acquisito dal cavaliere. Il 2° grado autorizza a partecipare a gare di salto ad ostacoli di categoria C135 o superiore"@it ;
                       rdfs:label "2° grado"@en ,
                                  "2° grado"@it .


#################################################################
#    Annotations
#################################################################

:AltaScuola <http://schema.org/image> <https://www.sef-italia.it/wp-content/uploads/2020/02/Schermata-2020-02-05-alle-14.52.05-768x712.png> ;
            rdfs:comment "E' uno sport equestre simile al Dressage che ha per scopo lo sviluppo armonioso dell'organismo e dei mezzi del cavallo"@it ,
                         "It is an equestrian sport similar to Dressage which has as its aim the harmonious development of the horse's organism and means"@en ;
            rdfs:label "Alta Scuola"@it ,
                       "Spanish riding school"@en .


:CrossCountry rdfs:comment "Cross-country is an Olympic equestrian sport, which consists of a speed test on varied terrain, and the overcoming of various types of fixed obstacles."@en ,
                           "Il cross-country è uno sport equestre olimpico, che consiste in una prova di velocità su terreno vario, e nel superamento di vari tipi di ostacoli fissi."@it ;
              rdfs:label "Cross-country"@en ,
                         "Cross-country"@it .


:Dressage rdfs:comment "Dressage is an Olympic equestrian discipline which is also called a training competition, as the horse and rider perform predominantly geometric movements on a rectangular field, measuring 20x40 meters for low level competitions and 20x60 in medium/high level ones."@en ,
                       "Il Dressage è una disciplina equestre olimpionica che viene anche chiamata gara di addestramento, in quanto cavallo e cavaliere eseguono movimenti prevalentemente geometrici su un campo di forma rettangolare, di dimensioni 20x40 metri per le gare di basso livello e 20x60 in quelle di livello medio/alto."@it ;
          rdfs:label "Dressage"@en ,
                     "Dressage"@it .


:Endurance rdfs:comment "Endurance is one of the most popular equestrian sports in the world. The competitions consist of endurance races on routes of various nature and a mileage that varies from 30 to 160 km depending on the categories."@en ,
                        "L'Endurance è uno degli sport equestri di maggior diffusione al mondo. Le competizioni consistono in corse di resistenza su percorsi di varia natura ed un chilometraggio che varia dai 30 ai 160 km a seconda delle categorie."@it ;
           rdfs:label "Endurance"@en ,
                      "Endurance"@it .


:Equiturismo rdfs:comment "Equestrian tourism is a practice of horse riding which consists in the use of the horse for the pleasure of riding in places far from civilization, for example the countryside, woods, hills or mountains."@en ,
                          "L'equiturismo è una pratica dell'equitazione che consiste nell'uso del cavallo per il piacere di cavalcare in luoghi lontani dalla civiltà, ad esempio i campagna, boschi, collina o montagna."@it ;
             rdfs:label "Equiturismo"@it ,
                        "Trail riding"@en .


:Eventing rdfs:comment "Full riding is a discipline that originates from the training of soldiers to face the difficulties of the campaign. At the same time they had to demonstrate perfect dressage training and also complete a show jumping course. The event trials are called \"three day events\" in the Anglo-Saxon world precisely because the three trials are spread over three days. Undoubtedly the most spectacular test is the countryside one, the cross country, during which the pairs have to face challenging natural obstacles such as trunks, ditches, uphill and downhill jumps, combinations and lakes."@en ,
                       "Il completo di equitazione è una disciplina che ha origine dall'addestramento dei militari per affrontare le difficoltà della campagna. Allo stesso tempo dovevano dimostrare un perfetto addestramento in dressage e superare anche un percorso di salto ostacoli. Le prove di completo sono chiamate nel mondo anglosassone \"three day event\" proprio perchè le tre prove sono distribuite su tre giornate. Indubbiamente la prova più spettacolare è quella di campagna, il cross country, durante la quale i binomi devono affrontare impegnativi ostacoli naturali come tronchi, fossi, salti in salita e discesa, combinazioni e laghetti."@it ;
          rdfs:label "Eventing"@it .


:SaltoAdOstacoli rdfs:comment "Il salto ostacoli è un termine che identifica una disciplina dell'equitazione, la quale vede impegnato il binomio uomo-cavallo, nell'interpretazione e risoluzione di un percorso ad ostacoli. L'altezza degli ostacoli, la difficoltà del percorso e il numero di ostacoli da superare dipende dalla categoria alla quale si partecipa e dalla preparazione atletica di cavallo e cavaliere. L'altezza degli ostacoli varia dai 40 cm a 1,60 m  con categorie intermedie di 60, 70, 80, 90, 100, 105, 110, 115, 120, 125,130, 135, 140,145, 150, 160. Il numero di ostacoli varia da 8 a 13 con eventuali combinazioni di più ostacoli dette gabbie."@it ,
                              "Show jumping is a term that identifies a discipline of horse riding, which involves the man-horse duo in the interpretation and resolution of an obstacle course. The height of the obstacles, the difficulty of the route and the number of obstacles to overcome depends on the category in which you participate and the athletic preparation of the horse and rider. The height of the obstacles varies from 40 cm to 1.60 m with intermediate categories of 60, 70, 80, 90, 100, 105, 110, 115, 120, 125,130, 135, 140,145, 150, 160. The number of obstacles varies from 8 to 13 with possible combinations of multiple obstacles called cages."@en ;
                 rdfs:label "Salto Ostacoli"@it ,
                            "Show jumping"@en .


:TiroAgricolo rdfs:comment "Use of the horse for agricultural work"@en ,
                           "Utilizzo del cavallo per lavori in campo agricolo"@it ;
              rdfs:label "Tiro agricolo"@it ,
                         "agricultural draft"@en .


:TrainoCarrozze rdfs:comment "Using the horse to pull carriages for the transport of goods or people"@en ,
                             "Utilizzo del cavallo per trainare carrozze per il trasporto di merci o persone"@it ;
                rdfs:label "Towing carriages"@en ,
                           "Traino carrozze"@it .


#################################################################
#    General axioms
#################################################################

[ rdf:type owl:AllDisjointClasses ;
  owl:members ( ontoHorse:CavalloAdulto
                ontoHorse:CavalloAnziano
                ontoHorse:Puledro
              )
] .


[ rdf:type owl:AllDisjointClasses ;
  owl:members ( ontoHorse:RazzaASangueCaldo
                ontoHorse:RazzaASangueFreddo
                ontoHorse:RazzaASangueMisto
              )
] .


[ rdf:type owl:AllDifferent ;
  owl:distinctMembers ( :AltaScuola
                        :CrossCountry
                        :Dressage
                        :Endurance
                        :Eventing
                        :SaltoAdOstacoli
                      )
] .


[ rdf:type owl:AllDifferent ;
  owl:distinctMembers ( :AngloAraboFrancese
                        :Appenninico
                        :Ard
                        :Ardennese
                        :BelgaDaTiro
                        :Boulonnais
                        :Bretone
                        :CavalloDelloJutland
                        :Clydesdale
                        :Frisone
                        :Hannover
                        :Holstein
                        :IrishSportHorse
                        :Lipizzano
                        :Lusitano
                        :Maremmano
                        :Murgese
                        :OlandeseASangueCaldo
                        :Oldemburghese
                        :Percheron
                        :PuroSangueInglese
                        :SellaFrancese
                        :Trakehner
                        :Westfalen
                        ontoHorse:Andaluso
                        ontoHorse:SellaItaliano
                      )
] .


[ rdf:type owl:AllDifferent ;
  owl:distinctMembers ( :sangueCaldo
                        :sangueFreddo
                        :sangueMisto
                      )
] .


[ rdf:type owl:AllDifferent ;
  owl:distinctMembers ( ontoHorse:C100
                        ontoHorse:C105
                        ontoHorse:C110
                        ontoHorse:C115
                        ontoHorse:C120
                        ontoHorse:C125
                        ontoHorse:C130
                        ontoHorse:C135
                        ontoHorse:C80
                        ontoHorse:C90
                      )
] .


[ rdf:type owl:AllDifferent ;
  owl:distinctMembers ( ontoHorse:CavaliereEsperto
                        ontoHorse:CavaliereIntermedio
                        ontoHorse:CavaliereMoltoEsperto
                        ontoHorse:CavalierePrincipiante
                      )
] .


###  Generated by the OWL API (version 4.5.26.2023-07-17T20:34:13Z) https://github.com/owlcs/owlapi
