<?xml version="1.0"?>
<rdf:RDF xmlns="http://www.semanticweb.org/annag/ontologies/2024/4/ontoHorsesInferred#"
     xml:base="http://www.semanticweb.org/annag/ontologies/2024/4/ontoHorsesInferred"
     xmlns:dc="http://purl.org/dc/elements/1.1/"
     xmlns:bag="http://www.ontologydesignpatterns.org/cp/owl/bag.owl#"
     xmlns:owl="http://www.w3.org/2002/07/owl#"
     xmlns:rdf="http://www.w3.org/1999/02/22-rdf-syntax-ns#"
     xmlns:xml="http://www.w3.org/XML/1998/namespace"
     xmlns:xsd="http://www.w3.org/2001/XMLSchema#"
     xmlns:rdfs="http://www.w3.org/2000/01/rdf-schema#"
     xmlns:skos="http://www.w3.org/2004/02/skos/core#"
     xmlns:vann="http://purl.org/vocab/vann/"
     xmlns:price="http://www.ontologydesignpatterns.org/cp/owl/price.owl#"
     xmlns:partof="http://www.ontologydesignpatterns.org/cp/owl/partof.owl#"
     xmlns:schema="http://schema.org/"
     xmlns:sequence="http://www.ontologydesignpatterns.org/cp/owl/sequence.owl#"
     xmlns:ontoHorses="http://www.semanticweb.org/annag/ontologies/2024/1/ontoHorses#"
     xmlns:collectionentity="http://www.ontologydesignpatterns.org/cp/owl/collectionentity.owl#"
     xmlns:cpannotationschema="http://www.ontologydesignpatterns.org/schemas/cpannotationschema.owl#">
    <owl:Ontology rdf:about="http://www.semanticweb.org/annag/ontologies/2024/4/ontoHorsesInferred">
        <dc:creator>Annalisa Sabatelli</dc:creator>
        <dc:date rdf:datatype="http://www.w3.org/2001/XMLSchema#dateTime">2024-03-01T09:00:00</dc:date>
        <dc:description xml:lang="en">Ontological representation of breeds, uses and main characteristics of horses and their sales announcements aimed at helping the user in purchasing a horse.</dc:description>
        <dc:description xml:lang="it">Rappresentazione ontologica di razze, impieghi e caratteristiche principali dei cavalli e annunci di vendita finalizzata ad aiutare l&apos;utente nell&apos;acquisto di un cavallo.</dc:description>
        <dc:title xml:lang="en">OntoHorses</dc:title>
        <vann:preferedNamespacePrefix xml:lang="it">http://www.semanticweb.org/annag/ontologies/2024/1/ontoHorses</vann:preferedNamespacePrefix>
        <vann:preferedNamespacePrefix xml:lang="en">oh</vann:preferedNamespacePrefix>
        <cpannotationschema:coversRequirements>What is before what?,What&apos;s next?,What&apos;s immediately following this?</cpannotationschema:coversRequirements>
        <cpannotationschema:coversRequirements>What things are contained in this collection (community, collective)? What collections this thing is member of?</cpannotationschema:coversRequirements>
        <cpannotationschema:coversRequirements>What are the items (elements) in this list?</cpannotationschema:coversRequirements>
        <cpannotationschema:coversRequirements>What are the items contained in this bag? </cpannotationschema:coversRequirements>
        <cpannotationschema:coversRequirements>What bag is this item an element of?</cpannotationschema:coversRequirements>
        <cpannotationschema:coversRequirements>What is the first/last item in this list?</cpannotationschema:coversRequirements>
        <cpannotationschema:coversRequirements>What is the length (size) of this list?</cpannotationschema:coversRequirements>
        <cpannotationschema:coversRequirements>What is the size of this bag?</cpannotationschema:coversRequirements>
        <cpannotationschema:coversRequirements>What is this entity part of? What are the parts of this entity?</cpannotationschema:coversRequirements>
        <cpannotationschema:coversRequirements>What it the next/previous item in the list?</cpannotationschema:coversRequirements>
        <cpannotationschema:coversRequirements>What resource does this item refer to?</cpannotationschema:coversRequirements>
        <cpannotationschema:coversRequirements>What resource does this list item contain?</cpannotationschema:coversRequirements>
        <cpannotationschema:extractedFrom>http://www.ontologydesignpatterns.org/ont/dul/DUL.owl</cpannotationschema:extractedFrom>
        <cpannotationschema:extractedFrom>http://swan.mindinformatics.org/ontologies/1.2/collections.owl</cpannotationschema:extractedFrom>
        <cpannotationschema:hasAuthor>Aldo Gangemi</cpannotationschema:hasAuthor>
        <cpannotationschema:hasAuthor>Sara Bernardini</cpannotationschema:hasAuthor>
        <cpannotationschema:hasAuthor>Valentina Presutti</cpannotationschema:hasAuthor>
        <cpannotationschema:hasAuthor>PaoloCiccarese</cpannotationschema:hasAuthor>
        <cpannotationschema:hasComponent>http://www.ontologydesignpatterns.org/cp/owl/collectionentity.owl</cpannotationschema:hasComponent>
        <cpannotationschema:hasComponent>http://www.ontologydesignpatterns.org/cp/owl/sequence.owl</cpannotationschema:hasComponent>
        <cpannotationschema:hasConsequences>Collections and their members can be associated. Time-indexed membership cannot be represented though (you need a situation-based pattern).</cpannotationschema:hasConsequences>
        <cpannotationschema:hasConsequences>We can represent and reason over transitive or intransitive sequences of any kind. However, since coreference cannot be expressed in OWL, it is not possible to represent and reason over loops and other sequences involving coreference.</cpannotationschema:hasConsequences>
        <cpannotationschema:hasConsequences>This CP allows designers to represent entities and their parts i.e., part-whole relations, with transitivity. The temporal aspect of this relation cannot be expressed; in order to solve this issue the time indexed part of CP can be used.</cpannotationschema:hasConsequences>
        <cpannotationschema:hasIntent>To represent domain (not set theory) membership.</cpannotationschema:hasIntent>
        <cpannotationschema:hasIntent>To represent sequence schemas. It defines the notion of transitive and intransitive precedence and their inverses. 
It can then be used between tasks, processes, time intervals, spatially locate objects, situations, etc.</cpannotationschema:hasIntent>
        <cpannotationschema:hasIntent>To model bags of items (elements). The Bag is characterized by a collection that can have multiple copies of each object. </cpannotationschema:hasIntent>
        <cpannotationschema:hasIntent>To represent ordered collections, i.e. lists.</cpannotationschema:hasIntent>
        <cpannotationschema:hasIntent>To represents entities and their parts.</cpannotationschema:hasIntent>
        <cpannotationschema:isSpecializationOf>http://www.ontologydesignpatterns.org/cp/owl/sequence.owl</cpannotationschema:isSpecializationOf>
        <cpannotationschema:reengineeredFrom>http://swan.mindinformatics.org/ontologies/1.2/collections.owl</cpannotationschema:reengineeredFrom>
        <cpannotationschema:relatedCPs>TimeIndexedMembership</cpannotationschema:relatedCPs>
        <cpannotationschema:relatedCPs>The time indexed part of is used as alternative when the temporal indexing has to be represented. Part of CP is specialized by componency. Sometimes this CP is wrongly used in order to model constituency and membership. These two modeling problems are addressed by constituency, and collection entity CPs, respectively.</cpannotationschema:relatedCPs>
        <cpannotationschema:relatedCPs>http://www.ontologydesignpatterns.org/cp/owl/bag.owl</cpannotationschema:relatedCPs>
        <cpannotationschema:relatedCPs>http://www.ontologydesignpatterns.org/cp/owl/list.owl</cpannotationschema:relatedCPs>
        <cpannotationschema:relatedCPs>http://www.ontologydesignpatterns.org/cp/owl/set.owl</cpannotationschema:relatedCPs>
        <cpannotationschema:scenarios>My saxophone collection includes a Mark VI tenor, a Balanced Action alto, and a Conn Transitional bari.</cpannotationschema:scenarios>
        <cpannotationschema:scenarios>Brain and heart are parts of the human body, substantia nigra is part of brain.</cpannotationschema:scenarios>
        <rdfs:comment>The collection entity pattern. 
It is extracted from DOLCE-UltraLite by partial clone of elements.</rdfs:comment>
        <rdfs:comment>The price content ontology design pattern. This CP represents the price of an entity in a certain currency.</rdfs:comment>
        <rdfs:comment>The Bag is characterized by a collection that can have multiple copies of each object. This is performed through the Item entity. The Item is linking exaclty one resource through the relationship itemContent.</rdfs:comment>
        <rdfs:label xml:lang="it">Ontologia sulle principali razze di cavallo europee</rdfs:label>
        <rdfs:label xml:lang="en">Ontology on the main European horse breeds</rdfs:label>
        <rdfs:label>collection entity</rdfs:label>
        <rdfs:label>membership</rdfs:label>
        <rdfs:label>ordering</rdfs:label>
        <rdfs:label>part of</rdfs:label>
        <rdfs:label>part-whole</rdfs:label>
        <rdfs:label>precedence</rdfs:label>
        <rdfs:label>sequence</rdfs:label>
        <owl:versionInfo>1.1
- Revised and annotated for ODP submission by Aldo Gangemi
1.0
- Created by Valentina Presutti and Sara Bernardini</owl:versionInfo>
        <owl:versionInfo>1.1 added rdfs:isDefinedBy for all named entities</owl:versionInfo>
        <owl:versionInfo>Created by Aldo Gangemi and Valentina Presutti</owl:versionInfo>
        <owl:versionInfo>Created by Valentina Presutti</owl:versionInfo>
        <owl:versionInfo>Created with TopBraid Composer</owl:versionInfo>
    </owl:Ontology>
    


    <!-- 
    ///////////////////////////////////////////////////////////////////////////////////////
    //
    // Annotation properties
    //
    ///////////////////////////////////////////////////////////////////////////////////////
     -->

    


    <!-- http://purl.org/dc/elements/1.1/creator -->

    <owl:AnnotationProperty rdf:about="http://purl.org/dc/elements/1.1/creator"/>
    


    <!-- http://purl.org/dc/elements/1.1/date -->

    <owl:AnnotationProperty rdf:about="http://purl.org/dc/elements/1.1/date"/>
    


    <!-- http://purl.org/dc/elements/1.1/description -->

    <owl:AnnotationProperty rdf:about="http://purl.org/dc/elements/1.1/description"/>
    


    <!-- http://purl.org/dc/elements/1.1/title -->

    <owl:AnnotationProperty rdf:about="http://purl.org/dc/elements/1.1/title"/>
    


    <!-- http://purl.org/vocab/vann/preferedNamespacePrefix -->

    <owl:AnnotationProperty rdf:about="http://purl.org/vocab/vann/preferedNamespacePrefix"/>
    


    <!-- http://schema.org/image -->

    <owl:AnnotationProperty rdf:about="http://schema.org/image"/>
    


    <!-- http://www.ontologydesignpatterns.org/schemas/cpannotationschema.owl#coversRequirements -->

    <owl:AnnotationProperty rdf:about="http://www.ontologydesignpatterns.org/schemas/cpannotationschema.owl#coversRequirements">
        <rdfs:comment>This annotation property is used for exemplifying possible requirements the content pattern provides a solution for. Requirements are expressed as natural language competency questions.</rdfs:comment>
    </owl:AnnotationProperty>
    


    <!-- http://www.ontologydesignpatterns.org/schemas/cpannotationschema.owl#extractedFrom -->

    <owl:AnnotationProperty rdf:about="http://www.ontologydesignpatterns.org/schemas/cpannotationschema.owl#extractedFrom">
        <rdfs:comment>This annotation property should be assigned with a URI, which points to the possible reference ontology which the annotated pattern was extracted from (i.e. the reference ontology that the ontology elements have been deeply or partially cloned by). The range is not explicit in the definition of the annotation property because it would turn the ontology to OWL Full. E.g. The participation pattern is extracted from the Dolce Ultra Lite ontology, hence the value for this annotation property is http://www.ontologydesignpatterns.org/ont/dul/DUL.owl</rdfs:comment>
    </owl:AnnotationProperty>
    


    <!-- http://www.ontologydesignpatterns.org/schemas/cpannotationschema.owl#hasAuthor -->

    <owl:AnnotationProperty rdf:about="http://www.ontologydesignpatterns.org/schemas/cpannotationschema.owl#hasAuthor"/>
    


    <!-- http://www.ontologydesignpatterns.org/schemas/cpannotationschema.owl#hasComponent -->

    <owl:AnnotationProperty rdf:about="http://www.ontologydesignpatterns.org/schemas/cpannotationschema.owl#hasComponent">
        <rdfs:comment>This annotation property is useful for content ontology design patterns. Its value is a URI, which refers to another content ontology design pattern which is a component of the annotated one.</rdfs:comment>
    </owl:AnnotationProperty>
    


    <!-- http://www.ontologydesignpatterns.org/schemas/cpannotationschema.owl#hasConsequences -->

    <owl:AnnotationProperty rdf:about="http://www.ontologydesignpatterns.org/schemas/cpannotationschema.owl#hasConsequences">
        <rdfs:comment>This annotation property is used for briefly describing the benefits and/or possible trade-offs when using the CP.</rdfs:comment>
    </owl:AnnotationProperty>
    


    <!-- http://www.ontologydesignpatterns.org/schemas/cpannotationschema.owl#hasIntent -->

    <owl:AnnotationProperty rdf:about="http://www.ontologydesignpatterns.org/schemas/cpannotationschema.owl#hasIntent">
        <rdfs:comment>This annotation property is used in order to describe the intent of the content pattern.</rdfs:comment>
    </owl:AnnotationProperty>
    


    <!-- http://www.ontologydesignpatterns.org/schemas/cpannotationschema.owl#isSpecializationOf -->

    <owl:AnnotationProperty rdf:about="http://www.ontologydesignpatterns.org/schemas/cpannotationschema.owl#isSpecializationOf">
        <rdfs:comment>This annotation property is useful for content ontology design patterns and its elements. Its value is a URI, which refers either to a content ontology design pattern that is specialized by the annotated one, or to an ontology element that is specialized by the annotated one.</rdfs:comment>
    </owl:AnnotationProperty>
    


    <!-- http://www.ontologydesignpatterns.org/schemas/cpannotationschema.owl#reengineeredFrom -->

    <owl:AnnotationProperty rdf:about="http://www.ontologydesignpatterns.org/schemas/cpannotationschema.owl#reengineeredFrom">
        <rdfs:comment>This annotation property should be assigned with a URI, which points to the concept schema, page, or anything else from which the annotated pattern was reengineered.  If the source does not have any URI e.g., a printed book, this property value should provide information as precise as possible in order to identify the source. This property is alternative to the extractedFrom property because it is used when the pattern come from a concept schema which is not an owl ontology. For example content ontology design patterns, which are reengineered from data model patterns, rdf schemas, etc. should be annotatd with this property. E.g. The basicpersonalfoaf pattern is extracted from the rdf FOAF specification, hence the value for this annotation property is http://xmlns.com/foaf/spec/20071002.rdf</rdfs:comment>
    </owl:AnnotationProperty>
    


    <!-- http://www.ontologydesignpatterns.org/schemas/cpannotationschema.owl#relatedCPs -->

    <owl:AnnotationProperty rdf:about="http://www.ontologydesignpatterns.org/schemas/cpannotationschema.owl#relatedCPs">
        <rdfs:comment>This annotation property can be used to indicate other CPs (if any) that specialize, generalize, inlcude, or are components of the CP. Furthermore, this field may indicate other CPs that are typically used in conjunction with the described one. Important similarities and differences with other patterns can be also described here.</rdfs:comment>
    </owl:AnnotationProperty>
    


    <!-- http://www.ontologydesignpatterns.org/schemas/cpannotationschema.owl#scenarios -->

    <owl:AnnotationProperty rdf:about="http://www.ontologydesignpatterns.org/schemas/cpannotationschema.owl#scenarios">
        <rdfs:comment>This annotation property is used for describing examples of instantiation of the Content OP. For example, for the part-of Content OP (which represents part-whole relations) a possible scenario is the sentence: &quot;the brain is part of the human body&quot;. Scenarios are expressed as natural language sentences.</rdfs:comment>
    </owl:AnnotationProperty>
    


    <!-- http://www.w3.org/2004/02/skos/core#exactMatch -->

    <owl:AnnotationProperty rdf:about="http://www.w3.org/2004/02/skos/core#exactMatch"/>
    


    <!-- http://www.w3.org/2004/02/skos/core#prefLabel -->

    <owl:AnnotationProperty rdf:about="http://www.w3.org/2004/02/skos/core#prefLabel"/>
    


    <!-- 
    ///////////////////////////////////////////////////////////////////////////////////////
    //
    // Object Properties
    //
    ///////////////////////////////////////////////////////////////////////////////////////
     -->

    


    <!-- http://www.ontologydesignpatterns.org/cp/owl/bag.owl#hasItem -->

    <owl:ObjectProperty rdf:about="http://www.ontologydesignpatterns.org/cp/owl/bag.owl#hasItem">
        <rdfs:subPropertyOf rdf:resource="http://www.ontologydesignpatterns.org/cp/owl/collectionentity.owl#hasMember"/>
        <rdfs:subPropertyOf>
            <rdf:Description>
                <owl:inverseOf rdf:resource="http://www.ontologydesignpatterns.org/cp/owl/collectionentity.owl#isMemberOf"/>
            </rdf:Description>
        </rdfs:subPropertyOf>
        <owl:inverseOf rdf:resource="http://www.ontologydesignpatterns.org/cp/owl/bag.owl#itemOf"/>
        <rdfs:domain rdf:resource="http://www.ontologydesignpatterns.org/cp/owl/bag.owl#Bag"/>
        <rdfs:range rdf:resource="http://www.ontologydesignpatterns.org/cp/owl/bag.owl#Item"/>
        <rdfs:comment>has item - The link to every item of the Bag</rdfs:comment>
        <rdfs:label>has item</rdfs:label>
    </owl:ObjectProperty>
    


    <!-- http://www.ontologydesignpatterns.org/cp/owl/bag.owl#itemContent -->

    <owl:ObjectProperty rdf:about="http://www.ontologydesignpatterns.org/cp/owl/bag.owl#itemContent">
        <rdfs:domain rdf:resource="http://www.ontologydesignpatterns.org/cp/owl/bag.owl#Item"/>
        <rdfs:range>
            <owl:Class>
                <owl:complementOf rdf:resource="http://www.ontologydesignpatterns.org/cp/owl/bag.owl#Item"/>
            </owl:Class>
        </rdfs:range>
        <rdfs:comment>itemContent - The link to the actual resource to which the item refers.</rdfs:comment>
        <rdfs:label>item content</rdfs:label>
    </owl:ObjectProperty>
    


    <!-- http://www.ontologydesignpatterns.org/cp/owl/bag.owl#itemOf -->

    <owl:ObjectProperty rdf:about="http://www.ontologydesignpatterns.org/cp/owl/bag.owl#itemOf">
        <rdfs:subPropertyOf rdf:resource="http://www.ontologydesignpatterns.org/cp/owl/collectionentity.owl#isMemberOf"/>
        <rdfs:subPropertyOf>
            <rdf:Description>
                <owl:inverseOf rdf:resource="http://www.ontologydesignpatterns.org/cp/owl/collectionentity.owl#hasMember"/>
            </rdf:Description>
        </rdfs:subPropertyOf>
        <rdfs:domain rdf:resource="http://www.ontologydesignpatterns.org/cp/owl/bag.owl#Item"/>
        <rdfs:range rdf:resource="http://www.ontologydesignpatterns.org/cp/owl/bag.owl#Bag"/>
        <rdfs:comment>item of - The link from an item to the Bag where it is contained</rdfs:comment>
        <rdfs:label>item of</rdfs:label>
    </owl:ObjectProperty>
    


    <!-- http://www.ontologydesignpatterns.org/cp/owl/collectionentity.owl#hasMember -->

    <owl:ObjectProperty rdf:about="http://www.ontologydesignpatterns.org/cp/owl/collectionentity.owl#hasMember">
        <owl:inverseOf rdf:resource="http://www.ontologydesignpatterns.org/cp/owl/collectionentity.owl#isMemberOf"/>
        <rdfs:domain rdf:resource="http://www.ontologydesignpatterns.org/cp/owl/collectionentity.owl#Collection"/>
        <rdfs:range rdf:resource="http://www.w3.org/2002/07/owl#Thing"/>
        <rdfs:comment>A relation between collections and entities, e.g. &apos;my collection of saxophones includes an old Adolphe Sax original alto&apos; (i.e. my collection has member an Adolphe Sax alto).</rdfs:comment>
        <rdfs:isDefinedBy rdf:resource="http://www.ontologydesignpatterns.org/cp/owl/collectionentity.owl"/>
        <rdfs:label xml:lang="en">has member</rdfs:label>
    </owl:ObjectProperty>
    


    <!-- http://www.ontologydesignpatterns.org/cp/owl/collectionentity.owl#isMemberOf -->

    <owl:ObjectProperty rdf:about="http://www.ontologydesignpatterns.org/cp/owl/collectionentity.owl#isMemberOf">
        <rdfs:domain rdf:resource="http://www.w3.org/2002/07/owl#Thing"/>
        <rdfs:range rdf:resource="http://www.ontologydesignpatterns.org/cp/owl/collectionentity.owl#Collection"/>
        <rdfs:isDefinedBy rdf:resource="http://www.ontologydesignpatterns.org/cp/owl/collectionentity.owl"/>
        <rdfs:label xml:lang="en">is member of</rdfs:label>
    </owl:ObjectProperty>
    


    <!-- http://www.ontologydesignpatterns.org/cp/owl/list.owl#firstItemOf -->

    <owl:ObjectProperty rdf:about="http://www.ontologydesignpatterns.org/cp/owl/list.owl#firstItemOf">
        <rdfs:subPropertyOf rdf:resource="http://www.ontologydesignpatterns.org/cp/owl/bag.owl#itemOf"/>
        <rdfs:subPropertyOf>
            <rdf:Description>
                <owl:inverseOf rdf:resource="http://www.ontologydesignpatterns.org/cp/owl/bag.owl#hasItem"/>
            </rdf:Description>
        </rdfs:subPropertyOf>
        <owl:inverseOf rdf:resource="http://www.ontologydesignpatterns.org/cp/owl/list.owl#hasFirstItem"/>
        <rdfs:domain rdf:resource="http://www.ontologydesignpatterns.org/cp/owl/list.owl#ListItem"/>
        <rdfs:range rdf:resource="http://www.ontologydesignpatterns.org/cp/owl/list.owl#List"/>
        <rdfs:label>first item of</rdfs:label>
    </owl:ObjectProperty>
    


    <!-- http://www.ontologydesignpatterns.org/cp/owl/list.owl#hasFirstItem -->

    <owl:ObjectProperty rdf:about="http://www.ontologydesignpatterns.org/cp/owl/list.owl#hasFirstItem">
        <rdfs:subPropertyOf rdf:resource="http://www.ontologydesignpatterns.org/cp/owl/bag.owl#hasItem"/>
        <rdfs:subPropertyOf>
            <rdf:Description>
                <owl:inverseOf rdf:resource="http://www.ontologydesignpatterns.org/cp/owl/bag.owl#itemOf"/>
            </rdf:Description>
        </rdfs:subPropertyOf>
        <rdf:type rdf:resource="http://www.w3.org/2002/07/owl#FunctionalProperty"/>
        <rdfs:domain rdf:resource="http://www.ontologydesignpatterns.org/cp/owl/list.owl#List"/>
        <rdfs:range rdf:resource="http://www.ontologydesignpatterns.org/cp/owl/list.owl#ListItem"/>
        <rdfs:comment>first item - The link to the first item of the list</rdfs:comment>
        <rdfs:label>has first item</rdfs:label>
    </owl:ObjectProperty>
    


    <!-- http://www.ontologydesignpatterns.org/cp/owl/list.owl#hasLastItem -->

    <owl:ObjectProperty rdf:about="http://www.ontologydesignpatterns.org/cp/owl/list.owl#hasLastItem">
        <rdfs:subPropertyOf rdf:resource="http://www.ontologydesignpatterns.org/cp/owl/bag.owl#hasItem"/>
        <rdfs:subPropertyOf>
            <rdf:Description>
                <owl:inverseOf rdf:resource="http://www.ontologydesignpatterns.org/cp/owl/bag.owl#itemOf"/>
            </rdf:Description>
        </rdfs:subPropertyOf>
        <owl:inverseOf rdf:resource="http://www.ontologydesignpatterns.org/cp/owl/list.owl#lastItemOf"/>
        <rdf:type rdf:resource="http://www.w3.org/2002/07/owl#FunctionalProperty"/>
        <rdfs:domain rdf:resource="http://www.ontologydesignpatterns.org/cp/owl/list.owl#List"/>
        <rdfs:range rdf:resource="http://www.ontologydesignpatterns.org/cp/owl/list.owl#ListItem"/>
        <rdfs:comment>last item - The link to the last item of the list</rdfs:comment>
        <rdfs:label>has last item</rdfs:label>
    </owl:ObjectProperty>
    


    <!-- http://www.ontologydesignpatterns.org/cp/owl/list.owl#lastItemOf -->

    <owl:ObjectProperty rdf:about="http://www.ontologydesignpatterns.org/cp/owl/list.owl#lastItemOf">
        <rdfs:subPropertyOf rdf:resource="http://www.ontologydesignpatterns.org/cp/owl/bag.owl#itemOf"/>
        <rdfs:subPropertyOf>
            <rdf:Description>
                <owl:inverseOf rdf:resource="http://www.ontologydesignpatterns.org/cp/owl/bag.owl#hasItem"/>
            </rdf:Description>
        </rdfs:subPropertyOf>
        <rdfs:domain rdf:resource="http://www.ontologydesignpatterns.org/cp/owl/list.owl#ListItem"/>
        <rdfs:range rdf:resource="http://www.ontologydesignpatterns.org/cp/owl/list.owl#List"/>
        <rdfs:label>last item of</rdfs:label>
    </owl:ObjectProperty>
    


    <!-- http://www.ontologydesignpatterns.org/cp/owl/list.owl#nextItem -->

    <owl:ObjectProperty rdf:about="http://www.ontologydesignpatterns.org/cp/owl/list.owl#nextItem">
        <rdfs:subPropertyOf rdf:resource="http://www.ontologydesignpatterns.org/cp/owl/sequence.owl#directlyFollows"/>
        <rdfs:subPropertyOf>
            <rdf:Description>
                <owl:inverseOf rdf:resource="http://www.ontologydesignpatterns.org/cp/owl/sequence.owl#directlyPrecedes"/>
            </rdf:Description>
        </rdfs:subPropertyOf>
        <owl:inverseOf rdf:resource="http://www.ontologydesignpatterns.org/cp/owl/list.owl#previousItem"/>
        <rdf:type rdf:resource="http://www.w3.org/2002/07/owl#FunctionalProperty"/>
        <rdfs:domain rdf:resource="http://www.ontologydesignpatterns.org/cp/owl/list.owl#ListItem"/>
        <rdfs:range rdf:resource="http://www.ontologydesignpatterns.org/cp/owl/list.owl#ListItem"/>
        <rdfs:comment>next item - The link to the next item in a list (ordered collection)</rdfs:comment>
        <rdfs:label>next item</rdfs:label>
    </owl:ObjectProperty>
    


    <!-- http://www.ontologydesignpatterns.org/cp/owl/list.owl#previousItem -->

    <owl:ObjectProperty rdf:about="http://www.ontologydesignpatterns.org/cp/owl/list.owl#previousItem">
        <rdfs:subPropertyOf rdf:resource="http://www.ontologydesignpatterns.org/cp/owl/sequence.owl#directlyPrecedes"/>
        <rdfs:subPropertyOf>
            <rdf:Description>
                <owl:inverseOf rdf:resource="http://www.ontologydesignpatterns.org/cp/owl/sequence.owl#directlyFollows"/>
            </rdf:Description>
        </rdfs:subPropertyOf>
        <rdf:type rdf:resource="http://www.w3.org/2002/07/owl#FunctionalProperty"/>
        <rdfs:domain rdf:resource="http://www.ontologydesignpatterns.org/cp/owl/list.owl#ListItem"/>
        <rdfs:range rdf:resource="http://www.ontologydesignpatterns.org/cp/owl/list.owl#ListItem"/>
        <rdfs:comment>previous item - The link to the previous item in a list (ordered collection)</rdfs:comment>
        <rdfs:label>previous item</rdfs:label>
    </owl:ObjectProperty>
    


    <!-- http://www.ontologydesignpatterns.org/cp/owl/partof.owl#hasPart -->

    <owl:ObjectProperty rdf:about="http://www.ontologydesignpatterns.org/cp/owl/partof.owl#hasPart">
        <owl:inverseOf rdf:resource="http://www.ontologydesignpatterns.org/cp/owl/partof.owl#isPartOf"/>
        <rdf:type rdf:resource="http://www.w3.org/2002/07/owl#TransitiveProperty"/>
        <rdfs:domain rdf:resource="http://www.semanticweb.org/annag/ontologies/2024/1/ontoHorses#AreaGeografica"/>
        <rdfs:domain rdf:resource="http://www.w3.org/2002/07/owl#Thing"/>
        <rdfs:range rdf:resource="http://www.semanticweb.org/annag/ontologies/2024/1/ontoHorses#AreaGeografica"/>
        <rdfs:range rdf:resource="http://www.w3.org/2002/07/owl#Thing"/>
        <rdfs:comment>A transitive relation expressing parthood between any entities, e.g. &apos;the human body has a brain as part&apos;. When specializing this pattern, take care of restricting the domain and range appropriately, since it could be counterintuitive to use this relation arbitrarily, e.g. between animals and planets. For an intransitive partof pattern, see &apos;componency&apos;.</rdfs:comment>
        <rdfs:isDefinedBy rdf:resource="http://www.ontologydesignpatterns.org/cp/owl/partof.owl"/>
        <rdfs:label xml:lang="en">has part</rdfs:label>
    </owl:ObjectProperty>
    


    <!-- http://www.ontologydesignpatterns.org/cp/owl/partof.owl#isPartOf -->

    <owl:ObjectProperty rdf:about="http://www.ontologydesignpatterns.org/cp/owl/partof.owl#isPartOf">
        <rdf:type rdf:resource="http://www.w3.org/2002/07/owl#TransitiveProperty"/>
        <rdfs:domain rdf:resource="http://www.semanticweb.org/annag/ontologies/2024/1/ontoHorses#AreaGeografica"/>
        <rdfs:domain rdf:resource="http://www.w3.org/2002/07/owl#Thing"/>
        <rdfs:range rdf:resource="http://www.semanticweb.org/annag/ontologies/2024/1/ontoHorses#AreaGeografica"/>
        <rdfs:range rdf:resource="http://www.w3.org/2002/07/owl#Thing"/>
        <rdfs:comment>A transitive relation expressing parthood between any entities, e.g. &apos;brain is a part of the human body&apos;. When specializing this pattern, take care of restricting the domain and range appropriately, since it could be counterintuitive to use this relation arbitrarily, e.g. between animals and planets. For an intransitive partof pattern, see &apos;componency&apos;.</rdfs:comment>
        <rdfs:isDefinedBy rdf:resource="http://www.ontologydesignpatterns.org/cp/owl/partof.owl"/>
        <rdfs:label xml:lang="en">is part of</rdfs:label>
    </owl:ObjectProperty>
    


    <!-- http://www.ontologydesignpatterns.org/cp/owl/price.owl#hasCurrency -->

    <owl:ObjectProperty rdf:about="http://www.ontologydesignpatterns.org/cp/owl/price.owl#hasCurrency">
        <rdfs:domain rdf:resource="http://www.ontologydesignpatterns.org/cp/owl/price.owl#Price"/>
        <rdfs:range rdf:resource="http://www.ontologydesignpatterns.org/cp/owl/price.owl#Currency"/>
        <rdfs:isDefinedBy rdf:resource="http://www.ontologydesignpatterns.org/cp/owl/price.owl"/>
        <rdfs:label xml:lang="en">has currency</rdfs:label>
    </owl:ObjectProperty>
    


    <!-- http://www.ontologydesignpatterns.org/cp/owl/price.owl#hasPrice -->

    <owl:ObjectProperty rdf:about="http://www.ontologydesignpatterns.org/cp/owl/price.owl#hasPrice">
        <owl:inverseOf rdf:resource="http://www.ontologydesignpatterns.org/cp/owl/price.owl#isPriceOf"/>
        <rdfs:domain rdf:resource="http://www.semanticweb.org/annag/ontologies/2024/1/ontoHorses#Cavallo"/>
        <rdfs:domain rdf:resource="http://www.w3.org/2002/07/owl#Thing"/>
        <rdfs:range rdf:resource="http://www.ontologydesignpatterns.org/cp/owl/price.owl#Price"/>
        <rdfs:isDefinedBy rdf:resource="http://www.ontologydesignpatterns.org/cp/owl/price.owl"/>
        <rdfs:label xml:lang="en">has price</rdfs:label>
    </owl:ObjectProperty>
    


    <!-- http://www.ontologydesignpatterns.org/cp/owl/price.owl#isPriceOf -->

    <owl:ObjectProperty rdf:about="http://www.ontologydesignpatterns.org/cp/owl/price.owl#isPriceOf">
        <rdfs:domain rdf:resource="http://www.ontologydesignpatterns.org/cp/owl/price.owl#Price"/>
        <rdfs:range rdf:resource="http://www.w3.org/2002/07/owl#Thing"/>
        <rdfs:isDefinedBy rdf:resource="http://www.ontologydesignpatterns.org/cp/owl/price.owl"/>
        <rdfs:label xml:lang="en">is price of</rdfs:label>
    </owl:ObjectProperty>
    


    <!-- http://www.ontologydesignpatterns.org/cp/owl/sequence.owl#directlyFollows -->

    <owl:ObjectProperty rdf:about="http://www.ontologydesignpatterns.org/cp/owl/sequence.owl#directlyFollows">
        <rdfs:subPropertyOf rdf:resource="http://www.ontologydesignpatterns.org/cp/owl/sequence.owl#follows"/>
        <rdfs:subPropertyOf>
            <rdf:Description>
                <owl:inverseOf rdf:resource="http://www.ontologydesignpatterns.org/cp/owl/sequence.owl#precedes"/>
            </rdf:Description>
        </rdfs:subPropertyOf>
        <owl:inverseOf rdf:resource="http://www.ontologydesignpatterns.org/cp/owl/sequence.owl#directlyPrecedes"/>
        <rdfs:domain rdf:resource="http://www.w3.org/2002/07/owl#Thing"/>
        <rdfs:range rdf:resource="http://www.w3.org/2002/07/owl#Thing"/>
        <rdfs:comment>The intransitive follows relation. For example, Wednesday directly precedes Thursday. Directness of precedence depends on the designer conceptualization.</rdfs:comment>
        <rdfs:isDefinedBy rdf:resource="http://www.ontologydesignpatterns.org/cp/owl/sequence.owl"/>
        <rdfs:label xml:lang="en">directly follows</rdfs:label>
        <rdfs:label xml:lang="it">segue direttamente</rdfs:label>
    </owl:ObjectProperty>
    


    <!-- http://www.ontologydesignpatterns.org/cp/owl/sequence.owl#directlyPrecedes -->

    <owl:ObjectProperty rdf:about="http://www.ontologydesignpatterns.org/cp/owl/sequence.owl#directlyPrecedes">
        <rdfs:subPropertyOf rdf:resource="http://www.ontologydesignpatterns.org/cp/owl/sequence.owl#precedes"/>
        <rdfs:subPropertyOf>
            <rdf:Description>
                <owl:inverseOf rdf:resource="http://www.ontologydesignpatterns.org/cp/owl/sequence.owl#follows"/>
            </rdf:Description>
        </rdfs:subPropertyOf>
        <rdfs:domain rdf:resource="http://www.w3.org/2002/07/owl#Thing"/>
        <rdfs:range rdf:resource="http://www.w3.org/2002/07/owl#Thing"/>
        <rdfs:comment>The intransitive precedes relation. For example, Monday directly precedes Tuesday. Directness of precedence depends on the designer conceptualization.</rdfs:comment>
        <rdfs:isDefinedBy rdf:resource="http://www.ontologydesignpatterns.org/cp/owl/sequence.owl"/>
        <rdfs:label xml:lang="en">directly precedes</rdfs:label>
        <rdfs:label xml:lang="it">precede direttamente</rdfs:label>
    </owl:ObjectProperty>
    


    <!-- http://www.ontologydesignpatterns.org/cp/owl/sequence.owl#follows -->

    <owl:ObjectProperty rdf:about="http://www.ontologydesignpatterns.org/cp/owl/sequence.owl#follows">
        <owl:inverseOf rdf:resource="http://www.ontologydesignpatterns.org/cp/owl/sequence.owl#precedes"/>
        <rdf:type rdf:resource="http://www.w3.org/2002/07/owl#TransitiveProperty"/>
        <rdfs:domain rdf:resource="http://www.w3.org/2002/07/owl#Thing"/>
        <rdfs:range rdf:resource="http://www.w3.org/2002/07/owl#Thing"/>
        <rdfs:comment>A relation between entities, expressing a &apos;sequence&apos; schema. 
E.g. &apos;year 2000 follows 1999&apos;, &apos;preparing coffee&apos; follows &apos;deciding what coffee to use&apos;, &apos;II World War follows I World War&apos;, etc. 
It can be used between tasks, processes or time intervals, and subproperties would fit best in order to distinguish the different uses.</rdfs:comment>
        <rdfs:isDefinedBy rdf:resource="http://www.ontologydesignpatterns.org/cp/owl/sequence.owl"/>
        <rdfs:label xml:lang="en">follows</rdfs:label>
        <rdfs:label xml:lang="it">segue</rdfs:label>
    </owl:ObjectProperty>
    


    <!-- http://www.ontologydesignpatterns.org/cp/owl/sequence.owl#precedes -->

    <owl:ObjectProperty rdf:about="http://www.ontologydesignpatterns.org/cp/owl/sequence.owl#precedes">
        <rdf:type rdf:resource="http://www.w3.org/2002/07/owl#TransitiveProperty"/>
        <rdfs:domain rdf:resource="http://www.w3.org/2002/07/owl#Thing"/>
        <rdfs:range rdf:resource="http://www.w3.org/2002/07/owl#Thing"/>
        <rdfs:comment>A relation between entities, expressing a &apos;sequence&apos; schema. 
E.g. &apos;year 1999 precedes 2000&apos;, &apos;deciding what coffee to use&apos; precedes &apos;preparing coffee&apos;, &apos;World War II follows World War I&apos;, &apos;in the Milan to Rome autoroute, Bologna precedes Florence&apos;, etc.
It can then be used between tasks, processes, time intervals, spatially locate objects, situations, etc. 
Subproperties can be defined in order to distinguish the different uses.</rdfs:comment>
        <rdfs:isDefinedBy rdf:resource="http://www.ontologydesignpatterns.org/cp/owl/sequence.owl"/>
        <rdfs:label xml:lang="it">precede</rdfs:label>
        <rdfs:label xml:lang="en">precedes</rdfs:label>
    </owl:ObjectProperty>
    


    <!-- http://www.semanticweb.org/annag/ontologies/2024/1/ontoHorses#adattoAlConseguimentoDi -->

    <owl:ObjectProperty rdf:about="http://www.semanticweb.org/annag/ontologies/2024/1/ontoHorses#adattoAlConseguimentoDi">
        <rdfs:domain rdf:resource="http://www.semanticweb.org/annag/ontologies/2024/1/ontoHorses#Cavallo"/>
        <rdfs:range rdf:resource="http://www.semanticweb.org/annag/ontologies/2024/1/ontoHorses#Patente"/>
        <owl:propertyChainAxiom rdf:parseType="Collection">
            <rdf:Description rdf:about="http://www.semanticweb.org/annag/ontologies/2024/1/ontoHorses#gareggiaNelleCategorieDiSalto"/>
            <rdf:Description rdf:about="http://www.semanticweb.org/annag/ontologies/2024/1/ontoHorses#permetteIlConseguimentoDi"/>
        </owl:propertyChainAxiom>
        <rdfs:comment xml:lang="en">Property that expresses the relationship between the horse&apos;s sporting performance and the riding licences it allows to achieve</rdfs:comment>
        <rdfs:comment xml:lang="it">Proprietà che esprime la relazione tra le prestazioni sportive del cavallo e le autorizzazioni a montare che permette di conseguire</rdfs:comment>
        <rdfs:label xml:lang="en">suitable for achieving</rdfs:label>
        <rdfs:label>adatto al conseguimento di</rdfs:label>
    </owl:ObjectProperty>
    


    <!-- http://www.semanticweb.org/annag/ontologies/2024/1/ontoHorses#consegue -->

    <owl:ObjectProperty rdf:about="http://www.semanticweb.org/annag/ontologies/2024/1/ontoHorses#consegue">
        <owl:inverseOf rdf:resource="http://www.semanticweb.org/annag/ontologies/2024/1/ontoHorses#vieneConseguitoDa"/>
        <rdfs:domain rdf:resource="http://www.semanticweb.org/annag/ontologies/2024/1/ontoHorses#Cavaliere"/>
        <rdfs:range rdf:resource="http://www.semanticweb.org/annag/ontologies/2024/1/ontoHorses#Patente"/>
        <rdfs:comment xml:lang="en">Property that expresses the relationship between the rider&apos;s experience and the riding licences he can achieve</rdfs:comment>
        <rdfs:comment xml:lang="it">Proprietà che esprime la relazione tra l&apos;esperienza del cavaliere e l&apos;&lt;utorizzazioni a montare che può conseguire</rdfs:comment>
        <rdfs:label xml:lang="en">achieve</rdfs:label>
        <rdfs:label xml:lang="it">consegue</rdfs:label>
    </owl:ObjectProperty>
    


    <!-- http://www.semanticweb.org/annag/ontologies/2024/1/ontoHorses#entitàWikidata -->

    <owl:ObjectProperty rdf:about="http://www.semanticweb.org/annag/ontologies/2024/1/ontoHorses#entitàWikidata">
        <rdf:type rdf:resource="http://www.w3.org/2002/07/owl#FunctionalProperty"/>
        <rdf:type rdf:resource="http://www.w3.org/2002/07/owl#InverseFunctionalProperty"/>
        <rdfs:domain rdf:resource="http://www.semanticweb.org/annag/ontologies/2024/1/ontoHorses#RazzaCavallo"/>
        <rdfs:range rdf:resource="http://www.w3.org/2002/07/owl#Thing"/>
        <rdfs:comment xml:lang="it">La corrispondente entità su Wikidata</rdfs:comment>
        <rdfs:comment xml:lang="en">The corrispondig entity on Wikidata</rdfs:comment>
        <rdfs:label xml:lang="it">Entità Wikidata</rdfs:label>
        <rdfs:label xml:lang="en">Wikidata Entity</rdfs:label>
    </owl:ObjectProperty>
    


    <!-- http://www.semanticweb.org/annag/ontologies/2024/1/ontoHorses#gareggiaNellaCategoriaDiDressage -->

    <owl:ObjectProperty rdf:about="http://www.semanticweb.org/annag/ontologies/2024/1/ontoHorses#gareggiaNellaCategoriaDiDressage">
        <rdfs:domain rdf:resource="http://dbpedia.org/ontology/horse"/>
        <rdfs:range rdf:resource="http://www.semanticweb.org/annag/ontologies/2024/1/ontoHorses#CategorieDressage"/>
        <rdfs:comment xml:lang="en">Property that expresses the category of  dressage competition in which the horse usually participates.</rdfs:comment>
        <rdfs:comment xml:lang="it">Proprietà che esprime la categoria di gara di dressage alla quale il cavallo di solito partecipa</rdfs:comment>
        <rdfs:label xml:lang="it">gareggia nella categoria di dressage</rdfs:label>
        <rdfs:label xml:lang="en">take part to dressage category</rdfs:label>
    </owl:ObjectProperty>
    


    <!-- http://www.semanticweb.org/annag/ontologies/2024/1/ontoHorses#gareggiaNelleCategorieDiSalto -->

    <owl:ObjectProperty rdf:about="http://www.semanticweb.org/annag/ontologies/2024/1/ontoHorses#gareggiaNelleCategorieDiSalto">
        <rdfs:domain rdf:resource="http://www.semanticweb.org/annag/ontologies/2024/1/ontoHorses#Cavallo"/>
        <rdfs:range rdf:resource="http://www.semanticweb.org/annag/ontologies/2024/1/ontoHorses#CategorieDiSalto"/>
        <rdfs:comment xml:lang="en">Property that expresses the category of  jumping competition in which the horse usually participates.</rdfs:comment>
        <rdfs:comment xml:lang="it">Proprietà che esprime la categoria di gare di salto ad ostacoli alle quali il cavallo di solito partecipa.</rdfs:comment>
        <rdfs:label xml:lang="it">gareggia nella categoria di salto ostacoli</rdfs:label>
        <rdfs:label xml:lang="en">take part to jumping categories</rdfs:label>
    </owl:ObjectProperty>
    


    <!-- http://www.semanticweb.org/annag/ontologies/2024/1/ontoHorses#haClassificazioneMorfologica -->

    <owl:ObjectProperty rdf:about="http://www.semanticweb.org/annag/ontologies/2024/1/ontoHorses#haClassificazioneMorfologica">
        <rdfs:domain rdf:resource="http://www.semanticweb.org/annag/ontologies/2024/1/ontoHorses#RazzaCavallo"/>
        <rdfs:range rdf:resource="http://www.semanticweb.org/annag/ontologies/2024/1/ontoHorses#RazzaCavallo"/>
        <rdfs:comment xml:lang="en">Property that expresses the morphological type to which the horse breed belongs</rdfs:comment>
        <rdfs:comment xml:lang="it">Proprietà che esprime il tipo morfologico al quale la razza di cavallo appartiene</rdfs:comment>
        <rdfs:label xml:lang="it">ha classificazione morfologica</rdfs:label>
        <rdfs:label xml:lang="en">has morphological classification</rdfs:label>
    </owl:ObjectProperty>
    


    <!-- http://www.semanticweb.org/annag/ontologies/2024/1/ontoHorses#haIndole -->

    <owl:ObjectProperty rdf:about="http://www.semanticweb.org/annag/ontologies/2024/1/ontoHorses#haIndole">
        <rdf:type rdf:resource="http://www.w3.org/2002/07/owl#FunctionalProperty"/>
        <rdfs:domain rdf:resource="http://www.semanticweb.org/annag/ontologies/2024/1/ontoHorses#RazzaCavallo"/>
        <rdfs:range rdf:resource="http://www.semanticweb.org/annag/ontologies/2024/1/ontoHorses#Indole"/>
        <rdfs:comment xml:lang="en">Property that expresses the temperament of a horse breed</rdfs:comment>
        <rdfs:comment xml:lang="it">Proprietà che esprime il temperamento di una razza di cavallo</rdfs:comment>
        <rdfs:label xml:lang="it">ha indole</rdfs:label>
        <rdfs:label xml:lang="en">has temperament</rdfs:label>
    </owl:ObjectProperty>
    


    <!-- http://www.semanticweb.org/annag/ontologies/2024/1/ontoHorses#haNazionalità -->

    <owl:ObjectProperty rdf:about="http://www.semanticweb.org/annag/ontologies/2024/1/ontoHorses#haNazionalità">
        <rdfs:domain rdf:resource="http://www.semanticweb.org/annag/ontologies/2024/1/ontoHorses#RazzaCavallo"/>
        <rdfs:range rdf:resource="http://www.semanticweb.org/annag/ontologies/2024/1/ontoHorses#AreaGeografica"/>
        <owl:propertyChainAxiom rdf:parseType="Collection">
            <rdf:Description rdf:about="http://www.semanticweb.org/annag/ontologies/2024/1/ontoHorses#haRegioneDiOrigine"/>
            <rdf:Description rdf:about="http://www.ontologydesignpatterns.org/cp/owl/partof.owl#isPartOf"/>
        </owl:propertyChainAxiom>
        <rdfs:comment xml:lang="en">Property that expresses the nation of origin of a horse breed</rdfs:comment>
        <rdfs:comment xml:lang="it">Proprietà che esprime la nazionalità di una razza di cavallo</rdfs:comment>
        <rdfs:label xml:lang="en">has nationality</rdfs:label>
        <rdfs:label>ha nazionalità</rdfs:label>
    </owl:ObjectProperty>
    


    <!-- http://www.semanticweb.org/annag/ontologies/2024/1/ontoHorses#haRazza -->

    <owl:ObjectProperty rdf:about="http://www.semanticweb.org/annag/ontologies/2024/1/ontoHorses#haRazza">
        <rdf:type rdf:resource="http://www.w3.org/2002/07/owl#FunctionalProperty"/>
        <rdfs:domain rdf:resource="http://www.semanticweb.org/annag/ontologies/2024/1/ontoHorses#Cavallo"/>
        <rdfs:range rdf:resource="http://www.semanticweb.org/annag/ontologies/2024/1/ontoHorses#RazzaCavallo"/>
        <rdfs:comment xml:lang="en">Property that expresses the breed of a horse</rdfs:comment>
        <rdfs:comment xml:lang="it">Proprietà che esprime la razza di un cavallo</rdfs:comment>
        <rdfs:label xml:lang="it">ha razza</rdfs:label>
        <rdfs:label xml:lang="en">has breed</rdfs:label>
    </owl:ObjectProperty>
    


    <!-- http://www.semanticweb.org/annag/ontologies/2024/1/ontoHorses#haRegioneDiOrigine -->

    <owl:ObjectProperty rdf:about="http://www.semanticweb.org/annag/ontologies/2024/1/ontoHorses#haRegioneDiOrigine">
        <rdfs:domain rdf:resource="http://www.semanticweb.org/annag/ontologies/2024/1/ontoHorses#RazzaCavallo"/>
        <rdfs:range rdf:resource="http://www.semanticweb.org/annag/ontologies/2024/1/ontoHorses#AreaGeografica"/>
        <rdfs:comment xml:lang="en">Property that expresses the territory of origin of a horse breed</rdfs:comment>
        <rdfs:comment xml:lang="it">Proprietà che esprime il territorio di origine di una razza di cavallo</rdfs:comment>
        <rdfs:label xml:lang="it">ha Regione di origine</rdfs:label>
        <rdfs:label xml:lang="en">has region of origin</rdfs:label>
    </owl:ObjectProperty>
    


    <!-- http://www.semanticweb.org/annag/ontologies/2024/1/ontoHorses#permetteIlConseguimentoDi -->

    <owl:ObjectProperty rdf:about="http://www.semanticweb.org/annag/ontologies/2024/1/ontoHorses#permetteIlConseguimentoDi">
        <rdfs:domain rdf:resource="http://www.semanticweb.org/annag/ontologies/2024/1/ontoHorses#CategorieDiSalto"/>
        <rdfs:range rdf:resource="http://www.semanticweb.org/annag/ontologies/2024/1/ontoHorses#Patente"/>
        <rdfs:comment xml:lang="en">Property that expresses the relationship between the jumping categories in which a rider competes and the riding licences he can obtain. In particular, the C80 allows the obtaining of the patent; the C115 allows the achievement of the 1st degree and the C135 the 2nd degree,</rdfs:comment>
        <rdfs:comment xml:lang="it">Proprietà che esprime la relazione tra le categorie di salto ad ostacoli in cui un cavaliera gareggia e le autorizzazioni a montare che può conseguire. In particolare la C80 permette il conseguimento del brevetto; la C115 permette il conseguimento del 1° grado e la C135 del 2° grado</rdfs:comment>
        <rdfs:label xml:lang="en">allows the achievement of</rdfs:label>
        <rdfs:label xml:lang="it">permette il conseguiimento di</rdfs:label>
    </owl:ObjectProperty>
    


    <!-- http://www.semanticweb.org/annag/ontologies/2024/1/ontoHorses#possiede -->

    <owl:ObjectProperty rdf:about="http://www.semanticweb.org/annag/ontologies/2024/1/ontoHorses#possiede">
        <owl:inverseOf rdf:resource="http://www.semanticweb.org/annag/ontologies/2024/1/ontoHorses#èPossedutoDa"/>
        <rdfs:comment xml:lang="en">Inverse proprerty of &quot;is owned by&quot;</rdfs:comment>
        <rdfs:comment xml:lang="it">Proprietà inversa di &quot;è posseduto da&quot;</rdfs:comment>
        <rdfs:label xml:lang="en">is owner</rdfs:label>
        <rdfs:label xml:lang="it">possiede</rdfs:label>
    </owl:ObjectProperty>
    


    <!-- http://www.semanticweb.org/annag/ontologies/2024/1/ontoHorses#puòEssereImpiegataIn -->

    <owl:ObjectProperty rdf:about="http://www.semanticweb.org/annag/ontologies/2024/1/ontoHorses#puòEssereImpiegataIn">
        <rdfs:domain rdf:resource="http://www.semanticweb.org/annag/ontologies/2024/1/ontoHorses#RazzaCavallo"/>
        <rdfs:range rdf:resource="http://www.semanticweb.org/annag/ontologies/2024/1/ontoHorses#Impiego"/>
        <rdfs:comment xml:lang="en">Property that expresses the possible uses of a breed in work or sport</rdfs:comment>
        <rdfs:comment xml:lang="it">Proprietà che esprime i possibili impieghi di una razza nel lavoro o nello sport</rdfs:comment>
        <rdfs:label xml:lang="en">can be used in</rdfs:label>
        <rdfs:label xml:lang="it">può essere impiegata in</rdfs:label>
    </owl:ObjectProperty>
    


    <!-- http://www.semanticweb.org/annag/ontologies/2024/1/ontoHorses#vieneConseguitoDa -->

    <owl:ObjectProperty rdf:about="http://www.semanticweb.org/annag/ontologies/2024/1/ontoHorses#vieneConseguitoDa">
        <rdfs:domain rdf:resource="http://www.semanticweb.org/annag/ontologies/2024/1/ontoHorses#Patente"/>
        <rdfs:range rdf:resource="http://www.semanticweb.org/annag/ontologies/2024/1/ontoHorses#Cavaliere"/>
        <rdfs:comment xml:lang="en">Inverse property of &quot;achieve&quot;</rdfs:comment>
        <rdfs:comment xml:lang="it">Proprietà inversa di &quot;consegue&quot;</rdfs:comment>
        <rdfs:label xml:lang="en">is achieved by</rdfs:label>
        <rdfs:label xml:lang="it">viene conseguito da</rdfs:label>
    </owl:ObjectProperty>
    


    <!-- http://www.semanticweb.org/annag/ontologies/2024/1/ontoHorses#vieneUtilizzatoPer -->

    <owl:ObjectProperty rdf:about="http://www.semanticweb.org/annag/ontologies/2024/1/ontoHorses#vieneUtilizzatoPer">
        <rdfs:domain rdf:resource="http://www.semanticweb.org/annag/ontologies/2024/1/ontoHorses#Cavallo"/>
        <rdfs:range rdf:resource="http://www.semanticweb.org/annag/ontologies/2024/1/ontoHorses#Impiego"/>
        <rdfs:comment xml:lang="en">Property that expresses the use made of a horse in work or sporting activities.</rdfs:comment>
        <rdfs:comment xml:lang="it">Proprietà che esprime l&apos;utilizzo che viene fatto di un cavallo in attività lavorative o sportive.</rdfs:comment>
        <rdfs:label xml:lang="en">is used for</rdfs:label>
        <rdfs:label xml:lang="it">viene utilizzato per</rdfs:label>
    </owl:ObjectProperty>
    


    <!-- http://www.semanticweb.org/annag/ontologies/2024/1/ontoHorses#èAdattoPer -->

    <owl:ObjectProperty rdf:about="http://www.semanticweb.org/annag/ontologies/2024/1/ontoHorses#èAdattoPer">
        <rdfs:domain rdf:resource="http://www.semanticweb.org/annag/ontologies/2024/1/ontoHorses#Cavallo"/>
        <rdfs:range rdf:resource="http://www.semanticweb.org/annag/ontologies/2024/1/ontoHorses#Cavaliere"/>
        <owl:propertyChainAxiom rdf:parseType="Collection">
            <rdf:Description rdf:about="http://www.semanticweb.org/annag/ontologies/2024/1/ontoHorses#adattoAlConseguimentoDi"/>
            <rdf:Description rdf:about="http://www.semanticweb.org/annag/ontologies/2024/1/ontoHorses#vieneConseguitoDa"/>
        </owl:propertyChainAxiom>
        <rdfs:comment xml:lang="en">Property that expresses the suitability of a horse for the sporting abilities of a rider. Generally horses that are used in very high jumping categories are not suitable for inexperienced riders.</rdfs:comment>
        <rdfs:comment xml:lang="it">Proprietà che esprime l&apos;adeguatezza di un cavallo alle capacità sportive di un cavaliere. Generalmente cavalli che vengono utilizzati in categorie di salto molto alte non sono idonei a cavalieri poco esperti.</rdfs:comment>
        <rdfs:label xml:lang="en">is suitable for</rdfs:label>
        <rdfs:label xml:lang="it">è adatto per</rdfs:label>
    </owl:ObjectProperty>
    


    <!-- http://www.semanticweb.org/annag/ontologies/2024/1/ontoHorses#èPossedutoDa -->

    <owl:ObjectProperty rdf:about="http://www.semanticweb.org/annag/ontologies/2024/1/ontoHorses#èPossedutoDa">
        <rdfs:domain rdf:resource="http://www.semanticweb.org/annag/ontologies/2024/1/ontoHorses#Cavallo"/>
        <rdfs:range rdf:resource="http://www.semanticweb.org/annag/ontologies/2024/1/ontoHorses#Proprietario"/>
        <rdfs:comment xml:lang="en">Property that expresses the relationship between the horse for sale and the current owner</rdfs:comment>
        <rdfs:comment xml:lang="it">Proprietà che esprime la relazione tra il cavallo in vendita e l&apos;attuale proprietario</rdfs:comment>
        <rdfs:label xml:lang="en">is owned by</rdfs:label>
        <rdfs:label xml:lang="it">è posseduto da</rdfs:label>
    </owl:ObjectProperty>
    


    <!-- http://www.semanticweb.org/annag/ontologies/2024/1/ontoHorses#èScuderizzatoIn -->

    <owl:ObjectProperty rdf:about="http://www.semanticweb.org/annag/ontologies/2024/1/ontoHorses#èScuderizzatoIn">
        <rdfs:domain rdf:resource="http://www.semanticweb.org/annag/ontologies/2024/1/ontoHorses#Cavallo"/>
        <rdfs:range rdf:resource="http://www.semanticweb.org/annag/ontologies/2024/1/ontoHorses#AreaGeografica"/>
        <owl:propertyChainAxiom rdf:parseType="Collection">
            <rdf:Description rdf:about="http://www.semanticweb.org/annag/ontologies/2024/1/ontoHorses#èScuderizzatoInCittàDi"/>
            <rdf:Description rdf:about="http://www.ontologydesignpatterns.org/cp/owl/partof.owl#isPartOf"/>
        </owl:propertyChainAxiom>
        <rdfs:comment xml:lang="en">Property that expresses the geographic area in terms of the State or Region in which the horse is stabled.</rdfs:comment>
        <rdfs:comment xml:lang="it">Proprietà che esprime l&apos;area geografica in termini di Stato o Regione in cui il cavallo è scuderizzato.</rdfs:comment>
        <rdfs:label xml:lang="en">is stabled in</rdfs:label>
        <rdfs:label xml:lang="it">è scuderizzato in</rdfs:label>
    </owl:ObjectProperty>
    


    <!-- http://www.semanticweb.org/annag/ontologies/2024/1/ontoHorses#èScuderizzatoInCittàDi -->

    <owl:ObjectProperty rdf:about="http://www.semanticweb.org/annag/ontologies/2024/1/ontoHorses#èScuderizzatoInCittàDi">
        <rdf:type rdf:resource="http://www.w3.org/2002/07/owl#FunctionalProperty"/>
        <rdfs:domain rdf:resource="http://www.semanticweb.org/annag/ontologies/2024/1/ontoHorses#Cavallo"/>
        <rdfs:comment xml:lang="en">Property that expresses the city in which the horse is stabled</rdfs:comment>
        <rdfs:comment xml:lang="it">Proprietà che esprime la Città in cui il cavallo è scuderizzato</rdfs:comment>
        <rdfs:label xml:lang="en">is stabled in the City of</rdfs:label>
        <rdfs:label xml:lang="it">è scuderizzato in Città di</rdfs:label>
    </owl:ObjectProperty>
    


    <!-- 
    ///////////////////////////////////////////////////////////////////////////////////////
    //
    // Data properties
    //
    ///////////////////////////////////////////////////////////////////////////////////////
     -->

    


    <!-- http://www.ontologydesignpatterns.org/cp/owl/bag.owl#size -->

    <owl:DatatypeProperty rdf:about="http://www.ontologydesignpatterns.org/cp/owl/bag.owl#size">
        <rdfs:domain rdf:resource="http://www.ontologydesignpatterns.org/cp/owl/collectionentity.owl#Collection"/>
        <rdfs:range rdf:resource="http://www.w3.org/2001/XMLSchema#integer"/>
        <rdfs:comment>size - The number of items belonging to a collection</rdfs:comment>
        <rdfs:label>size</rdfs:label>
    </owl:DatatypeProperty>
    


    <!-- http://www.ontologydesignpatterns.org/cp/owl/price.owl#hasValue -->

    <owl:DatatypeProperty rdf:about="http://www.ontologydesignpatterns.org/cp/owl/price.owl#hasValue">
        <rdfs:domain rdf:resource="http://www.ontologydesignpatterns.org/cp/owl/price.owl#Price"/>
        <rdfs:range rdf:resource="http://www.w3.org/2001/XMLSchema#float"/>
    </owl:DatatypeProperty>
    


    <!-- http://www.semanticweb.org/annag/ontologies/2024/1/ontoHorses#altezzaGarrese -->

    <owl:DatatypeProperty rdf:about="http://www.semanticweb.org/annag/ontologies/2024/1/ontoHorses#altezzaGarrese">
        <rdfs:domain rdf:resource="http://www.semanticweb.org/annag/ontologies/2024/1/ontoHorses#Cavallo"/>
        <rdfs:range rdf:resource="http://www.w3.org/2001/XMLSchema#decimal"/>
        <schema:image rdf:resource="https://www.kramer.it/$WS/kraemer-pferdesport/websale8_shop-kraemer-pferdesport/benutzer/templates/ws-customer/Serviceseiten/images/content/blankets_ita.jpg"/>
        <rdfs:comment xml:lang="it">L&apos;altezza di un animale quadrupede si misura al garrese che è il punto più alto del dorso e si trova tra il collo e il tronco nella zona di incontro tra collo e scapole</rdfs:comment>
        <rdfs:comment xml:lang="en">The height of a quadruped animal is measured at the withers which is the highest point of the back and is located between the neck and the trunk in the area where the neck and shoulder blades meet</rdfs:comment>
        <rdfs:label xml:lang="en">Height at the withers [cm]</rdfs:label>
        <rdfs:label>altezza al garrese [cm]</rdfs:label>
    </owl:DatatypeProperty>
    


    <!-- http://www.semanticweb.org/annag/ontologies/2024/1/ontoHorses#altezzaMediaGarrese -->

    <owl:DatatypeProperty rdf:about="http://www.semanticweb.org/annag/ontologies/2024/1/ontoHorses#altezzaMediaGarrese">
        <rdfs:domain rdf:resource="http://www.semanticweb.org/annag/ontologies/2024/1/ontoHorses#RazzaCavallo"/>
        <rdfs:range rdf:resource="http://www.w3.org/2001/XMLSchema#decimal"/>
        <rdfs:comment xml:lang="en">Average height at the withers of a horse breed</rdfs:comment>
        <rdfs:comment xml:lang="it">Valore medio dell&apos;altezza al garrese di una razza di cavallo</rdfs:comment>
        <rdfs:label xml:lang="en">average height at the withers [cm]</rdfs:label>
        <rdfs:label>altezza media al garrese [cm]</rdfs:label>
    </owl:DatatypeProperty>
    


    <!-- http://www.semanticweb.org/annag/ontologies/2024/1/ontoHorses#eta -->

    <owl:DatatypeProperty rdf:about="http://www.semanticweb.org/annag/ontologies/2024/1/ontoHorses#eta">
        <rdf:type rdf:resource="http://www.w3.org/2002/07/owl#FunctionalProperty"/>
        <rdfs:domain rdf:resource="http://www.semanticweb.org/annag/ontologies/2024/1/ontoHorses#Cavallo"/>
        <rdfs:range rdf:resource="http://www.w3.org/2001/XMLSchema#integer"/>
        <rdfs:comment xml:lang="en">age of horse for sale</rdfs:comment>
        <rdfs:comment xml:lang="it">età del cavallo in vendita</rdfs:comment>
        <rdfs:label xml:lang="en">age</rdfs:label>
        <rdfs:label xml:lang="it">età</rdfs:label>
    </owl:DatatypeProperty>
    


    <!-- http://www.semanticweb.org/annag/ontologies/2024/1/ontoHorses#haColoreMantello -->

    <owl:DatatypeProperty rdf:about="http://www.semanticweb.org/annag/ontologies/2024/1/ontoHorses#haColoreMantello">
        <rdfs:domain rdf:resource="http://www.semanticweb.org/annag/ontologies/2024/1/ontoHorses#RazzaCavallo"/>
        <rdfs:range>
            <rdfs:Datatype>
                <owl:oneOf>
                    <rdf:Description>
                        <rdf:type rdf:resource="http://www.w3.org/1999/02/22-rdf-syntax-ns#List"/>
                        <rdf:first>apaloosa</rdf:first>
                        <rdf:rest>
                            <rdf:Description>
                                <rdf:type rdf:resource="http://www.w3.org/1999/02/22-rdf-syntax-ns#List"/>
                                <rdf:first>baio</rdf:first>
                                <rdf:rest>
                                    <rdf:Description>
                                        <rdf:type rdf:resource="http://www.w3.org/1999/02/22-rdf-syntax-ns#List"/>
                                        <rdf:first>crema</rdf:first>
                                        <rdf:rest>
                                            <rdf:Description>
                                                <rdf:type rdf:resource="http://www.w3.org/1999/02/22-rdf-syntax-ns#List"/>
                                                <rdf:first>falbo</rdf:first>
                                                <rdf:rest>
                                                    <rdf:Description>
                                                        <rdf:type rdf:resource="http://www.w3.org/1999/02/22-rdf-syntax-ns#List"/>
                                                        <rdf:first>grigio</rdf:first>
                                                        <rdf:rest>
                                                            <rdf:Description>
                                                                <rdf:type rdf:resource="http://www.w3.org/1999/02/22-rdf-syntax-ns#List"/>
                                                                <rdf:first>isabella</rdf:first>
                                                                <rdf:rest>
                                                                    <rdf:Description>
                                                                        <rdf:type rdf:resource="http://www.w3.org/1999/02/22-rdf-syntax-ns#List"/>
                                                                        <rdf:first>mantello coniugato</rdf:first>
                                                                        <rdf:rest>
                                                                            <rdf:Description>
                                                                                <rdf:type rdf:resource="http://www.w3.org/1999/02/22-rdf-syntax-ns#List"/>
                                                                                <rdf:first>morello</rdf:first>
                                                                                <rdf:rest>
                                                                                    <rdf:Description>
                                                                                        <rdf:type rdf:resource="http://www.w3.org/1999/02/22-rdf-syntax-ns#List"/>
                                                                                        <rdf:first>palomino</rdf:first>
                                                                                        <rdf:rest>
                                                                                            <rdf:Description>
                                                                                                <rdf:type rdf:resource="http://www.w3.org/1999/02/22-rdf-syntax-ns#List"/>
                                                                                                <rdf:first>pezzato</rdf:first>
                                                                                                <rdf:rest>
                                                                                                    <rdf:Description>
                                                                                                        <rdf:type rdf:resource="http://www.w3.org/1999/02/22-rdf-syntax-ns#List"/>
                                                                                                        <rdf:first>roano</rdf:first>
                                                                                                        <rdf:rest>
                                                                                                            <rdf:Description>
                                                                                                                <rdf:type rdf:resource="http://www.w3.org/1999/02/22-rdf-syntax-ns#List"/>
                                                                                                                <rdf:first>sauro</rdf:first>
                                                                                                                <rdf:rest>
                                                                                                                    <rdf:Description>
                                                                                                                        <rdf:type rdf:resource="http://www.w3.org/1999/02/22-rdf-syntax-ns#List"/>
                                                                                                                        <rdf:first>sorcino</rdf:first>
                                                                                                                        <rdf:rest>
                                                                                                                            <rdf:Description>
                                                                                                                                <rdf:type rdf:resource="http://www.w3.org/1999/02/22-rdf-syntax-ns#List"/>
                                                                                                                                <rdf:first>ubero</rdf:first>
                                                                                                                                <rdf:rest rdf:resource="http://www.w3.org/1999/02/22-rdf-syntax-ns#nil"/>
                                                                                                                            </rdf:Description>
                                                                                                                        </rdf:rest>
                                                                                                                    </rdf:Description>
                                                                                                                </rdf:rest>
                                                                                                            </rdf:Description>
                                                                                                        </rdf:rest>
                                                                                                    </rdf:Description>
                                                                                                </rdf:rest>
                                                                                            </rdf:Description>
                                                                                        </rdf:rest>
                                                                                    </rdf:Description>
                                                                                </rdf:rest>
                                                                            </rdf:Description>
                                                                        </rdf:rest>
                                                                    </rdf:Description>
                                                                </rdf:rest>
                                                            </rdf:Description>
                                                        </rdf:rest>
                                                    </rdf:Description>
                                                </rdf:rest>
                                            </rdf:Description>
                                        </rdf:rest>
                                    </rdf:Description>
                                </rdf:rest>
                            </rdf:Description>
                        </rdf:rest>
                    </rdf:Description>
                </owl:oneOf>
            </rdfs:Datatype>
        </rdfs:range>
        <rdfs:comment xml:lang="it">Insieme dei colori del mantello ammessi per una razza di cavallo</rdfs:comment>
        <rdfs:comment xml:lang="en">Set of coat colors allowed for a horse breed</rdfs:comment>
        <rdfs:label xml:lang="en">admittet coat colors</rdfs:label>
        <rdfs:label xml:lang="it">ha colori mantello ammessi</rdfs:label>
    </owl:DatatypeProperty>
    


    <!-- http://www.semanticweb.org/annag/ontologies/2024/1/ontoHorses#haSesso -->

    <owl:DatatypeProperty rdf:about="http://www.semanticweb.org/annag/ontologies/2024/1/ontoHorses#haSesso">
        <rdf:type rdf:resource="http://www.w3.org/2002/07/owl#FunctionalProperty"/>
        <rdfs:domain rdf:resource="http://www.semanticweb.org/annag/ontologies/2024/1/ontoHorses#Cavallo"/>
        <rdfs:range>
            <rdfs:Datatype>
                <owl:oneOf>
                    <rdf:Description>
                        <rdf:type rdf:resource="http://www.w3.org/1999/02/22-rdf-syntax-ns#List"/>
                        <rdf:first>castrone</rdf:first>
                        <rdf:rest>
                            <rdf:Description>
                                <rdf:type rdf:resource="http://www.w3.org/1999/02/22-rdf-syntax-ns#List"/>
                                <rdf:first>femmina</rdf:first>
                                <rdf:rest>
                                    <rdf:Description>
                                        <rdf:type rdf:resource="http://www.w3.org/1999/02/22-rdf-syntax-ns#List"/>
                                        <rdf:first>maschio</rdf:first>
                                        <rdf:rest rdf:resource="http://www.w3.org/1999/02/22-rdf-syntax-ns#nil"/>
                                    </rdf:Description>
                                </rdf:rest>
                            </rdf:Description>
                        </rdf:rest>
                    </rdf:Description>
                </owl:oneOf>
            </rdfs:Datatype>
        </rdfs:range>
        <rdfs:comment xml:lang="en">Horse sex for sale</rdfs:comment>
        <rdfs:comment>Sesso del cavallo in vendita</rdfs:comment>
        <rdfs:label xml:lang="it">ha sesso</rdfs:label>
        <rdfs:label xml:lang="en">has sex</rdfs:label>
    </owl:DatatypeProperty>
    


    <!-- http://www.semanticweb.org/annag/ontologies/2024/1/ontoHorses#nomeCavallo -->

    <owl:DatatypeProperty rdf:about="http://www.semanticweb.org/annag/ontologies/2024/1/ontoHorses#nomeCavallo">
        <rdfs:domain rdf:resource="http://www.semanticweb.org/annag/ontologies/2024/1/ontoHorses#Cavallo"/>
        <rdfs:range rdf:resource="http://www.w3.org/2001/XMLSchema#string"/>
        <rdfs:comment xml:lang="en">Horse name for sale</rdfs:comment>
        <rdfs:comment xml:lang="it">Nome del cavallo in vendita</rdfs:comment>
        <rdfs:label xml:lang="en">Horse name</rdfs:label>
        <rdfs:label xml:lang="it">Nome del cavallo</rdfs:label>
    </owl:DatatypeProperty>
    


    <!-- http://www.semanticweb.org/annag/ontologies/2024/1/ontoHorses#pesoMedio -->

    <owl:DatatypeProperty rdf:about="http://www.semanticweb.org/annag/ontologies/2024/1/ontoHorses#pesoMedio">
        <rdf:type rdf:resource="http://www.w3.org/2002/07/owl#FunctionalProperty"/>
        <rdfs:domain rdf:resource="http://www.semanticweb.org/annag/ontologies/2024/1/ontoHorses#RazzaCavallo"/>
        <rdfs:range rdf:resource="http://www.w3.org/2001/XMLSchema#integer"/>
        <rdfs:comment xml:lang="en">Average mass value of a specific horse breed</rdfs:comment>
        <rdfs:comment xml:lang="it">Valore medio della massa di una specifica razza di cavallo</rdfs:comment>
        <rdfs:label xml:lang="en">medium weight [Kg]</rdfs:label>
        <rdfs:label xml:lang="it">peso medio [Kg]</rdfs:label>
    </owl:DatatypeProperty>
    


    <!-- 
    ///////////////////////////////////////////////////////////////////////////////////////
    //
    // Classes
    //
    ///////////////////////////////////////////////////////////////////////////////////////
     -->

    


    <!-- http://dbpedia.org/ontology/HorseRider -->

    <owl:Class rdf:about="http://dbpedia.org/ontology/HorseRider">
        <owl:equivalentClass rdf:resource="http://www.semanticweb.org/annag/ontologies/2024/1/ontoHorses#Cavaliere"/>
        <rdfs:subClassOf rdf:resource="http://www.semanticweb.org/annag/ontologies/2024/1/ontoHorses#Persona"/>
        <rdfs:subClassOf rdf:resource="http://xmlns.com/foaf/0.1/person"/>
    </owl:Class>
    


    <!-- http://dbpedia.org/ontology/horse -->

    <owl:Class rdf:about="http://dbpedia.org/ontology/horse">
        <owl:equivalentClass rdf:resource="http://www.semanticweb.org/annag/ontologies/2024/1/ontoHorses#Cavallo"/>
    </owl:Class>
    


    <!-- http://dbpedia.org/ontology/horseRidingDiscipline -->

    <owl:Class rdf:about="http://dbpedia.org/ontology/horseRidingDiscipline">
        <owl:equivalentClass rdf:resource="http://www.semanticweb.org/annag/ontologies/2024/1/ontoHorses#Sella"/>
        <rdfs:subClassOf rdf:resource="http://www.semanticweb.org/annag/ontologies/2024/1/ontoHorses#Impiego"/>
    </owl:Class>
    


    <!-- http://schema.org/Place -->

    <owl:Class rdf:about="http://schema.org/Place">
        <owl:equivalentClass rdf:resource="http://www.semanticweb.org/annag/ontologies/2024/1/ontoHorses#AreaGeografica"/>
    </owl:Class>
    


    <!-- http://www.ontologydesignpatterns.org/cp/owl/bag.owl#Bag -->

    <owl:Class rdf:about="http://www.ontologydesignpatterns.org/cp/owl/bag.owl#Bag">
        <rdfs:subClassOf rdf:resource="http://www.ontologydesignpatterns.org/cp/owl/collectionentity.owl#Collection"/>
        <rdfs:subClassOf rdf:resource="http://www.semanticweb.org/annag/ontologies/2024/1/ontoHorses#CatalogoAutorizzazioniAMontareFise"/>
        <rdfs:comment>Bag - Collection that can have a number of copies of each object</rdfs:comment>
        <rdfs:label>(collections) Bag</rdfs:label>
    </owl:Class>
    


    <!-- http://www.ontologydesignpatterns.org/cp/owl/bag.owl#Item -->

    <owl:Class rdf:about="http://www.ontologydesignpatterns.org/cp/owl/bag.owl#Item">
        <rdfs:subClassOf rdf:resource="http://www.w3.org/2002/07/owl#Thing"/>
        <rdfs:subClassOf>
            <owl:Restriction>
                <owl:onProperty rdf:resource="http://www.ontologydesignpatterns.org/cp/owl/bag.owl#itemContent"/>
                <owl:cardinality rdf:datatype="http://www.w3.org/2001/XMLSchema#nonNegativeInteger">1</owl:cardinality>
            </owl:Restriction>
        </rdfs:subClassOf>
        <owl:disjointWith rdf:resource="http://www.ontologydesignpatterns.org/cp/owl/collectionentity.owl#Collection"/>
        <rdfs:comment>Item - Element belonging to a Bag</rdfs:comment>
        <rdfs:label>item</rdfs:label>
    </owl:Class>
    


    <!-- http://www.ontologydesignpatterns.org/cp/owl/collectionentity.owl#Collection -->

    <owl:Class rdf:about="http://www.ontologydesignpatterns.org/cp/owl/collectionentity.owl#Collection">
        <owl:equivalentClass rdf:resource="http://www.semanticweb.org/annag/ontologies/2024/1/ontoHorses#CatalogoAutorizzazioniAMontareFise"/>
        <rdfs:comment>Any container for entities that share one or more common properties. E.g. &quot;stone objects&quot;, &quot;the nurses&quot;, &quot;the Louvre Aegyptian collection&quot;. A collection is not a logical class: a collection is a first-order entity, while a class is a second-order one.</rdfs:comment>
        <rdfs:isDefinedBy rdf:resource="http://www.ontologydesignpatterns.org/cp/owl/collectionentity.owl"/>
        <rdfs:label xml:lang="en">Collection</rdfs:label>
    </owl:Class>
    


    <!-- http://www.ontologydesignpatterns.org/cp/owl/list.owl#List -->

    <owl:Class rdf:about="http://www.ontologydesignpatterns.org/cp/owl/list.owl#List">
        <rdfs:subClassOf rdf:resource="http://www.ontologydesignpatterns.org/cp/owl/bag.owl#Bag"/>
        <rdfs:comment>List - An ordered array of items, that can be present in multiple copies</rdfs:comment>
        <rdfs:label>list</rdfs:label>
    </owl:Class>
    


    <!-- http://www.ontologydesignpatterns.org/cp/owl/list.owl#ListItem -->

    <owl:Class rdf:about="http://www.ontologydesignpatterns.org/cp/owl/list.owl#ListItem">
        <rdfs:subClassOf rdf:resource="http://www.ontologydesignpatterns.org/cp/owl/bag.owl#Item"/>
        <rdfs:comment>ListItem - Element belonging to a list</rdfs:comment>
        <rdfs:label>list item</rdfs:label>
    </owl:Class>
    


    <!-- http://www.ontologydesignpatterns.org/cp/owl/price.owl#Currency -->

    <owl:Class rdf:about="http://www.ontologydesignpatterns.org/cp/owl/price.owl#Currency">
        <rdfs:subClassOf rdf:resource="http://dbpedia.org/ontology/horse"/>
        <rdfs:subClassOf rdf:resource="http://www.semanticweb.org/annag/ontologies/2024/1/ontoHorses#Cavallo"/>
        <owl:disjointWith rdf:resource="http://www.ontologydesignpatterns.org/cp/owl/price.owl#Price"/>
        <rdfs:comment>A system of money in general use in a particular country.</rdfs:comment>
        <rdfs:isDefinedBy rdf:resource="http://www.ontologydesignpatterns.org/cp/owl/price.owl"/>
        <rdfs:label xml:lang="en">Currency</rdfs:label>
    </owl:Class>
    


    <!-- http://www.ontologydesignpatterns.org/cp/owl/price.owl#Price -->

    <owl:Class rdf:about="http://www.ontologydesignpatterns.org/cp/owl/price.owl#Price">
        <rdfs:subClassOf>
            <owl:Restriction>
                <owl:onProperty rdf:resource="http://www.ontologydesignpatterns.org/cp/owl/price.owl#hasCurrency"/>
                <owl:cardinality rdf:datatype="http://www.w3.org/2001/XMLSchema#nonNegativeInteger">1</owl:cardinality>
            </owl:Restriction>
        </rdfs:subClassOf>
        <rdfs:subClassOf>
            <owl:Restriction>
                <owl:onProperty rdf:resource="http://www.ontologydesignpatterns.org/cp/owl/price.owl#hasValue"/>
                <owl:minCardinality rdf:datatype="http://www.w3.org/2001/XMLSchema#nonNegativeInteger">1</owl:minCardinality>
            </owl:Restriction>
        </rdfs:subClassOf>
        <rdfs:comment>The amount of money expected, required, or given in payment for something.</rdfs:comment>
        <rdfs:isDefinedBy rdf:resource="http://www.ontologydesignpatterns.org/cp/owl/price.owl"/>
        <rdfs:label xml:lang="en">Price</rdfs:label>
    </owl:Class>
    


    <!-- http://www.semanticweb.org/annag/ontologies/2024/1/ontoHorses#AltaScuola -->

    <owl:Class rdf:about="http://www.semanticweb.org/annag/ontologies/2024/1/ontoHorses#AltaScuola">
        <rdfs:subClassOf rdf:resource="http://www.semanticweb.org/annag/ontologies/2024/1/ontoHorses#SportEquestre"/>
    </owl:Class>
    


    <!-- http://www.semanticweb.org/annag/ontologies/2024/1/ontoHorses#AreaGeografica -->

    <owl:Class rdf:about="http://www.semanticweb.org/annag/ontologies/2024/1/ontoHorses#AreaGeografica">
        <rdfs:comment xml:lang="it">Area spaziale univocamente identificato da coordinate geografiche di latitudine e longitudine</rdfs:comment>
        <rdfs:comment xml:lang="en">Spatial area uniquely identified by geographical coordinates of latitude and longitude</rdfs:comment>
        <rdfs:label xml:lang="it">Area geografica</rdfs:label>
        <rdfs:label xml:lang="en">Geographical area</rdfs:label>
    </owl:Class>
    


    <!-- http://www.semanticweb.org/annag/ontologies/2024/1/ontoHorses#CatalogoAutorizzazioniAMontareFise -->

    <owl:Class rdf:about="http://www.semanticweb.org/annag/ontologies/2024/1/ontoHorses#CatalogoAutorizzazioniAMontareFise">
        <rdfs:comment xml:lang="en">Catalog of horse riding licences defined by Federazione Italiana Sport Equestri</rdfs:comment>
        <rdfs:comment xml:lang="it">Catalogo di tutte le autorizzazioni a montare previste dalla Federazione Italiana Sport Equestri</rdfs:comment>
        <rdfs:label xml:lang="en">Catalog of horse riding licences FISE</rdfs:label>
        <rdfs:label xml:lang="it">Catalogo autorizzazioni a montare FISE</rdfs:label>
    </owl:Class>
    


    <!-- http://www.semanticweb.org/annag/ontologies/2024/1/ontoHorses#CategorieDiSalto -->

    <owl:Class rdf:about="http://www.semanticweb.org/annag/ontologies/2024/1/ontoHorses#CategorieDiSalto">
        <owl:equivalentClass>
            <owl:Class>
                <owl:oneOf rdf:parseType="Collection">
                    <rdf:Description rdf:about="http://www.semanticweb.org/annag/ontologies/2024/1/ontoHorses#C100"/>
                    <rdf:Description rdf:about="http://www.semanticweb.org/annag/ontologies/2024/1/ontoHorses#C105"/>
                    <rdf:Description rdf:about="http://www.semanticweb.org/annag/ontologies/2024/1/ontoHorses#C110"/>
                    <rdf:Description rdf:about="http://www.semanticweb.org/annag/ontologies/2024/1/ontoHorses#C115"/>
                    <rdf:Description rdf:about="http://www.semanticweb.org/annag/ontologies/2024/1/ontoHorses#C120"/>
                    <rdf:Description rdf:about="http://www.semanticweb.org/annag/ontologies/2024/1/ontoHorses#C125"/>
                    <rdf:Description rdf:about="http://www.semanticweb.org/annag/ontologies/2024/1/ontoHorses#C130"/>
                    <rdf:Description rdf:about="http://www.semanticweb.org/annag/ontologies/2024/1/ontoHorses#C135"/>
                    <rdf:Description rdf:about="http://www.semanticweb.org/annag/ontologies/2024/1/ontoHorses#C80"/>
                    <rdf:Description rdf:about="http://www.semanticweb.org/annag/ontologies/2024/1/ontoHorses#C90"/>
                </owl:oneOf>
            </owl:Class>
        </owl:equivalentClass>
        <rdfs:subClassOf rdf:resource="http://www.semanticweb.org/annag/ontologies/2024/1/ontoHorses#SaltoAdOstacoli"/>
        <rdfs:comment xml:lang="it">Categorie di difficoltà del salto ad ostacoli</rdfs:comment>
        <rdfs:comment xml:lang="en">Difficulty categories of jumping</rdfs:comment>
        <rdfs:label xml:lang="it">Categoria di salto ad ostacoli</rdfs:label>
        <rdfs:label xml:lang="en">Show jumping category</rdfs:label>
    </owl:Class>
    


    <!-- http://www.semanticweb.org/annag/ontologies/2024/1/ontoHorses#CategorieDressage -->

    <owl:Class rdf:about="http://www.semanticweb.org/annag/ontologies/2024/1/ontoHorses#CategorieDressage">
        <owl:equivalentClass>
            <owl:Class>
                <owl:oneOf rdf:parseType="Collection">
                    <rdf:Description rdf:about="http://www.semanticweb.org/annag/ontologies/2024/1/ontoHorses#D"/>
                    <rdf:Description rdf:about="http://www.semanticweb.org/annag/ontologies/2024/1/ontoHorses#E"/>
                    <rdf:Description rdf:about="http://www.semanticweb.org/annag/ontologies/2024/1/ontoHorses#F"/>
                    <rdf:Description rdf:about="http://www.semanticweb.org/annag/ontologies/2024/1/ontoHorses#M"/>
                </owl:oneOf>
            </owl:Class>
        </owl:equivalentClass>
        <rdfs:subClassOf rdf:resource="http://www.semanticweb.org/annag/ontologies/2024/1/ontoHorses#Dressage"/>
        <rdfs:comment xml:lang="it">Categorie di difficoltà del  Dressage</rdfs:comment>
        <rdfs:comment xml:lang="en">Difficulty categories of Dressage</rdfs:comment>
        <rdfs:label xml:lang="it">Categoria di dressage</rdfs:label>
        <rdfs:label xml:lang="en">Dressage Category</rdfs:label>
    </owl:Class>
    


    <!-- http://www.semanticweb.org/annag/ontologies/2024/1/ontoHorses#Cavaliere -->

    <owl:Class rdf:about="http://www.semanticweb.org/annag/ontologies/2024/1/ontoHorses#Cavaliere">
        <owl:equivalentClass>
            <owl:Class>
                <owl:oneOf rdf:parseType="Collection">
                    <rdf:Description rdf:about="http://www.semanticweb.org/annag/ontologies/2024/1/ontoHorses#CavaliereEsperto"/>
                    <rdf:Description rdf:about="http://www.semanticweb.org/annag/ontologies/2024/1/ontoHorses#CavaliereIntermedio"/>
                    <rdf:Description rdf:about="http://www.semanticweb.org/annag/ontologies/2024/1/ontoHorses#CavaliereMoltoEsperto"/>
                    <rdf:Description rdf:about="http://www.semanticweb.org/annag/ontologies/2024/1/ontoHorses#CavalierePrincipiante"/>
                </owl:oneOf>
            </owl:Class>
        </owl:equivalentClass>
        <rdfs:subClassOf rdf:resource="http://www.semanticweb.org/annag/ontologies/2024/1/ontoHorses#Persona"/>
        <rdfs:subClassOf rdf:resource="http://xmlns.com/foaf/0.1/person"/>
        <rdfs:comment xml:lang="en">Individual who practices equestrian sports</rdfs:comment>
        <rdfs:comment xml:lang="it">Individuo che pratica sport equestri</rdfs:comment>
        <rdfs:label xml:lang="it">Cavaliere</rdfs:label>
        <rdfs:label xml:lang="en">Horse rider</rdfs:label>
    </owl:Class>
    


    <!-- http://www.semanticweb.org/annag/ontologies/2024/1/ontoHorses#Cavallo -->

    <owl:Class rdf:about="http://www.semanticweb.org/annag/ontologies/2024/1/ontoHorses#Cavallo">
        <owl:equivalentClass>
            <owl:Restriction>
                <owl:onProperty rdf:resource="http://www.semanticweb.org/annag/ontologies/2024/1/ontoHorses#haRazza"/>
                <owl:someValuesFrom rdf:resource="http://www.semanticweb.org/annag/ontologies/2024/1/ontoHorses#RazzaCavallo"/>
            </owl:Restriction>
        </owl:equivalentClass>
        <owl:equivalentClass>
            <owl:Restriction>
                <owl:onProperty rdf:resource="http://www.semanticweb.org/annag/ontologies/2024/1/ontoHorses#eta"/>
                <owl:someValuesFrom rdf:resource="http://www.w3.org/2001/XMLSchema#integer"/>
            </owl:Restriction>
        </owl:equivalentClass>
        <owl:equivalentClass>
            <owl:Restriction>
                <owl:onProperty rdf:resource="http://www.semanticweb.org/annag/ontologies/2024/1/ontoHorses#haSesso"/>
                <owl:someValuesFrom rdf:resource="http://www.w3.org/2001/XMLSchema#string"/>
            </owl:Restriction>
        </owl:equivalentClass>
        <rdfs:comment xml:lang="it">Il cavallo è un mammifero perissodattilo di medio-grossa taglia appartenente alla famiglia degli Equidi.</rdfs:comment>
        <rdfs:comment xml:lang="en">The horse is a medium-large sized perissodactyl mammal belonging to the Equidae family.</rdfs:comment>
        <rdfs:label xml:lang="it">Cavallo</rdfs:label>
        <rdfs:label xml:lang="en">Horse</rdfs:label>
    </owl:Class>
    


    <!-- http://www.semanticweb.org/annag/ontologies/2024/1/ontoHorses#CavalloASangueCaldo -->

    <owl:Class rdf:about="http://www.semanticweb.org/annag/ontologies/2024/1/ontoHorses#CavalloASangueCaldo">
        <owl:equivalentClass>
            <owl:Class>
                <owl:intersectionOf rdf:parseType="Collection">
                    <rdf:Description rdf:about="http://www.semanticweb.org/annag/ontologies/2024/1/ontoHorses#Cavallo"/>
                    <owl:Restriction>
                        <owl:onProperty rdf:resource="http://www.semanticweb.org/annag/ontologies/2024/1/ontoHorses#haRazza"/>
                        <owl:someValuesFrom rdf:resource="http://www.semanticweb.org/annag/ontologies/2024/1/ontoHorses#RazzaASangueCaldo"/>
                    </owl:Restriction>
                </owl:intersectionOf>
            </owl:Class>
        </owl:equivalentClass>
        <rdfs:subClassOf rdf:resource="http://dbpedia.org/ontology/horse"/>
        <rdfs:subClassOf rdf:resource="http://www.semanticweb.org/annag/ontologies/2024/1/ontoHorses#Cavallo"/>
        <rdfs:comment xml:lang="it">Cavallo la cui razza è a sangue caldo</rdfs:comment>
        <rdfs:comment xml:lang="en">Horse whose breed is warm-blooded</rdfs:comment>
        <rdfs:label xml:lang="it">Cavallo a sangue caldo</rdfs:label>
        <rdfs:label xml:lang="en">Warm blooded horse</rdfs:label>
    </owl:Class>
    


    <!-- http://www.semanticweb.org/annag/ontologies/2024/1/ontoHorses#CavalloASangueFreddo -->

    <owl:Class rdf:about="http://www.semanticweb.org/annag/ontologies/2024/1/ontoHorses#CavalloASangueFreddo">
        <owl:equivalentClass>
            <owl:Class>
                <owl:intersectionOf rdf:parseType="Collection">
                    <rdf:Description rdf:about="http://www.semanticweb.org/annag/ontologies/2024/1/ontoHorses#Cavallo"/>
                    <owl:Restriction>
                        <owl:onProperty rdf:resource="http://www.semanticweb.org/annag/ontologies/2024/1/ontoHorses#haRazza"/>
                        <owl:someValuesFrom rdf:resource="http://www.semanticweb.org/annag/ontologies/2024/1/ontoHorses#RazzaASangueFreddo"/>
                    </owl:Restriction>
                </owl:intersectionOf>
            </owl:Class>
        </owl:equivalentClass>
        <rdfs:subClassOf rdf:resource="http://dbpedia.org/ontology/horse"/>
        <rdfs:subClassOf rdf:resource="http://www.semanticweb.org/annag/ontologies/2024/1/ontoHorses#Cavallo"/>
        <rdfs:comment xml:lang="it">Cavallo la cui razza è a sangue freddo</rdfs:comment>
        <rdfs:comment xml:lang="en">Horse whose breed is cold-blooded</rdfs:comment>
        <rdfs:label xml:lang="it">Cavallo a sangue freddo</rdfs:label>
        <rdfs:label xml:lang="en">Cold-blooded horse</rdfs:label>
    </owl:Class>
    


    <!-- http://www.semanticweb.org/annag/ontologies/2024/1/ontoHorses#CavalloASangueMisto -->

    <owl:Class rdf:about="http://www.semanticweb.org/annag/ontologies/2024/1/ontoHorses#CavalloASangueMisto">
        <owl:equivalentClass>
            <owl:Class>
                <owl:intersectionOf rdf:parseType="Collection">
                    <rdf:Description rdf:about="http://www.semanticweb.org/annag/ontologies/2024/1/ontoHorses#Cavallo"/>
                    <owl:Restriction>
                        <owl:onProperty rdf:resource="http://www.semanticweb.org/annag/ontologies/2024/1/ontoHorses#haRazza"/>
                        <owl:someValuesFrom rdf:resource="http://www.semanticweb.org/annag/ontologies/2024/1/ontoHorses#RazzaASangueMisto"/>
                    </owl:Restriction>
                </owl:intersectionOf>
            </owl:Class>
        </owl:equivalentClass>
        <rdfs:subClassOf rdf:resource="http://dbpedia.org/ontology/horse"/>
        <rdfs:subClassOf rdf:resource="http://www.semanticweb.org/annag/ontologies/2024/1/ontoHorses#Cavallo"/>
        <rdfs:comment xml:lang="it">Cavallo la cui razza è a sangue misto</rdfs:comment>
        <rdfs:comment xml:lang="en">Horse whose breed is mixed blood</rdfs:comment>
        <rdfs:label xml:lang="it">Cavallo a sangue misto</rdfs:label>
        <rdfs:label xml:lang="en">Mixed-blooded horse</rdfs:label>
    </owl:Class>
    


    <!-- http://www.semanticweb.org/annag/ontologies/2024/1/ontoHorses#CavalloAdulto -->

    <owl:Class rdf:about="http://www.semanticweb.org/annag/ontologies/2024/1/ontoHorses#CavalloAdulto">
        <owl:equivalentClass>
            <owl:Class>
                <owl:intersectionOf rdf:parseType="Collection">
                    <rdf:Description rdf:about="http://www.semanticweb.org/annag/ontologies/2024/1/ontoHorses#Cavallo"/>
                    <owl:Restriction>
                        <owl:onProperty rdf:resource="http://www.semanticweb.org/annag/ontologies/2024/1/ontoHorses#eta"/>
                        <owl:someValuesFrom>
                            <rdfs:Datatype>
                                <owl:onDatatype rdf:resource="http://www.w3.org/2001/XMLSchema#integer"/>
                                <owl:withRestrictions rdf:parseType="Collection">
                                    <rdf:Description>
                                        <xsd:minExclusive rdf:datatype="http://www.w3.org/2001/XMLSchema#integer">6</xsd:minExclusive>
                                    </rdf:Description>
                                    <rdf:Description>
                                        <xsd:maxInclusive rdf:datatype="http://www.w3.org/2001/XMLSchema#integer">18</xsd:maxInclusive>
                                    </rdf:Description>
                                </owl:withRestrictions>
                            </rdfs:Datatype>
                        </owl:someValuesFrom>
                    </owl:Restriction>
                </owl:intersectionOf>
            </owl:Class>
        </owl:equivalentClass>
        <rdfs:subClassOf rdf:resource="http://dbpedia.org/ontology/horse"/>
        <rdfs:subClassOf rdf:resource="http://www.semanticweb.org/annag/ontologies/2024/1/ontoHorses#Cavallo"/>
        <rdfs:comment xml:lang="it">Cavallo con età superiore ai 6 anni</rdfs:comment>
        <rdfs:comment xml:lang="en">Horse over 6 years old</rdfs:comment>
        <rdfs:label xml:lang="en">Adult horse</rdfs:label>
        <rdfs:label xml:lang="it">Cavallo adulto</rdfs:label>
    </owl:Class>
    


    <!-- http://www.semanticweb.org/annag/ontologies/2024/1/ontoHorses#CavalloAnziano -->

    <owl:Class rdf:about="http://www.semanticweb.org/annag/ontologies/2024/1/ontoHorses#CavalloAnziano">
        <owl:equivalentClass>
            <owl:Class>
                <owl:intersectionOf rdf:parseType="Collection">
                    <rdf:Description rdf:about="http://www.semanticweb.org/annag/ontologies/2024/1/ontoHorses#Cavallo"/>
                    <owl:Restriction>
                        <owl:onProperty rdf:resource="http://www.semanticweb.org/annag/ontologies/2024/1/ontoHorses#eta"/>
                        <owl:someValuesFrom>
                            <rdfs:Datatype>
                                <owl:onDatatype rdf:resource="http://www.w3.org/2001/XMLSchema#integer"/>
                                <owl:withRestrictions rdf:parseType="Collection">
                                    <rdf:Description>
                                        <xsd:minExclusive rdf:datatype="http://www.w3.org/2001/XMLSchema#integer">18</xsd:minExclusive>
                                    </rdf:Description>
                                </owl:withRestrictions>
                            </rdfs:Datatype>
                        </owl:someValuesFrom>
                    </owl:Restriction>
                </owl:intersectionOf>
            </owl:Class>
        </owl:equivalentClass>
        <rdfs:subClassOf rdf:resource="http://dbpedia.org/ontology/horse"/>
        <rdfs:subClassOf rdf:resource="http://www.semanticweb.org/annag/ontologies/2024/1/ontoHorses#Cavallo"/>
        <rdfs:comment xml:lang="it">Cavallo con età superiore o uguale ai 18 anni</rdfs:comment>
        <rdfs:comment xml:lang="en">Horse aged 18 years or older</rdfs:comment>
        <rdfs:label xml:lang="it">Cavallo anziano</rdfs:label>
        <rdfs:label xml:lang="en">Old horse</rdfs:label>
    </owl:Class>
    


    <!-- http://www.semanticweb.org/annag/ontologies/2024/1/ontoHorses#CavalloCastrone -->

    <owl:Class rdf:about="http://www.semanticweb.org/annag/ontologies/2024/1/ontoHorses#CavalloCastrone">
        <owl:equivalentClass>
            <owl:Class>
                <owl:intersectionOf rdf:parseType="Collection">
                    <rdf:Description rdf:about="http://www.semanticweb.org/annag/ontologies/2024/1/ontoHorses#Cavallo"/>
                    <owl:Restriction>
                        <owl:onProperty rdf:resource="http://www.semanticweb.org/annag/ontologies/2024/1/ontoHorses#haSesso"/>
                        <owl:hasValue>castrone</owl:hasValue>
                    </owl:Restriction>
                </owl:intersectionOf>
            </owl:Class>
        </owl:equivalentClass>
        <rdfs:subClassOf rdf:resource="http://dbpedia.org/ontology/horse"/>
        <rdfs:subClassOf rdf:resource="http://www.semanticweb.org/annag/ontologies/2024/1/ontoHorses#Cavallo"/>
        <rdfs:comment xml:lang="en">Castrated male horse of any age</rdfs:comment>
        <rdfs:comment xml:lang="it">Cavallo maschio castrato di qualsiasi età</rdfs:comment>
        <rdfs:label xml:lang="it">Cavallo castrone</rdfs:label>
        <rdfs:label xml:lang="en">Gelding horse</rdfs:label>
    </owl:Class>
    


    <!-- http://www.semanticweb.org/annag/ontologies/2024/1/ontoHorses#CavalloDaEquiturismo -->

    <owl:Class rdf:about="http://www.semanticweb.org/annag/ontologies/2024/1/ontoHorses#CavalloDaEquiturismo">
        <owl:equivalentClass>
            <owl:Class>
                <owl:intersectionOf rdf:parseType="Collection">
                    <rdf:Description rdf:about="http://www.semanticweb.org/annag/ontologies/2024/1/ontoHorses#CavalloDaSella"/>
                    <owl:Restriction>
                        <owl:onProperty rdf:resource="http://www.semanticweb.org/annag/ontologies/2024/1/ontoHorses#vieneUtilizzatoPer"/>
                        <owl:hasValue rdf:resource="http://www.semanticweb.org/annag/ontologies/2024/1/ontoHorses#Equiturismo"/>
                    </owl:Restriction>
                </owl:intersectionOf>
            </owl:Class>
        </owl:equivalentClass>
        <rdfs:subClassOf rdf:resource="http://www.semanticweb.org/annag/ontologies/2024/1/ontoHorses#CavalloDaSella"/>
        <rdfs:comment xml:lang="it">Cavallo utilizzato per equiturismo</rdfs:comment>
        <rdfs:comment xml:lang="en">Horse used for equestrian tourism</rdfs:comment>
        <rdfs:label xml:lang="it">Cavallo da equiturismo</rdfs:label>
        <rdfs:label xml:lang="en">Equestrian tourism horse</rdfs:label>
    </owl:Class>
    


    <!-- http://www.semanticweb.org/annag/ontologies/2024/1/ontoHorses#CavalloDaLavoro -->

    <owl:Class rdf:about="http://www.semanticweb.org/annag/ontologies/2024/1/ontoHorses#CavalloDaLavoro">
        <owl:equivalentClass>
            <owl:Class>
                <owl:intersectionOf rdf:parseType="Collection">
                    <rdf:Description rdf:about="http://www.semanticweb.org/annag/ontologies/2024/1/ontoHorses#Cavallo"/>
                    <owl:Restriction>
                        <owl:onProperty rdf:resource="http://www.semanticweb.org/annag/ontologies/2024/1/ontoHorses#vieneUtilizzatoPer"/>
                        <owl:minQualifiedCardinality rdf:datatype="http://www.w3.org/2001/XMLSchema#nonNegativeInteger">1</owl:minQualifiedCardinality>
                        <owl:onClass rdf:resource="http://www.semanticweb.org/annag/ontologies/2024/1/ontoHorses#Lavoro"/>
                    </owl:Restriction>
                </owl:intersectionOf>
            </owl:Class>
        </owl:equivalentClass>
        <rdfs:subClassOf rdf:resource="http://dbpedia.org/ontology/horse"/>
        <rdfs:subClassOf rdf:resource="http://www.semanticweb.org/annag/ontologies/2024/1/ontoHorses#Cavallo"/>
        <rdfs:comment xml:lang="it">Cavallo impiegato nel lavoro agricolo o nel traino carrozze e/o carichi</rdfs:comment>
        <rdfs:comment xml:lang="en">Horse used in agricultural work or in pulling carriages and/or loads</rdfs:comment>
        <rdfs:label xml:lang="it">Cavallo da lavoro</rdfs:label>
        <rdfs:label xml:lang="en">Work horse</rdfs:label>
    </owl:Class>
    


    <!-- http://www.semanticweb.org/annag/ontologies/2024/1/ontoHorses#CavalloDaSella -->

    <owl:Class rdf:about="http://www.semanticweb.org/annag/ontologies/2024/1/ontoHorses#CavalloDaSella">
        <owl:equivalentClass>
            <owl:Class>
                <owl:intersectionOf rdf:parseType="Collection">
                    <rdf:Description rdf:about="http://www.semanticweb.org/annag/ontologies/2024/1/ontoHorses#Cavallo"/>
                    <owl:Restriction>
                        <owl:onProperty rdf:resource="http://www.semanticweb.org/annag/ontologies/2024/1/ontoHorses#vieneUtilizzatoPer"/>
                        <owl:someValuesFrom rdf:resource="http://www.semanticweb.org/annag/ontologies/2024/1/ontoHorses#Sella"/>
                    </owl:Restriction>
                </owl:intersectionOf>
            </owl:Class>
        </owl:equivalentClass>
        <rdfs:subClassOf rdf:resource="http://dbpedia.org/ontology/horse"/>
        <rdfs:subClassOf rdf:resource="http://www.semanticweb.org/annag/ontologies/2024/1/ontoHorses#Cavallo"/>
        <rdfs:comment xml:lang="it">Cavallo che ha attitudine alla sella</rdfs:comment>
        <rdfs:comment xml:lang="en">Horse suitable for the saddle</rdfs:comment>
        <rdfs:label xml:lang="it">Cavallo da sella</rdfs:label>
        <rdfs:label xml:lang="en">Riding horse</rdfs:label>
    </owl:Class>
    


    <!-- http://www.semanticweb.org/annag/ontologies/2024/1/ontoHorses#CavalloDaTiroAgricolo -->

    <owl:Class rdf:about="http://www.semanticweb.org/annag/ontologies/2024/1/ontoHorses#CavalloDaTiroAgricolo">
        <owl:equivalentClass>
            <owl:Class>
                <owl:intersectionOf rdf:parseType="Collection">
                    <rdf:Description rdf:about="http://www.semanticweb.org/annag/ontologies/2024/1/ontoHorses#CavalloDaLavoro"/>
                    <owl:Restriction>
                        <owl:onProperty rdf:resource="http://www.semanticweb.org/annag/ontologies/2024/1/ontoHorses#vieneUtilizzatoPer"/>
                        <owl:hasValue rdf:resource="http://www.semanticweb.org/annag/ontologies/2024/1/ontoHorses#TiroAgricolo"/>
                    </owl:Restriction>
                </owl:intersectionOf>
            </owl:Class>
        </owl:equivalentClass>
        <rdfs:subClassOf rdf:resource="http://www.semanticweb.org/annag/ontologies/2024/1/ontoHorses#CavalloDaLavoro"/>
        <rdfs:comment xml:lang="it">Cavallo utilizzato nei lavori agricoli</rdfs:comment>
        <rdfs:comment xml:lang="en">Horse used in agricultural work</rdfs:comment>
        <rdfs:label xml:lang="en">Agricultural wor horse</rdfs:label>
        <rdfs:label xml:lang="it">Cavallo da tiro agricolo</rdfs:label>
    </owl:Class>
    


    <!-- http://www.semanticweb.org/annag/ontologies/2024/1/ontoHorses#CavalloDaTrainoCarrozze -->

    <owl:Class rdf:about="http://www.semanticweb.org/annag/ontologies/2024/1/ontoHorses#CavalloDaTrainoCarrozze">
        <owl:equivalentClass>
            <owl:Class>
                <owl:intersectionOf rdf:parseType="Collection">
                    <rdf:Description rdf:about="http://www.semanticweb.org/annag/ontologies/2024/1/ontoHorses#CavalloDaLavoro"/>
                    <owl:Restriction>
                        <owl:onProperty rdf:resource="http://www.semanticweb.org/annag/ontologies/2024/1/ontoHorses#vieneUtilizzatoPer"/>
                        <owl:hasValue rdf:resource="http://www.semanticweb.org/annag/ontologies/2024/1/ontoHorses#TrainoCarrozze"/>
                    </owl:Restriction>
                </owl:intersectionOf>
            </owl:Class>
        </owl:equivalentClass>
        <rdfs:subClassOf rdf:resource="http://www.semanticweb.org/annag/ontologies/2024/1/ontoHorses#CavalloDaLavoro"/>
        <rdfs:comment xml:lang="it">Cavallo utilizzato per il traino di carrozze merci o passeggeri</rdfs:comment>
        <rdfs:comment xml:lang="en">Horse used for pulling freight or passenger carriages</rdfs:comment>
        <rdfs:label xml:lang="it">Cavallo da traino carrozze</rdfs:label>
        <rdfs:label xml:lang="en">Horse for pulling carriages</rdfs:label>
    </owl:Class>
    


    <!-- http://www.semanticweb.org/annag/ontologies/2024/1/ontoHorses#CavalloFemmina -->

    <owl:Class rdf:about="http://www.semanticweb.org/annag/ontologies/2024/1/ontoHorses#CavalloFemmina">
        <owl:equivalentClass>
            <owl:Class>
                <owl:intersectionOf rdf:parseType="Collection">
                    <rdf:Description rdf:about="http://www.semanticweb.org/annag/ontologies/2024/1/ontoHorses#Cavallo"/>
                    <owl:Restriction>
                        <owl:onProperty rdf:resource="http://www.semanticweb.org/annag/ontologies/2024/1/ontoHorses#haSesso"/>
                        <owl:hasValue>femmina</owl:hasValue>
                    </owl:Restriction>
                </owl:intersectionOf>
            </owl:Class>
        </owl:equivalentClass>
        <rdfs:subClassOf rdf:resource="http://dbpedia.org/ontology/horse"/>
        <rdfs:subClassOf rdf:resource="http://www.semanticweb.org/annag/ontologies/2024/1/ontoHorses#Cavallo"/>
        <rdfs:comment xml:lang="it">Cavallo il cui sesso è femmina</rdfs:comment>
        <rdfs:comment xml:lang="en">Horse whose sex is female</rdfs:comment>
        <rdfs:label xml:lang="it">Cavallo femmina</rdfs:label>
        <rdfs:label xml:lang="en">Female horse</rdfs:label>
    </owl:Class>
    


    <!-- http://www.semanticweb.org/annag/ontologies/2024/1/ontoHorses#CavalloMaschio -->

    <owl:Class rdf:about="http://www.semanticweb.org/annag/ontologies/2024/1/ontoHorses#CavalloMaschio">
        <owl:equivalentClass>
            <owl:Class>
                <owl:intersectionOf rdf:parseType="Collection">
                    <rdf:Description rdf:about="http://www.semanticweb.org/annag/ontologies/2024/1/ontoHorses#Cavallo"/>
                    <owl:Restriction>
                        <owl:onProperty rdf:resource="http://www.semanticweb.org/annag/ontologies/2024/1/ontoHorses#haSesso"/>
                        <owl:hasValue>maschio</owl:hasValue>
                    </owl:Restriction>
                </owl:intersectionOf>
            </owl:Class>
        </owl:equivalentClass>
        <rdfs:subClassOf rdf:resource="http://dbpedia.org/ontology/horse"/>
        <rdfs:subClassOf rdf:resource="http://www.semanticweb.org/annag/ontologies/2024/1/ontoHorses#Cavallo"/>
        <rdfs:comment xml:lang="it">Cavallo il cui sesso è maschio e non è castrato</rdfs:comment>
        <rdfs:comment xml:lang="en">Horse whose sex is male and is not castrated</rdfs:comment>
        <rdfs:label xml:lang="it">Cavallo maschio</rdfs:label>
        <rdfs:label xml:lang="en">Male horse</rdfs:label>
    </owl:Class>
    


    <!-- http://www.semanticweb.org/annag/ontologies/2024/1/ontoHorses#CavalloPerAltaScuola -->

    <owl:Class rdf:about="http://www.semanticweb.org/annag/ontologies/2024/1/ontoHorses#CavalloPerAltaScuola">
        <owl:equivalentClass>
            <owl:Class>
                <owl:intersectionOf rdf:parseType="Collection">
                    <rdf:Description rdf:about="http://www.semanticweb.org/annag/ontologies/2024/1/ontoHorses#CavalloSportivo"/>
                    <owl:Restriction>
                        <owl:onProperty rdf:resource="http://www.semanticweb.org/annag/ontologies/2024/1/ontoHorses#vieneUtilizzatoPer"/>
                        <owl:hasValue rdf:resource="http://www.semanticweb.org/annag/ontologies/2024/1/ontoHorses#AltaScuola"/>
                    </owl:Restriction>
                </owl:intersectionOf>
            </owl:Class>
        </owl:equivalentClass>
        <rdfs:subClassOf rdf:resource="http://www.semanticweb.org/annag/ontologies/2024/1/ontoHorses#CavalloSportivo"/>
        <rdfs:comment xml:lang="it">Cavallo utilizzato nella disciplina sportiva equestre dell&apos;Alta Scuola</rdfs:comment>
        <rdfs:comment xml:lang="en">Horse used in the equestrian sport of Spanish riding school</rdfs:comment>
        <rdfs:label xml:lang="it">Cavallo per Alta Scuola</rdfs:label>
        <rdfs:label xml:lang="en">Spanish riding school horse</rdfs:label>
    </owl:Class>
    


    <!-- http://www.semanticweb.org/annag/ontologies/2024/1/ontoHorses#CavalloPerCrossCountry -->

    <owl:Class rdf:about="http://www.semanticweb.org/annag/ontologies/2024/1/ontoHorses#CavalloPerCrossCountry">
        <owl:equivalentClass>
            <owl:Class>
                <owl:intersectionOf rdf:parseType="Collection">
                    <rdf:Description rdf:about="http://www.semanticweb.org/annag/ontologies/2024/1/ontoHorses#CavalloSportivo"/>
                    <owl:Restriction>
                        <owl:onProperty rdf:resource="http://www.semanticweb.org/annag/ontologies/2024/1/ontoHorses#vieneUtilizzatoPer"/>
                        <owl:hasValue rdf:resource="http://www.semanticweb.org/annag/ontologies/2024/1/ontoHorses#CrossCountry"/>
                    </owl:Restriction>
                </owl:intersectionOf>
            </owl:Class>
        </owl:equivalentClass>
        <rdfs:subClassOf rdf:resource="http://www.semanticweb.org/annag/ontologies/2024/1/ontoHorses#CavalloSportivo"/>
        <rdfs:comment xml:lang="it">Cavallo usato nella disciplina sportiva equestre del cross-country</rdfs:comment>
        <rdfs:comment xml:lang="en">Horse used in the equestrian sport discipline of cross-country</rdfs:comment>
        <rdfs:label xml:lang="it">Cavallo per cross-country</rdfs:label>
        <rdfs:label xml:lang="en">Cross-country horse</rdfs:label>
    </owl:Class>
    


    <!-- http://www.semanticweb.org/annag/ontologies/2024/1/ontoHorses#CavalloPerDressage -->

    <owl:Class rdf:about="http://www.semanticweb.org/annag/ontologies/2024/1/ontoHorses#CavalloPerDressage">
        <owl:equivalentClass>
            <owl:Class>
                <owl:intersectionOf rdf:parseType="Collection">
                    <rdf:Description rdf:about="http://www.semanticweb.org/annag/ontologies/2024/1/ontoHorses#CavalloSportivo"/>
                    <owl:Class>
                        <owl:unionOf rdf:parseType="Collection">
                            <owl:Restriction>
                                <owl:onProperty rdf:resource="http://www.semanticweb.org/annag/ontologies/2024/1/ontoHorses#gareggiaNellaCategoriaDiDressage"/>
                                <owl:someValuesFrom rdf:resource="http://www.semanticweb.org/annag/ontologies/2024/1/ontoHorses#CategorieDressage"/>
                            </owl:Restriction>
                            <owl:Restriction>
                                <owl:onProperty rdf:resource="http://www.semanticweb.org/annag/ontologies/2024/1/ontoHorses#vieneUtilizzatoPer"/>
                                <owl:hasValue rdf:resource="http://www.semanticweb.org/annag/ontologies/2024/1/ontoHorses#Dressage"/>
                            </owl:Restriction>
                        </owl:unionOf>
                    </owl:Class>
                </owl:intersectionOf>
            </owl:Class>
        </owl:equivalentClass>
        <rdfs:subClassOf rdf:resource="http://www.semanticweb.org/annag/ontologies/2024/1/ontoHorses#CavalloSportivo"/>
        <rdfs:comment xml:lang="it">Cavallo utilizzato nella disciplina sportiva equestre del dressage</rdfs:comment>
        <rdfs:comment xml:lang="en">Horse used in the equestrian sport discipline of dressage</rdfs:comment>
        <rdfs:label xml:lang="it">Cavallo per Dressage</rdfs:label>
        <rdfs:label xml:lang="en">Dressage horse</rdfs:label>
    </owl:Class>
    


    <!-- http://www.semanticweb.org/annag/ontologies/2024/1/ontoHorses#CavalloPerEndurance -->

    <owl:Class rdf:about="http://www.semanticweb.org/annag/ontologies/2024/1/ontoHorses#CavalloPerEndurance">
        <owl:equivalentClass>
            <owl:Class>
                <owl:intersectionOf rdf:parseType="Collection">
                    <rdf:Description rdf:about="http://www.semanticweb.org/annag/ontologies/2024/1/ontoHorses#CavalloSportivo"/>
                    <owl:Restriction>
                        <owl:onProperty rdf:resource="http://www.semanticweb.org/annag/ontologies/2024/1/ontoHorses#vieneUtilizzatoPer"/>
                        <owl:hasValue rdf:resource="http://www.semanticweb.org/annag/ontologies/2024/1/ontoHorses#Endurance"/>
                    </owl:Restriction>
                </owl:intersectionOf>
            </owl:Class>
        </owl:equivalentClass>
        <rdfs:subClassOf rdf:resource="http://www.semanticweb.org/annag/ontologies/2024/1/ontoHorses#CavalloSportivo"/>
        <rdfs:comment xml:lang="it">Cavallo utilizzato nella disciplina sportiva equestre dell&apos;endurance</rdfs:comment>
        <rdfs:comment xml:lang="en">Horse used in the equestrian sport discipline of endurance</rdfs:comment>
        <rdfs:label xml:lang="it">Cavallo per Endurance</rdfs:label>
        <rdfs:label xml:lang="en">Endurance horse</rdfs:label>
    </owl:Class>
    


    <!-- http://www.semanticweb.org/annag/ontologies/2024/1/ontoHorses#CavalloPerEventing -->

    <owl:Class rdf:about="http://www.semanticweb.org/annag/ontologies/2024/1/ontoHorses#CavalloPerEventing">
        <owl:equivalentClass>
            <owl:Class>
                <owl:intersectionOf rdf:parseType="Collection">
                    <rdf:Description rdf:about="http://www.semanticweb.org/annag/ontologies/2024/1/ontoHorses#CavalloSportivo"/>
                    <owl:Restriction>
                        <owl:onProperty rdf:resource="http://www.semanticweb.org/annag/ontologies/2024/1/ontoHorses#vieneUtilizzatoPer"/>
                        <owl:hasValue rdf:resource="http://www.semanticweb.org/annag/ontologies/2024/1/ontoHorses#Eventing"/>
                    </owl:Restriction>
                </owl:intersectionOf>
            </owl:Class>
        </owl:equivalentClass>
        <rdfs:subClassOf rdf:resource="http://www.semanticweb.org/annag/ontologies/2024/1/ontoHorses#CavalloSportivo"/>
        <rdfs:comment xml:lang="it">Cavallo utilizzato nella disciplina sportiva equestre dell&apos;eventing</rdfs:comment>
        <rdfs:comment xml:lang="en">Horse used in the equestrian sport discipline of eventing</rdfs:comment>
        <rdfs:label xml:lang="it">Cavallo per Eventing</rdfs:label>
        <rdfs:label xml:lang="en">Eventing horse</rdfs:label>
    </owl:Class>
    


    <!-- http://www.semanticweb.org/annag/ontologies/2024/1/ontoHorses#CavalloPerSaltoOstacoli -->

    <owl:Class rdf:about="http://www.semanticweb.org/annag/ontologies/2024/1/ontoHorses#CavalloPerSaltoOstacoli">
        <owl:equivalentClass>
            <owl:Class>
                <owl:intersectionOf rdf:parseType="Collection">
                    <rdf:Description rdf:about="http://www.semanticweb.org/annag/ontologies/2024/1/ontoHorses#CavalloPerSaltoOstacoli"/>
                    <owl:Class>
                        <owl:unionOf rdf:parseType="Collection">
                            <owl:Restriction>
                                <owl:onProperty rdf:resource="http://www.semanticweb.org/annag/ontologies/2024/1/ontoHorses#gareggiaNelleCategorieDiSalto"/>
                                <owl:someValuesFrom rdf:resource="http://www.semanticweb.org/annag/ontologies/2024/1/ontoHorses#CategorieDiSalto"/>
                            </owl:Restriction>
                            <owl:Restriction>
                                <owl:onProperty rdf:resource="http://www.semanticweb.org/annag/ontologies/2024/1/ontoHorses#vieneUtilizzatoPer"/>
                                <owl:hasValue rdf:resource="http://www.semanticweb.org/annag/ontologies/2024/1/ontoHorses#SaltoAdOstacoli"/>
                            </owl:Restriction>
                        </owl:unionOf>
                    </owl:Class>
                </owl:intersectionOf>
            </owl:Class>
        </owl:equivalentClass>
        <rdfs:subClassOf rdf:resource="http://www.semanticweb.org/annag/ontologies/2024/1/ontoHorses#CavalloSportivo"/>
        <rdfs:comment xml:lang="it">Cavallo utilizzato nella disciplina sportiva equestre del salto ostacoli</rdfs:comment>
        <rdfs:comment xml:lang="en">Horse used in the equestrian sport discipline of jumping</rdfs:comment>
        <rdfs:label xml:lang="it">Cavallo per salto ostacoli</rdfs:label>
        <rdfs:label xml:lang="en">Jumping horse</rdfs:label>
    </owl:Class>
    


    <!-- http://www.semanticweb.org/annag/ontologies/2024/1/ontoHorses#CavalloSportivo -->

    <owl:Class rdf:about="http://www.semanticweb.org/annag/ontologies/2024/1/ontoHorses#CavalloSportivo">
        <owl:equivalentClass>
            <owl:Class>
                <owl:intersectionOf rdf:parseType="Collection">
                    <rdf:Description rdf:about="http://www.semanticweb.org/annag/ontologies/2024/1/ontoHorses#CavalloDaSella"/>
                    <owl:Restriction>
                        <owl:onProperty rdf:resource="http://www.semanticweb.org/annag/ontologies/2024/1/ontoHorses#vieneUtilizzatoPer"/>
                        <owl:minQualifiedCardinality rdf:datatype="http://www.w3.org/2001/XMLSchema#nonNegativeInteger">1</owl:minQualifiedCardinality>
                        <owl:onClass rdf:resource="http://www.semanticweb.org/annag/ontologies/2024/1/ontoHorses#SportEquestre"/>
                    </owl:Restriction>
                </owl:intersectionOf>
            </owl:Class>
        </owl:equivalentClass>
        <rdfs:subClassOf rdf:resource="http://www.semanticweb.org/annag/ontologies/2024/1/ontoHorses#CavalloDaSella"/>
        <rdfs:comment xml:lang="it">Cavallo utilizzato nello sport equestre</rdfs:comment>
        <rdfs:comment xml:lang="en">Horse used in some equestrian sports</rdfs:comment>
        <rdfs:label xml:lang="it">Cavallo sportivo</rdfs:label>
        <rdfs:label xml:lang="en">Sport horse</rdfs:label>
    </owl:Class>
    


    <!-- http://www.semanticweb.org/annag/ontologies/2024/1/ontoHorses#CrossCountry -->

    <owl:Class rdf:about="http://www.semanticweb.org/annag/ontologies/2024/1/ontoHorses#CrossCountry">
        <rdfs:subClassOf rdf:resource="http://www.semanticweb.org/annag/ontologies/2024/1/ontoHorses#SportEquestre"/>
    </owl:Class>
    


    <!-- http://www.semanticweb.org/annag/ontologies/2024/1/ontoHorses#Dressage -->

    <owl:Class rdf:about="http://www.semanticweb.org/annag/ontologies/2024/1/ontoHorses#Dressage">
        <rdfs:subClassOf rdf:resource="http://www.semanticweb.org/annag/ontologies/2024/1/ontoHorses#SportEquestre"/>
    </owl:Class>
    


    <!-- http://www.semanticweb.org/annag/ontologies/2024/1/ontoHorses#Endurance -->

    <owl:Class rdf:about="http://www.semanticweb.org/annag/ontologies/2024/1/ontoHorses#Endurance">
        <rdfs:subClassOf rdf:resource="http://www.semanticweb.org/annag/ontologies/2024/1/ontoHorses#SportEquestre"/>
    </owl:Class>
    


    <!-- http://www.semanticweb.org/annag/ontologies/2024/1/ontoHorses#Equiturismo -->

    <owl:Class rdf:about="http://www.semanticweb.org/annag/ontologies/2024/1/ontoHorses#Equiturismo">
        <rdfs:subClassOf rdf:resource="http://dbpedia.org/ontology/horseRidingDiscipline"/>
        <rdfs:subClassOf rdf:resource="http://www.semanticweb.org/annag/ontologies/2024/1/ontoHorses#Sella"/>
    </owl:Class>
    


    <!-- http://www.semanticweb.org/annag/ontologies/2024/1/ontoHorses#Eventing -->

    <owl:Class rdf:about="http://www.semanticweb.org/annag/ontologies/2024/1/ontoHorses#Eventing">
        <rdfs:subClassOf rdf:resource="http://www.semanticweb.org/annag/ontologies/2024/1/ontoHorses#SportEquestre"/>
    </owl:Class>
    


    <!-- http://www.semanticweb.org/annag/ontologies/2024/1/ontoHorses#Impiego -->

    <owl:Class rdf:about="http://www.semanticweb.org/annag/ontologies/2024/1/ontoHorses#Impiego">
        <rdfs:comment xml:lang="it">I possibili impieghi del cavallo</rdfs:comment>
        <rdfs:comment xml:lang="en">The possible uses of the horse</rdfs:comment>
        <rdfs:label xml:lang="it">Impiego</rdfs:label>
        <rdfs:label xml:lang="en">Use</rdfs:label>
    </owl:Class>
    


    <!-- http://www.semanticweb.org/annag/ontologies/2024/1/ontoHorses#Indole -->

    <owl:Class rdf:about="http://www.semanticweb.org/annag/ontologies/2024/1/ontoHorses#Indole">
        <owl:equivalentClass>
            <owl:Class>
                <owl:oneOf rdf:parseType="Collection">
                    <rdf:Description rdf:about="http://www.semanticweb.org/annag/ontologies/2024/1/ontoHorses#sangueCaldo"/>
                    <rdf:Description rdf:about="http://www.semanticweb.org/annag/ontologies/2024/1/ontoHorses#sangueFreddo"/>
                    <rdf:Description rdf:about="http://www.semanticweb.org/annag/ontologies/2024/1/ontoHorses#sangueMisto"/>
                </owl:oneOf>
            </owl:Class>
        </owl:equivalentClass>
        <rdfs:comment xml:lang="it">L&apos;indole o temperamento è uno dei classici parametri di classificazione dei cavalli</rdfs:comment>
        <rdfs:comment xml:lang="en">The nature or temperament is one of the classic classification parameters of horses</rdfs:comment>
        <rdfs:label xml:lang="it">Indole</rdfs:label>
        <rdfs:label xml:lang="en">Nature</rdfs:label>
    </owl:Class>
    


    <!-- http://www.semanticweb.org/annag/ontologies/2024/1/ontoHorses#Lavoro -->

    <owl:Class rdf:about="http://www.semanticweb.org/annag/ontologies/2024/1/ontoHorses#Lavoro">
        <rdfs:subClassOf rdf:resource="http://www.semanticweb.org/annag/ontologies/2024/1/ontoHorses#Impiego"/>
        <rdfs:comment xml:lang="it">Impiego del cavallo in attività lavorative</rdfs:comment>
        <rdfs:comment xml:lang="en">Use of the horse in work activities</rdfs:comment>
        <rdfs:label xml:lang="it">Lavoro</rdfs:label>
        <rdfs:label xml:lang="en">Work</rdfs:label>
    </owl:Class>
    


    <!-- http://www.semanticweb.org/annag/ontologies/2024/1/ontoHorses#Morfologia -->

    <owl:Class rdf:about="http://www.semanticweb.org/annag/ontologies/2024/1/ontoHorses#Morfologia">
        <owl:equivalentClass>
            <owl:Class>
                <owl:oneOf rdf:parseType="Collection">
                    <rdf:Description rdf:about="http://www.semanticweb.org/annag/ontologies/2024/1/ontoHorses#brachimorfo"/>
                    <rdf:Description rdf:about="http://www.semanticweb.org/annag/ontologies/2024/1/ontoHorses#dolicomorfo"/>
                    <rdf:Description rdf:about="http://www.semanticweb.org/annag/ontologies/2024/1/ontoHorses#mesoBrachimorfo"/>
                    <rdf:Description rdf:about="http://www.semanticweb.org/annag/ontologies/2024/1/ontoHorses#mesoDolicomorfo"/>
                    <rdf:Description rdf:about="http://www.semanticweb.org/annag/ontologies/2024/1/ontoHorses#mesomorfo"/>
                </owl:oneOf>
            </owl:Class>
        </owl:equivalentClass>
        <rdfs:subClassOf rdf:resource="http://www.semanticweb.org/annag/ontologies/2024/1/ontoHorses#RazzaCavallo"/>
        <rdfs:comment xml:lang="en">Main physical traits of a horse that can possibly determine its classification</rdfs:comment>
        <rdfs:comment xml:lang="it">Tratti fisici principali di un cavallo che eventualmente ne possono determinare una classificazione</rdfs:comment>
        <rdfs:label xml:lang="it">Morfologia</rdfs:label>
        <rdfs:label xml:lang="en">Morphology</rdfs:label>
    </owl:Class>
    


    <!-- http://www.semanticweb.org/annag/ontologies/2024/1/ontoHorses#Patente -->

    <owl:Class rdf:about="http://www.semanticweb.org/annag/ontologies/2024/1/ontoHorses#Patente">
        <rdfs:subClassOf rdf:resource="http://www.ontologydesignpatterns.org/cp/owl/list.owl#ListItem"/>
        <rdfs:comment xml:lang="en">Authorization to ride issued by FISE on the basis of the skills acquired, the competitions in which one participates and any exams taken.</rdfs:comment>
        <rdfs:comment xml:lang="it">Autorizzazione a montare rilasciata dalla FISE sulla base dell&apos;abilità acquisita, delle competizioni a cui si partecipa e degli eventuali esami sostenuti.</rdfs:comment>
        <rdfs:label xml:lang="en">FISE riding licence</rdfs:label>
        <rdfs:label xml:lang="it">Patente FISE</rdfs:label>
    </owl:Class>
    


    <!-- http://www.semanticweb.org/annag/ontologies/2024/1/ontoHorses#Persona -->

    <owl:Class rdf:about="http://www.semanticweb.org/annag/ontologies/2024/1/ontoHorses#Persona">
        <owl:equivalentClass rdf:resource="http://xmlns.com/foaf/0.1/person"/>
        <rdfs:comment xml:lang="en">Individual of the human species</rdfs:comment>
        <rdfs:comment xml:lang="it">Individuo della specie umana</rdfs:comment>
        <rdfs:label xml:lang="en">Person</rdfs:label>
        <rdfs:label xml:lang="it">Persona</rdfs:label>
    </owl:Class>
    


    <!-- http://www.semanticweb.org/annag/ontologies/2024/1/ontoHorses#Proprietario -->

    <owl:Class rdf:about="http://www.semanticweb.org/annag/ontologies/2024/1/ontoHorses#Proprietario">
        <owl:equivalentClass>
            <owl:Class>
                <owl:intersectionOf rdf:parseType="Collection">
                    <rdf:Description rdf:about="http://www.semanticweb.org/annag/ontologies/2024/1/ontoHorses#Persona"/>
                    <owl:Restriction>
                        <owl:onProperty rdf:resource="http://www.semanticweb.org/annag/ontologies/2024/1/ontoHorses#possiede"/>
                        <owl:minQualifiedCardinality rdf:datatype="http://www.w3.org/2001/XMLSchema#nonNegativeInteger">1</owl:minQualifiedCardinality>
                        <owl:onClass rdf:resource="http://www.semanticweb.org/annag/ontologies/2024/1/ontoHorses#Cavallo"/>
                    </owl:Restriction>
                </owl:intersectionOf>
            </owl:Class>
        </owl:equivalentClass>
        <rdfs:subClassOf rdf:resource="http://www.semanticweb.org/annag/ontologies/2024/1/ontoHorses#Persona"/>
        <rdfs:subClassOf rdf:resource="http://xmlns.com/foaf/0.1/person"/>
        <rdfs:comment xml:lang="it">La persona che detiene la proprietà del cavallo e ne è autorizzato alla vendita</rdfs:comment>
        <rdfs:comment xml:lang="en">The person who holds title to the horse and is authorized to sell it</rdfs:comment>
        <rdfs:label xml:lang="en">Horse owner</rdfs:label>
        <rdfs:label xml:lang="it">Proprietario</rdfs:label>
    </owl:Class>
    


    <!-- http://www.semanticweb.org/annag/ontologies/2024/1/ontoHorses#Puledro -->

    <owl:Class rdf:about="http://www.semanticweb.org/annag/ontologies/2024/1/ontoHorses#Puledro">
        <owl:equivalentClass>
            <owl:Class>
                <owl:intersectionOf rdf:parseType="Collection">
                    <rdf:Description rdf:about="http://www.semanticweb.org/annag/ontologies/2024/1/ontoHorses#Cavallo"/>
                    <owl:Restriction>
                        <owl:onProperty rdf:resource="http://www.semanticweb.org/annag/ontologies/2024/1/ontoHorses#eta"/>
                        <owl:someValuesFrom>
                            <rdfs:Datatype>
                                <owl:onDatatype rdf:resource="http://www.w3.org/2001/XMLSchema#integer"/>
                                <owl:withRestrictions rdf:parseType="Collection">
                                    <rdf:Description>
                                        <xsd:maxInclusive rdf:datatype="http://www.w3.org/2001/XMLSchema#integer">6</xsd:maxInclusive>
                                    </rdf:Description>
                                </owl:withRestrictions>
                            </rdfs:Datatype>
                        </owl:someValuesFrom>
                    </owl:Restriction>
                </owl:intersectionOf>
            </owl:Class>
        </owl:equivalentClass>
        <rdfs:subClassOf rdf:resource="http://dbpedia.org/ontology/horse"/>
        <rdfs:subClassOf rdf:resource="http://www.semanticweb.org/annag/ontologies/2024/1/ontoHorses#Cavallo"/>
        <rdfs:comment xml:lang="it">Cavallo di età inferiore ai 6 anni</rdfs:comment>
        <rdfs:comment xml:lang="en">Horse under 6 years of age</rdfs:comment>
        <rdfs:label xml:lang="en">Foal</rdfs:label>
        <rdfs:label xml:lang="it">Puledro</rdfs:label>
    </owl:Class>
    


    <!-- http://www.semanticweb.org/annag/ontologies/2024/1/ontoHorses#RazzaASangueCaldo -->

    <owl:Class rdf:about="http://www.semanticweb.org/annag/ontologies/2024/1/ontoHorses#RazzaASangueCaldo">
        <owl:equivalentClass>
            <owl:Class>
                <owl:intersectionOf rdf:parseType="Collection">
                    <rdf:Description rdf:about="http://www.semanticweb.org/annag/ontologies/2024/1/ontoHorses#RazzaCavallo"/>
                    <owl:Restriction>
                        <owl:onProperty rdf:resource="http://www.semanticweb.org/annag/ontologies/2024/1/ontoHorses#haIndole"/>
                        <owl:hasValue rdf:resource="http://www.semanticweb.org/annag/ontologies/2024/1/ontoHorses#sangueCaldo"/>
                    </owl:Restriction>
                </owl:intersectionOf>
            </owl:Class>
        </owl:equivalentClass>
        <rdfs:subClassOf rdf:resource="http://www.semanticweb.org/annag/ontologies/2024/1/ontoHorses#RazzaCavallo"/>
        <rdfs:comment xml:lang="en">Horse breed with warm-blooded temperament</rdfs:comment>
        <rdfs:comment xml:lang="it">Razza di cavallo con temperamento a sangue caldo</rdfs:comment>
        <rdfs:label xml:lang="it">Razza di cavallo a sangue caldo</rdfs:label>
        <rdfs:label xml:lang="en">warm-blooded horse breed</rdfs:label>
    </owl:Class>
    


    <!-- http://www.semanticweb.org/annag/ontologies/2024/1/ontoHorses#RazzaASangueFreddo -->

    <owl:Class rdf:about="http://www.semanticweb.org/annag/ontologies/2024/1/ontoHorses#RazzaASangueFreddo">
        <owl:equivalentClass>
            <owl:Class>
                <owl:intersectionOf rdf:parseType="Collection">
                    <rdf:Description rdf:about="http://www.semanticweb.org/annag/ontologies/2024/1/ontoHorses#RazzaCavallo"/>
                    <owl:Restriction>
                        <owl:onProperty rdf:resource="http://www.semanticweb.org/annag/ontologies/2024/1/ontoHorses#haIndole"/>
                        <owl:hasValue rdf:resource="http://www.semanticweb.org/annag/ontologies/2024/1/ontoHorses#sangueFreddo"/>
                    </owl:Restriction>
                </owl:intersectionOf>
            </owl:Class>
        </owl:equivalentClass>
        <rdfs:subClassOf rdf:resource="http://www.semanticweb.org/annag/ontologies/2024/1/ontoHorses#RazzaCavallo"/>
        <rdfs:comment xml:lang="en">Horse breed with cold-blooded temperament</rdfs:comment>
        <rdfs:comment xml:lang="it">Razza di cavallo con temperamento a sangue freddo</rdfs:comment>
        <rdfs:label xml:lang="en">Cold-blooded horse breed</rdfs:label>
        <rdfs:label xml:lang="it">Razza di cavallo a sangue freddo</rdfs:label>
    </owl:Class>
    


    <!-- http://www.semanticweb.org/annag/ontologies/2024/1/ontoHorses#RazzaASangueMisto -->

    <owl:Class rdf:about="http://www.semanticweb.org/annag/ontologies/2024/1/ontoHorses#RazzaASangueMisto">
        <owl:equivalentClass>
            <owl:Class>
                <owl:intersectionOf rdf:parseType="Collection">
                    <rdf:Description rdf:about="http://www.semanticweb.org/annag/ontologies/2024/1/ontoHorses#RazzaCavallo"/>
                    <owl:Restriction>
                        <owl:onProperty rdf:resource="http://www.semanticweb.org/annag/ontologies/2024/1/ontoHorses#haIndole"/>
                        <owl:hasValue rdf:resource="http://www.semanticweb.org/annag/ontologies/2024/1/ontoHorses#sangueMisto"/>
                    </owl:Restriction>
                </owl:intersectionOf>
            </owl:Class>
        </owl:equivalentClass>
        <rdfs:subClassOf rdf:resource="http://www.semanticweb.org/annag/ontologies/2024/1/ontoHorses#RazzaCavallo"/>
        <rdfs:comment xml:lang="en">Horse breed with mixed-blooded temperament</rdfs:comment>
        <rdfs:comment xml:lang="it">Razza di cavallo con temperamento a sangue misto</rdfs:comment>
        <rdfs:label xml:lang="en">Mixed-blooded horse breed</rdfs:label>
        <rdfs:label xml:lang="it">Razza di cavallo a sangue misto</rdfs:label>
    </owl:Class>
    


    <!-- http://www.semanticweb.org/annag/ontologies/2024/1/ontoHorses#RazzaBelga -->

    <owl:Class rdf:about="http://www.semanticweb.org/annag/ontologies/2024/1/ontoHorses#RazzaBelga">
        <owl:equivalentClass>
            <owl:Class>
                <owl:intersectionOf rdf:parseType="Collection">
                    <rdf:Description rdf:about="http://www.semanticweb.org/annag/ontologies/2024/1/ontoHorses#RazzaEuropea"/>
                    <owl:Restriction>
                        <owl:onProperty rdf:resource="http://www.semanticweb.org/annag/ontologies/2024/1/ontoHorses#haNazionalità"/>
                        <owl:hasValue rdf:resource="http://www.semanticweb.org/annag/ontologies/2024/1/ontoHorses#Belgio"/>
                    </owl:Restriction>
                </owl:intersectionOf>
            </owl:Class>
        </owl:equivalentClass>
        <rdfs:subClassOf rdf:resource="http://www.semanticweb.org/annag/ontologies/2024/1/ontoHorses#RazzaEuropea"/>
        <rdfs:comment xml:lang="en">Horse breed originated from Belgium</rdfs:comment>
        <rdfs:comment xml:lang="it">Razza di cavallo originaria del Belgio</rdfs:comment>
        <rdfs:label xml:lang="en">Belgian horse breed</rdfs:label>
        <rdfs:label xml:lang="it">Razza belga</rdfs:label>
    </owl:Class>
    


    <!-- http://www.semanticweb.org/annag/ontologies/2024/1/ontoHorses#RazzaBrachimorfa -->

    <owl:Class rdf:about="http://www.semanticweb.org/annag/ontologies/2024/1/ontoHorses#RazzaBrachimorfa">
        <owl:equivalentClass>
            <owl:Class>
                <owl:intersectionOf rdf:parseType="Collection">
                    <rdf:Description rdf:about="http://www.semanticweb.org/annag/ontologies/2024/1/ontoHorses#RazzaCavallo"/>
                    <owl:Restriction>
                        <owl:onProperty rdf:resource="http://www.semanticweb.org/annag/ontologies/2024/1/ontoHorses#haClassificazioneMorfologica"/>
                        <owl:hasValue rdf:resource="http://www.semanticweb.org/annag/ontologies/2024/1/ontoHorses#brachimorfo"/>
                    </owl:Restriction>
                </owl:intersectionOf>
            </owl:Class>
        </owl:equivalentClass>
        <rdfs:subClassOf rdf:resource="http://www.semanticweb.org/annag/ontologies/2024/1/ontoHorses#RazzaCavallo"/>
        <rdfs:comment xml:lang="en">Horse breed more inclined to the development of musculature, with a wide chest, powerful, massive and not very long shapes.</rdfs:comment>
        <rdfs:comment xml:lang="it">Razza di cavallo  più propenso allo sviluppo di muscolatura, con un torace ampio, forme potenti, massicce e non molto lungo.</rdfs:comment>
        <rdfs:label xml:lang="en">Brachymorphic horse breed</rdfs:label>
        <rdfs:label xml:lang="it">Razza brachimorfa</rdfs:label>
    </owl:Class>
    


    <!-- http://www.semanticweb.org/annag/ontologies/2024/1/ontoHorses#RazzaCavallo -->

    <owl:Class rdf:about="http://www.semanticweb.org/annag/ontologies/2024/1/ontoHorses#RazzaCavallo">
        <owl:equivalentClass>
            <owl:Restriction>
                <owl:onProperty rdf:resource="http://www.semanticweb.org/annag/ontologies/2024/1/ontoHorses#haClassificazioneMorfologica"/>
                <owl:someValuesFrom rdf:resource="http://www.semanticweb.org/annag/ontologies/2024/1/ontoHorses#Morfologia"/>
            </owl:Restriction>
        </owl:equivalentClass>
        <owl:equivalentClass>
            <owl:Restriction>
                <owl:onProperty rdf:resource="http://www.semanticweb.org/annag/ontologies/2024/1/ontoHorses#haIndole"/>
                <owl:someValuesFrom rdf:resource="http://www.semanticweb.org/annag/ontologies/2024/1/ontoHorses#Indole"/>
            </owl:Restriction>
        </owl:equivalentClass>
        <owl:equivalentClass>
            <owl:Restriction>
                <owl:onProperty rdf:resource="http://www.semanticweb.org/annag/ontologies/2024/1/ontoHorses#haRegioneDiOrigine"/>
                <owl:someValuesFrom rdf:resource="http://www.semanticweb.org/annag/ontologies/2024/1/ontoHorses#AreaGeografica"/>
            </owl:Restriction>
        </owl:equivalentClass>
        <owl:equivalentClass>
            <owl:Restriction>
                <owl:onProperty rdf:resource="http://www.semanticweb.org/annag/ontologies/2024/1/ontoHorses#puòEssereImpiegataIn"/>
                <owl:minQualifiedCardinality rdf:datatype="http://www.w3.org/2001/XMLSchema#nonNegativeInteger">1</owl:minQualifiedCardinality>
                <owl:onClass rdf:resource="http://www.semanticweb.org/annag/ontologies/2024/1/ontoHorses#Impiego"/>
            </owl:Restriction>
        </owl:equivalentClass>
        <rdfs:comment xml:lang="en">Defines the main horse breeds and their possible classifications.</rdfs:comment>
        <rdfs:comment xml:lang="it">Definisce le principali razze equine e le loro possibili classificazioni.</rdfs:comment>
        <rdfs:label xml:lang="en">Horse breed</rdfs:label>
        <rdfs:label xml:lang="it">Razza cavallo</rdfs:label>
    </owl:Class>
    


    <!-- http://www.semanticweb.org/annag/ontologies/2024/1/ontoHorses#RazzaDaAltaScuola -->

    <owl:Class rdf:about="http://www.semanticweb.org/annag/ontologies/2024/1/ontoHorses#RazzaDaAltaScuola">
        <owl:equivalentClass>
            <owl:Class>
                <owl:intersectionOf rdf:parseType="Collection">
                    <rdf:Description rdf:about="http://www.semanticweb.org/annag/ontologies/2024/1/ontoHorses#RazzaSportiva"/>
                    <owl:Restriction>
                        <owl:onProperty rdf:resource="http://www.semanticweb.org/annag/ontologies/2024/1/ontoHorses#puòEssereImpiegataIn"/>
                        <owl:hasValue rdf:resource="http://www.semanticweb.org/annag/ontologies/2024/1/ontoHorses#AltaScuola"/>
                    </owl:Restriction>
                </owl:intersectionOf>
            </owl:Class>
        </owl:equivalentClass>
        <rdfs:subClassOf rdf:resource="http://www.semanticweb.org/annag/ontologies/2024/1/ontoHorses#RazzaSportiva"/>
        <rdfs:comment xml:lang="en">Horse breed that can be used in the equestrian sport discipline of Spanish riding school</rdfs:comment>
        <rdfs:comment xml:lang="it">Razza di cavallo che può essere utilizzata nella disciplina di sport equestre dell&apos;Alta Scuola</rdfs:comment>
        <rdfs:label xml:lang="it">Razza da Alta Scuola</rdfs:label>
        <rdfs:label xml:lang="en">Spanish riding school horse breed</rdfs:label>
    </owl:Class>
    


    <!-- http://www.semanticweb.org/annag/ontologies/2024/1/ontoHorses#RazzaDaAttacchi -->

    <owl:Class rdf:about="http://www.semanticweb.org/annag/ontologies/2024/1/ontoHorses#RazzaDaAttacchi">
        <owl:equivalentClass>
            <owl:Class>
                <owl:intersectionOf rdf:parseType="Collection">
                    <rdf:Description rdf:about="http://www.semanticweb.org/annag/ontologies/2024/1/ontoHorses#RazzaDaAttacchi"/>
                    <owl:Restriction>
                        <owl:onProperty rdf:resource="http://www.semanticweb.org/annag/ontologies/2024/1/ontoHorses#puòEssereImpiegataIn"/>
                        <owl:hasValue rdf:resource="http://www.semanticweb.org/annag/ontologies/2024/1/ontoHorses#TrainoCarrozze"/>
                    </owl:Restriction>
                </owl:intersectionOf>
            </owl:Class>
        </owl:equivalentClass>
        <rdfs:subClassOf rdf:resource="http://www.semanticweb.org/annag/ontologies/2024/1/ontoHorses#RazzaDaLavoro"/>
        <rdfs:comment xml:lang="en">Horse breed used for pulling carriages</rdfs:comment>
        <rdfs:comment xml:lang="it">Razza di cavallo utilizzata per il traino carrozze</rdfs:comment>
        <rdfs:label xml:lang="en">Horse breed pulling carriages</rdfs:label>
        <rdfs:label xml:lang="it">Razza da attacchi</rdfs:label>
    </owl:Class>
    


    <!-- http://www.semanticweb.org/annag/ontologies/2024/1/ontoHorses#RazzaDaCrossCountry -->

    <owl:Class rdf:about="http://www.semanticweb.org/annag/ontologies/2024/1/ontoHorses#RazzaDaCrossCountry">
        <owl:equivalentClass>
            <owl:Class>
                <owl:intersectionOf rdf:parseType="Collection">
                    <rdf:Description rdf:about="http://www.semanticweb.org/annag/ontologies/2024/1/ontoHorses#RazzaSportiva"/>
                    <owl:Restriction>
                        <owl:onProperty rdf:resource="http://www.semanticweb.org/annag/ontologies/2024/1/ontoHorses#puòEssereImpiegataIn"/>
                        <owl:hasValue rdf:resource="http://www.semanticweb.org/annag/ontologies/2024/1/ontoHorses#CrossCountry"/>
                    </owl:Restriction>
                </owl:intersectionOf>
            </owl:Class>
        </owl:equivalentClass>
        <rdfs:subClassOf rdf:resource="http://www.semanticweb.org/annag/ontologies/2024/1/ontoHorses#RazzaSportiva"/>
        <rdfs:comment xml:lang="it">Razza di cavallo che può essere utilizzata nella disciplina di sport equestre del cross-country</rdfs:comment>
        <rdfs:label xml:lang="en">Cross-country horse breed</rdfs:label>
        <rdfs:label xml:lang="en">Horse breed that can be used in the equestrian sport discipline of cross-country</rdfs:label>
        <rdfs:label xml:lang="it">Razza da cross-country</rdfs:label>
    </owl:Class>
    


    <!-- http://www.semanticweb.org/annag/ontologies/2024/1/ontoHorses#RazzaDaDressage -->

    <owl:Class rdf:about="http://www.semanticweb.org/annag/ontologies/2024/1/ontoHorses#RazzaDaDressage">
        <owl:equivalentClass>
            <owl:Class>
                <owl:intersectionOf rdf:parseType="Collection">
                    <rdf:Description rdf:about="http://www.semanticweb.org/annag/ontologies/2024/1/ontoHorses#RazzaSportiva"/>
                    <owl:Restriction>
                        <owl:onProperty rdf:resource="http://www.semanticweb.org/annag/ontologies/2024/1/ontoHorses#puòEssereImpiegataIn"/>
                        <owl:hasValue rdf:resource="http://www.semanticweb.org/annag/ontologies/2024/1/ontoHorses#Dressage"/>
                    </owl:Restriction>
                </owl:intersectionOf>
            </owl:Class>
        </owl:equivalentClass>
        <rdfs:subClassOf rdf:resource="http://www.semanticweb.org/annag/ontologies/2024/1/ontoHorses#RazzaSportiva"/>
        <rdfs:comment xml:lang="en">Horse breed that can be used in the equestrian sport discipline of Dressage</rdfs:comment>
        <rdfs:comment xml:lang="it">Razza di cavallo che può essere utilizzata nella disciplina di sport equestre del Dressage</rdfs:comment>
        <rdfs:label xml:lang="en">Dressage horse breed</rdfs:label>
        <rdfs:label xml:lang="it">Razza da dressage</rdfs:label>
    </owl:Class>
    


    <!-- http://www.semanticweb.org/annag/ontologies/2024/1/ontoHorses#RazzaDaEquiturismo -->

    <owl:Class rdf:about="http://www.semanticweb.org/annag/ontologies/2024/1/ontoHorses#RazzaDaEquiturismo">
        <owl:equivalentClass>
            <owl:Class>
                <owl:intersectionOf rdf:parseType="Collection">
                    <rdf:Description rdf:about="http://www.semanticweb.org/annag/ontologies/2024/1/ontoHorses#RazzaDaSella"/>
                    <owl:Restriction>
                        <owl:onProperty rdf:resource="http://www.semanticweb.org/annag/ontologies/2024/1/ontoHorses#puòEssereImpiegataIn"/>
                        <owl:hasValue rdf:resource="http://www.semanticweb.org/annag/ontologies/2024/1/ontoHorses#Equiturismo"/>
                    </owl:Restriction>
                </owl:intersectionOf>
            </owl:Class>
        </owl:equivalentClass>
        <rdfs:subClassOf rdf:resource="http://www.semanticweb.org/annag/ontologies/2024/1/ontoHorses#RazzaDaSella"/>
        <rdfs:comment xml:lang="en">Horse breed that can be used for equestrian tourism (or trekking)</rdfs:comment>
        <rdfs:comment xml:lang="it">Razza di cavallo che può essere utilizzata per il turismo equestre (o trekking)</rdfs:comment>
        <rdfs:label xml:lang="en">Equestrian tourism horse breed</rdfs:label>
        <rdfs:label xml:lang="it">Razza da equiturismo</rdfs:label>
    </owl:Class>
    


    <!-- http://www.semanticweb.org/annag/ontologies/2024/1/ontoHorses#RazzaDaEventing -->

    <owl:Class rdf:about="http://www.semanticweb.org/annag/ontologies/2024/1/ontoHorses#RazzaDaEventing">
        <owl:equivalentClass>
            <owl:Class>
                <owl:intersectionOf rdf:parseType="Collection">
                    <rdf:Description rdf:about="http://www.semanticweb.org/annag/ontologies/2024/1/ontoHorses#RazzaSportiva"/>
                    <owl:Restriction>
                        <owl:onProperty rdf:resource="http://www.semanticweb.org/annag/ontologies/2024/1/ontoHorses#puòEssereImpiegataIn"/>
                        <owl:hasValue rdf:resource="http://www.semanticweb.org/annag/ontologies/2024/1/ontoHorses#Eventing"/>
                    </owl:Restriction>
                </owl:intersectionOf>
            </owl:Class>
        </owl:equivalentClass>
        <rdfs:subClassOf rdf:resource="http://www.semanticweb.org/annag/ontologies/2024/1/ontoHorses#RazzaSportiva"/>
        <rdfs:comment xml:lang="en">Horse breed that can be used in the equestrian sport discipline of eventing</rdfs:comment>
        <rdfs:comment xml:lang="it">Razza di cavallo che può essere utilizzata nella disciplina di sport equestre dell&apos;eventing</rdfs:comment>
        <rdfs:label xml:lang="en">Eventing horse breed</rdfs:label>
        <rdfs:label xml:lang="it">Razza da eventing</rdfs:label>
    </owl:Class>
    


    <!-- http://www.semanticweb.org/annag/ontologies/2024/1/ontoHorses#RazzaDaLavoro -->

    <owl:Class rdf:about="http://www.semanticweb.org/annag/ontologies/2024/1/ontoHorses#RazzaDaLavoro">
        <owl:equivalentClass>
            <owl:Class>
                <owl:intersectionOf rdf:parseType="Collection">
                    <rdf:Description rdf:about="http://www.semanticweb.org/annag/ontologies/2024/1/ontoHorses#RazzaCavallo"/>
                    <owl:Restriction>
                        <owl:onProperty rdf:resource="http://www.semanticweb.org/annag/ontologies/2024/1/ontoHorses#puòEssereImpiegataIn"/>
                        <owl:minQualifiedCardinality rdf:datatype="http://www.w3.org/2001/XMLSchema#nonNegativeInteger">1</owl:minQualifiedCardinality>
                        <owl:onClass rdf:resource="http://www.semanticweb.org/annag/ontologies/2024/1/ontoHorses#Lavoro"/>
                    </owl:Restriction>
                </owl:intersectionOf>
            </owl:Class>
        </owl:equivalentClass>
        <rdfs:subClassOf rdf:resource="http://www.semanticweb.org/annag/ontologies/2024/1/ontoHorses#RazzaCavallo"/>
        <rdfs:comment xml:lang="en">Breed of horse used in agricultural work or for pulling carriages</rdfs:comment>
        <rdfs:comment xml:lang="it">Razza di cavallo impiegata in attività lavorative agricole o di traino carrozze</rdfs:comment>
        <rdfs:label xml:lang="en">Horse breed for work</rdfs:label>
        <rdfs:label xml:lang="it">Razza da lavoro</rdfs:label>
    </owl:Class>
    


    <!-- http://www.semanticweb.org/annag/ontologies/2024/1/ontoHorses#RazzaDaSaltoOstacoli -->

    <owl:Class rdf:about="http://www.semanticweb.org/annag/ontologies/2024/1/ontoHorses#RazzaDaSaltoOstacoli">
        <owl:equivalentClass>
            <owl:Class>
                <owl:intersectionOf rdf:parseType="Collection">
                    <rdf:Description rdf:about="http://www.semanticweb.org/annag/ontologies/2024/1/ontoHorses#RazzaSportiva"/>
                    <owl:Restriction>
                        <owl:onProperty rdf:resource="http://www.semanticweb.org/annag/ontologies/2024/1/ontoHorses#puòEssereImpiegataIn"/>
                        <owl:hasValue rdf:resource="http://www.semanticweb.org/annag/ontologies/2024/1/ontoHorses#SaltoAdOstacoli"/>
                    </owl:Restriction>
                </owl:intersectionOf>
            </owl:Class>
        </owl:equivalentClass>
        <rdfs:subClassOf rdf:resource="http://www.semanticweb.org/annag/ontologies/2024/1/ontoHorses#RazzaSportiva"/>
        <rdfs:comment xml:lang="en">Horse breed that can be used in the equestrian sport discipline of jumping</rdfs:comment>
        <rdfs:comment xml:lang="it">Razza di cavallo che può essere utilizzata nella disciplina di sport equestre del salto ostacoli</rdfs:comment>
        <rdfs:label xml:lang="en">Jumping horse breed</rdfs:label>
        <rdfs:label xml:lang="it">Razza da salto ostacoli</rdfs:label>
    </owl:Class>
    


    <!-- http://www.semanticweb.org/annag/ontologies/2024/1/ontoHorses#RazzaDaSella -->

    <owl:Class rdf:about="http://www.semanticweb.org/annag/ontologies/2024/1/ontoHorses#RazzaDaSella">
        <owl:equivalentClass>
            <owl:Class>
                <owl:intersectionOf rdf:parseType="Collection">
                    <rdf:Description rdf:about="http://www.semanticweb.org/annag/ontologies/2024/1/ontoHorses#RazzaCavallo"/>
                    <owl:Restriction>
                        <owl:onProperty rdf:resource="http://www.semanticweb.org/annag/ontologies/2024/1/ontoHorses#puòEssereImpiegataIn"/>
                        <owl:someValuesFrom rdf:resource="http://www.semanticweb.org/annag/ontologies/2024/1/ontoHorses#Sella"/>
                    </owl:Restriction>
                </owl:intersectionOf>
            </owl:Class>
        </owl:equivalentClass>
        <rdfs:subClassOf rdf:resource="http://www.semanticweb.org/annag/ontologies/2024/1/ontoHorses#RazzaCavallo"/>
        <rdfs:comment xml:lang="en">Horse breed suitable for the saddle</rdfs:comment>
        <rdfs:comment xml:lang="it">Razza di cavallo che ha attitudine alla sella</rdfs:comment>
        <rdfs:label xml:lang="it">Razza da sella</rdfs:label>
        <rdfs:label xml:lang="en">Riding horse breed</rdfs:label>
    </owl:Class>
    


    <!-- http://www.semanticweb.org/annag/ontologies/2024/1/ontoHorses#RazzaDaTiroAgricolo -->

    <owl:Class rdf:about="http://www.semanticweb.org/annag/ontologies/2024/1/ontoHorses#RazzaDaTiroAgricolo">
        <owl:equivalentClass>
            <owl:Class>
                <owl:intersectionOf rdf:parseType="Collection">
                    <rdf:Description rdf:about="http://www.semanticweb.org/annag/ontologies/2024/1/ontoHorses#RazzaDaLavoro"/>
                    <owl:Restriction>
                        <owl:onProperty rdf:resource="http://www.semanticweb.org/annag/ontologies/2024/1/ontoHorses#puòEssereImpiegataIn"/>
                        <owl:hasValue rdf:resource="http://www.semanticweb.org/annag/ontologies/2024/1/ontoHorses#TiroAgricolo"/>
                    </owl:Restriction>
                </owl:intersectionOf>
            </owl:Class>
        </owl:equivalentClass>
        <rdfs:subClassOf rdf:resource="http://www.semanticweb.org/annag/ontologies/2024/1/ontoHorses#RazzaDaLavoro"/>
        <rdfs:comment xml:lang="en">Horse breed used for agricultural work</rdfs:comment>
        <rdfs:comment xml:lang="it">Razza di cavallo utilizzata nelle attività agricole</rdfs:comment>
        <rdfs:label xml:lang="en">Horse breed for agricultural work</rdfs:label>
        <rdfs:label xml:lang="it">Razza da tiro agricolo</rdfs:label>
    </owl:Class>
    


    <!-- http://www.semanticweb.org/annag/ontologies/2024/1/ontoHorses#RazzaDanese -->

    <owl:Class rdf:about="http://www.semanticweb.org/annag/ontologies/2024/1/ontoHorses#RazzaDanese">
        <owl:equivalentClass>
            <owl:Class>
                <owl:intersectionOf rdf:parseType="Collection">
                    <rdf:Description rdf:about="http://www.semanticweb.org/annag/ontologies/2024/1/ontoHorses#RazzaEuropea"/>
                    <owl:Restriction>
                        <owl:onProperty rdf:resource="http://www.semanticweb.org/annag/ontologies/2024/1/ontoHorses#haNazionalità"/>
                        <owl:hasValue rdf:resource="http://www.semanticweb.org/annag/ontologies/2024/1/ontoHorses#Danimarca"/>
                    </owl:Restriction>
                </owl:intersectionOf>
            </owl:Class>
        </owl:equivalentClass>
        <rdfs:subClassOf rdf:resource="http://www.semanticweb.org/annag/ontologies/2024/1/ontoHorses#RazzaEuropea"/>
        <rdfs:comment xml:lang="en">Horse breed originated from Denmark</rdfs:comment>
        <rdfs:comment xml:lang="it">Razza di cavallo originaria della Danimarca</rdfs:comment>
        <rdfs:label xml:lang="en">Danish horse breed</rdfs:label>
        <rdfs:label xml:lang="it">Razza danese</rdfs:label>
    </owl:Class>
    


    <!-- http://www.semanticweb.org/annag/ontologies/2024/1/ontoHorses#RazzaDolicomorfa -->

    <owl:Class rdf:about="http://www.semanticweb.org/annag/ontologies/2024/1/ontoHorses#RazzaDolicomorfa">
        <owl:equivalentClass>
            <owl:Class>
                <owl:intersectionOf rdf:parseType="Collection">
                    <rdf:Description rdf:about="http://www.semanticweb.org/annag/ontologies/2024/1/ontoHorses#RazzaCavallo"/>
                    <owl:Restriction>
                        <owl:onProperty rdf:resource="http://www.semanticweb.org/annag/ontologies/2024/1/ontoHorses#haClassificazioneMorfologica"/>
                        <owl:hasValue rdf:resource="http://www.semanticweb.org/annag/ontologies/2024/1/ontoHorses#dolicomorfo"/>
                    </owl:Restriction>
                </owl:intersectionOf>
            </owl:Class>
        </owl:equivalentClass>
        <rdfs:subClassOf rdf:resource="http://www.semanticweb.org/annag/ontologies/2024/1/ontoHorses#RazzaCavallo"/>
        <rdfs:comment xml:lang="en">Horse breed more suitable for fast and long gaits than for tests of strength: it has a deep chest, elongated lines and joints with very open angles. The figure is agile, light and slender.</rdfs:comment>
        <rdfs:comment xml:lang="it">Razza di cavallo più idoneo alle andature veloci e allungate che alle prove di forza: ha torace profondo, linee allungate e articolazioni con angoli molto aperti. La figura è agile, leggera e slanciata.</rdfs:comment>
        <rdfs:label xml:lang="en">Dolicomorphic horse breed</rdfs:label>
        <rdfs:label xml:lang="it">Razza dolicomorfa</rdfs:label>
    </owl:Class>
    


    <!-- http://www.semanticweb.org/annag/ontologies/2024/1/ontoHorses#RazzaEndurance -->

    <owl:Class rdf:about="http://www.semanticweb.org/annag/ontologies/2024/1/ontoHorses#RazzaEndurance">
        <owl:equivalentClass>
            <owl:Class>
                <owl:intersectionOf rdf:parseType="Collection">
                    <rdf:Description rdf:about="http://www.semanticweb.org/annag/ontologies/2024/1/ontoHorses#RazzaSportiva"/>
                    <owl:Restriction>
                        <owl:onProperty rdf:resource="http://www.semanticweb.org/annag/ontologies/2024/1/ontoHorses#puòEssereImpiegataIn"/>
                        <owl:hasValue rdf:resource="http://www.semanticweb.org/annag/ontologies/2024/1/ontoHorses#Endurance"/>
                    </owl:Restriction>
                </owl:intersectionOf>
            </owl:Class>
        </owl:equivalentClass>
        <rdfs:subClassOf rdf:resource="http://www.semanticweb.org/annag/ontologies/2024/1/ontoHorses#RazzaSportiva"/>
        <rdfs:comment xml:lang="en">Horse breed that can be used in the equestrian sport discipline of endurance</rdfs:comment>
        <rdfs:comment xml:lang="it">Razza di cavallo che può essere utilizzata nella disciplina di sport equestre dell&apos;endurance</rdfs:comment>
        <rdfs:label xml:lang="en">Endurance horse breed</rdfs:label>
        <rdfs:label xml:lang="it">Razza da endurance</rdfs:label>
    </owl:Class>
    


    <!-- http://www.semanticweb.org/annag/ontologies/2024/1/ontoHorses#RazzaEuropea -->

    <owl:Class rdf:about="http://www.semanticweb.org/annag/ontologies/2024/1/ontoHorses#RazzaEuropea">
        <rdfs:subClassOf rdf:resource="http://www.semanticweb.org/annag/ontologies/2024/1/ontoHorses#RazzaCavallo"/>
        <rdfs:comment xml:lang="en">Horse breed originating from Europe</rdfs:comment>
        <rdfs:comment xml:lang="it">Razza di cavallo originaria dell&apos;Europa</rdfs:comment>
        <rdfs:label xml:lang="en">European horse breed</rdfs:label>
        <rdfs:label xml:lang="it">Razza europea</rdfs:label>
    </owl:Class>
    


    <!-- http://www.semanticweb.org/annag/ontologies/2024/1/ontoHorses#RazzaFrancese -->

    <owl:Class rdf:about="http://www.semanticweb.org/annag/ontologies/2024/1/ontoHorses#RazzaFrancese">
        <owl:equivalentClass>
            <owl:Class>
                <owl:intersectionOf rdf:parseType="Collection">
                    <rdf:Description rdf:about="http://www.semanticweb.org/annag/ontologies/2024/1/ontoHorses#RazzaEuropea"/>
                    <owl:Restriction>
                        <owl:onProperty rdf:resource="http://www.semanticweb.org/annag/ontologies/2024/1/ontoHorses#haNazionalità"/>
                        <owl:hasValue rdf:resource="http://www.semanticweb.org/annag/ontologies/2024/1/ontoHorses#Francia"/>
                    </owl:Restriction>
                </owl:intersectionOf>
            </owl:Class>
        </owl:equivalentClass>
        <rdfs:subClassOf rdf:resource="http://www.semanticweb.org/annag/ontologies/2024/1/ontoHorses#RazzaEuropea"/>
        <rdfs:comment xml:lang="en">Horse breed originated from France</rdfs:comment>
        <rdfs:comment xml:lang="it">Razza di cavallo originaria della Francia</rdfs:comment>
        <rdfs:label xml:lang="en">French horse breed</rdfs:label>
        <rdfs:label xml:lang="it">Razza francese</rdfs:label>
    </owl:Class>
    


    <!-- http://www.semanticweb.org/annag/ontologies/2024/1/ontoHorses#RazzaInglese -->

    <owl:Class rdf:about="http://www.semanticweb.org/annag/ontologies/2024/1/ontoHorses#RazzaInglese">
        <owl:equivalentClass>
            <owl:Class>
                <owl:intersectionOf rdf:parseType="Collection">
                    <rdf:Description rdf:about="http://www.semanticweb.org/annag/ontologies/2024/1/ontoHorses#RazzaEuropea"/>
                    <owl:Restriction>
                        <owl:onProperty rdf:resource="http://www.semanticweb.org/annag/ontologies/2024/1/ontoHorses#haNazionalità"/>
                        <owl:hasValue rdf:resource="http://www.semanticweb.org/annag/ontologies/2024/1/ontoHorses#RegnoUnito"/>
                    </owl:Restriction>
                </owl:intersectionOf>
            </owl:Class>
        </owl:equivalentClass>
        <rdfs:subClassOf rdf:resource="http://www.semanticweb.org/annag/ontologies/2024/1/ontoHorses#RazzaEuropea"/>
        <rdfs:comment xml:lang="en">Horse breed originated from United Kingdom</rdfs:comment>
        <rdfs:comment xml:lang="it">Razza di cavallo originaria del Regno Unito</rdfs:comment>
        <rdfs:label xml:lang="en">English horse breed</rdfs:label>
        <rdfs:label xml:lang="it">Razza inglese</rdfs:label>
    </owl:Class>
    


    <!-- http://www.semanticweb.org/annag/ontologies/2024/1/ontoHorses#RazzaItaliana -->

    <owl:Class rdf:about="http://www.semanticweb.org/annag/ontologies/2024/1/ontoHorses#RazzaItaliana">
        <owl:equivalentClass>
            <owl:Class>
                <owl:intersectionOf rdf:parseType="Collection">
                    <rdf:Description rdf:about="http://www.semanticweb.org/annag/ontologies/2024/1/ontoHorses#RazzaEuropea"/>
                    <owl:Restriction>
                        <owl:onProperty rdf:resource="http://www.semanticweb.org/annag/ontologies/2024/1/ontoHorses#haNazionalità"/>
                        <owl:hasValue rdf:resource="http://www.semanticweb.org/annag/ontologies/2024/1/ontoHorses#Italia"/>
                    </owl:Restriction>
                </owl:intersectionOf>
            </owl:Class>
        </owl:equivalentClass>
        <rdfs:subClassOf rdf:resource="http://www.semanticweb.org/annag/ontologies/2024/1/ontoHorses#RazzaEuropea"/>
        <rdfs:comment xml:lang="en">Horse breed originated from Italy</rdfs:comment>
        <rdfs:comment xml:lang="it">Razza di cavallo originaria dell&apos;Italia</rdfs:comment>
        <rdfs:label xml:lang="en">Italian horse breed</rdfs:label>
        <rdfs:label xml:lang="it">Razza italiana</rdfs:label>
    </owl:Class>
    


    <!-- http://www.semanticweb.org/annag/ontologies/2024/1/ontoHorses#RazzaMesoBrachimorfa -->

    <owl:Class rdf:about="http://www.semanticweb.org/annag/ontologies/2024/1/ontoHorses#RazzaMesoBrachimorfa">
        <owl:equivalentClass>
            <owl:Class>
                <owl:intersectionOf rdf:parseType="Collection">
                    <rdf:Description rdf:about="http://www.semanticweb.org/annag/ontologies/2024/1/ontoHorses#RazzaCavallo"/>
                    <owl:Restriction>
                        <owl:onProperty rdf:resource="http://www.semanticweb.org/annag/ontologies/2024/1/ontoHorses#haClassificazioneMorfologica"/>
                        <owl:hasValue rdf:resource="http://www.semanticweb.org/annag/ontologies/2024/1/ontoHorses#mesoBrachimorfo"/>
                    </owl:Restriction>
                </owl:intersectionOf>
            </owl:Class>
        </owl:equivalentClass>
        <rdfs:subClassOf rdf:resource="http://www.semanticweb.org/annag/ontologies/2024/1/ontoHorses#RazzaCavallo"/>
        <rdfs:comment xml:lang="en">Horse breed between draft horses and riding horses.</rdfs:comment>
        <rdfs:comment xml:lang="it">Razza di cavallo a metà strada tra i cavalli da tiro e i cavalli da sella.</rdfs:comment>
        <rdfs:label xml:lang="en">Meso-brachimorphyc horse breed</rdfs:label>
        <rdfs:label xml:lang="it">Razza meso-brachimorfa</rdfs:label>
    </owl:Class>
    


    <!-- http://www.semanticweb.org/annag/ontologies/2024/1/ontoHorses#RazzaMesoDolicomorfa -->

    <owl:Class rdf:about="http://www.semanticweb.org/annag/ontologies/2024/1/ontoHorses#RazzaMesoDolicomorfa">
        <owl:equivalentClass>
            <owl:Class>
                <owl:intersectionOf rdf:parseType="Collection">
                    <rdf:Description rdf:about="http://www.semanticweb.org/annag/ontologies/2024/1/ontoHorses#RazzaCavallo"/>
                    <owl:Restriction>
                        <owl:onProperty rdf:resource="http://www.semanticweb.org/annag/ontologies/2024/1/ontoHorses#haClassificazioneMorfologica"/>
                        <owl:hasValue rdf:resource="http://www.semanticweb.org/annag/ontologies/2024/1/ontoHorses#mesoDolicomorfo"/>
                    </owl:Restriction>
                </owl:intersectionOf>
            </owl:Class>
        </owl:equivalentClass>
        <rdfs:subClassOf rdf:resource="http://www.semanticweb.org/annag/ontologies/2024/1/ontoHorses#RazzaCavallo"/>
        <rdfs:comment xml:lang="en">Powerful horse breed, strong but at the same time agile and noble in bearing.</rdfs:comment>
        <rdfs:comment xml:lang="it">Razza di cavallo potente, forte ma contemporaneamente agile e nobile nel portamento.</rdfs:comment>
        <rdfs:label xml:lang="en">Meso-dolicomorphic horse breed</rdfs:label>
        <rdfs:label xml:lang="it">Razza meso-dolicomorfa</rdfs:label>
    </owl:Class>
    


    <!-- http://www.semanticweb.org/annag/ontologies/2024/1/ontoHorses#RazzaOlandese -->

    <owl:Class rdf:about="http://www.semanticweb.org/annag/ontologies/2024/1/ontoHorses#RazzaOlandese">
        <owl:equivalentClass>
            <owl:Class>
                <owl:intersectionOf rdf:parseType="Collection">
                    <rdf:Description rdf:about="http://www.semanticweb.org/annag/ontologies/2024/1/ontoHorses#RazzaEuropea"/>
                    <owl:Restriction>
                        <owl:onProperty rdf:resource="http://www.semanticweb.org/annag/ontologies/2024/1/ontoHorses#haNazionalità"/>
                        <owl:hasValue rdf:resource="http://www.semanticweb.org/annag/ontologies/2024/1/ontoHorses#PaesiBassi"/>
                    </owl:Restriction>
                </owl:intersectionOf>
            </owl:Class>
        </owl:equivalentClass>
        <rdfs:subClassOf rdf:resource="http://www.semanticweb.org/annag/ontologies/2024/1/ontoHorses#RazzaEuropea"/>
        <rdfs:comment xml:lang="en">Horse breed originated from Holland</rdfs:comment>
        <rdfs:comment xml:lang="it">Razza di cavallo originaria dei Paesi Bassi</rdfs:comment>
        <rdfs:label xml:lang="en">Dutch horse breed</rdfs:label>
        <rdfs:label xml:lang="it">Razza olandese</rdfs:label>
    </owl:Class>
    


    <!-- http://www.semanticweb.org/annag/ontologies/2024/1/ontoHorses#RazzaPortoghese -->

    <owl:Class rdf:about="http://www.semanticweb.org/annag/ontologies/2024/1/ontoHorses#RazzaPortoghese">
        <owl:equivalentClass>
            <owl:Class>
                <owl:intersectionOf rdf:parseType="Collection">
                    <rdf:Description rdf:about="http://www.semanticweb.org/annag/ontologies/2024/1/ontoHorses#RazzaEuropea"/>
                    <owl:Restriction>
                        <owl:onProperty rdf:resource="http://www.semanticweb.org/annag/ontologies/2024/1/ontoHorses#haNazionalità"/>
                        <owl:hasValue rdf:resource="http://www.semanticweb.org/annag/ontologies/2024/1/ontoHorses#Portogallo"/>
                    </owl:Restriction>
                </owl:intersectionOf>
            </owl:Class>
        </owl:equivalentClass>
        <rdfs:subClassOf rdf:resource="http://www.semanticweb.org/annag/ontologies/2024/1/ontoHorses#RazzaEuropea"/>
        <rdfs:comment xml:lang="en">Horse breed originated from Portugal</rdfs:comment>
        <rdfs:comment xml:lang="it">Razza di cavallo originaria del Portogallo</rdfs:comment>
        <rdfs:label xml:lang="en">Portoguese horse breed</rdfs:label>
        <rdfs:label xml:lang="it">Razza portoghese</rdfs:label>
    </owl:Class>
    


    <!-- http://www.semanticweb.org/annag/ontologies/2024/1/ontoHorses#RazzaSpagnola -->

    <owl:Class rdf:about="http://www.semanticweb.org/annag/ontologies/2024/1/ontoHorses#RazzaSpagnola">
        <owl:equivalentClass>
            <owl:Class>
                <owl:intersectionOf rdf:parseType="Collection">
                    <rdf:Description rdf:about="http://www.semanticweb.org/annag/ontologies/2024/1/ontoHorses#RazzaEuropea"/>
                    <owl:Restriction>
                        <owl:onProperty rdf:resource="http://www.semanticweb.org/annag/ontologies/2024/1/ontoHorses#haNazionalità"/>
                        <owl:hasValue rdf:resource="http://www.semanticweb.org/annag/ontologies/2024/1/ontoHorses#Spagna"/>
                    </owl:Restriction>
                </owl:intersectionOf>
            </owl:Class>
        </owl:equivalentClass>
        <rdfs:subClassOf rdf:resource="http://www.semanticweb.org/annag/ontologies/2024/1/ontoHorses#RazzaEuropea"/>
        <rdfs:comment xml:lang="en">Horse breed originated from Spain</rdfs:comment>
        <rdfs:comment xml:lang="it">Razza di cavallo originaria della Spagna</rdfs:comment>
        <rdfs:label xml:lang="it">Razza spagnola</rdfs:label>
        <rdfs:label xml:lang="en">Spanish horse breed</rdfs:label>
    </owl:Class>
    


    <!-- http://www.semanticweb.org/annag/ontologies/2024/1/ontoHorses#RazzaSportiva -->

    <owl:Class rdf:about="http://www.semanticweb.org/annag/ontologies/2024/1/ontoHorses#RazzaSportiva">
        <owl:equivalentClass>
            <owl:Class>
                <owl:intersectionOf rdf:parseType="Collection">
                    <rdf:Description rdf:about="http://www.semanticweb.org/annag/ontologies/2024/1/ontoHorses#RazzaDaSella"/>
                    <owl:Restriction>
                        <owl:onProperty rdf:resource="http://www.semanticweb.org/annag/ontologies/2024/1/ontoHorses#puòEssereImpiegataIn"/>
                        <owl:minQualifiedCardinality rdf:datatype="http://www.w3.org/2001/XMLSchema#nonNegativeInteger">1</owl:minQualifiedCardinality>
                        <owl:onClass rdf:resource="http://www.semanticweb.org/annag/ontologies/2024/1/ontoHorses#SportEquestre"/>
                    </owl:Restriction>
                </owl:intersectionOf>
            </owl:Class>
        </owl:equivalentClass>
        <rdfs:subClassOf rdf:resource="http://www.semanticweb.org/annag/ontologies/2024/1/ontoHorses#RazzaDaSella"/>
        <rdfs:comment xml:lang="en">Horse breed that can be used in equestrian sports</rdfs:comment>
        <rdfs:comment xml:lang="it">Razza di cavallo che può essere utilizzata negli sport equestri</rdfs:comment>
        <rdfs:label xml:lang="it">Razza sportiva</rdfs:label>
        <rdfs:label xml:lang="en">Sport horse breed</rdfs:label>
    </owl:Class>
    


    <!-- http://www.semanticweb.org/annag/ontologies/2024/1/ontoHorses#RazzamMesomorfa -->

    <owl:Class rdf:about="http://www.semanticweb.org/annag/ontologies/2024/1/ontoHorses#RazzamMesomorfa">
        <owl:equivalentClass>
            <owl:Class>
                <owl:intersectionOf rdf:parseType="Collection">
                    <rdf:Description rdf:about="http://www.semanticweb.org/annag/ontologies/2024/1/ontoHorses#RazzaCavallo"/>
                    <owl:Restriction>
                        <owl:onProperty rdf:resource="http://www.semanticweb.org/annag/ontologies/2024/1/ontoHorses#haClassificazioneMorfologica"/>
                        <owl:hasValue rdf:resource="http://www.semanticweb.org/annag/ontologies/2024/1/ontoHorses#mesomorfo"/>
                    </owl:Restriction>
                </owl:intersectionOf>
            </owl:Class>
        </owl:equivalentClass>
        <rdfs:subClassOf rdf:resource="http://www.semanticweb.org/annag/ontologies/2024/1/ontoHorses#RazzaCavallo"/>
        <rdfs:comment xml:lang="en">Horse breed with a much lighter physical structure than the brachymorph, but still powerful and compact.</rdfs:comment>
        <rdfs:comment xml:lang="it">Razza di cavallo con una struttura fisica molto più leggera rispetto al brachimorfo, ma comunque potente e compatta.</rdfs:comment>
        <rdfs:label xml:lang="en">Mesomorphic horse breed</rdfs:label>
        <rdfs:label xml:lang="it">Razza mesomorfa</rdfs:label>
    </owl:Class>
    


    <!-- http://www.semanticweb.org/annag/ontologies/2024/1/ontoHorses#SaltoAdOstacoli -->

    <owl:Class rdf:about="http://www.semanticweb.org/annag/ontologies/2024/1/ontoHorses#SaltoAdOstacoli">
        <rdfs:subClassOf rdf:resource="http://www.semanticweb.org/annag/ontologies/2024/1/ontoHorses#SportEquestre"/>
    </owl:Class>
    


    <!-- http://www.semanticweb.org/annag/ontologies/2024/1/ontoHorses#Sella -->

    <owl:Class rdf:about="http://www.semanticweb.org/annag/ontologies/2024/1/ontoHorses#Sella">
        <rdfs:subClassOf rdf:resource="http://www.semanticweb.org/annag/ontologies/2024/1/ontoHorses#Impiego"/>
        <rdfs:comment xml:lang="it">Impiego del cavallo che ha attitudine alla sella per turismo o sport</rdfs:comment>
        <rdfs:comment xml:lang="en">Use of the horse that is suited to the saddle for tourism or sport</rdfs:comment>
        <rdfs:label xml:lang="en">Saddle</rdfs:label>
        <rdfs:label xml:lang="it">Sella</rdfs:label>
    </owl:Class>
    


    <!-- http://www.semanticweb.org/annag/ontologies/2024/1/ontoHorses#SportEquestre -->

    <owl:Class rdf:about="http://www.semanticweb.org/annag/ontologies/2024/1/ontoHorses#SportEquestre">
        <rdfs:subClassOf rdf:resource="http://dbpedia.org/ontology/horseRidingDiscipline"/>
        <rdfs:subClassOf rdf:resource="http://www.semanticweb.org/annag/ontologies/2024/1/ontoHorses#Sella"/>
        <rdfs:comment xml:lang="it">Insieme degli sport che prevedono la monta di un cavallo</rdfs:comment>
        <rdfs:comment xml:lang="en">Set of sports that involve riding a horse</rdfs:comment>
        <rdfs:label xml:lang="en">Equestrian sport</rdfs:label>
        <rdfs:label xml:lang="it">Sport equestre</rdfs:label>
    </owl:Class>
    


    <!-- http://www.semanticweb.org/annag/ontologies/2024/1/ontoHorses#TiroAgricolo -->

    <owl:Class rdf:about="http://www.semanticweb.org/annag/ontologies/2024/1/ontoHorses#TiroAgricolo">
        <rdfs:subClassOf rdf:resource="http://www.semanticweb.org/annag/ontologies/2024/1/ontoHorses#Lavoro"/>
    </owl:Class>
    


    <!-- http://www.semanticweb.org/annag/ontologies/2024/1/ontoHorses#TrainoCarrozze -->

    <owl:Class rdf:about="http://www.semanticweb.org/annag/ontologies/2024/1/ontoHorses#TrainoCarrozze">
        <rdfs:subClassOf rdf:resource="http://www.semanticweb.org/annag/ontologies/2024/1/ontoHorses#Lavoro"/>
    </owl:Class>
    


    <!-- http://xmlns.com/foaf/0.1/person -->

    <owl:Class rdf:about="http://xmlns.com/foaf/0.1/person"/>
    


    <!-- 
    ///////////////////////////////////////////////////////////////////////////////////////
    //
    // Individuals
    //
    ///////////////////////////////////////////////////////////////////////////////////////
     -->

    


    <!-- http://www.semanticweb.org/annag/ontologies/2024/1/ontoHorses#AltaScuola -->

    <owl:NamedIndividual rdf:about="http://www.semanticweb.org/annag/ontologies/2024/1/ontoHorses#AltaScuola">
        <rdf:type rdf:resource="http://dbpedia.org/ontology/horseRidingDiscipline"/>
        <rdf:type rdf:resource="http://www.semanticweb.org/annag/ontologies/2024/1/ontoHorses#Impiego"/>
        <rdf:type rdf:resource="http://www.semanticweb.org/annag/ontologies/2024/1/ontoHorses#Sella"/>
        <rdf:type rdf:resource="http://www.semanticweb.org/annag/ontologies/2024/1/ontoHorses#SportEquestre"/>
    </owl:NamedIndividual>
    


    <!-- http://www.semanticweb.org/annag/ontologies/2024/1/ontoHorses#Andalusia -->

    <owl:NamedIndividual rdf:about="http://www.semanticweb.org/annag/ontologies/2024/1/ontoHorses#Andalusia">
        <rdf:type rdf:resource="http://schema.org/Place"/>
        <rdf:type rdf:resource="http://www.semanticweb.org/annag/ontologies/2024/1/ontoHorses#AreaGeografica"/>
        <partof:isPartOf rdf:resource="http://www.semanticweb.org/annag/ontologies/2024/1/ontoHorses#Spagna"/>
        <schema:image rdf:resource="https://upload.wikimedia.org/wikipedia/commons/thumb/2/2e/Andalucia_in_Spain_%28plus_Canarias%29.svg/260px-Andalucia_in_Spain_%28plus_Canarias%29.svg.png"/>
        <rdfs:comment xml:lang="en">Andalusia is one of the seventeen autonomous communities of Spain and has Seville as its capital</rdfs:comment>
        <rdfs:comment xml:lang="it">L&apos;Andalusìa  è una delle diciassette comunità autonome della Spagna ed ha Siviglia come capoluogo</rdfs:comment>
        <rdfs:label xml:lang="en">Andalusia</rdfs:label>
        <rdfs:label xml:lang="it">Andalusia</rdfs:label>
    </owl:NamedIndividual>
    


    <!-- http://www.semanticweb.org/annag/ontologies/2024/1/ontoHorses#Andaluso -->

    <owl:NamedIndividual rdf:about="http://www.semanticweb.org/annag/ontologies/2024/1/ontoHorses#Andaluso">
        <rdf:type rdf:resource="http://www.semanticweb.org/annag/ontologies/2024/1/ontoHorses#RazzaASangueCaldo"/>
        <rdf:type rdf:resource="http://www.semanticweb.org/annag/ontologies/2024/1/ontoHorses#RazzaCavallo"/>
        <rdf:type rdf:resource="http://www.semanticweb.org/annag/ontologies/2024/1/ontoHorses#RazzaDaAltaScuola"/>
        <rdf:type rdf:resource="http://www.semanticweb.org/annag/ontologies/2024/1/ontoHorses#RazzaDaDressage"/>
        <rdf:type rdf:resource="http://www.semanticweb.org/annag/ontologies/2024/1/ontoHorses#RazzaDaSella"/>
        <rdf:type rdf:resource="http://www.semanticweb.org/annag/ontologies/2024/1/ontoHorses#RazzaSportiva"/>
        <rdf:type rdf:resource="http://www.semanticweb.org/annag/ontologies/2024/1/ontoHorses#RazzamMesomorfa"/>
        <ontoHorses:entitàWikidata rdf:resource="http://www.wikidata.org/entity/Q489798"/>
        <ontoHorses:haClassificazioneMorfologica rdf:resource="http://www.semanticweb.org/annag/ontologies/2024/1/ontoHorses#mesomorfo"/>
        <ontoHorses:haIndole rdf:resource="http://www.semanticweb.org/annag/ontologies/2024/1/ontoHorses#sangueCaldo"/>
        <ontoHorses:haNazionalità rdf:resource="http://www.semanticweb.org/annag/ontologies/2024/1/ontoHorses#Spagna"/>
        <ontoHorses:haRegioneDiOrigine rdf:resource="http://www.semanticweb.org/annag/ontologies/2024/1/ontoHorses#Andalusia"/>
        <ontoHorses:puòEssereImpiegataIn rdf:resource="http://www.semanticweb.org/annag/ontologies/2024/1/ontoHorses#AltaScuola"/>
        <ontoHorses:puòEssereImpiegataIn rdf:resource="http://www.semanticweb.org/annag/ontologies/2024/1/ontoHorses#Dressage"/>
        <ontoHorses:altezzaMediaGarrese rdf:datatype="http://www.w3.org/2001/XMLSchema#integer">160</ontoHorses:altezzaMediaGarrese>
        <ontoHorses:haColoreMantello>baio</ontoHorses:haColoreMantello>
        <ontoHorses:haColoreMantello>grigio</ontoHorses:haColoreMantello>
        <ontoHorses:haColoreMantello>roano</ontoHorses:haColoreMantello>
        <ontoHorses:pesoMedio rdf:datatype="http://www.w3.org/2001/XMLSchema#integer">470</ontoHorses:pesoMedio>
        <schema:image rdf:resource="https://upload.wikimedia.org/wikipedia/commons/1/10/Fotografo-caballos-pura-raza.jpg"/>
        <rdfs:comment xml:lang="en">Mesomorphic Spanish horse breed with a noble and elegant bearing</rdfs:comment>
        <rdfs:comment xml:lang="it">Razza di cavallo Spagnola mesomorfa dal portamento nobile ed elegante</rdfs:comment>
        <skos:exactMatch xml:lang="it">http://www.wikidata.org/entity/Q489798</skos:exactMatch>
        <skos:prefLabel xml:lang="en">Andalusian Horse</skos:prefLabel>
        <skos:prefLabel xml:lang="it">Andaluso</skos:prefLabel>
    </owl:NamedIndividual>
    


    <!-- http://www.semanticweb.org/annag/ontologies/2024/1/ontoHorses#AngloAraboFrancese -->

    <owl:NamedIndividual rdf:about="http://www.semanticweb.org/annag/ontologies/2024/1/ontoHorses#AngloAraboFrancese">
        <rdf:type rdf:resource="http://www.semanticweb.org/annag/ontologies/2024/1/ontoHorses#RazzaASangueCaldo"/>
        <rdf:type rdf:resource="http://www.semanticweb.org/annag/ontologies/2024/1/ontoHorses#RazzaCavallo"/>
        <rdf:type rdf:resource="http://www.semanticweb.org/annag/ontologies/2024/1/ontoHorses#RazzaDaCrossCountry"/>
        <rdf:type rdf:resource="http://www.semanticweb.org/annag/ontologies/2024/1/ontoHorses#RazzaDaEventing"/>
        <rdf:type rdf:resource="http://www.semanticweb.org/annag/ontologies/2024/1/ontoHorses#RazzaDaSaltoOstacoli"/>
        <rdf:type rdf:resource="http://www.semanticweb.org/annag/ontologies/2024/1/ontoHorses#RazzaDaSella"/>
        <rdf:type rdf:resource="http://www.semanticweb.org/annag/ontologies/2024/1/ontoHorses#RazzaDolicomorfa"/>
        <rdf:type rdf:resource="http://www.semanticweb.org/annag/ontologies/2024/1/ontoHorses#RazzaEndurance"/>
        <rdf:type rdf:resource="http://www.semanticweb.org/annag/ontologies/2024/1/ontoHorses#RazzaSportiva"/>
        <ontoHorses:entitàWikidata rdf:resource="http://www.wikidata.org/entity/Q7029480"/>
        <ontoHorses:haClassificazioneMorfologica rdf:resource="http://www.semanticweb.org/annag/ontologies/2024/1/ontoHorses#dolicomorfo"/>
        <ontoHorses:haIndole rdf:resource="http://www.semanticweb.org/annag/ontologies/2024/1/ontoHorses#sangueCaldo"/>
        <ontoHorses:haNazionalità rdf:resource="http://www.semanticweb.org/annag/ontologies/2024/1/ontoHorses#Francia"/>
        <ontoHorses:haRegioneDiOrigine rdf:resource="http://www.semanticweb.org/annag/ontologies/2024/1/ontoHorses#Normandia"/>
        <ontoHorses:puòEssereImpiegataIn rdf:resource="http://www.semanticweb.org/annag/ontologies/2024/1/ontoHorses#CrossCountry"/>
        <ontoHorses:puòEssereImpiegataIn rdf:resource="http://www.semanticweb.org/annag/ontologies/2024/1/ontoHorses#Endurance"/>
        <ontoHorses:puòEssereImpiegataIn rdf:resource="http://www.semanticweb.org/annag/ontologies/2024/1/ontoHorses#Eventing"/>
        <ontoHorses:puòEssereImpiegataIn rdf:resource="http://www.semanticweb.org/annag/ontologies/2024/1/ontoHorses#SaltoAdOstacoli"/>
        <ontoHorses:altezzaMediaGarrese rdf:datatype="http://www.w3.org/2001/XMLSchema#integer">161</ontoHorses:altezzaMediaGarrese>
        <ontoHorses:haColoreMantello>baio</ontoHorses:haColoreMantello>
        <ontoHorses:haColoreMantello>grigio</ontoHorses:haColoreMantello>
        <ontoHorses:haColoreMantello>morello</ontoHorses:haColoreMantello>
        <ontoHorses:haColoreMantello>sauro</ontoHorses:haColoreMantello>
        <ontoHorses:pesoMedio rdf:datatype="http://www.w3.org/2001/XMLSchema#integer">475</ontoHorses:pesoMedio>
        <schema:image rdf:resource="https://upload.wikimedia.org/wikipedia/commons/thumb/8/87/Anglo-arabe-portrait02.JPG/220px-Anglo-arabe-portrait02.JPG"/>
        <rdfs:comment xml:lang="it">L&apos;anglo-arabo francese  è un cavallo sportivo di tipo dolicomorfo che ha caratteristiche intermedie tra il cavallo Arabo ed il Purosangue inglese.</rdfs:comment>
        <rdfs:comment xml:lang="en">The French Anglo-Arab is a dolichomorphic sport horse that has intermediate characteristics between the Arabian horse and the English Thoroughbred.</rdfs:comment>
        <skos:exactMatch xml:lang="it">http://www.wikidata.org/entity/Q7029480</skos:exactMatch>
        <skos:prefLabel xml:lang="it">Anglo-Arabo francese</skos:prefLabel>
        <skos:prefLabel xml:lang="en">French Anglo-Arab</skos:prefLabel>
    </owl:NamedIndividual>
    


    <!-- http://www.semanticweb.org/annag/ontologies/2024/1/ontoHorses#AngloAraboSpagnolo -->

    <owl:NamedIndividual rdf:about="http://www.semanticweb.org/annag/ontologies/2024/1/ontoHorses#AngloAraboSpagnolo">
        <rdf:type rdf:resource="http://www.semanticweb.org/annag/ontologies/2024/1/ontoHorses#RazzaASangueCaldo"/>
        <rdf:type rdf:resource="http://www.semanticweb.org/annag/ontologies/2024/1/ontoHorses#RazzaCavallo"/>
        <rdf:type rdf:resource="http://www.semanticweb.org/annag/ontologies/2024/1/ontoHorses#RazzaDaDressage"/>
        <rdf:type rdf:resource="http://www.semanticweb.org/annag/ontologies/2024/1/ontoHorses#RazzaDaEquiturismo"/>
        <rdf:type rdf:resource="http://www.semanticweb.org/annag/ontologies/2024/1/ontoHorses#RazzaDaSella"/>
        <rdf:type rdf:resource="http://www.semanticweb.org/annag/ontologies/2024/1/ontoHorses#RazzaDolicomorfa"/>
        <rdf:type rdf:resource="http://www.semanticweb.org/annag/ontologies/2024/1/ontoHorses#RazzaSportiva"/>
        <ontoHorses:entitàWikidata rdf:resource="http://www.wikidata.org/entity/Q3617386"/>
        <ontoHorses:haClassificazioneMorfologica rdf:resource="http://www.semanticweb.org/annag/ontologies/2024/1/ontoHorses#dolicomorfo"/>
        <ontoHorses:haIndole rdf:resource="http://www.semanticweb.org/annag/ontologies/2024/1/ontoHorses#sangueCaldo"/>
        <ontoHorses:haNazionalità rdf:resource="http://www.semanticweb.org/annag/ontologies/2024/1/ontoHorses#Spagna"/>
        <ontoHorses:haRegioneDiOrigine rdf:resource="http://www.semanticweb.org/annag/ontologies/2024/1/ontoHorses#Andalusia"/>
        <ontoHorses:puòEssereImpiegataIn rdf:resource="http://www.semanticweb.org/annag/ontologies/2024/1/ontoHorses#Dressage"/>
        <ontoHorses:puòEssereImpiegataIn rdf:resource="http://www.semanticweb.org/annag/ontologies/2024/1/ontoHorses#Equiturismo"/>
        <ontoHorses:altezzaMediaGarrese rdf:datatype="http://www.w3.org/2001/XMLSchema#integer">160</ontoHorses:altezzaMediaGarrese>
        <ontoHorses:haColoreMantello>baio</ontoHorses:haColoreMantello>
        <ontoHorses:haColoreMantello>grigio</ontoHorses:haColoreMantello>
        <ontoHorses:haColoreMantello>sauro</ontoHorses:haColoreMantello>
        <ontoHorses:pesoMedio rdf:datatype="http://www.w3.org/2001/XMLSchema#integer">500</ontoHorses:pesoMedio>
        <schema:image rdf:resource="https://www.ideegreen.it/wp-content/uploads/2020/10/cavallo-anglo-arabo-spagnolo.jpg"/>
        <rdfs:comment xml:lang="it">L&apos;anglo-arabo spagnolo è un cavallo maneggevole, agile nei movimenti, progenitore dell&apos;Andaluso</rdfs:comment>
        <rdfs:comment xml:lang="en">The Spanish Anglo-Arab is a manageable horse, agile in movement, progenitor of the Andalusian</rdfs:comment>
        <skos:exactMatch xml:lang="it">http://www.wikidata.org/entity/Q3617386</skos:exactMatch>
        <skos:prefLabel xml:lang="en">Anglo-Arabic Spanish</skos:prefLabel>
        <skos:prefLabel xml:lang="it">Anglo-Arabo spagnolo</skos:prefLabel>
    </owl:NamedIndividual>
    


    <!-- http://www.semanticweb.org/annag/ontologies/2024/1/ontoHorses#Appenninico -->

    <owl:NamedIndividual rdf:about="http://www.semanticweb.org/annag/ontologies/2024/1/ontoHorses#Appenninico">
        <rdf:type rdf:resource="http://www.semanticweb.org/annag/ontologies/2024/1/ontoHorses#RazzaASangueFreddo"/>
        <rdf:type rdf:resource="http://www.semanticweb.org/annag/ontologies/2024/1/ontoHorses#RazzaCavallo"/>
        <rdf:type rdf:resource="http://www.semanticweb.org/annag/ontologies/2024/1/ontoHorses#RazzaDaEquiturismo"/>
        <rdf:type rdf:resource="http://www.semanticweb.org/annag/ontologies/2024/1/ontoHorses#RazzaDaLavoro"/>
        <rdf:type rdf:resource="http://www.semanticweb.org/annag/ontologies/2024/1/ontoHorses#RazzaDaSella"/>
        <rdf:type rdf:resource="http://www.semanticweb.org/annag/ontologies/2024/1/ontoHorses#RazzamMesomorfa"/>
        <ontoHorses:entitàWikidata rdf:resource="http://www.wikidata.org/entity/Q3620866"/>
        <ontoHorses:haClassificazioneMorfologica rdf:resource="http://www.semanticweb.org/annag/ontologies/2024/1/ontoHorses#mesomorfo"/>
        <ontoHorses:haIndole rdf:resource="http://www.semanticweb.org/annag/ontologies/2024/1/ontoHorses#sangueFreddo"/>
        <ontoHorses:haNazionalità rdf:resource="http://www.semanticweb.org/annag/ontologies/2024/1/ontoHorses#Italia"/>
        <ontoHorses:haRegioneDiOrigine rdf:resource="http://www.semanticweb.org/annag/ontologies/2024/1/ontoHorses#AppenninoToscoEmiliano"/>
        <ontoHorses:puòEssereImpiegataIn rdf:resource="http://www.semanticweb.org/annag/ontologies/2024/1/ontoHorses#Equiturismo"/>
        <ontoHorses:puòEssereImpiegataIn rdf:resource="http://www.semanticweb.org/annag/ontologies/2024/1/ontoHorses#TrainoCarrozze"/>
        <ontoHorses:altezzaMediaGarrese rdf:datatype="http://www.w3.org/2001/XMLSchema#integer">155</ontoHorses:altezzaMediaGarrese>
        <ontoHorses:haColoreMantello>baio</ontoHorses:haColoreMantello>
        <ontoHorses:haColoreMantello>sauro</ontoHorses:haColoreMantello>
        <ontoHorses:pesoMedio rdf:datatype="http://www.w3.org/2001/XMLSchema#integer">575</ontoHorses:pesoMedio>
        <schema:image rdf:resource="https://www.sef-italia.it/wp-content/uploads/2017/06/a_cavallo_sull_Appennino5.jpg"/>
        <rdfs:comment xml:lang="it">L&apos;Appenninico è una razza di cavallo rustico e adattabile originario dall&apos;Appenino tosco-emiliano.</rdfs:comment>
        <rdfs:comment xml:lang="en">The Appenninico is a rustic and adaptable horse breed originating from the Tuscan-Emilian Apennines.</rdfs:comment>
        <skos:exactMatch xml:lang="it">http://www.wikidata.org/entity/Q3620866</skos:exactMatch>
        <skos:prefLabel xml:lang="en">Appenninico</skos:prefLabel>
        <skos:prefLabel xml:lang="it">Appenninico</skos:prefLabel>
    </owl:NamedIndividual>
    


    <!-- http://www.semanticweb.org/annag/ontologies/2024/1/ontoHorses#AppenninoToscoEmiliano -->

    <owl:NamedIndividual rdf:about="http://www.semanticweb.org/annag/ontologies/2024/1/ontoHorses#AppenninoToscoEmiliano">
        <rdf:type rdf:resource="http://schema.org/Place"/>
        <rdf:type rdf:resource="http://www.semanticweb.org/annag/ontologies/2024/1/ontoHorses#AreaGeografica"/>
        <partof:isPartOf rdf:resource="http://www.semanticweb.org/annag/ontologies/2024/1/ontoHorses#Italia"/>
        <rdfs:comment xml:lang="en">It is a subdivision of the Apennine chain, in particular a stretch of the northern Apennines, which affects the border and adjacent areas of Tuscany and Emilia-Romagna</rdfs:comment>
        <rdfs:comment xml:lang="it">Si tratta di una suddivisione della catena degli Appennini, in particolare un tratto dell&apos;Appennino settentrionale, che interessa il confine e le aree adiacenti di Toscana e Emilia-Romagna</rdfs:comment>
        <rdfs:label xml:lang="it">Appenino Tosco-Emiliano</rdfs:label>
        <rdfs:label xml:lang="en">Tuscan-Emilian Apennines</rdfs:label>
    </owl:NamedIndividual>
    


    <!-- http://www.semanticweb.org/annag/ontologies/2024/1/ontoHorses#Ardenne -->

    <owl:NamedIndividual rdf:about="http://www.semanticweb.org/annag/ontologies/2024/1/ontoHorses#Ardenne">
        <rdf:type rdf:resource="http://schema.org/Place"/>
        <rdf:type rdf:resource="http://www.semanticweb.org/annag/ontologies/2024/1/ontoHorses#AreaGeografica"/>
        <partof:isPartOf rdf:resource="http://www.semanticweb.org/annag/ontologies/2024/1/ontoHorses#Belgio"/>
        <rdfs:comment xml:lang="it">Le Ardenne sono una regione collinare coperta da foreste, che si trova principalmente in Belgio e Lussemburgo e Francia</rdfs:comment>
        <rdfs:comment xml:lang="en">The Ardennes is a hilly, forested region, found mainly in Belgium and Luxembourg and France</rdfs:comment>
        <rdfs:label xml:lang="it">Ardenne</rdfs:label>
        <rdfs:label xml:lang="en">Ardennes</rdfs:label>
    </owl:NamedIndividual>
    


    <!-- http://www.semanticweb.org/annag/ontologies/2024/1/ontoHorses#Ardennese -->

    <owl:NamedIndividual rdf:about="http://www.semanticweb.org/annag/ontologies/2024/1/ontoHorses#Ardennese">
        <rdf:type rdf:resource="http://www.semanticweb.org/annag/ontologies/2024/1/ontoHorses#RazzaASangueFreddo"/>
        <rdf:type rdf:resource="http://www.semanticweb.org/annag/ontologies/2024/1/ontoHorses#RazzaBrachimorfa"/>
        <rdf:type rdf:resource="http://www.semanticweb.org/annag/ontologies/2024/1/ontoHorses#RazzaCavallo"/>
        <rdf:type rdf:resource="http://www.semanticweb.org/annag/ontologies/2024/1/ontoHorses#RazzaDaLavoro"/>
        <ontoHorses:entitàWikidata rdf:resource="http://www.wikidata.org/entity/Q638976"/>
        <ontoHorses:haClassificazioneMorfologica rdf:resource="http://www.semanticweb.org/annag/ontologies/2024/1/ontoHorses#brachimorfo"/>
        <ontoHorses:haIndole rdf:resource="http://www.semanticweb.org/annag/ontologies/2024/1/ontoHorses#sangueFreddo"/>
        <ontoHorses:haNazionalità rdf:resource="http://www.semanticweb.org/annag/ontologies/2024/1/ontoHorses#Belgio"/>
        <ontoHorses:haRegioneDiOrigine rdf:resource="http://www.semanticweb.org/annag/ontologies/2024/1/ontoHorses#Ardenne"/>
        <ontoHorses:puòEssereImpiegataIn rdf:resource="http://www.semanticweb.org/annag/ontologies/2024/1/ontoHorses#TrainoCarrozze"/>
        <ontoHorses:altezzaMediaGarrese rdf:datatype="http://www.w3.org/2001/XMLSchema#integer">160</ontoHorses:altezzaMediaGarrese>
        <ontoHorses:haColoreMantello>baio</ontoHorses:haColoreMantello>
        <ontoHorses:haColoreMantello>isabella</ontoHorses:haColoreMantello>
        <ontoHorses:haColoreMantello>roano</ontoHorses:haColoreMantello>
        <ontoHorses:haColoreMantello>sauro</ontoHorses:haColoreMantello>
        <ontoHorses:haColoreMantello>ubero</ontoHorses:haColoreMantello>
        <ontoHorses:pesoMedio rdf:datatype="http://www.w3.org/2001/XMLSchema#integer">800</ontoHorses:pesoMedio>
        <schema:image rdf:resource="https://upload.wikimedia.org/wikipedia/commons/thumb/4/41/Ardenner.jpg/240px-Ardenner.jpg"/>
        <rdfs:comment xml:lang="it">L&apos;Ardennese è  una razza di cavallo brachimorfo adatto al tiro pesante E&apos; un antico cavallo noto ai tempi di Giulio Cesare</rdfs:comment>
        <rdfs:comment xml:lang="en">The Ardennese is a brachymorphic horse breed suitable for heavy shooting. It is an ancient horse known at the time of Julius Caesar</rdfs:comment>
        <skos:exactMatch xml:lang="it">http://www.wikidata.org/entity/Q638976</skos:exactMatch>
        <skos:prefLabel xml:lang="en">Ardennes Horse</skos:prefLabel>
        <skos:prefLabel xml:lang="it">Ardennese</skos:prefLabel>
    </owl:NamedIndividual>
    


    <!-- http://www.semanticweb.org/annag/ontologies/2024/1/ontoHorses#BelgaDaTiro -->

    <owl:NamedIndividual rdf:about="http://www.semanticweb.org/annag/ontologies/2024/1/ontoHorses#BelgaDaTiro">
        <rdf:type rdf:resource="http://www.semanticweb.org/annag/ontologies/2024/1/ontoHorses#RazzaASangueFreddo"/>
        <rdf:type rdf:resource="http://www.semanticweb.org/annag/ontologies/2024/1/ontoHorses#RazzaBrachimorfa"/>
        <rdf:type rdf:resource="http://www.semanticweb.org/annag/ontologies/2024/1/ontoHorses#RazzaCavallo"/>
        <rdf:type rdf:resource="http://www.semanticweb.org/annag/ontologies/2024/1/ontoHorses#RazzaDaLavoro"/>
        <rdf:type rdf:resource="http://www.semanticweb.org/annag/ontologies/2024/1/ontoHorses#RazzaDaTiroAgricolo"/>
        <ontoHorses:entitàWikidata rdf:resource="http://www.wikidata.org/entity/Q896476"/>
        <ontoHorses:haClassificazioneMorfologica rdf:resource="http://www.semanticweb.org/annag/ontologies/2024/1/ontoHorses#brachimorfo"/>
        <ontoHorses:haIndole rdf:resource="http://www.semanticweb.org/annag/ontologies/2024/1/ontoHorses#sangueFreddo"/>
        <ontoHorses:haNazionalità rdf:resource="http://www.semanticweb.org/annag/ontologies/2024/1/ontoHorses#Belgio"/>
        <ontoHorses:haRegioneDiOrigine rdf:resource="http://www.semanticweb.org/annag/ontologies/2024/1/ontoHorses#Ardenne"/>
        <ontoHorses:puòEssereImpiegataIn rdf:resource="http://www.semanticweb.org/annag/ontologies/2024/1/ontoHorses#TiroAgricolo"/>
        <ontoHorses:puòEssereImpiegataIn rdf:resource="http://www.semanticweb.org/annag/ontologies/2024/1/ontoHorses#TrainoCarrozze"/>
        <ontoHorses:altezzaMediaGarrese rdf:datatype="http://www.w3.org/2001/XMLSchema#integer">160</ontoHorses:altezzaMediaGarrese>
        <ontoHorses:haColoreMantello>baio</ontoHorses:haColoreMantello>
        <ontoHorses:haColoreMantello>roano</ontoHorses:haColoreMantello>
        <ontoHorses:haColoreMantello>sauro</ontoHorses:haColoreMantello>
        <ontoHorses:pesoMedio rdf:datatype="http://www.w3.org/2001/XMLSchema#integer">750</ontoHorses:pesoMedio>
        <schema:image rdf:resource="https://upload.wikimedia.org/wikipedia/commons/thumb/7/77/Belgisk_hest-2.jpg/240px-Belgisk_hest-2.jpg"/>
        <rdfs:comment xml:lang="it">Il Belga da tiro è una razza di cavallo originaria del Belgio: è un cavallo massiccio, uno dei più grandi, usato per il traino di oggetti sin dall&apos;antichità</rdfs:comment>
        <rdfs:comment xml:lang="en">The Belgian draft horse is a breed of horse originating from Belgium: it is a massive horse, one of the largest, used for pulling objects since ancient times</rdfs:comment>
        <skos:exactMatch xml:lang="it">http://www.wikidata.org/entity/Q896476</skos:exactMatch>
        <skos:prefLabel xml:lang="it">Belga Da Tiro</skos:prefLabel>
        <skos:prefLabel xml:lang="en">Belgian Draught</skos:prefLabel>
    </owl:NamedIndividual>
    


    <!-- http://www.semanticweb.org/annag/ontologies/2024/1/ontoHorses#Belgio -->

    <owl:NamedIndividual rdf:about="http://www.semanticweb.org/annag/ontologies/2024/1/ontoHorses#Belgio">
        <rdf:type rdf:resource="http://schema.org/Place"/>
        <rdf:type rdf:resource="http://www.semanticweb.org/annag/ontologies/2024/1/ontoHorses#AreaGeografica"/>
        <partof:hasPart rdf:resource="http://www.semanticweb.org/annag/ontologies/2024/1/ontoHorses#Ardenne"/>
        <schema:image rdf:resource="https://upload.wikimedia.org/wikipedia/commons/thumb/6/65/Flag_of_Belgium.svg/188px-Flag_of_Belgium.svg.png"/>
        <rdfs:comment xml:lang="en">Belgium, officially the Kingdom of Belgium, is a country in Northwestern Europe.</rdfs:comment>
        <rdfs:comment xml:lang="it">Il Belgio, ufficialmente Regno del Belgio, è uno Stato federale retto da una monarchia parlamentare  situato nell&apos;Europa occidentale.</rdfs:comment>
        <rdfs:label xml:lang="it">Belgio</rdfs:label>
        <rdfs:label xml:lang="en">Belgium</rdfs:label>
    </owl:NamedIndividual>
    


    <!-- http://www.semanticweb.org/annag/ontologies/2024/1/ontoHorses#Boulonnais -->

    <owl:NamedIndividual rdf:about="http://www.semanticweb.org/annag/ontologies/2024/1/ontoHorses#Boulonnais">
        <rdf:type rdf:resource="http://www.semanticweb.org/annag/ontologies/2024/1/ontoHorses#RazzaASangueFreddo"/>
        <rdf:type rdf:resource="http://www.semanticweb.org/annag/ontologies/2024/1/ontoHorses#RazzaBrachimorfa"/>
        <rdf:type rdf:resource="http://www.semanticweb.org/annag/ontologies/2024/1/ontoHorses#RazzaCavallo"/>
        <rdf:type rdf:resource="http://www.semanticweb.org/annag/ontologies/2024/1/ontoHorses#RazzaDaLavoro"/>
        <rdf:type rdf:resource="http://www.semanticweb.org/annag/ontologies/2024/1/ontoHorses#RazzaDaTiroAgricolo"/>
        <ontoHorses:entitàWikidata rdf:resource="http://www.wikidata.org/entity/Q588252"/>
        <ontoHorses:haClassificazioneMorfologica rdf:resource="http://www.semanticweb.org/annag/ontologies/2024/1/ontoHorses#brachimorfo"/>
        <ontoHorses:haIndole rdf:resource="http://www.semanticweb.org/annag/ontologies/2024/1/ontoHorses#sangueFreddo"/>
        <ontoHorses:haNazionalità rdf:resource="http://www.semanticweb.org/annag/ontologies/2024/1/ontoHorses#Francia"/>
        <ontoHorses:haRegioneDiOrigine rdf:resource="http://www.semanticweb.org/annag/ontologies/2024/1/ontoHorses#RegioneBoullonnais"/>
        <ontoHorses:puòEssereImpiegataIn rdf:resource="http://www.semanticweb.org/annag/ontologies/2024/1/ontoHorses#TiroAgricolo"/>
        <ontoHorses:altezzaMediaGarrese rdf:datatype="http://www.w3.org/2001/XMLSchema#integer">163</ontoHorses:altezzaMediaGarrese>
        <ontoHorses:haColoreMantello>baio</ontoHorses:haColoreMantello>
        <ontoHorses:haColoreMantello>grigio</ontoHorses:haColoreMantello>
        <ontoHorses:haColoreMantello>morello</ontoHorses:haColoreMantello>
        <ontoHorses:haColoreMantello>roano</ontoHorses:haColoreMantello>
        <ontoHorses:haColoreMantello>sauro</ontoHorses:haColoreMantello>
        <ontoHorses:pesoMedio rdf:datatype="http://www.w3.org/2001/XMLSchema#integer">800</ontoHorses:pesoMedio>
        <schema:image rdf:resource="https://upload.wikimedia.org/wikipedia/commons/thumb/4/47/T%C3%AAte_jument_boulonnaise_2.jpg/260px-T%C3%AAte_jument_boulonnaise_2.jpg"/>
        <rdfs:comment xml:lang="it">Il Boulonnais è una razza di cavallo da tiro, soprannominato &quot;cavallo purosangue line&quot; o &quot;colosso di marmo bianco&quot;, originario della regione di Boulogne-sur-Mer nel nord della Francia.</rdfs:comment>
        <rdfs:comment xml:lang="en">The Boulonnais is a breed of draft horse, nicknamed &quot;thoroughbred line horse&quot; or &quot;colossus of white marble&quot;, native to the Boulogne-sur-Mer region of northern France.</rdfs:comment>
        <skos:exactMatch xml:lang="it">http://www.wikidata.org/entity/Q588252</skos:exactMatch>
        <skos:prefLabel xml:lang="en">Boulonnais</skos:prefLabel>
        <skos:prefLabel xml:lang="it">Boulonnais</skos:prefLabel>
    </owl:NamedIndividual>
    


    <!-- http://www.semanticweb.org/annag/ontologies/2024/1/ontoHorses#Bretagna -->

    <owl:NamedIndividual rdf:about="http://www.semanticweb.org/annag/ontologies/2024/1/ontoHorses#Bretagna">
        <rdf:type rdf:resource="http://schema.org/Place"/>
        <rdf:type rdf:resource="http://www.semanticweb.org/annag/ontologies/2024/1/ontoHorses#AreaGeografica"/>
        <partof:isPartOf rdf:resource="http://www.semanticweb.org/annag/ontologies/2024/1/ontoHorses#Francia"/>
        <schema:image rdf:resource="https://upload.wikimedia.org/wikipedia/commons/thumb/4/4b/Brittany_in_France_2016.svg/260px-Brittany_in_France_2016.svg.png"/>
        <rdfs:comment xml:lang="en">Brittany is a historical and administrative region of France that forms a vast promontory towards the English Channel and the Atlantic Ocean</rdfs:comment>
        <rdfs:comment xml:lang="it">La Bretagna  è una regione storica e amministrativa della Francia che forma un vasto promontorio verso la Manica e l&apos;Oceano Atlantico</rdfs:comment>
        <rdfs:label xml:lang="it">Bretagna</rdfs:label>
        <rdfs:label xml:lang="en">Brittany</rdfs:label>
    </owl:NamedIndividual>
    


    <!-- http://www.semanticweb.org/annag/ontologies/2024/1/ontoHorses#Bretone -->

    <owl:NamedIndividual rdf:about="http://www.semanticweb.org/annag/ontologies/2024/1/ontoHorses#Bretone">
        <rdf:type rdf:resource="http://www.semanticweb.org/annag/ontologies/2024/1/ontoHorses#RazzaASangueFreddo"/>
        <rdf:type rdf:resource="http://www.semanticweb.org/annag/ontologies/2024/1/ontoHorses#RazzaBrachimorfa"/>
        <rdf:type rdf:resource="http://www.semanticweb.org/annag/ontologies/2024/1/ontoHorses#RazzaCavallo"/>
        <rdf:type rdf:resource="http://www.semanticweb.org/annag/ontologies/2024/1/ontoHorses#RazzaDaLavoro"/>
        <rdf:type rdf:resource="http://www.semanticweb.org/annag/ontologies/2024/1/ontoHorses#RazzaDaTiroAgricolo"/>
        <ontoHorses:entitàWikidata rdf:resource="http://www.wikidata.org/entity/Q514553"/>
        <ontoHorses:haClassificazioneMorfologica rdf:resource="http://www.semanticweb.org/annag/ontologies/2024/1/ontoHorses#brachimorfo"/>
        <ontoHorses:haIndole rdf:resource="http://www.semanticweb.org/annag/ontologies/2024/1/ontoHorses#sangueFreddo"/>
        <ontoHorses:haNazionalità rdf:resource="http://www.semanticweb.org/annag/ontologies/2024/1/ontoHorses#Francia"/>
        <ontoHorses:haRegioneDiOrigine rdf:resource="http://www.semanticweb.org/annag/ontologies/2024/1/ontoHorses#Bretagna"/>
        <ontoHorses:puòEssereImpiegataIn rdf:resource="http://www.semanticweb.org/annag/ontologies/2024/1/ontoHorses#TiroAgricolo"/>
        <ontoHorses:puòEssereImpiegataIn rdf:resource="http://www.semanticweb.org/annag/ontologies/2024/1/ontoHorses#TrainoCarrozze"/>
        <ontoHorses:altezzaMediaGarrese rdf:datatype="http://www.w3.org/2001/XMLSchema#integer">155</ontoHorses:altezzaMediaGarrese>
        <ontoHorses:haColoreMantello>sauro</ontoHorses:haColoreMantello>
        <ontoHorses:pesoMedio rdf:datatype="http://www.w3.org/2001/XMLSchema#integer">800</ontoHorses:pesoMedio>
        <schema:image rdf:resource="https://upload.wikimedia.org/wikipedia/commons/thumb/f/fa/Breton_%C3%A9talon_SDA2012.JPG/220px-Breton_%C3%A9talon_SDA2012.JPG"/>
        <rdfs:comment xml:lang="it">Il  Bretone è una razza di cavallo da tiro pesante, originario della Francia, un tempo utilizzato specialmente nei lavori agricoli</rdfs:comment>
        <rdfs:comment xml:lang="en">The Breton is a breed of heavy draft horse, originally from France, once used especially in agricultural work</rdfs:comment>
        <skos:exactMatch xml:lang="it">http://www.wikidata.org/entity/Q514553</skos:exactMatch>
        <skos:prefLabel xml:lang="it">Bretone</skos:prefLabel>
        <skos:prefLabel>Breton Horse</skos:prefLabel>
    </owl:NamedIndividual>
    


    <!-- http://www.semanticweb.org/annag/ontologies/2024/1/ontoHorses#C100 -->

    <owl:NamedIndividual rdf:about="http://www.semanticweb.org/annag/ontologies/2024/1/ontoHorses#C100">
        <rdf:type rdf:resource="http://dbpedia.org/ontology/horseRidingDiscipline"/>
        <rdf:type rdf:resource="http://www.semanticweb.org/annag/ontologies/2024/1/ontoHorses#CategorieDiSalto"/>
        <rdf:type rdf:resource="http://www.semanticweb.org/annag/ontologies/2024/1/ontoHorses#Impiego"/>
        <rdf:type rdf:resource="http://www.semanticweb.org/annag/ontologies/2024/1/ontoHorses#SaltoAdOstacoli"/>
        <rdf:type rdf:resource="http://www.semanticweb.org/annag/ontologies/2024/1/ontoHorses#Sella"/>
        <rdf:type rdf:resource="http://www.semanticweb.org/annag/ontologies/2024/1/ontoHorses#SportEquestre"/>
        <ontoHorses:permetteIlConseguimentoDi rdf:resource="http://www.semanticweb.org/annag/ontologies/2024/1/ontoHorses#brevetto"/>
        <rdfs:comment xml:lang="it">Categoria di salto ad ostacoli in cui l&apos;altezza degli ostacoli lungo il percorso di gara non è mai superiore ai 100 cm</rdfs:comment>
        <rdfs:comment xml:lang="en">Show jumping category in which the height of the obstacles along the competition course is never higher than 100 cm</rdfs:comment>
        <rdfs:label xml:lang="en">C100</rdfs:label>
        <rdfs:label xml:lang="it">C100</rdfs:label>
    </owl:NamedIndividual>
    


    <!-- http://www.semanticweb.org/annag/ontologies/2024/1/ontoHorses#C105 -->

    <owl:NamedIndividual rdf:about="http://www.semanticweb.org/annag/ontologies/2024/1/ontoHorses#C105">
        <rdf:type rdf:resource="http://dbpedia.org/ontology/horseRidingDiscipline"/>
        <rdf:type rdf:resource="http://www.semanticweb.org/annag/ontologies/2024/1/ontoHorses#CategorieDiSalto"/>
        <rdf:type rdf:resource="http://www.semanticweb.org/annag/ontologies/2024/1/ontoHorses#Impiego"/>
        <rdf:type rdf:resource="http://www.semanticweb.org/annag/ontologies/2024/1/ontoHorses#SaltoAdOstacoli"/>
        <rdf:type rdf:resource="http://www.semanticweb.org/annag/ontologies/2024/1/ontoHorses#Sella"/>
        <rdf:type rdf:resource="http://www.semanticweb.org/annag/ontologies/2024/1/ontoHorses#SportEquestre"/>
        <ontoHorses:permetteIlConseguimentoDi rdf:resource="http://www.semanticweb.org/annag/ontologies/2024/1/ontoHorses#brevetto"/>
        <rdfs:comment xml:lang="it">Categoria di salto ad ostacoli in cui l&apos;altezza degli ostacoli lungo il percorso di gara non è mai superiore ai 105 cm</rdfs:comment>
        <rdfs:comment xml:lang="en">Show jumping category in which the height of the obstacles along the competition course is never higher than 105 cm</rdfs:comment>
        <rdfs:label xml:lang="en">C105</rdfs:label>
        <rdfs:label xml:lang="it">C105</rdfs:label>
    </owl:NamedIndividual>
    


    <!-- http://www.semanticweb.org/annag/ontologies/2024/1/ontoHorses#C110 -->

    <owl:NamedIndividual rdf:about="http://www.semanticweb.org/annag/ontologies/2024/1/ontoHorses#C110">
        <rdf:type rdf:resource="http://dbpedia.org/ontology/horseRidingDiscipline"/>
        <rdf:type rdf:resource="http://www.semanticweb.org/annag/ontologies/2024/1/ontoHorses#CategorieDiSalto"/>
        <rdf:type rdf:resource="http://www.semanticweb.org/annag/ontologies/2024/1/ontoHorses#Impiego"/>
        <rdf:type rdf:resource="http://www.semanticweb.org/annag/ontologies/2024/1/ontoHorses#SaltoAdOstacoli"/>
        <rdf:type rdf:resource="http://www.semanticweb.org/annag/ontologies/2024/1/ontoHorses#Sella"/>
        <rdf:type rdf:resource="http://www.semanticweb.org/annag/ontologies/2024/1/ontoHorses#SportEquestre"/>
        <ontoHorses:permetteIlConseguimentoDi rdf:resource="http://www.semanticweb.org/annag/ontologies/2024/1/ontoHorses#brevetto"/>
        <rdfs:comment xml:lang="it">Categoria di salto ad ostacoli in cui l&apos;altezza degli ostacoli lungo il percorso di gara non è mai superiore ai 110 cm</rdfs:comment>
        <rdfs:comment xml:lang="en">Show jumping category in which the height of the obstacles along the competition course is never higher than 110 cm</rdfs:comment>
        <rdfs:label xml:lang="en">C110</rdfs:label>
        <rdfs:label xml:lang="it">C110</rdfs:label>
    </owl:NamedIndividual>
    


    <!-- http://www.semanticweb.org/annag/ontologies/2024/1/ontoHorses#C115 -->

    <owl:NamedIndividual rdf:about="http://www.semanticweb.org/annag/ontologies/2024/1/ontoHorses#C115">
        <rdf:type rdf:resource="http://dbpedia.org/ontology/horseRidingDiscipline"/>
        <rdf:type rdf:resource="http://www.semanticweb.org/annag/ontologies/2024/1/ontoHorses#CategorieDiSalto"/>
        <rdf:type rdf:resource="http://www.semanticweb.org/annag/ontologies/2024/1/ontoHorses#Impiego"/>
        <rdf:type rdf:resource="http://www.semanticweb.org/annag/ontologies/2024/1/ontoHorses#SaltoAdOstacoli"/>
        <rdf:type rdf:resource="http://www.semanticweb.org/annag/ontologies/2024/1/ontoHorses#Sella"/>
        <rdf:type rdf:resource="http://www.semanticweb.org/annag/ontologies/2024/1/ontoHorses#SportEquestre"/>
        <ontoHorses:permetteIlConseguimentoDi rdf:resource="http://www.semanticweb.org/annag/ontologies/2024/1/ontoHorses#brevetto"/>
        <ontoHorses:permetteIlConseguimentoDi rdf:resource="http://www.semanticweb.org/annag/ontologies/2024/1/ontoHorses#primoGrado"/>
        <rdfs:comment xml:lang="it">Categoria di salto ad ostacoli in cui l&apos;altezza degli ostacoli lungo il percorso di gara non è mai superiore ai 115 cm</rdfs:comment>
        <rdfs:comment xml:lang="en">Show jumping category in which the height of the obstacles along the competition course is never higher than 115 cm</rdfs:comment>
        <rdfs:label xml:lang="en">C115</rdfs:label>
        <rdfs:label xml:lang="it">C115</rdfs:label>
    </owl:NamedIndividual>
    


    <!-- http://www.semanticweb.org/annag/ontologies/2024/1/ontoHorses#C120 -->

    <owl:NamedIndividual rdf:about="http://www.semanticweb.org/annag/ontologies/2024/1/ontoHorses#C120">
        <rdf:type rdf:resource="http://dbpedia.org/ontology/horseRidingDiscipline"/>
        <rdf:type rdf:resource="http://www.semanticweb.org/annag/ontologies/2024/1/ontoHorses#CategorieDiSalto"/>
        <rdf:type rdf:resource="http://www.semanticweb.org/annag/ontologies/2024/1/ontoHorses#Impiego"/>
        <rdf:type rdf:resource="http://www.semanticweb.org/annag/ontologies/2024/1/ontoHorses#SaltoAdOstacoli"/>
        <rdf:type rdf:resource="http://www.semanticweb.org/annag/ontologies/2024/1/ontoHorses#Sella"/>
        <rdf:type rdf:resource="http://www.semanticweb.org/annag/ontologies/2024/1/ontoHorses#SportEquestre"/>
        <ontoHorses:permetteIlConseguimentoDi rdf:resource="http://www.semanticweb.org/annag/ontologies/2024/1/ontoHorses#primoGrado"/>
        <rdfs:comment xml:lang="it">Categoria di salto ad ostacoli in cui l&apos;altezza degli ostacoli lungo il percorso di gara non è mai superiore ai 120 cm</rdfs:comment>
        <rdfs:comment xml:lang="en">Show jumping category in which the height of the obstacles along the competition course is never higher than 120 cm</rdfs:comment>
        <rdfs:label xml:lang="en">C120</rdfs:label>
        <rdfs:label xml:lang="it">C120</rdfs:label>
    </owl:NamedIndividual>
    


    <!-- http://www.semanticweb.org/annag/ontologies/2024/1/ontoHorses#C125 -->

    <owl:NamedIndividual rdf:about="http://www.semanticweb.org/annag/ontologies/2024/1/ontoHorses#C125">
        <rdf:type rdf:resource="http://dbpedia.org/ontology/horseRidingDiscipline"/>
        <rdf:type rdf:resource="http://www.semanticweb.org/annag/ontologies/2024/1/ontoHorses#CategorieDiSalto"/>
        <rdf:type rdf:resource="http://www.semanticweb.org/annag/ontologies/2024/1/ontoHorses#Impiego"/>
        <rdf:type rdf:resource="http://www.semanticweb.org/annag/ontologies/2024/1/ontoHorses#SaltoAdOstacoli"/>
        <rdf:type rdf:resource="http://www.semanticweb.org/annag/ontologies/2024/1/ontoHorses#Sella"/>
        <rdf:type rdf:resource="http://www.semanticweb.org/annag/ontologies/2024/1/ontoHorses#SportEquestre"/>
        <ontoHorses:permetteIlConseguimentoDi rdf:resource="http://www.semanticweb.org/annag/ontologies/2024/1/ontoHorses#primoGrado"/>
        <rdfs:comment xml:lang="it">Categoria di salto ad ostacoli in cui l&apos;altezza degli ostacoli lungo il percorso di gara non è mai superiore ai 125 cm</rdfs:comment>
        <rdfs:comment xml:lang="en">Show jumping category in which the height of the obstacles along the competition course is never higher than 125 cm</rdfs:comment>
        <rdfs:label xml:lang="en">C125</rdfs:label>
        <rdfs:label xml:lang="it">C125</rdfs:label>
    </owl:NamedIndividual>
    


    <!-- http://www.semanticweb.org/annag/ontologies/2024/1/ontoHorses#C130 -->

    <owl:NamedIndividual rdf:about="http://www.semanticweb.org/annag/ontologies/2024/1/ontoHorses#C130">
        <rdf:type rdf:resource="http://dbpedia.org/ontology/horseRidingDiscipline"/>
        <rdf:type rdf:resource="http://www.semanticweb.org/annag/ontologies/2024/1/ontoHorses#CategorieDiSalto"/>
        <rdf:type rdf:resource="http://www.semanticweb.org/annag/ontologies/2024/1/ontoHorses#Impiego"/>
        <rdf:type rdf:resource="http://www.semanticweb.org/annag/ontologies/2024/1/ontoHorses#SaltoAdOstacoli"/>
        <rdf:type rdf:resource="http://www.semanticweb.org/annag/ontologies/2024/1/ontoHorses#Sella"/>
        <rdf:type rdf:resource="http://www.semanticweb.org/annag/ontologies/2024/1/ontoHorses#SportEquestre"/>
        <ontoHorses:permetteIlConseguimentoDi rdf:resource="http://www.semanticweb.org/annag/ontologies/2024/1/ontoHorses#primoGrado"/>
        <rdfs:comment xml:lang="it">Categoria di salto ad ostacoli in cui l&apos;altezza degli ostacoli lungo il percorso di gara non è mai superiore ai 130 cm</rdfs:comment>
        <rdfs:comment xml:lang="en">Show jumping category in which the height of the obstacles along the competition course is never higher than 130 cm</rdfs:comment>
        <rdfs:label xml:lang="en">C130</rdfs:label>
        <rdfs:label xml:lang="it">C130</rdfs:label>
    </owl:NamedIndividual>
    


    <!-- http://www.semanticweb.org/annag/ontologies/2024/1/ontoHorses#C135 -->

    <owl:NamedIndividual rdf:about="http://www.semanticweb.org/annag/ontologies/2024/1/ontoHorses#C135">
        <rdf:type rdf:resource="http://dbpedia.org/ontology/horseRidingDiscipline"/>
        <rdf:type rdf:resource="http://www.semanticweb.org/annag/ontologies/2024/1/ontoHorses#CategorieDiSalto"/>
        <rdf:type rdf:resource="http://www.semanticweb.org/annag/ontologies/2024/1/ontoHorses#Impiego"/>
        <rdf:type rdf:resource="http://www.semanticweb.org/annag/ontologies/2024/1/ontoHorses#SaltoAdOstacoli"/>
        <rdf:type rdf:resource="http://www.semanticweb.org/annag/ontologies/2024/1/ontoHorses#Sella"/>
        <rdf:type rdf:resource="http://www.semanticweb.org/annag/ontologies/2024/1/ontoHorses#SportEquestre"/>
        <ontoHorses:permetteIlConseguimentoDi rdf:resource="http://www.semanticweb.org/annag/ontologies/2024/1/ontoHorses#primoGrado"/>
        <ontoHorses:permetteIlConseguimentoDi rdf:resource="http://www.semanticweb.org/annag/ontologies/2024/1/ontoHorses#secondoGrado"/>
        <rdfs:comment xml:lang="it">Categoria di salto ad ostacoli in cui l&apos;altezza degli ostacoli lungo il percorso di gara non è mai superiore ai 135 cm</rdfs:comment>
        <rdfs:comment xml:lang="en">Show jumping category in which the height of the obstacles along the competition course is never higher than 135 cm</rdfs:comment>
        <rdfs:label xml:lang="en">C135</rdfs:label>
        <rdfs:label xml:lang="it">C135</rdfs:label>
    </owl:NamedIndividual>
    


    <!-- http://www.semanticweb.org/annag/ontologies/2024/1/ontoHorses#C80 -->

    <owl:NamedIndividual rdf:about="http://www.semanticweb.org/annag/ontologies/2024/1/ontoHorses#C80">
        <rdf:type rdf:resource="http://dbpedia.org/ontology/horseRidingDiscipline"/>
        <rdf:type rdf:resource="http://www.semanticweb.org/annag/ontologies/2024/1/ontoHorses#CategorieDiSalto"/>
        <rdf:type rdf:resource="http://www.semanticweb.org/annag/ontologies/2024/1/ontoHorses#Impiego"/>
        <rdf:type rdf:resource="http://www.semanticweb.org/annag/ontologies/2024/1/ontoHorses#SaltoAdOstacoli"/>
        <rdf:type rdf:resource="http://www.semanticweb.org/annag/ontologies/2024/1/ontoHorses#Sella"/>
        <rdf:type rdf:resource="http://www.semanticweb.org/annag/ontologies/2024/1/ontoHorses#SportEquestre"/>
        <ontoHorses:permetteIlConseguimentoDi rdf:resource="http://www.semanticweb.org/annag/ontologies/2024/1/ontoHorses#brevetto"/>
        <rdfs:comment xml:lang="it">Categoria di salto ad ostacoli in cui l&apos;altezza degli ostacoli lungo il percorso di gara non è mai superiore ai 80 cm</rdfs:comment>
        <rdfs:comment xml:lang="en">Show jumping category in which the height of the obstacles along the competition course is never higher than 80 cm</rdfs:comment>
        <rdfs:label xml:lang="en">C80</rdfs:label>
        <rdfs:label xml:lang="it">C80</rdfs:label>
    </owl:NamedIndividual>
    


    <!-- http://www.semanticweb.org/annag/ontologies/2024/1/ontoHorses#C90 -->

    <owl:NamedIndividual rdf:about="http://www.semanticweb.org/annag/ontologies/2024/1/ontoHorses#C90">
        <rdf:type rdf:resource="http://dbpedia.org/ontology/horseRidingDiscipline"/>
        <rdf:type rdf:resource="http://www.semanticweb.org/annag/ontologies/2024/1/ontoHorses#CategorieDiSalto"/>
        <rdf:type rdf:resource="http://www.semanticweb.org/annag/ontologies/2024/1/ontoHorses#Impiego"/>
        <rdf:type rdf:resource="http://www.semanticweb.org/annag/ontologies/2024/1/ontoHorses#SaltoAdOstacoli"/>
        <rdf:type rdf:resource="http://www.semanticweb.org/annag/ontologies/2024/1/ontoHorses#Sella"/>
        <rdf:type rdf:resource="http://www.semanticweb.org/annag/ontologies/2024/1/ontoHorses#SportEquestre"/>
        <ontoHorses:permetteIlConseguimentoDi rdf:resource="http://www.semanticweb.org/annag/ontologies/2024/1/ontoHorses#brevetto"/>
        <rdfs:comment xml:lang="it">Categoria di salto ad ostacoli in cui l&apos;altezza degli ostacoli lungo il percorso di gara non è mai superiore ai 90 cm</rdfs:comment>
        <rdfs:comment xml:lang="en">Show jumping category in which the height of the obstacles along the competition course is never higher than 90 cm</rdfs:comment>
        <rdfs:label xml:lang="en">C90</rdfs:label>
        <rdfs:label xml:lang="it">C90</rdfs:label>
    </owl:NamedIndividual>
    


    <!-- http://www.semanticweb.org/annag/ontologies/2024/1/ontoHorses#CastroneAngloAraboFrancese -->

    <owl:NamedIndividual rdf:about="http://www.semanticweb.org/annag/ontologies/2024/1/ontoHorses#CastroneAngloAraboFrancese">
        <rdf:type rdf:resource="http://dbpedia.org/ontology/horse"/>
        <rdf:type rdf:resource="http://www.semanticweb.org/annag/ontologies/2024/1/ontoHorses#Cavallo"/>
        <rdf:type rdf:resource="http://www.semanticweb.org/annag/ontologies/2024/1/ontoHorses#CavalloASangueCaldo"/>
        <rdf:type rdf:resource="http://www.semanticweb.org/annag/ontologies/2024/1/ontoHorses#CavalloAdulto"/>
        <rdf:type rdf:resource="http://www.semanticweb.org/annag/ontologies/2024/1/ontoHorses#CavalloCastrone"/>
        <rdf:type rdf:resource="http://www.semanticweb.org/annag/ontologies/2024/1/ontoHorses#CavalloDaSella"/>
        <rdf:type rdf:resource="http://www.semanticweb.org/annag/ontologies/2024/1/ontoHorses#CavalloPerCrossCountry"/>
        <rdf:type rdf:resource="http://www.semanticweb.org/annag/ontologies/2024/1/ontoHorses#CavalloSportivo"/>
        <price:hasPrice rdf:resource="http://www.semanticweb.org/annag/ontologies/2024/1/ontoHorses#15000Euro"/>
        <ontoHorses:haRazza rdf:resource="http://www.semanticweb.org/annag/ontologies/2024/1/ontoHorses#AngloAraboFrancese"/>
        <ontoHorses:vieneUtilizzatoPer rdf:resource="http://www.semanticweb.org/annag/ontologies/2024/1/ontoHorses#CrossCountry"/>
        <ontoHorses:èAdattoPer rdf:resource="http://www.semanticweb.org/annag/ontologies/2024/1/ontoHorses#CavaliereIntermedio"/>
        <ontoHorses:èPossedutoDa rdf:resource="http://www.semanticweb.org/annag/ontologies/2024/1/ontoHorses#claudioCavallo"/>
        <ontoHorses:èScuderizzatoIn rdf:resource="http://www.semanticweb.org/annag/ontologies/2024/1/ontoHorses#Italia"/>
        <ontoHorses:èScuderizzatoIn rdf:resource="http://www.semanticweb.org/annag/ontologies/2024/1/ontoHorses#Sicilia"/>
        <ontoHorses:èScuderizzatoInCittàDi rdf:resource="http://www.semanticweb.org/annag/ontologies/2024/1/ontoHorses#siracusa"/>
        <ontoHorses:altezzaGarrese rdf:datatype="http://www.w3.org/2001/XMLSchema#integer">158</ontoHorses:altezzaGarrese>
        <ontoHorses:eta rdf:datatype="http://www.w3.org/2001/XMLSchema#integer">15</ontoHorses:eta>
        <ontoHorses:haSesso>castrone</ontoHorses:haSesso>
        <ontoHorses:nomeCavallo>Filè</ontoHorses:nomeCavallo>
        <schema:image rdf:resource="https://www.equirodi.it/images/annonces/l/857696_1711550997_1626.jpg"/>
        <rdfs:comment xml:lang="en">15 year old French Anglo-Arab gelding for sale. Not suitable for beginners. Currently used for cross-country competitions.</rdfs:comment>
        <rdfs:comment xml:lang="it">Esemplare di cavallo castrone anglo-arabo francese di 15 anni  in vendita. Non adatto a principianti. Attualmente utilizzato per competizioni di cross-country.</rdfs:comment>
        <rdfs:label xml:lang="it">Castrone anglo-arabo francese</rdfs:label>
        <rdfs:label xml:lang="en">French Anglo-Arabic gelding</rdfs:label>
    </owl:NamedIndividual>
    


    <!-- http://www.semanticweb.org/annag/ontologies/2024/1/ontoHorses#CastroneFrancese -->

    <owl:NamedIndividual rdf:about="http://www.semanticweb.org/annag/ontologies/2024/1/ontoHorses#CastroneFrancese">
        <rdf:type rdf:resource="http://dbpedia.org/ontology/horse"/>
        <rdf:type rdf:resource="http://www.semanticweb.org/annag/ontologies/2024/1/ontoHorses#Cavallo"/>
        <rdf:type rdf:resource="http://www.semanticweb.org/annag/ontologies/2024/1/ontoHorses#CavalloASangueCaldo"/>
        <rdf:type rdf:resource="http://www.semanticweb.org/annag/ontologies/2024/1/ontoHorses#CavalloAdulto"/>
        <rdf:type rdf:resource="http://www.semanticweb.org/annag/ontologies/2024/1/ontoHorses#CavalloCastrone"/>
        <rdf:type rdf:resource="http://www.semanticweb.org/annag/ontologies/2024/1/ontoHorses#CavalloDaSella"/>
        <rdf:type rdf:resource="http://www.semanticweb.org/annag/ontologies/2024/1/ontoHorses#CavalloSportivo"/>
        <price:hasPrice rdf:resource="http://www.semanticweb.org/annag/ontologies/2024/1/ontoHorses#18000Euro"/>
        <ontoHorses:adattoAlConseguimentoDi rdf:resource="http://www.semanticweb.org/annag/ontologies/2024/1/ontoHorses#brevetto"/>
        <ontoHorses:adattoAlConseguimentoDi rdf:resource="http://www.semanticweb.org/annag/ontologies/2024/1/ontoHorses#primoGrado"/>
        <ontoHorses:gareggiaNelleCategorieDiSalto rdf:resource="http://www.semanticweb.org/annag/ontologies/2024/1/ontoHorses#C110"/>
        <ontoHorses:gareggiaNelleCategorieDiSalto rdf:resource="http://www.semanticweb.org/annag/ontologies/2024/1/ontoHorses#C125"/>
        <ontoHorses:haRazza rdf:resource="http://www.semanticweb.org/annag/ontologies/2024/1/ontoHorses#SellaFrancese"/>
        <ontoHorses:vieneUtilizzatoPer rdf:resource="http://www.semanticweb.org/annag/ontologies/2024/1/ontoHorses#SaltoAdOstacoli"/>
        <ontoHorses:èAdattoPer rdf:resource="http://www.semanticweb.org/annag/ontologies/2024/1/ontoHorses#CavaliereEsperto"/>
        <ontoHorses:èAdattoPer rdf:resource="http://www.semanticweb.org/annag/ontologies/2024/1/ontoHorses#CavaliereIntermedio"/>
        <ontoHorses:èAdattoPer rdf:resource="http://www.semanticweb.org/annag/ontologies/2024/1/ontoHorses#CavalierePrincipiante"/>
        <ontoHorses:èPossedutoDa rdf:resource="http://www.semanticweb.org/annag/ontologies/2024/1/ontoHorses#gianlucaCamoletto"/>
        <ontoHorses:èScuderizzatoIn rdf:resource="http://www.semanticweb.org/annag/ontologies/2024/1/ontoHorses#Italia"/>
        <ontoHorses:èScuderizzatoIn rdf:resource="http://www.semanticweb.org/annag/ontologies/2024/1/ontoHorses#Piemonte"/>
        <ontoHorses:èScuderizzatoInCittàDi rdf:resource="http://www.semanticweb.org/annag/ontologies/2024/1/ontoHorses#leini"/>
        <ontoHorses:altezzaGarrese rdf:datatype="http://www.w3.org/2001/XMLSchema#integer">167</ontoHorses:altezzaGarrese>
        <ontoHorses:eta rdf:datatype="http://www.w3.org/2001/XMLSchema#integer">8</ontoHorses:eta>
        <ontoHorses:haSesso>castrone</ontoHorses:haSesso>
        <ontoHorses:nomeCavallo>Elton</ontoHorses:nomeCavallo>
        <schema:image rdf:resource="https://www.equirodi.it/images/annonces/xl/855373_1710395667_3888.jpg"/>
        <rdfs:comment xml:lang="it">Esemplare di castrone francese in vendita. Anno 2016. Attualmente impegnato in salto ad ostacoli nelle categorie C110 e C125. Adatto a tutti. Facile gestione sia a terra che in sella. Adatto come primo cavallo per il conseguimento del brevetto.</rdfs:comment>
        <rdfs:comment xml:lang="en">French gelding for sale. Year 2016. Currently involved in show jumping in the C110 and C125 categories. Suitable for everyone. Easy management both on the ground and in the saddle. Suitable as the first horse for obtaining the licence.</rdfs:comment>
        <rdfs:label xml:lang="it">Castrone Francese</rdfs:label>
        <rdfs:label xml:lang="en">French gelding horse</rdfs:label>
    </owl:NamedIndividual>
    


    <!-- http://www.semanticweb.org/annag/ontologies/2024/1/ontoHorses#CastroneItaliano -->

    <owl:NamedIndividual rdf:about="http://www.semanticweb.org/annag/ontologies/2024/1/ontoHorses#CastroneItaliano">
        <rdf:type rdf:resource="http://dbpedia.org/ontology/horse"/>
        <rdf:type rdf:resource="http://www.semanticweb.org/annag/ontologies/2024/1/ontoHorses#Cavallo"/>
        <rdf:type rdf:resource="http://www.semanticweb.org/annag/ontologies/2024/1/ontoHorses#CavalloASangueCaldo"/>
        <rdf:type rdf:resource="http://www.semanticweb.org/annag/ontologies/2024/1/ontoHorses#CavalloAdulto"/>
        <rdf:type rdf:resource="http://www.semanticweb.org/annag/ontologies/2024/1/ontoHorses#CavalloCastrone"/>
        <rdf:type rdf:resource="http://www.semanticweb.org/annag/ontologies/2024/1/ontoHorses#CavalloDaSella"/>
        <rdf:type rdf:resource="http://www.semanticweb.org/annag/ontologies/2024/1/ontoHorses#CavalloSportivo"/>
        <price:hasPrice rdf:resource="http://www.semanticweb.org/annag/ontologies/2024/1/ontoHorses#12000Euro"/>
        <ontoHorses:adattoAlConseguimentoDi rdf:resource="http://www.semanticweb.org/annag/ontologies/2024/1/ontoHorses#brevetto"/>
        <ontoHorses:gareggiaNelleCategorieDiSalto rdf:resource="http://www.semanticweb.org/annag/ontologies/2024/1/ontoHorses#C100"/>
        <ontoHorses:gareggiaNelleCategorieDiSalto rdf:resource="http://www.semanticweb.org/annag/ontologies/2024/1/ontoHorses#C80"/>
        <ontoHorses:haRazza rdf:resource="http://www.semanticweb.org/annag/ontologies/2024/1/ontoHorses#SellaItaliano"/>
        <ontoHorses:vieneUtilizzatoPer rdf:resource="http://www.semanticweb.org/annag/ontologies/2024/1/ontoHorses#SaltoAdOstacoli"/>
        <ontoHorses:èAdattoPer rdf:resource="http://www.semanticweb.org/annag/ontologies/2024/1/ontoHorses#CavalierePrincipiante"/>
        <ontoHorses:èPossedutoDa rdf:resource="http://www.semanticweb.org/annag/ontologies/2024/1/ontoHorses#brunoGramaglia"/>
        <ontoHorses:èScuderizzatoIn rdf:resource="http://www.semanticweb.org/annag/ontologies/2024/1/ontoHorses#Italia"/>
        <ontoHorses:èScuderizzatoIn rdf:resource="http://www.semanticweb.org/annag/ontologies/2024/1/ontoHorses#Piemonte"/>
        <ontoHorses:èScuderizzatoInCittàDi rdf:resource="http://www.semanticweb.org/annag/ontologies/2024/1/ontoHorses#sanMauro"/>
        <ontoHorses:altezzaGarrese rdf:datatype="http://www.w3.org/2001/XMLSchema#integer">160</ontoHorses:altezzaGarrese>
        <ontoHorses:eta rdf:datatype="http://www.w3.org/2001/XMLSchema#integer">11</ontoHorses:eta>
        <ontoHorses:haSesso>castrone</ontoHorses:haSesso>
        <ontoHorses:nomeCavallo>Dracon&apos;s Breaker</ontoHorses:nomeCavallo>
        <schema:image rdf:resource="https://www.equirodi.it/images/annonces/xl/857207_1711357444_2037.jpg"/>
        <rdfs:comment xml:lang="en">11 year old Italian gelding horse for sale. Currently involved in show jumping in the C100 categories. Suitable for beginners with a minimum of experience. Difficult management in the box.</rdfs:comment>
        <rdfs:comment xml:lang="it">Esemplare di cavallo castrone italiano di 11 anni in vendita. Attualmente impegnato nel salto ad ostacoli nelle categorie C100. Adatto a principianti con un minimo di esperienza. Difficile gestione in box.</rdfs:comment>
        <rdfs:label xml:lang="it">Castrone italiano</rdfs:label>
        <rdfs:label xml:lang="en">Italian Gelding horse</rdfs:label>
    </owl:NamedIndividual>
    


    <!-- http://www.semanticweb.org/annag/ontologies/2024/1/ontoHorses#CavaliereEsperto -->

    <owl:NamedIndividual rdf:about="http://www.semanticweb.org/annag/ontologies/2024/1/ontoHorses#CavaliereEsperto">
        <rdf:type rdf:resource="http://dbpedia.org/ontology/HorseRider"/>
        <rdf:type rdf:resource="http://www.semanticweb.org/annag/ontologies/2024/1/ontoHorses#Cavaliere"/>
        <rdf:type rdf:resource="http://www.semanticweb.org/annag/ontologies/2024/1/ontoHorses#Persona"/>
        <rdf:type rdf:resource="http://xmlns.com/foaf/0.1/person"/>
        <ontoHorses:consegue rdf:resource="http://www.semanticweb.org/annag/ontologies/2024/1/ontoHorses#primoGrado"/>
        <rdfs:comment xml:lang="it">Cavaliere la cui abilità di di salto ostacoli è superiore alla categoria C115 ma inferiore alla categoria C130</rdfs:comment>
        <rdfs:comment xml:lang="en">Horse rider whose jumping ability is above category C115 but below category C130</rdfs:comment>
        <rdfs:label xml:lang="it">Cavaliere esperto</rdfs:label>
        <rdfs:label xml:lang="en">Expert horse rider</rdfs:label>
    </owl:NamedIndividual>
    


    <!-- http://www.semanticweb.org/annag/ontologies/2024/1/ontoHorses#CavaliereIntermedio -->

    <owl:NamedIndividual rdf:about="http://www.semanticweb.org/annag/ontologies/2024/1/ontoHorses#CavaliereIntermedio">
        <rdf:type rdf:resource="http://dbpedia.org/ontology/HorseRider"/>
        <rdf:type rdf:resource="http://www.semanticweb.org/annag/ontologies/2024/1/ontoHorses#Cavaliere"/>
        <rdf:type rdf:resource="http://www.semanticweb.org/annag/ontologies/2024/1/ontoHorses#Persona"/>
        <rdf:type rdf:resource="http://xmlns.com/foaf/0.1/person"/>
        <ontoHorses:consegue rdf:resource="http://www.semanticweb.org/annag/ontologies/2024/1/ontoHorses#primoGrado"/>
        <rdfs:comment xml:lang="it">Cavaliere la cui abilità di di salto ostacoli è inferiore alla categoria C115</rdfs:comment>
        <rdfs:comment xml:lang="en">Horse rider whose jumping ability is below category C115</rdfs:comment>
        <rdfs:label xml:lang="it">Cavaliere intermedio</rdfs:label>
        <rdfs:label xml:lang="en">Intermediate horse rider</rdfs:label>
    </owl:NamedIndividual>
    


    <!-- http://www.semanticweb.org/annag/ontologies/2024/1/ontoHorses#CavaliereMoltoEsperto -->

    <owl:NamedIndividual rdf:about="http://www.semanticweb.org/annag/ontologies/2024/1/ontoHorses#CavaliereMoltoEsperto">
        <rdf:type rdf:resource="http://dbpedia.org/ontology/HorseRider"/>
        <rdf:type rdf:resource="http://www.semanticweb.org/annag/ontologies/2024/1/ontoHorses#Cavaliere"/>
        <rdf:type rdf:resource="http://www.semanticweb.org/annag/ontologies/2024/1/ontoHorses#Persona"/>
        <rdf:type rdf:resource="http://xmlns.com/foaf/0.1/person"/>
        <ontoHorses:consegue rdf:resource="http://www.semanticweb.org/annag/ontologies/2024/1/ontoHorses#secondoGrado"/>
        <rdfs:comment xml:lang="it">Cavaliere la cui abilità di di salto ostacoli è uguale o superiore alla categoria C135</rdfs:comment>
        <rdfs:comment xml:lang="en">Horse rider whose show jumping ability is equal to or greater than category C135</rdfs:comment>
        <rdfs:label xml:lang="it">Cavaliere molto esperto</rdfs:label>
        <rdfs:label xml:lang="en">Very experienced horse rider</rdfs:label>
    </owl:NamedIndividual>
    


    <!-- http://www.semanticweb.org/annag/ontologies/2024/1/ontoHorses#CavalierePrincipiante -->

    <owl:NamedIndividual rdf:about="http://www.semanticweb.org/annag/ontologies/2024/1/ontoHorses#CavalierePrincipiante">
        <rdf:type rdf:resource="http://dbpedia.org/ontology/HorseRider"/>
        <rdf:type rdf:resource="http://www.semanticweb.org/annag/ontologies/2024/1/ontoHorses#Cavaliere"/>
        <rdf:type rdf:resource="http://www.semanticweb.org/annag/ontologies/2024/1/ontoHorses#Persona"/>
        <rdf:type rdf:resource="http://xmlns.com/foaf/0.1/person"/>
        <ontoHorses:consegue rdf:resource="http://www.semanticweb.org/annag/ontologies/2024/1/ontoHorses#brevetto"/>
        <ontoHorses:consegue rdf:resource="http://www.semanticweb.org/annag/ontologies/2024/1/ontoHorses#patenteLudicaA"/>
        <rdfs:comment xml:lang="it">Cavaliere la cui abilità di di salto ostacoli è inferiore alla categoria C80</rdfs:comment>
        <rdfs:comment xml:lang="en">Horse rider whose jumping ability is below category C80</rdfs:comment>
        <rdfs:label xml:lang="en">Beginner horse rider</rdfs:label>
        <rdfs:label xml:lang="it">Cavaliere principiante</rdfs:label>
    </owl:NamedIndividual>
    


    <!-- http://www.semanticweb.org/annag/ontologies/2024/1/ontoHorses#CavalloDelloJutland -->

    <owl:NamedIndividual rdf:about="http://www.semanticweb.org/annag/ontologies/2024/1/ontoHorses#CavalloDelloJutland">
        <rdf:type rdf:resource="http://www.semanticweb.org/annag/ontologies/2024/1/ontoHorses#RazzaASangueFreddo"/>
        <rdf:type rdf:resource="http://www.semanticweb.org/annag/ontologies/2024/1/ontoHorses#RazzaBrachimorfa"/>
        <rdf:type rdf:resource="http://www.semanticweb.org/annag/ontologies/2024/1/ontoHorses#RazzaCavallo"/>
        <rdf:type rdf:resource="http://www.semanticweb.org/annag/ontologies/2024/1/ontoHorses#RazzaDaLavoro"/>
        <rdf:type rdf:resource="http://www.semanticweb.org/annag/ontologies/2024/1/ontoHorses#RazzaDaTiroAgricolo"/>
        <ontoHorses:entitàWikidata rdf:resource="http://www.wikidata.org/entity/Q1684175"/>
        <ontoHorses:haClassificazioneMorfologica rdf:resource="http://www.semanticweb.org/annag/ontologies/2024/1/ontoHorses#brachimorfo"/>
        <ontoHorses:haIndole rdf:resource="http://www.semanticweb.org/annag/ontologies/2024/1/ontoHorses#sangueFreddo"/>
        <ontoHorses:haNazionalità rdf:resource="http://www.semanticweb.org/annag/ontologies/2024/1/ontoHorses#Danimarca"/>
        <ontoHorses:haRegioneDiOrigine rdf:resource="http://www.semanticweb.org/annag/ontologies/2024/1/ontoHorses#Jutland"/>
        <ontoHorses:puòEssereImpiegataIn rdf:resource="http://www.semanticweb.org/annag/ontologies/2024/1/ontoHorses#TiroAgricolo"/>
        <ontoHorses:altezzaMediaGarrese rdf:datatype="http://www.w3.org/2001/XMLSchema#integer">160</ontoHorses:altezzaMediaGarrese>
        <ontoHorses:haColoreMantello>baio</ontoHorses:haColoreMantello>
        <ontoHorses:haColoreMantello>grigio</ontoHorses:haColoreMantello>
        <ontoHorses:haColoreMantello>roano</ontoHorses:haColoreMantello>
        <ontoHorses:haColoreMantello>sauro</ontoHorses:haColoreMantello>
        <ontoHorses:pesoMedio rdf:datatype="http://www.w3.org/2001/XMLSchema#integer">725</ontoHorses:pesoMedio>
        <schema:image rdf:resource="https://upload.wikimedia.org/wikipedia/commons/thumb/4/49/Jydske_heste_vorup_enge.jpg/240px-Jydske_heste_vorup_enge.jpg"/>
        <rdfs:comment xml:lang="it">Il cavallo dello Jutland è un cavallo da tiro pesante, di razza danese, il cui nome deriva dalla penisola dello Jutland, in cui viene allevato dal XII secolo</rdfs:comment>
        <rdfs:comment xml:lang="en">The Jutland horse is a heavy draft horse, of Danish breed, whose name derives from the Jutland peninsula, where it has been bred since the 12th century</rdfs:comment>
        <skos:exactMatch xml:lang="it">http://www.wikidata.org/entity/Q1684175</skos:exactMatch>
        <skos:prefLabel xml:lang="it">Cavallo dello Jutland</skos:prefLabel>
        <skos:prefLabel xml:lang="en">Jutland Horse</skos:prefLabel>
    </owl:NamedIndividual>
    


    <!-- http://www.semanticweb.org/annag/ontologies/2024/1/ontoHorses#Clydesdale -->

    <owl:NamedIndividual rdf:about="http://www.semanticweb.org/annag/ontologies/2024/1/ontoHorses#Clydesdale">
        <rdf:type rdf:resource="http://www.semanticweb.org/annag/ontologies/2024/1/ontoHorses#RazzaASangueFreddo"/>
        <rdf:type rdf:resource="http://www.semanticweb.org/annag/ontologies/2024/1/ontoHorses#RazzaBrachimorfa"/>
        <rdf:type rdf:resource="http://www.semanticweb.org/annag/ontologies/2024/1/ontoHorses#RazzaCavallo"/>
        <rdf:type rdf:resource="http://www.semanticweb.org/annag/ontologies/2024/1/ontoHorses#RazzaDaLavoro"/>
        <rdf:type rdf:resource="http://www.semanticweb.org/annag/ontologies/2024/1/ontoHorses#RazzaDaTiroAgricolo"/>
        <ontoHorses:entitàWikidata rdf:resource="http://www.wikidata.org/entity/Q844058"/>
        <ontoHorses:haClassificazioneMorfologica rdf:resource="http://www.semanticweb.org/annag/ontologies/2024/1/ontoHorses#brachimorfo"/>
        <ontoHorses:haIndole rdf:resource="http://www.semanticweb.org/annag/ontologies/2024/1/ontoHorses#sangueFreddo"/>
        <ontoHorses:haNazionalità rdf:resource="http://www.semanticweb.org/annag/ontologies/2024/1/ontoHorses#RegnoUnito"/>
        <ontoHorses:haRegioneDiOrigine rdf:resource="http://www.semanticweb.org/annag/ontologies/2024/1/ontoHorses#Scozia"/>
        <ontoHorses:puòEssereImpiegataIn rdf:resource="http://www.semanticweb.org/annag/ontologies/2024/1/ontoHorses#TiroAgricolo"/>
        <ontoHorses:altezzaMediaGarrese rdf:datatype="http://www.w3.org/2001/XMLSchema#integer">168</ontoHorses:altezzaMediaGarrese>
        <ontoHorses:haColoreMantello>baio</ontoHorses:haColoreMantello>
        <ontoHorses:haColoreMantello>grigio</ontoHorses:haColoreMantello>
        <ontoHorses:haColoreMantello>morello</ontoHorses:haColoreMantello>
        <ontoHorses:haColoreMantello>roano</ontoHorses:haColoreMantello>
        <ontoHorses:haColoreMantello>sauro</ontoHorses:haColoreMantello>
        <ontoHorses:pesoMedio rdf:datatype="http://www.w3.org/2001/XMLSchema#integer">850</ontoHorses:pesoMedio>
        <schema:image rdf:resource="https://upload.wikimedia.org/wikipedia/commons/thumb/0/07/I_feel_pretty._Oh_so_pretty..jpg/220px-I_feel_pretty._Oh_so_pretty..jpg"/>
        <rdfs:comment xml:lang="it">Il Clydesdale è una razza di cavalli da tiro pesante lentoil cui nome deriva dalle fattorie presenti nella contea di Clydesdale, situata in Scozia.</rdfs:comment>
        <rdfs:comment xml:lang="en">The Clydesdale is a breed of slow heavy draft horse whose name derives from the farms present in the county of Clydesdale, located in Scotland</rdfs:comment>
        <skos:exactMatch xml:lang="it">http://www.wikidata.org/entity/Q844058</skos:exactMatch>
        <skos:prefLabel xml:lang="it">Clydesdale</skos:prefLabel>
        <skos:prefLabel xml:lang="en">Clydesdale Horse</skos:prefLabel>
    </owl:NamedIndividual>
    


    <!-- http://www.semanticweb.org/annag/ontologies/2024/1/ontoHorses#CrossCountry -->

    <owl:NamedIndividual rdf:about="http://www.semanticweb.org/annag/ontologies/2024/1/ontoHorses#CrossCountry">
        <rdf:type rdf:resource="http://dbpedia.org/ontology/horseRidingDiscipline"/>
        <rdf:type rdf:resource="http://www.semanticweb.org/annag/ontologies/2024/1/ontoHorses#Impiego"/>
        <rdf:type rdf:resource="http://www.semanticweb.org/annag/ontologies/2024/1/ontoHorses#Sella"/>
        <rdf:type rdf:resource="http://www.semanticweb.org/annag/ontologies/2024/1/ontoHorses#SportEquestre"/>
    </owl:NamedIndividual>
    


    <!-- http://www.semanticweb.org/annag/ontologies/2024/1/ontoHorses#D -->

    <owl:NamedIndividual rdf:about="http://www.semanticweb.org/annag/ontologies/2024/1/ontoHorses#D">
        <rdf:type rdf:resource="http://dbpedia.org/ontology/horseRidingDiscipline"/>
        <rdf:type rdf:resource="http://www.semanticweb.org/annag/ontologies/2024/1/ontoHorses#CategorieDressage"/>
        <rdf:type rdf:resource="http://www.semanticweb.org/annag/ontologies/2024/1/ontoHorses#Dressage"/>
        <rdf:type rdf:resource="http://www.semanticweb.org/annag/ontologies/2024/1/ontoHorses#Impiego"/>
        <rdf:type rdf:resource="http://www.semanticweb.org/annag/ontologies/2024/1/ontoHorses#Sella"/>
        <rdf:type rdf:resource="http://www.semanticweb.org/annag/ontologies/2024/1/ontoHorses#SportEquestre"/>
        <rdfs:comment xml:lang="it">E&apos; la categoria di Dressage con la massima difficoltà, detta anche Gran Premio</rdfs:comment>
        <rdfs:comment xml:lang="en">It is the Dressage category with the greatest difficulty, also called Grand Prix</rdfs:comment>
        <rdfs:label xml:lang="en">D</rdfs:label>
        <rdfs:label xml:lang="it">D</rdfs:label>
    </owl:NamedIndividual>
    


    <!-- http://www.semanticweb.org/annag/ontologies/2024/1/ontoHorses#Danimarca -->

    <owl:NamedIndividual rdf:about="http://www.semanticweb.org/annag/ontologies/2024/1/ontoHorses#Danimarca">
        <rdf:type rdf:resource="http://schema.org/Place"/>
        <rdf:type rdf:resource="http://www.semanticweb.org/annag/ontologies/2024/1/ontoHorses#AreaGeografica"/>
        <partof:hasPart rdf:resource="http://www.semanticweb.org/annag/ontologies/2024/1/ontoHorses#Jutland"/>
        <schema:image rdf:resource="https://upload.wikimedia.org/wikipedia/commons/thumb/9/9c/Flag_of_Denmark.svg/1280px-Flag_of_Denmark.svg.png"/>
        <rdfs:comment xml:lang="en">Denmark, officially the Kingdom of Denmark, is a member state of the European Union and the smallest and southernmost state in Scandinavia.</rdfs:comment>
        <rdfs:comment xml:lang="it">La Danimarca, ufficialmente Regno di Danimarca , è uno Stato membro dell&apos;Unione europea e lo Stato più piccolo e più meridionale della Scandinavia.</rdfs:comment>
        <rdfs:label xml:lang="it">Danimarca</rdfs:label>
        <rdfs:label xml:lang="en">Denmark</rdfs:label>
    </owl:NamedIndividual>
    


    <!-- http://www.semanticweb.org/annag/ontologies/2024/1/ontoHorses#Dressage -->

    <owl:NamedIndividual rdf:about="http://www.semanticweb.org/annag/ontologies/2024/1/ontoHorses#Dressage">
        <rdf:type rdf:resource="http://dbpedia.org/ontology/horseRidingDiscipline"/>
        <rdf:type rdf:resource="http://www.semanticweb.org/annag/ontologies/2024/1/ontoHorses#Impiego"/>
        <rdf:type rdf:resource="http://www.semanticweb.org/annag/ontologies/2024/1/ontoHorses#Sella"/>
        <rdf:type rdf:resource="http://www.semanticweb.org/annag/ontologies/2024/1/ontoHorses#SportEquestre"/>
    </owl:NamedIndividual>
    


    <!-- http://www.semanticweb.org/annag/ontologies/2024/1/ontoHorses#E -->

    <owl:NamedIndividual rdf:about="http://www.semanticweb.org/annag/ontologies/2024/1/ontoHorses#E">
        <rdf:type rdf:resource="http://dbpedia.org/ontology/horseRidingDiscipline"/>
        <rdf:type rdf:resource="http://www.semanticweb.org/annag/ontologies/2024/1/ontoHorses#CategorieDressage"/>
        <rdf:type rdf:resource="http://www.semanticweb.org/annag/ontologies/2024/1/ontoHorses#Dressage"/>
        <rdf:type rdf:resource="http://www.semanticweb.org/annag/ontologies/2024/1/ontoHorses#Impiego"/>
        <rdf:type rdf:resource="http://www.semanticweb.org/annag/ontologies/2024/1/ontoHorses#Sella"/>
        <rdf:type rdf:resource="http://www.semanticweb.org/annag/ontologies/2024/1/ontoHorses#SportEquestre"/>
        <rdfs:comment xml:lang="it">Categoria elementare di Dressage</rdfs:comment>
        <rdfs:comment xml:lang="en">Elementary Dressage category</rdfs:comment>
        <rdfs:label xml:lang="en">E</rdfs:label>
        <rdfs:label xml:lang="it">E</rdfs:label>
    </owl:NamedIndividual>
    


    <!-- http://www.semanticweb.org/annag/ontologies/2024/1/ontoHorses#Endurance -->

    <owl:NamedIndividual rdf:about="http://www.semanticweb.org/annag/ontologies/2024/1/ontoHorses#Endurance">
        <rdf:type rdf:resource="http://dbpedia.org/ontology/horseRidingDiscipline"/>
        <rdf:type rdf:resource="http://www.semanticweb.org/annag/ontologies/2024/1/ontoHorses#Impiego"/>
        <rdf:type rdf:resource="http://www.semanticweb.org/annag/ontologies/2024/1/ontoHorses#Sella"/>
        <rdf:type rdf:resource="http://www.semanticweb.org/annag/ontologies/2024/1/ontoHorses#SportEquestre"/>
    </owl:NamedIndividual>
    


    <!-- http://www.semanticweb.org/annag/ontologies/2024/1/ontoHorses#Equiturismo -->

    <owl:Class rdf:about="http://www.semanticweb.org/annag/ontologies/2024/1/ontoHorses#Equiturismo">
        <rdf:type rdf:resource="http://www.w3.org/2002/07/owl#NamedIndividual"/>
        <rdf:type rdf:resource="http://dbpedia.org/ontology/horseRidingDiscipline"/>
        <rdf:type rdf:resource="http://www.semanticweb.org/annag/ontologies/2024/1/ontoHorses#Equiturismo"/>
        <rdf:type rdf:resource="http://www.semanticweb.org/annag/ontologies/2024/1/ontoHorses#Impiego"/>
        <rdf:type rdf:resource="http://www.semanticweb.org/annag/ontologies/2024/1/ontoHorses#Sella"/>
    </owl:Class>
    


    <!-- http://www.semanticweb.org/annag/ontologies/2024/1/ontoHorses#Euro -->

    <owl:NamedIndividual rdf:about="http://www.semanticweb.org/annag/ontologies/2024/1/ontoHorses#Euro">
        <rdf:type rdf:resource="http://dbpedia.org/ontology/horse"/>
        <rdf:type rdf:resource="http://www.ontologydesignpatterns.org/cp/owl/price.owl#Currency"/>
        <rdf:type rdf:resource="http://www.semanticweb.org/annag/ontologies/2024/1/ontoHorses#Cavallo"/>
        <rdfs:comment xml:lang="en">European Currency</rdfs:comment>
        <rdfs:comment xml:lang="it">Moneta europea</rdfs:comment>
        <rdfs:label xml:lang="en">Euro</rdfs:label>
        <rdfs:label xml:lang="it">Euro</rdfs:label>
    </owl:NamedIndividual>
    


    <!-- http://www.semanticweb.org/annag/ontologies/2024/1/ontoHorses#Eventing -->

    <owl:NamedIndividual rdf:about="http://www.semanticweb.org/annag/ontologies/2024/1/ontoHorses#Eventing">
        <rdf:type rdf:resource="http://dbpedia.org/ontology/horseRidingDiscipline"/>
        <rdf:type rdf:resource="http://www.semanticweb.org/annag/ontologies/2024/1/ontoHorses#Impiego"/>
        <rdf:type rdf:resource="http://www.semanticweb.org/annag/ontologies/2024/1/ontoHorses#Sella"/>
        <rdf:type rdf:resource="http://www.semanticweb.org/annag/ontologies/2024/1/ontoHorses#SportEquestre"/>
    </owl:NamedIndividual>
    


    <!-- http://www.semanticweb.org/annag/ontologies/2024/1/ontoHorses#F -->

    <owl:NamedIndividual rdf:about="http://www.semanticweb.org/annag/ontologies/2024/1/ontoHorses#F">
        <rdf:type rdf:resource="http://dbpedia.org/ontology/horseRidingDiscipline"/>
        <rdf:type rdf:resource="http://www.semanticweb.org/annag/ontologies/2024/1/ontoHorses#CategorieDressage"/>
        <rdf:type rdf:resource="http://www.semanticweb.org/annag/ontologies/2024/1/ontoHorses#Dressage"/>
        <rdf:type rdf:resource="http://www.semanticweb.org/annag/ontologies/2024/1/ontoHorses#Impiego"/>
        <rdf:type rdf:resource="http://www.semanticweb.org/annag/ontologies/2024/1/ontoHorses#Sella"/>
        <rdf:type rdf:resource="http://www.semanticweb.org/annag/ontologies/2024/1/ontoHorses#SportEquestre"/>
        <rdfs:comment xml:lang="it">Categoria facile di Dressage</rdfs:comment>
        <rdfs:comment xml:lang="en">Easy Dressage category</rdfs:comment>
        <rdfs:label xml:lang="en">F</rdfs:label>
        <rdfs:label xml:lang="it">F</rdfs:label>
    </owl:NamedIndividual>
    


    <!-- http://www.semanticweb.org/annag/ontologies/2024/1/ontoHorses#FemminaBretone -->

    <owl:NamedIndividual rdf:about="http://www.semanticweb.org/annag/ontologies/2024/1/ontoHorses#FemminaBretone">
        <rdf:type rdf:resource="http://dbpedia.org/ontology/horse"/>
        <rdf:type rdf:resource="http://www.semanticweb.org/annag/ontologies/2024/1/ontoHorses#Cavallo"/>
        <rdf:type rdf:resource="http://www.semanticweb.org/annag/ontologies/2024/1/ontoHorses#CavalloASangueFreddo"/>
        <rdf:type rdf:resource="http://www.semanticweb.org/annag/ontologies/2024/1/ontoHorses#CavalloAdulto"/>
        <rdf:type rdf:resource="http://www.semanticweb.org/annag/ontologies/2024/1/ontoHorses#CavalloDaLavoro"/>
        <rdf:type rdf:resource="http://www.semanticweb.org/annag/ontologies/2024/1/ontoHorses#CavalloDaTiroAgricolo"/>
        <rdf:type rdf:resource="http://www.semanticweb.org/annag/ontologies/2024/1/ontoHorses#CavalloFemmina"/>
        <price:hasPrice rdf:resource="http://www.semanticweb.org/annag/ontologies/2024/1/ontoHorses#2500Euro"/>
        <ontoHorses:haRazza rdf:resource="http://www.semanticweb.org/annag/ontologies/2024/1/ontoHorses#Bretone"/>
        <ontoHorses:vieneUtilizzatoPer rdf:resource="http://www.semanticweb.org/annag/ontologies/2024/1/ontoHorses#TiroAgricolo"/>
        <ontoHorses:èAdattoPer rdf:resource="http://www.semanticweb.org/annag/ontologies/2024/1/ontoHorses#CavalierePrincipiante"/>
        <ontoHorses:èPossedutoDa rdf:resource="http://www.semanticweb.org/annag/ontologies/2024/1/ontoHorses#claudioCavallo"/>
        <ontoHorses:èScuderizzatoIn rdf:resource="http://www.semanticweb.org/annag/ontologies/2024/1/ontoHorses#Italia"/>
        <ontoHorses:èScuderizzatoIn rdf:resource="http://www.semanticweb.org/annag/ontologies/2024/1/ontoHorses#Sicilia"/>
        <ontoHorses:èScuderizzatoInCittàDi rdf:resource="http://www.semanticweb.org/annag/ontologies/2024/1/ontoHorses#siracusa"/>
        <ontoHorses:altezzaGarrese rdf:datatype="http://www.w3.org/2001/XMLSchema#integer">150</ontoHorses:altezzaGarrese>
        <ontoHorses:eta rdf:datatype="http://www.w3.org/2001/XMLSchema#integer">18</ontoHorses:eta>
        <ontoHorses:haSesso>femmina</ontoHorses:haSesso>
        <ontoHorses:nomeCavallo>Carmen</ontoHorses:nomeCavallo>
        <schema:image rdf:resource="https://www.equirodi.it/images/annonces/xl/857985_1711659932_3839.jpg"/>
        <rdfs:comment xml:lang="en">18 year old Breton female specimen for sale ideal for agricultural work. Good temper</rdfs:comment>
        <rdfs:comment xml:lang="it">Esemplare di femmina bretone di 18 anni in vendita ideale per lavori agricoli. Buon carattere.</rdfs:comment>
        <rdfs:label xml:lang="en">Female breton horse</rdfs:label>
        <rdfs:label xml:lang="it">Femmina bretone</rdfs:label>
    </owl:NamedIndividual>
    


    <!-- http://www.semanticweb.org/annag/ontologies/2024/1/ontoHorses#FemminaMaremmano -->

    <owl:NamedIndividual rdf:about="http://www.semanticweb.org/annag/ontologies/2024/1/ontoHorses#FemminaMaremmano">
        <rdf:type rdf:resource="http://dbpedia.org/ontology/horse"/>
        <rdf:type rdf:resource="http://www.semanticweb.org/annag/ontologies/2024/1/ontoHorses#Cavallo"/>
        <rdf:type rdf:resource="http://www.semanticweb.org/annag/ontologies/2024/1/ontoHorses#CavalloASangueFreddo"/>
        <rdf:type rdf:resource="http://www.semanticweb.org/annag/ontologies/2024/1/ontoHorses#CavalloAnziano"/>
        <rdf:type rdf:resource="http://www.semanticweb.org/annag/ontologies/2024/1/ontoHorses#CavalloDaEquiturismo"/>
        <rdf:type rdf:resource="http://www.semanticweb.org/annag/ontologies/2024/1/ontoHorses#CavalloDaLavoro"/>
        <rdf:type rdf:resource="http://www.semanticweb.org/annag/ontologies/2024/1/ontoHorses#CavalloDaSella"/>
        <rdf:type rdf:resource="http://www.semanticweb.org/annag/ontologies/2024/1/ontoHorses#CavalloDaTrainoCarrozze"/>
        <rdf:type rdf:resource="http://www.semanticweb.org/annag/ontologies/2024/1/ontoHorses#CavalloFemmina"/>
        <price:hasPrice rdf:resource="http://www.semanticweb.org/annag/ontologies/2024/1/ontoHorses#5000Euro"/>
        <ontoHorses:haRazza rdf:resource="http://www.semanticweb.org/annag/ontologies/2024/1/ontoHorses#Maremmano"/>
        <ontoHorses:vieneUtilizzatoPer rdf:resource="http://www.semanticweb.org/annag/ontologies/2024/1/ontoHorses#Equiturismo"/>
        <ontoHorses:vieneUtilizzatoPer rdf:resource="http://www.semanticweb.org/annag/ontologies/2024/1/ontoHorses#TrainoCarrozze"/>
        <ontoHorses:èAdattoPer rdf:resource="http://www.semanticweb.org/annag/ontologies/2024/1/ontoHorses#CavalierePrincipiante"/>
        <ontoHorses:èPossedutoDa rdf:resource="http://www.semanticweb.org/annag/ontologies/2024/1/ontoHorses#claudioCavallo"/>
        <ontoHorses:èScuderizzatoIn rdf:resource="http://www.semanticweb.org/annag/ontologies/2024/1/ontoHorses#Italia"/>
        <ontoHorses:èScuderizzatoIn rdf:resource="http://www.semanticweb.org/annag/ontologies/2024/1/ontoHorses#Sicilia"/>
        <ontoHorses:èScuderizzatoInCittàDi rdf:resource="http://www.semanticweb.org/annag/ontologies/2024/1/ontoHorses#siracusa"/>
        <ontoHorses:altezzaGarrese rdf:datatype="http://www.w3.org/2001/XMLSchema#integer">162</ontoHorses:altezzaGarrese>
        <ontoHorses:eta rdf:datatype="http://www.w3.org/2001/XMLSchema#integer">20</ontoHorses:eta>
        <ontoHorses:haSesso>femmina</ontoHorses:haSesso>
        <ontoHorses:nomeCavallo>Penelope</ontoHorses:nomeCavallo>
        <schema:image rdf:resource="http://www.anamcavallomaremmano.com/typo3temp/pics/d887dddef7.jpg"/>
        <rdfs:comment xml:lang="it">Esemplare di femmina maremmano in vendita. Anno 2004. Adatto a tutti. Facile gestione anche in passeggiata</rdfs:comment>
        <rdfs:comment xml:lang="en">Female Maremma for sale. Suitable for everyone. Year 2004. Easy management even when walking</rdfs:comment>
        <rdfs:label xml:lang="en">Female maremmano horse</rdfs:label>
        <rdfs:label xml:lang="it">Femmina maremmano</rdfs:label>
    </owl:NamedIndividual>
    


    <!-- http://www.semanticweb.org/annag/ontologies/2024/1/ontoHorses#FemminaMurgese -->

    <owl:NamedIndividual rdf:about="http://www.semanticweb.org/annag/ontologies/2024/1/ontoHorses#FemminaMurgese">
        <rdf:type rdf:resource="http://dbpedia.org/ontology/horse"/>
        <rdf:type rdf:resource="http://www.semanticweb.org/annag/ontologies/2024/1/ontoHorses#Cavallo"/>
        <rdf:type rdf:resource="http://www.semanticweb.org/annag/ontologies/2024/1/ontoHorses#CavalloASangueCaldo"/>
        <rdf:type rdf:resource="http://www.semanticweb.org/annag/ontologies/2024/1/ontoHorses#CavalloDaEquiturismo"/>
        <rdf:type rdf:resource="http://www.semanticweb.org/annag/ontologies/2024/1/ontoHorses#CavalloDaSella"/>
        <rdf:type rdf:resource="http://www.semanticweb.org/annag/ontologies/2024/1/ontoHorses#CavalloFemmina"/>
        <rdf:type rdf:resource="http://www.semanticweb.org/annag/ontologies/2024/1/ontoHorses#CavalloPerDressage"/>
        <rdf:type rdf:resource="http://www.semanticweb.org/annag/ontologies/2024/1/ontoHorses#CavalloSportivo"/>
        <rdf:type rdf:resource="http://www.semanticweb.org/annag/ontologies/2024/1/ontoHorses#Puledro"/>
        <price:hasPrice rdf:resource="http://www.semanticweb.org/annag/ontologies/2024/1/ontoHorses#4800Euro"/>
        <ontoHorses:adattoAlConseguimentoDi rdf:resource="http://www.semanticweb.org/annag/ontologies/2024/1/ontoHorses#brevetto"/>
        <ontoHorses:gareggiaNellaCategoriaDiDressage rdf:resource="http://www.semanticweb.org/annag/ontologies/2024/1/ontoHorses#D"/>
        <ontoHorses:gareggiaNelleCategorieDiSalto rdf:resource="http://www.semanticweb.org/annag/ontologies/2024/1/ontoHorses#C80"/>
        <ontoHorses:haRazza rdf:resource="http://www.semanticweb.org/annag/ontologies/2024/1/ontoHorses#Murgese"/>
        <ontoHorses:vieneUtilizzatoPer rdf:resource="http://www.semanticweb.org/annag/ontologies/2024/1/ontoHorses#Dressage"/>
        <ontoHorses:vieneUtilizzatoPer rdf:resource="http://www.semanticweb.org/annag/ontologies/2024/1/ontoHorses#Equiturismo"/>
        <ontoHorses:vieneUtilizzatoPer rdf:resource="http://www.semanticweb.org/annag/ontologies/2024/1/ontoHorses#SaltoAdOstacoli"/>
        <ontoHorses:èAdattoPer rdf:resource="http://www.semanticweb.org/annag/ontologies/2024/1/ontoHorses#CavalierePrincipiante"/>
        <ontoHorses:èPossedutoDa rdf:resource="http://www.semanticweb.org/annag/ontologies/2024/1/ontoHorses#paoloGrassi"/>
        <ontoHorses:èScuderizzatoIn rdf:resource="http://www.semanticweb.org/annag/ontologies/2024/1/ontoHorses#Italia"/>
        <ontoHorses:èScuderizzatoIn rdf:resource="http://www.semanticweb.org/annag/ontologies/2024/1/ontoHorses#Puglia"/>
        <ontoHorses:èScuderizzatoInCittàDi rdf:resource="http://www.semanticweb.org/annag/ontologies/2024/1/ontoHorses#taranto"/>
        <ontoHorses:altezzaGarrese rdf:datatype="http://www.w3.org/2001/XMLSchema#integer">158</ontoHorses:altezzaGarrese>
        <ontoHorses:eta rdf:datatype="http://www.w3.org/2001/XMLSchema#integer">4</ontoHorses:eta>
        <ontoHorses:haSesso>femmina</ontoHorses:haSesso>
        <ontoHorses:nomeCavallo>Queen</ontoHorses:nomeCavallo>
        <schema:image rdf:resource="https://www.equirodi.it/images/annonces/xl/855775_1710607148_7462.jpg"/>
        <rdfs:comment xml:lang="en">4 year old Murgese female for sale. Excellent for dressage and show jumping up to patent category. Very easy management on the go and in the box. Suitable for beginners.</rdfs:comment>
        <rdfs:comment xml:lang="it">Esemplare di femmina murgese di 4 anni in vendita. Ottima per dressage e salto ad ostacoli fino a categoria brevetto. Facilissima gestione in passeggiata e in box. Adatta a principianti.</rdfs:comment>
        <rdfs:label xml:lang="en">Female murgese</rdfs:label>
        <rdfs:label xml:lang="it">Femmina murgese</rdfs:label>
    </owl:NamedIndividual>
    


    <!-- http://www.semanticweb.org/annag/ontologies/2024/1/ontoHorses#Francia -->

    <owl:NamedIndividual rdf:about="http://www.semanticweb.org/annag/ontologies/2024/1/ontoHorses#Francia">
        <rdf:type rdf:resource="http://schema.org/Place"/>
        <rdf:type rdf:resource="http://www.semanticweb.org/annag/ontologies/2024/1/ontoHorses#AreaGeografica"/>
        <partof:hasPart rdf:resource="http://www.semanticweb.org/annag/ontologies/2024/1/ontoHorses#Bretagna"/>
        <partof:hasPart rdf:resource="http://www.semanticweb.org/annag/ontologies/2024/1/ontoHorses#Normandia"/>
        <partof:hasPart rdf:resource="http://www.semanticweb.org/annag/ontologies/2024/1/ontoHorses#Perche"/>
        <partof:hasPart rdf:resource="http://www.semanticweb.org/annag/ontologies/2024/1/ontoHorses#RegioneBoullonnais"/>
        <schema:image rdf:resource="https://upload.wikimedia.org/wikipedia/commons/thumb/9/93/Flag_of_France_%281794%E2%80%931815%2C_1830%E2%80%931974%29.svg/1280px-Flag_of_France_%281794%E2%80%931815%2C_1830%E2%80%931974%29.svg.png"/>
        <rdfs:comment xml:lang="en">France, officially the French Republic, is a state located in Western Europe and Southern Europe, but which also has territories spread across multiple oceans and other continents.</rdfs:comment>
        <rdfs:comment xml:lang="it">La Francia,  ufficialmente Repubblica francese, è uno Stato situato nell&apos;Europa occidentale e nell&apos;Europa meridionale, ma che possiede ugualmente territori disseminati su più oceani e altri continenti.</rdfs:comment>
        <rdfs:label xml:lang="en">France</rdfs:label>
        <rdfs:label xml:lang="it">Francia</rdfs:label>
    </owl:NamedIndividual>
    


    <!-- http://www.semanticweb.org/annag/ontologies/2024/1/ontoHorses#Frisia -->

    <owl:NamedIndividual rdf:about="http://www.semanticweb.org/annag/ontologies/2024/1/ontoHorses#Frisia">
        <rdf:type rdf:resource="http://schema.org/Place"/>
        <rdf:type rdf:resource="http://www.semanticweb.org/annag/ontologies/2024/1/ontoHorses#AreaGeografica"/>
        <partof:isPartOf rdf:resource="http://www.semanticweb.org/annag/ontologies/2024/1/ontoHorses#PaesiBassi"/>
        <rdfs:comment xml:lang="en">Friesland is a province of the Netherlands</rdfs:comment>
        <rdfs:comment xml:lang="it">La Frisia è una provincia dei Paesi Bassi</rdfs:comment>
        <rdfs:label xml:lang="en">Friesland</rdfs:label>
        <rdfs:label xml:lang="it">Frisia</rdfs:label>
    </owl:NamedIndividual>
    


    <!-- http://www.semanticweb.org/annag/ontologies/2024/1/ontoHorses#Frisone -->

    <owl:NamedIndividual rdf:about="http://www.semanticweb.org/annag/ontologies/2024/1/ontoHorses#Frisone">
        <rdf:type rdf:resource="http://www.semanticweb.org/annag/ontologies/2024/1/ontoHorses#RazzaASangueFreddo"/>
        <rdf:type rdf:resource="http://www.semanticweb.org/annag/ontologies/2024/1/ontoHorses#RazzaCavallo"/>
        <rdf:type rdf:resource="http://www.semanticweb.org/annag/ontologies/2024/1/ontoHorses#RazzaDaDressage"/>
        <rdf:type rdf:resource="http://www.semanticweb.org/annag/ontologies/2024/1/ontoHorses#RazzaDaLavoro"/>
        <rdf:type rdf:resource="http://www.semanticweb.org/annag/ontologies/2024/1/ontoHorses#RazzaDaSella"/>
        <rdf:type rdf:resource="http://www.semanticweb.org/annag/ontologies/2024/1/ontoHorses#RazzaMesoBrachimorfa"/>
        <rdf:type rdf:resource="http://www.semanticweb.org/annag/ontologies/2024/1/ontoHorses#RazzaSportiva"/>
        <ontoHorses:entitàWikidata rdf:resource="http://www.wikidata.org/entity/Q388952"/>
        <ontoHorses:haClassificazioneMorfologica rdf:resource="http://www.semanticweb.org/annag/ontologies/2024/1/ontoHorses#mesoBrachimorfo"/>
        <ontoHorses:haIndole rdf:resource="http://www.semanticweb.org/annag/ontologies/2024/1/ontoHorses#sangueFreddo"/>
        <ontoHorses:haNazionalità rdf:resource="http://www.semanticweb.org/annag/ontologies/2024/1/ontoHorses#PaesiBassi"/>
        <ontoHorses:haRegioneDiOrigine rdf:resource="http://www.semanticweb.org/annag/ontologies/2024/1/ontoHorses#Frisia"/>
        <ontoHorses:puòEssereImpiegataIn rdf:resource="http://www.semanticweb.org/annag/ontologies/2024/1/ontoHorses#Dressage"/>
        <ontoHorses:puòEssereImpiegataIn rdf:resource="http://www.semanticweb.org/annag/ontologies/2024/1/ontoHorses#TrainoCarrozze"/>
        <ontoHorses:altezzaMediaGarrese rdf:datatype="http://www.w3.org/2001/XMLSchema#integer">160</ontoHorses:altezzaMediaGarrese>
        <ontoHorses:haColoreMantello>morello</ontoHorses:haColoreMantello>
        <ontoHorses:pesoMedio rdf:datatype="http://www.w3.org/2001/XMLSchema#integer">525</ontoHorses:pesoMedio>
        <schema:image rdf:resource="https://upload.wikimedia.org/wikipedia/commons/thumb/7/7c/Friese.jpg/220px-Friese.jpg"/>
        <rdfs:comment xml:lang="it">Il Frisone occidentale è originario della Frisia ed è una razza di cavallo robusto, possente e infaticabile, utilizzato in passato, soprattutto durante il Medioevo, come cavallo da guerra. Oggi è particolarmente apprezzato nel dressage e negli attacchi.</rdfs:comment>
        <rdfs:comment xml:lang="en">The West Friesian originates from Friesland and is a robust, powerful and tireless breed of horse, used in the past, especially during the Middle Ages, as a war horse. Today it is particularly appreciated in dressage and driving.</rdfs:comment>
        <skos:exactMatch xml:lang="it">http://www.wikidata.org/entity/Q388952</skos:exactMatch>
        <skos:prefLabel xml:lang="en">Friesian horse</skos:prefLabel>
        <skos:prefLabel xml:lang="it">Frisone</skos:prefLabel>
    </owl:NamedIndividual>
    


    <!-- http://www.semanticweb.org/annag/ontologies/2024/1/ontoHorses#Germania -->

    <owl:NamedIndividual rdf:about="http://www.semanticweb.org/annag/ontologies/2024/1/ontoHorses#Germania">
        <rdf:type rdf:resource="http://schema.org/Place"/>
        <rdf:type rdf:resource="http://www.semanticweb.org/annag/ontologies/2024/1/ontoHorses#AreaGeografica"/>
        <partof:hasPart rdf:resource="http://www.semanticweb.org/annag/ontologies/2024/1/ontoHorses#RegioneHannover"/>
        <partof:hasPart rdf:resource="http://www.semanticweb.org/annag/ontologies/2024/1/ontoHorses#Schleswig-Holstein"/>
        <partof:hasPart rdf:resource="http://www.semanticweb.org/annag/ontologies/2024/1/ontoHorses#Vestfalia"/>
        <schema:image rdf:resource="https://upload.wikimedia.org/wikipedia/en/thumb/b/ba/Flag_of_Germany.svg/1920px-Flag_of_Germany.svg.png"/>
        <rdfs:comment xml:lang="en">Germany, officially the Federal Republic of Germany, is a member state of the European Union located in central-western Europe.</rdfs:comment>
        <rdfs:comment xml:lang="it">La Germania, ufficialmente Repubblica Federale di Germania, è uno Stato membro dell&apos;Unione europea situato nell&apos;Europa centro-occidentale.</rdfs:comment>
        <rdfs:label xml:lang="it">Germania</rdfs:label>
        <rdfs:label xml:lang="en">Germany</rdfs:label>
    </owl:NamedIndividual>
    


    <!-- http://www.semanticweb.org/annag/ontologies/2024/1/ontoHorses#Hannover -->

    <owl:NamedIndividual rdf:about="http://www.semanticweb.org/annag/ontologies/2024/1/ontoHorses#Hannover">
        <rdf:type rdf:resource="http://www.semanticweb.org/annag/ontologies/2024/1/ontoHorses#RazzaASangueCaldo"/>
        <rdf:type rdf:resource="http://www.semanticweb.org/annag/ontologies/2024/1/ontoHorses#RazzaCavallo"/>
        <rdf:type rdf:resource="http://www.semanticweb.org/annag/ontologies/2024/1/ontoHorses#RazzaDaDressage"/>
        <rdf:type rdf:resource="http://www.semanticweb.org/annag/ontologies/2024/1/ontoHorses#RazzaDaSaltoOstacoli"/>
        <rdf:type rdf:resource="http://www.semanticweb.org/annag/ontologies/2024/1/ontoHorses#RazzaDaSella"/>
        <rdf:type rdf:resource="http://www.semanticweb.org/annag/ontologies/2024/1/ontoHorses#RazzaSportiva"/>
        <rdf:type rdf:resource="http://www.semanticweb.org/annag/ontologies/2024/1/ontoHorses#RazzamMesomorfa"/>
        <ontoHorses:entitàWikidata rdf:resource="http://www.wikidata.org/entity/Q1501738"/>
        <ontoHorses:haClassificazioneMorfologica rdf:resource="http://www.semanticweb.org/annag/ontologies/2024/1/ontoHorses#mesomorfo"/>
        <ontoHorses:haIndole rdf:resource="http://www.semanticweb.org/annag/ontologies/2024/1/ontoHorses#sangueCaldo"/>
        <ontoHorses:haNazionalità rdf:resource="http://www.semanticweb.org/annag/ontologies/2024/1/ontoHorses#Germania"/>
        <ontoHorses:haRegioneDiOrigine rdf:resource="http://www.semanticweb.org/annag/ontologies/2024/1/ontoHorses#RegioneHannover"/>
        <ontoHorses:puòEssereImpiegataIn rdf:resource="http://www.semanticweb.org/annag/ontologies/2024/1/ontoHorses#Dressage"/>
        <ontoHorses:puòEssereImpiegataIn rdf:resource="http://www.semanticweb.org/annag/ontologies/2024/1/ontoHorses#SaltoAdOstacoli"/>
        <ontoHorses:altezzaMediaGarrese rdf:datatype="http://www.w3.org/2001/XMLSchema#integer">168</ontoHorses:altezzaMediaGarrese>
        <ontoHorses:haColoreMantello>baio</ontoHorses:haColoreMantello>
        <ontoHorses:haColoreMantello>grigio</ontoHorses:haColoreMantello>
        <ontoHorses:haColoreMantello>morello</ontoHorses:haColoreMantello>
        <ontoHorses:haColoreMantello>sauro</ontoHorses:haColoreMantello>
        <ontoHorses:pesoMedio rdf:datatype="http://www.w3.org/2001/XMLSchema#integer">575</ontoHorses:pesoMedio>
        <schema:image rdf:resource="https://upload.wikimedia.org/wikipedia/commons/thumb/c/cc/RCMP_Farm_Hannoverian2.jpg/240px-RCMP_Farm_Hannoverian2.jpg"/>
        <rdfs:comment xml:lang="it">L&apos; Hannover è una razza di cavallo a sangue caldo, originaria della Germania, più precisamente della regione di Hannover</rdfs:comment>
        <rdfs:comment xml:lang="en">The Hanoverian is a breed of warm-blooded horse, originating from Germany, more precisely from the Hanover region</rdfs:comment>
        <skos:exactMatch xml:lang="it">http://www.wikidata.org/entity/Q1501738</skos:exactMatch>
        <skos:prefLabel xml:lang="it">Hannover</skos:prefLabel>
        <skos:prefLabel xml:lang="en">Hanoverian horse</skos:prefLabel>
    </owl:NamedIndividual>
    


    <!-- http://www.semanticweb.org/annag/ontologies/2024/1/ontoHorses#Holstein -->

    <owl:NamedIndividual rdf:about="http://www.semanticweb.org/annag/ontologies/2024/1/ontoHorses#Holstein">
        <rdf:type rdf:resource="http://www.semanticweb.org/annag/ontologies/2024/1/ontoHorses#RazzaASangueMisto"/>
        <rdf:type rdf:resource="http://www.semanticweb.org/annag/ontologies/2024/1/ontoHorses#RazzaCavallo"/>
        <rdf:type rdf:resource="http://www.semanticweb.org/annag/ontologies/2024/1/ontoHorses#RazzaDaDressage"/>
        <rdf:type rdf:resource="http://www.semanticweb.org/annag/ontologies/2024/1/ontoHorses#RazzaDaSaltoOstacoli"/>
        <rdf:type rdf:resource="http://www.semanticweb.org/annag/ontologies/2024/1/ontoHorses#RazzaDaSella"/>
        <rdf:type rdf:resource="http://www.semanticweb.org/annag/ontologies/2024/1/ontoHorses#RazzaSportiva"/>
        <rdf:type rdf:resource="http://www.semanticweb.org/annag/ontologies/2024/1/ontoHorses#RazzamMesomorfa"/>
        <ontoHorses:entitàWikidata rdf:resource="http://www.wikidata.org/entity/Q571149"/>
        <ontoHorses:haClassificazioneMorfologica rdf:resource="http://www.semanticweb.org/annag/ontologies/2024/1/ontoHorses#mesomorfo"/>
        <ontoHorses:haIndole rdf:resource="http://www.semanticweb.org/annag/ontologies/2024/1/ontoHorses#sangueMisto"/>
        <ontoHorses:haNazionalità rdf:resource="http://www.semanticweb.org/annag/ontologies/2024/1/ontoHorses#Germania"/>
        <ontoHorses:haRegioneDiOrigine rdf:resource="http://www.semanticweb.org/annag/ontologies/2024/1/ontoHorses#Schleswig-Holstein"/>
        <ontoHorses:puòEssereImpiegataIn rdf:resource="http://www.semanticweb.org/annag/ontologies/2024/1/ontoHorses#Dressage"/>
        <ontoHorses:puòEssereImpiegataIn rdf:resource="http://www.semanticweb.org/annag/ontologies/2024/1/ontoHorses#SaltoAdOstacoli"/>
        <ontoHorses:altezzaMediaGarrese rdf:datatype="http://www.w3.org/2001/XMLSchema#integer">168</ontoHorses:altezzaMediaGarrese>
        <ontoHorses:haColoreMantello>baio</ontoHorses:haColoreMantello>
        <ontoHorses:haColoreMantello>grigio</ontoHorses:haColoreMantello>
        <ontoHorses:haColoreMantello>morello</ontoHorses:haColoreMantello>
        <ontoHorses:haColoreMantello>sauro</ontoHorses:haColoreMantello>
        <ontoHorses:pesoMedio rdf:datatype="http://www.w3.org/2001/XMLSchema#integer">575</ontoHorses:pesoMedio>
        <schema:image rdf:resource="https://upload.wikimedia.org/wikipedia/commons/thumb/e/ea/Holstein_cavallo.jpg/192px-Holstein_cavallo.jpg"/>
        <rdfs:comment xml:lang="it">L&apos;Holstein è una razza che nasce dall&apos;idea di incrociare il cavallo agricolo tedesco nativo della regione Schleswing-Holstein con i purosangue per creare all&apos;inizio un cavallo da tiro leggero e successivamente un cavallo da sella adatto alle attività sportive</rdfs:comment>
        <rdfs:comment xml:lang="en">The Holstein is a breed that was born from the idea of crossing the German agricultural horse native to the Schleswing-Holstein region with thoroughbreds to initially create a light draft horse and subsequently a saddle horse suitable for sporting activities</rdfs:comment>
        <skos:exactMatch xml:lang="it">http://www.wikidata.org/entity/Q571149</skos:exactMatch>
        <skos:prefLabel xml:lang="it">Holstein</skos:prefLabel>
        <skos:prefLabel xml:lang="en">Holsteiner</skos:prefLabel>
    </owl:NamedIndividual>
    


    <!-- http://www.semanticweb.org/annag/ontologies/2024/1/ontoHorses#IrishSportHorse -->

    <owl:NamedIndividual rdf:about="http://www.semanticweb.org/annag/ontologies/2024/1/ontoHorses#IrishSportHorse">
        <rdf:type rdf:resource="http://www.semanticweb.org/annag/ontologies/2024/1/ontoHorses#RazzaASangueCaldo"/>
        <rdf:type rdf:resource="http://www.semanticweb.org/annag/ontologies/2024/1/ontoHorses#RazzaCavallo"/>
        <rdf:type rdf:resource="http://www.semanticweb.org/annag/ontologies/2024/1/ontoHorses#RazzaDaDressage"/>
        <rdf:type rdf:resource="http://www.semanticweb.org/annag/ontologies/2024/1/ontoHorses#RazzaDaEventing"/>
        <rdf:type rdf:resource="http://www.semanticweb.org/annag/ontologies/2024/1/ontoHorses#RazzaDaSaltoOstacoli"/>
        <rdf:type rdf:resource="http://www.semanticweb.org/annag/ontologies/2024/1/ontoHorses#RazzaDaSella"/>
        <rdf:type rdf:resource="http://www.semanticweb.org/annag/ontologies/2024/1/ontoHorses#RazzaSportiva"/>
        <rdf:type rdf:resource="http://www.semanticweb.org/annag/ontologies/2024/1/ontoHorses#RazzamMesomorfa"/>
        <ontoHorses:entitàWikidata rdf:resource="http://www.wikidata.org/entity/Q1665430"/>
        <ontoHorses:haClassificazioneMorfologica rdf:resource="http://www.semanticweb.org/annag/ontologies/2024/1/ontoHorses#mesomorfo"/>
        <ontoHorses:haIndole rdf:resource="http://www.semanticweb.org/annag/ontologies/2024/1/ontoHorses#sangueCaldo"/>
        <ontoHorses:haNazionalità rdf:resource="http://www.semanticweb.org/annag/ontologies/2024/1/ontoHorses#Irlanda"/>
        <ontoHorses:puòEssereImpiegataIn rdf:resource="http://www.semanticweb.org/annag/ontologies/2024/1/ontoHorses#Dressage"/>
        <ontoHorses:puòEssereImpiegataIn rdf:resource="http://www.semanticweb.org/annag/ontologies/2024/1/ontoHorses#Eventing"/>
        <ontoHorses:puòEssereImpiegataIn rdf:resource="http://www.semanticweb.org/annag/ontologies/2024/1/ontoHorses#SaltoAdOstacoli"/>
        <ontoHorses:altezzaMediaGarrese rdf:datatype="http://www.w3.org/2001/XMLSchema#integer">163</ontoHorses:altezzaMediaGarrese>
        <ontoHorses:haColoreMantello>baio</ontoHorses:haColoreMantello>
        <ontoHorses:haColoreMantello>crema</ontoHorses:haColoreMantello>
        <ontoHorses:haColoreMantello>grigio</ontoHorses:haColoreMantello>
        <ontoHorses:haColoreMantello>morello</ontoHorses:haColoreMantello>
        <ontoHorses:haColoreMantello>sauro</ontoHorses:haColoreMantello>
        <ontoHorses:pesoMedio rdf:datatype="http://www.w3.org/2001/XMLSchema#integer">600</ontoHorses:pesoMedio>
        <schema:image rdf:resource="https://upload.wikimedia.org/wikipedia/commons/thumb/e/ea/Irish_Sport_Horse_foal_and_mare.jpg/220px-Irish_Sport_Horse_foal_and_mare.jpg"/>
        <rdfs:comment xml:lang="it">L&apos;Irish Sport Horse (ISH), o Irish Hunter, è una razza irlandese di cavalli sportivi a sangue caldo, utilizzata principalmente per dressage, completo e salto ostacoli</rdfs:comment>
        <rdfs:comment xml:lang="en">The Irish Sport Horse (ISH), or Irish Hunter, is an Irish breed of warmblood sport horse, used primarily for dressage, eventing, and show jumping</rdfs:comment>
        <skos:exactMatch xml:lang="it">http://www.wikidata.org/entity/Q1665430</skos:exactMatch>
        <skos:prefLabel xml:lang="en">Irish Sport Horse</skos:prefLabel>
        <skos:prefLabel xml:lang="it">Irish Sport Horse</skos:prefLabel>
    </owl:NamedIndividual>
    


    <!-- http://www.semanticweb.org/annag/ontologies/2024/1/ontoHorses#Irlanda -->

    <owl:NamedIndividual rdf:about="http://www.semanticweb.org/annag/ontologies/2024/1/ontoHorses#Irlanda">
        <rdf:type rdf:resource="http://schema.org/Place"/>
        <rdf:type rdf:resource="http://www.semanticweb.org/annag/ontologies/2024/1/ontoHorses#AreaGeografica"/>
        <schema:image rdf:resource="https://upload.wikimedia.org/wikipedia/commons/thumb/4/45/Flag_of_Ireland.svg/1920px-Flag_of_Ireland.svg.png"/>
        <rdfs:comment xml:lang="en">Ireland, officially the Republic of Ireland, is a member country of the European Union.</rdfs:comment>
        <rdfs:comment xml:lang="it">L&apos;Irlanda, ufficialmente Repubblica d&apos;Irlanda, è un Paese membro dell&apos;Unione europea.</rdfs:comment>
        <rdfs:label xml:lang="it">Irlanda</rdfs:label>
        <rdfs:label xml:lang="en">Republic of Ireland</rdfs:label>
    </owl:NamedIndividual>
    


    <!-- http://www.semanticweb.org/annag/ontologies/2024/1/ontoHorses#Italia -->

    <owl:NamedIndividual rdf:about="http://www.semanticweb.org/annag/ontologies/2024/1/ontoHorses#Italia">
        <rdf:type rdf:resource="http://schema.org/Place"/>
        <rdf:type rdf:resource="http://www.semanticweb.org/annag/ontologies/2024/1/ontoHorses#AreaGeografica"/>
        <partof:hasPart rdf:resource="http://www.semanticweb.org/annag/ontologies/2024/1/ontoHorses#AppenninoToscoEmiliano"/>
        <partof:hasPart rdf:resource="http://www.semanticweb.org/annag/ontologies/2024/1/ontoHorses#Lombardia"/>
        <partof:hasPart rdf:resource="http://www.semanticweb.org/annag/ontologies/2024/1/ontoHorses#Maremma"/>
        <partof:hasPart rdf:resource="http://www.semanticweb.org/annag/ontologies/2024/1/ontoHorses#Murge"/>
        <partof:hasPart rdf:resource="http://www.semanticweb.org/annag/ontologies/2024/1/ontoHorses#Piemonte"/>
        <partof:hasPart rdf:resource="http://www.semanticweb.org/annag/ontologies/2024/1/ontoHorses#Puglia"/>
        <partof:hasPart rdf:resource="http://www.semanticweb.org/annag/ontologies/2024/1/ontoHorses#Sicilia"/>
        <partof:hasPart rdf:resource="http://www.semanticweb.org/annag/ontologies/2024/1/ontoHorses#TrentinoAltoAdige"/>
        <partof:hasPart rdf:resource="http://www.semanticweb.org/annag/ontologies/2024/1/ontoHorses#bergamo"/>
        <partof:hasPart rdf:resource="http://www.semanticweb.org/annag/ontologies/2024/1/ontoHorses#leini"/>
        <partof:hasPart rdf:resource="http://www.semanticweb.org/annag/ontologies/2024/1/ontoHorses#sanMauro"/>
        <partof:hasPart rdf:resource="http://www.semanticweb.org/annag/ontologies/2024/1/ontoHorses#siracusa"/>
        <partof:hasPart rdf:resource="http://www.semanticweb.org/annag/ontologies/2024/1/ontoHorses#taranto"/>
        <schema:image rdf:resource="https://upload.wikimedia.org/wikipedia/commons/thumb/0/03/Flag_of_Italy.svg/1280px-Flag_of_Italy.svg.png"/>
        <rdfs:comment xml:lang="en">Italy, officially the Italian Republic, is a member state of the European Union, located in southern and western Europe, whose territory largely coincides with the geographical region of the same name.</rdfs:comment>
        <rdfs:comment xml:lang="it">L&apos;Italia, ufficialmente Repubblica Italiana, è uno Stato membro dell&apos;Unione europea, situato nell&apos;Europa meridionale e occidentale, il cui territorio coincide in gran parte con l&apos;omonima regione geografica.</rdfs:comment>
        <rdfs:label xml:lang="it">Italia</rdfs:label>
        <rdfs:label xml:lang="en">Italy</rdfs:label>
    </owl:NamedIndividual>
    


    <!-- http://www.semanticweb.org/annag/ontologies/2024/1/ontoHorses#Jutland -->

    <owl:NamedIndividual rdf:about="http://www.semanticweb.org/annag/ontologies/2024/1/ontoHorses#Jutland">
        <rdf:type rdf:resource="http://schema.org/Place"/>
        <rdf:type rdf:resource="http://www.semanticweb.org/annag/ontologies/2024/1/ontoHorses#AreaGeografica"/>
        <partof:isPartOf rdf:resource="http://www.semanticweb.org/annag/ontologies/2024/1/ontoHorses#Danimarca"/>
        <rdfs:comment xml:lang="en">Jutland is a peninsula in northern Europe divided between Germany, to the south, and Denmark, of which it constitutes the peninsular part.</rdfs:comment>
        <rdfs:comment xml:lang="it">Lo Jutland è una penisola del nord Europa divisa tra Germania, a sud, e Danimarca, di cui costituisce la parte peninsulare.</rdfs:comment>
        <rdfs:label xml:lang="en">Jutland</rdfs:label>
        <rdfs:label xml:lang="it">Jutland</rdfs:label>
    </owl:NamedIndividual>
    


    <!-- http://www.semanticweb.org/annag/ontologies/2024/1/ontoHorses#Lipizzano -->

    <owl:NamedIndividual rdf:about="http://www.semanticweb.org/annag/ontologies/2024/1/ontoHorses#Lipizzano">
        <rdf:type rdf:resource="http://www.semanticweb.org/annag/ontologies/2024/1/ontoHorses#RazzaASangueMisto"/>
        <rdf:type rdf:resource="http://www.semanticweb.org/annag/ontologies/2024/1/ontoHorses#RazzaCavallo"/>
        <rdf:type rdf:resource="http://www.semanticweb.org/annag/ontologies/2024/1/ontoHorses#RazzaDaAltaScuola"/>
        <rdf:type rdf:resource="http://www.semanticweb.org/annag/ontologies/2024/1/ontoHorses#RazzaDaDressage"/>
        <rdf:type rdf:resource="http://www.semanticweb.org/annag/ontologies/2024/1/ontoHorses#RazzaDaLavoro"/>
        <rdf:type rdf:resource="http://www.semanticweb.org/annag/ontologies/2024/1/ontoHorses#RazzaDaSella"/>
        <rdf:type rdf:resource="http://www.semanticweb.org/annag/ontologies/2024/1/ontoHorses#RazzaDaTiroAgricolo"/>
        <rdf:type rdf:resource="http://www.semanticweb.org/annag/ontologies/2024/1/ontoHorses#RazzaMesoDolicomorfa"/>
        <rdf:type rdf:resource="http://www.semanticweb.org/annag/ontologies/2024/1/ontoHorses#RazzaSportiva"/>
        <ontoHorses:entitàWikidata rdf:resource="http://www.wikidata.org/entity/Q217671"/>
        <ontoHorses:haClassificazioneMorfologica rdf:resource="http://www.semanticweb.org/annag/ontologies/2024/1/ontoHorses#mesoDolicomorfo"/>
        <ontoHorses:haIndole rdf:resource="http://www.semanticweb.org/annag/ontologies/2024/1/ontoHorses#sangueMisto"/>
        <ontoHorses:haNazionalità rdf:resource="http://www.semanticweb.org/annag/ontologies/2024/1/ontoHorses#Italia"/>
        <ontoHorses:haRegioneDiOrigine rdf:resource="http://www.semanticweb.org/annag/ontologies/2024/1/ontoHorses#TrentinoAltoAdige"/>
        <ontoHorses:puòEssereImpiegataIn rdf:resource="http://www.semanticweb.org/annag/ontologies/2024/1/ontoHorses#AltaScuola"/>
        <ontoHorses:puòEssereImpiegataIn rdf:resource="http://www.semanticweb.org/annag/ontologies/2024/1/ontoHorses#Dressage"/>
        <ontoHorses:puòEssereImpiegataIn rdf:resource="http://www.semanticweb.org/annag/ontologies/2024/1/ontoHorses#TiroAgricolo"/>
        <ontoHorses:altezzaMediaGarrese rdf:datatype="http://www.w3.org/2001/XMLSchema#integer">155</ontoHorses:altezzaMediaGarrese>
        <ontoHorses:haColoreMantello>baio</ontoHorses:haColoreMantello>
        <ontoHorses:haColoreMantello>grigio</ontoHorses:haColoreMantello>
        <ontoHorses:haColoreMantello>morello</ontoHorses:haColoreMantello>
        <ontoHorses:haColoreMantello>roano</ontoHorses:haColoreMantello>
        <ontoHorses:pesoMedio rdf:datatype="http://www.w3.org/2001/XMLSchema#integer">520</ontoHorses:pesoMedio>
        <schema:image rdf:resource="https://upload.wikimedia.org/wikipedia/commons/thumb/c/cb/Favory_Pallavicina.jpg/330px-Favory_Pallavicina.jpg"/>
        <rdfs:comment xml:lang="it">Il Lipizzano è una razza di cavallo che deve il suo nome alla città di Lipizza e originariamente  fu usato per trainare le carrozze dei monarchi e nell&apos;esercito</rdfs:comment>
        <rdfs:comment xml:lang="en">The Lipizzan is a breed of horse that owes its name to the city of Lipica and was originally used to pull the carriages of monarchs and in the army</rdfs:comment>
        <skos:exactMatch xml:lang="it">http://www.wikidata.org/entity/Q217671</skos:exactMatch>
        <skos:prefLabel xml:lang="en">Lipizzan</skos:prefLabel>
        <skos:prefLabel xml:lang="it">Lipizzano</skos:prefLabel>
    </owl:NamedIndividual>
    


    <!-- http://www.semanticweb.org/annag/ontologies/2024/1/ontoHorses#Lombardia -->

    <owl:NamedIndividual rdf:about="http://www.semanticweb.org/annag/ontologies/2024/1/ontoHorses#Lombardia">
        <rdf:type rdf:resource="http://schema.org/Place"/>
        <rdf:type rdf:resource="http://www.semanticweb.org/annag/ontologies/2024/1/ontoHorses#AreaGeografica"/>
        <partof:hasPart rdf:resource="http://www.semanticweb.org/annag/ontologies/2024/1/ontoHorses#bergamo"/>
        <partof:isPartOf rdf:resource="http://www.semanticweb.org/annag/ontologies/2024/1/ontoHorses#Italia"/>
        <rdfs:comment xml:lang="it">La Lombardia  è una regione italiana a statuto ordinario di 10 020 528 abitanti dell&apos;Italia nord-occidentale che ha il suo capoluogo nella città di Milano. La regione si posiziona prima in Italia per popolazione, densità abitativa e numero di enti locali, mentre è quarta per superficie, dopo Sicilia, Piemonte e Sardegna.</rdfs:comment>
        <rdfs:comment xml:lang="en">Lombardy is an Italian region with ordinary statute of 10,020,528 inhabitants in north-western Italy which has its capital in the city of Milan. The region ranks first in Italy in terms of population, population density and number of local authorities, while it is fourth in terms of surface area, after Sicily, Piedmont and Sardinia.</rdfs:comment>
        <rdfs:label xml:lang="it">Lombardia</rdfs:label>
        <rdfs:label xml:lang="en">Lombardy</rdfs:label>
    </owl:NamedIndividual>
    


    <!-- http://www.semanticweb.org/annag/ontologies/2024/1/ontoHorses#Lusitano -->

    <owl:NamedIndividual rdf:about="http://www.semanticweb.org/annag/ontologies/2024/1/ontoHorses#Lusitano">
        <rdf:type rdf:resource="http://www.semanticweb.org/annag/ontologies/2024/1/ontoHorses#RazzaASangueCaldo"/>
        <rdf:type rdf:resource="http://www.semanticweb.org/annag/ontologies/2024/1/ontoHorses#RazzaCavallo"/>
        <rdf:type rdf:resource="http://www.semanticweb.org/annag/ontologies/2024/1/ontoHorses#RazzaDaAltaScuola"/>
        <rdf:type rdf:resource="http://www.semanticweb.org/annag/ontologies/2024/1/ontoHorses#RazzaDaDressage"/>
        <rdf:type rdf:resource="http://www.semanticweb.org/annag/ontologies/2024/1/ontoHorses#RazzaDaSella"/>
        <rdf:type rdf:resource="http://www.semanticweb.org/annag/ontologies/2024/1/ontoHorses#RazzaMesoDolicomorfa"/>
        <rdf:type rdf:resource="http://www.semanticweb.org/annag/ontologies/2024/1/ontoHorses#RazzaSportiva"/>
        <ontoHorses:entitàWikidata rdf:resource="http://www.wikidata.org/entity/Q937595"/>
        <ontoHorses:haClassificazioneMorfologica rdf:resource="http://www.semanticweb.org/annag/ontologies/2024/1/ontoHorses#mesoDolicomorfo"/>
        <ontoHorses:haIndole rdf:resource="http://www.semanticweb.org/annag/ontologies/2024/1/ontoHorses#sangueCaldo"/>
        <ontoHorses:haNazionalità rdf:resource="http://www.semanticweb.org/annag/ontologies/2024/1/ontoHorses#Portogallo"/>
        <ontoHorses:puòEssereImpiegataIn rdf:resource="http://www.semanticweb.org/annag/ontologies/2024/1/ontoHorses#AltaScuola"/>
        <ontoHorses:puòEssereImpiegataIn rdf:resource="http://www.semanticweb.org/annag/ontologies/2024/1/ontoHorses#Dressage"/>
        <ontoHorses:altezzaMediaGarrese rdf:datatype="http://www.w3.org/2001/XMLSchema#integer">157</ontoHorses:altezzaMediaGarrese>
        <ontoHorses:haColoreMantello>baio</ontoHorses:haColoreMantello>
        <ontoHorses:haColoreMantello>crema</ontoHorses:haColoreMantello>
        <ontoHorses:haColoreMantello>grigio</ontoHorses:haColoreMantello>
        <ontoHorses:haColoreMantello>isabella</ontoHorses:haColoreMantello>
        <ontoHorses:haColoreMantello>palomino</ontoHorses:haColoreMantello>
        <ontoHorses:haColoreMantello>sauro</ontoHorses:haColoreMantello>
        <ontoHorses:pesoMedio rdf:datatype="http://www.w3.org/2001/XMLSchema#integer">525</ontoHorses:pesoMedio>
        <schema:image rdf:resource="https://upload.wikimedia.org/wikipedia/commons/thumb/0/00/Beja_lusitano.JPG/220px-Beja_lusitano.JPG"/>
        <rdfs:comment xml:lang="it">Il Lusitano deriva il suo nome dalla Lusitania, attuale Portogallo ed è il cavallo simbolo di questa nazione. Di origine antica, il Lusitano originariamente era allevato per essere utilizzato in guerra e nelle corride</rdfs:comment>
        <rdfs:comment xml:lang="en">The Lusitano derives its name from Lusitania, now Portugal and is the symbolic horse of this nation. Of ancient origin, the Lusitano was originally bred for use in war and bullfights</rdfs:comment>
        <skos:exactMatch xml:lang="it">http://www.wikidata.org/entity/Q937595</skos:exactMatch>
        <skos:prefLabel xml:lang="en">Lusitano</skos:prefLabel>
        <skos:prefLabel xml:lang="it">Lusitano</skos:prefLabel>
    </owl:NamedIndividual>
    


    <!-- http://www.semanticweb.org/annag/ontologies/2024/1/ontoHorses#M -->

    <owl:NamedIndividual rdf:about="http://www.semanticweb.org/annag/ontologies/2024/1/ontoHorses#M">
        <rdf:type rdf:resource="http://dbpedia.org/ontology/horseRidingDiscipline"/>
        <rdf:type rdf:resource="http://www.semanticweb.org/annag/ontologies/2024/1/ontoHorses#CategorieDressage"/>
        <rdf:type rdf:resource="http://www.semanticweb.org/annag/ontologies/2024/1/ontoHorses#Dressage"/>
        <rdf:type rdf:resource="http://www.semanticweb.org/annag/ontologies/2024/1/ontoHorses#Impiego"/>
        <rdf:type rdf:resource="http://www.semanticweb.org/annag/ontologies/2024/1/ontoHorses#Sella"/>
        <rdf:type rdf:resource="http://www.semanticweb.org/annag/ontologies/2024/1/ontoHorses#SportEquestre"/>
        <rdfs:comment xml:lang="it">Categoria di Dressage di media difficoltà</rdfs:comment>
        <rdfs:comment xml:lang="en">Medium difficulty Dressage category</rdfs:comment>
        <rdfs:label xml:lang="en">M</rdfs:label>
        <rdfs:label xml:lang="it">M</rdfs:label>
    </owl:NamedIndividual>
    


    <!-- http://www.semanticweb.org/annag/ontologies/2024/1/ontoHorses#Maremma -->

    <owl:NamedIndividual rdf:about="http://www.semanticweb.org/annag/ontologies/2024/1/ontoHorses#Maremma">
        <rdf:type rdf:resource="http://schema.org/Place"/>
        <rdf:type rdf:resource="http://www.semanticweb.org/annag/ontologies/2024/1/ontoHorses#AreaGeografica"/>
        <partof:isPartOf rdf:resource="http://www.semanticweb.org/annag/ontologies/2024/1/ontoHorses#Italia"/>
        <rdfs:comment xml:lang="it">La Maremma  è una vasta regione geografica compresa fra Toscana e Lazio, di circa 5000 km², che si affaccia sul Mar Tirreno e sul Mar Ligure.</rdfs:comment>
        <rdfs:comment xml:lang="en">Maremma is a vast geographical region between Tuscany and Lazio, of approximately 5000 km², which overlooks the Tyrrhenian Sea and the Ligurian Sea.</rdfs:comment>
        <rdfs:label xml:lang="en">Maremma</rdfs:label>
        <rdfs:label xml:lang="it">Maremma</rdfs:label>
    </owl:NamedIndividual>
    


    <!-- http://www.semanticweb.org/annag/ontologies/2024/1/ontoHorses#Maremmano -->

    <owl:NamedIndividual rdf:about="http://www.semanticweb.org/annag/ontologies/2024/1/ontoHorses#Maremmano">
        <rdf:type rdf:resource="http://www.semanticweb.org/annag/ontologies/2024/1/ontoHorses#RazzaASangueFreddo"/>
        <rdf:type rdf:resource="http://www.semanticweb.org/annag/ontologies/2024/1/ontoHorses#RazzaCavallo"/>
        <rdf:type rdf:resource="http://www.semanticweb.org/annag/ontologies/2024/1/ontoHorses#RazzaDaEquiturismo"/>
        <rdf:type rdf:resource="http://www.semanticweb.org/annag/ontologies/2024/1/ontoHorses#RazzaDaSella"/>
        <rdf:type rdf:resource="http://www.semanticweb.org/annag/ontologies/2024/1/ontoHorses#RazzaMesoDolicomorfa"/>
        <ontoHorses:entitàWikidata rdf:resource="http://www.wikidata.org/entity/Q1894708"/>
        <ontoHorses:haClassificazioneMorfologica rdf:resource="http://www.semanticweb.org/annag/ontologies/2024/1/ontoHorses#mesoDolicomorfo"/>
        <ontoHorses:haIndole rdf:resource="http://www.semanticweb.org/annag/ontologies/2024/1/ontoHorses#sangueFreddo"/>
        <ontoHorses:haNazionalità rdf:resource="http://www.semanticweb.org/annag/ontologies/2024/1/ontoHorses#Italia"/>
        <ontoHorses:haRegioneDiOrigine rdf:resource="http://www.semanticweb.org/annag/ontologies/2024/1/ontoHorses#Maremma"/>
        <ontoHorses:puòEssereImpiegataIn rdf:resource="http://www.semanticweb.org/annag/ontologies/2024/1/ontoHorses#Equiturismo"/>
        <ontoHorses:altezzaMediaGarrese rdf:datatype="http://www.w3.org/2001/XMLSchema#integer">155</ontoHorses:altezzaMediaGarrese>
        <ontoHorses:haColoreMantello>baio</ontoHorses:haColoreMantello>
        <ontoHorses:haColoreMantello>morello</ontoHorses:haColoreMantello>
        <ontoHorses:pesoMedio rdf:datatype="http://www.w3.org/2001/XMLSchema#integer">500</ontoHorses:pesoMedio>
        <schema:image rdf:resource="https://www.politicheagricole.it/flex/images/d/7/5/D.1bb62598304e4dec51c6/maremmano_large.jpg"/>
        <rdfs:comment xml:lang="it">Il cavallo di razza Maremmano è una razza equina italiana i cui primi esemplari sembra risalgano ai tempi degli Etruschi</rdfs:comment>
        <rdfs:comment xml:lang="en">The Maremmano Horse is an Italian horse breed whose first specimens seem to date back to Etruscan times</rdfs:comment>
        <skos:exactMatch xml:lang="it">http://www.wikidata.org/entity/Q1894708</skos:exactMatch>
        <skos:prefLabel xml:lang="en">Maremmano</skos:prefLabel>
        <skos:prefLabel xml:lang="it">Maremmano</skos:prefLabel>
    </owl:NamedIndividual>
    


    <!-- http://www.semanticweb.org/annag/ontologies/2024/1/ontoHorses#MaschioAndaluso -->

    <owl:NamedIndividual rdf:about="http://www.semanticweb.org/annag/ontologies/2024/1/ontoHorses#MaschioAndaluso">
        <rdf:type rdf:resource="http://dbpedia.org/ontology/horse"/>
        <rdf:type rdf:resource="http://www.semanticweb.org/annag/ontologies/2024/1/ontoHorses#Cavallo"/>
        <rdf:type rdf:resource="http://www.semanticweb.org/annag/ontologies/2024/1/ontoHorses#CavalloASangueCaldo"/>
        <rdf:type rdf:resource="http://www.semanticweb.org/annag/ontologies/2024/1/ontoHorses#CavalloDaSella"/>
        <rdf:type rdf:resource="http://www.semanticweb.org/annag/ontologies/2024/1/ontoHorses#CavalloMaschio"/>
        <rdf:type rdf:resource="http://www.semanticweb.org/annag/ontologies/2024/1/ontoHorses#CavalloPerAltaScuola"/>
        <rdf:type rdf:resource="http://www.semanticweb.org/annag/ontologies/2024/1/ontoHorses#CavalloPerDressage"/>
        <rdf:type rdf:resource="http://www.semanticweb.org/annag/ontologies/2024/1/ontoHorses#CavalloSportivo"/>
        <rdf:type rdf:resource="http://www.semanticweb.org/annag/ontologies/2024/1/ontoHorses#Puledro"/>
        <price:hasPrice rdf:resource="http://www.semanticweb.org/annag/ontologies/2024/1/ontoHorses#7000Euro"/>
        <ontoHorses:gareggiaNellaCategoriaDiDressage rdf:resource="http://www.semanticweb.org/annag/ontologies/2024/1/ontoHorses#F"/>
        <ontoHorses:haRazza rdf:resource="http://www.semanticweb.org/annag/ontologies/2024/1/ontoHorses#Andaluso"/>
        <ontoHorses:vieneUtilizzatoPer rdf:resource="http://www.semanticweb.org/annag/ontologies/2024/1/ontoHorses#AltaScuola"/>
        <ontoHorses:èAdattoPer rdf:resource="http://www.semanticweb.org/annag/ontologies/2024/1/ontoHorses#CavaliereIntermedio"/>
        <ontoHorses:èPossedutoDa rdf:resource="http://www.semanticweb.org/annag/ontologies/2024/1/ontoHorses#brunoGramaglia"/>
        <ontoHorses:èScuderizzatoIn rdf:resource="http://www.semanticweb.org/annag/ontologies/2024/1/ontoHorses#Italia"/>
        <ontoHorses:èScuderizzatoIn rdf:resource="http://www.semanticweb.org/annag/ontologies/2024/1/ontoHorses#Piemonte"/>
        <ontoHorses:èScuderizzatoInCittàDi rdf:resource="http://www.semanticweb.org/annag/ontologies/2024/1/ontoHorses#sanMauro"/>
        <ontoHorses:altezzaGarrese rdf:datatype="http://www.w3.org/2001/XMLSchema#integer">165</ontoHorses:altezzaGarrese>
        <ontoHorses:eta rdf:datatype="http://www.w3.org/2001/XMLSchema#integer">4</ontoHorses:eta>
        <ontoHorses:haSesso>maschio</ontoHorses:haSesso>
        <ontoHorses:nomeCavallo>Fuser</ontoHorses:nomeCavallo>
        <schema:image rdf:resource="https://cdn.ehorses.media/image/blur/big/andaluso-giumenta-11anni-160-cm-grigio-cavalli-per-ricreazione-cavalli-da-dressage-wellheim_22ccd770-84e8-4983-8669-b3fd22c544cd.jpg"/>
        <rdfs:comment xml:lang="it">Esemplare di cavallo maschio andaluso in vendita. Anno 2020. Ottima genealogia. Utilizzato in gare di dressage ed Alta scuola. Adatto a cavalieri con un minimo di esperienza.</rdfs:comment>
        <rdfs:comment xml:lang="en">Male Andalusian horse for sale. Year 2020. Excellent genealogy. Used in dressage and high school competitions. Suitable for riders with a minimum of experience.</rdfs:comment>
        <rdfs:label xml:lang="en">Andalusian male</rdfs:label>
        <rdfs:label xml:lang="it">Maschio andaluso</rdfs:label>
    </owl:NamedIndividual>
    


    <!-- http://www.semanticweb.org/annag/ontologies/2024/1/ontoHorses#MaschioOlandese -->

    <owl:NamedIndividual rdf:about="http://www.semanticweb.org/annag/ontologies/2024/1/ontoHorses#MaschioOlandese">
        <rdf:type rdf:resource="http://dbpedia.org/ontology/horse"/>
        <rdf:type rdf:resource="http://www.semanticweb.org/annag/ontologies/2024/1/ontoHorses#Cavallo"/>
        <rdf:type rdf:resource="http://www.semanticweb.org/annag/ontologies/2024/1/ontoHorses#CavalloASangueCaldo"/>
        <rdf:type rdf:resource="http://www.semanticweb.org/annag/ontologies/2024/1/ontoHorses#CavalloAdulto"/>
        <rdf:type rdf:resource="http://www.semanticweb.org/annag/ontologies/2024/1/ontoHorses#CavalloDaSella"/>
        <rdf:type rdf:resource="http://www.semanticweb.org/annag/ontologies/2024/1/ontoHorses#CavalloMaschio"/>
        <rdf:type rdf:resource="http://www.semanticweb.org/annag/ontologies/2024/1/ontoHorses#CavalloSportivo"/>
        <price:hasPrice rdf:resource="http://www.semanticweb.org/annag/ontologies/2024/1/ontoHorses#35000Euro"/>
        <ontoHorses:adattoAlConseguimentoDi rdf:resource="http://www.semanticweb.org/annag/ontologies/2024/1/ontoHorses#primoGrado"/>
        <ontoHorses:adattoAlConseguimentoDi rdf:resource="http://www.semanticweb.org/annag/ontologies/2024/1/ontoHorses#secondoGrado"/>
        <ontoHorses:gareggiaNelleCategorieDiSalto rdf:resource="http://www.semanticweb.org/annag/ontologies/2024/1/ontoHorses#C135"/>
        <ontoHorses:haRazza rdf:resource="http://www.semanticweb.org/annag/ontologies/2024/1/ontoHorses#OlandeseASangueCaldo"/>
        <ontoHorses:vieneUtilizzatoPer rdf:resource="http://www.semanticweb.org/annag/ontologies/2024/1/ontoHorses#SaltoAdOstacoli"/>
        <ontoHorses:èAdattoPer rdf:resource="http://www.semanticweb.org/annag/ontologies/2024/1/ontoHorses#CavaliereEsperto"/>
        <ontoHorses:èAdattoPer rdf:resource="http://www.semanticweb.org/annag/ontologies/2024/1/ontoHorses#CavaliereIntermedio"/>
        <ontoHorses:èAdattoPer rdf:resource="http://www.semanticweb.org/annag/ontologies/2024/1/ontoHorses#CavaliereMoltoEsperto"/>
        <ontoHorses:èPossedutoDa rdf:resource="http://www.semanticweb.org/annag/ontologies/2024/1/ontoHorses#gianlucaCamoletto"/>
        <ontoHorses:èScuderizzatoIn rdf:resource="http://www.semanticweb.org/annag/ontologies/2024/1/ontoHorses#Italia"/>
        <ontoHorses:èScuderizzatoIn rdf:resource="http://www.semanticweb.org/annag/ontologies/2024/1/ontoHorses#Piemonte"/>
        <ontoHorses:èScuderizzatoInCittàDi rdf:resource="http://www.semanticweb.org/annag/ontologies/2024/1/ontoHorses#leini"/>
        <ontoHorses:altezzaGarrese rdf:datatype="http://www.w3.org/2001/XMLSchema#integer">170</ontoHorses:altezzaGarrese>
        <ontoHorses:eta rdf:datatype="http://www.w3.org/2001/XMLSchema#integer">12</ontoHorses:eta>
        <ontoHorses:haSesso>maschio</ontoHorses:haSesso>
        <ontoHorses:nomeCavallo>Mufasa</ontoHorses:nomeCavallo>
        <schema:image rdf:resource="https://www.equirodi.it/images/annonces/xl/854164_1709831119_8149.jpg"/>
        <rdfs:comment xml:lang="en">12 year old male Dutch horse for sale. Excellent for obtaining 1st and 2nd degrees. Suitable for experienced riders. Difficult management on the ground.</rdfs:comment>
        <rdfs:comment xml:lang="it">Esemplare di cavallo maschio olandese di 12 anni  in vendita. Ottimo per il conseguimento di 1° e 2° grado. Adatto a cavalieri esperti. Difficile gestione a terra.</rdfs:comment>
        <rdfs:label xml:lang="en">Dutch male</rdfs:label>
        <rdfs:label xml:lang="it">Maschio olandese</rdfs:label>
    </owl:NamedIndividual>
    


    <!-- http://www.semanticweb.org/annag/ontologies/2024/1/ontoHorses#MaschioPuroSangueInglese -->

    <owl:NamedIndividual rdf:about="http://www.semanticweb.org/annag/ontologies/2024/1/ontoHorses#MaschioPuroSangueInglese">
        <rdf:type rdf:resource="http://dbpedia.org/ontology/horse"/>
        <rdf:type rdf:resource="http://www.semanticweb.org/annag/ontologies/2024/1/ontoHorses#Cavallo"/>
        <rdf:type rdf:resource="http://www.semanticweb.org/annag/ontologies/2024/1/ontoHorses#CavalloASangueCaldo"/>
        <rdf:type rdf:resource="http://www.semanticweb.org/annag/ontologies/2024/1/ontoHorses#CavalloAdulto"/>
        <rdf:type rdf:resource="http://www.semanticweb.org/annag/ontologies/2024/1/ontoHorses#CavalloDaSella"/>
        <rdf:type rdf:resource="http://www.semanticweb.org/annag/ontologies/2024/1/ontoHorses#CavalloMaschio"/>
        <rdf:type rdf:resource="http://www.semanticweb.org/annag/ontologies/2024/1/ontoHorses#CavalloPerEndurance"/>
        <rdf:type rdf:resource="http://www.semanticweb.org/annag/ontologies/2024/1/ontoHorses#CavalloSportivo"/>
        <price:hasPrice rdf:resource="http://www.semanticweb.org/annag/ontologies/2024/1/ontoHorses#20000Euro"/>
        <ontoHorses:haRazza rdf:resource="http://www.semanticweb.org/annag/ontologies/2024/1/ontoHorses#PuroSangueInglese"/>
        <ontoHorses:vieneUtilizzatoPer rdf:resource="http://www.semanticweb.org/annag/ontologies/2024/1/ontoHorses#Endurance"/>
        <ontoHorses:èAdattoPer rdf:resource="http://www.semanticweb.org/annag/ontologies/2024/1/ontoHorses#CavaliereMoltoEsperto"/>
        <ontoHorses:èPossedutoDa rdf:resource="http://www.semanticweb.org/annag/ontologies/2024/1/ontoHorses#brunoGramaglia"/>
        <ontoHorses:èScuderizzatoIn rdf:resource="http://www.semanticweb.org/annag/ontologies/2024/1/ontoHorses#Italia"/>
        <ontoHorses:èScuderizzatoIn rdf:resource="http://www.semanticweb.org/annag/ontologies/2024/1/ontoHorses#Piemonte"/>
        <ontoHorses:èScuderizzatoInCittàDi rdf:resource="http://www.semanticweb.org/annag/ontologies/2024/1/ontoHorses#sanMauro"/>
        <ontoHorses:altezzaGarrese rdf:datatype="http://www.w3.org/2001/XMLSchema#integer">161</ontoHorses:altezzaGarrese>
        <ontoHorses:eta rdf:datatype="http://www.w3.org/2001/XMLSchema#integer">10</ontoHorses:eta>
        <ontoHorses:haSesso>maschio</ontoHorses:haSesso>
        <ontoHorses:nomeCavallo>Fulmine Del Monte Acuto</ontoHorses:nomeCavallo>
        <schema:image rdf:resource="https://cdn.ehorses.media/image/blur/big/purosangue-inglese-castrone-11anni-167-cm-sauro-cavalli-da-completo-langenhagen_c785185a-0bc2-41c5-9eb5-077fb8170f36.jpg"/>
        <rdfs:comment xml:lang="en">English Thoroughbred example for sale. Year 2014. Excellent results in endurance competitions. It requires a very experienced rider. Easy handling on the ground.</rdfs:comment>
        <rdfs:comment xml:lang="it">Esemplare di purosangue inglese in vendita. Anno 2014. Ottimi risultati nelle competizioni di endurance. Richiede un cavaliere molto esperto. Facile gestione a terra.</rdfs:comment>
        <rdfs:label xml:lang="it">Maschio purosangue inglese</rdfs:label>
        <rdfs:label xml:lang="en">Thoroughbred male</rdfs:label>
    </owl:NamedIndividual>
    


    <!-- http://www.semanticweb.org/annag/ontologies/2024/1/ontoHorses#MaschioTedesco -->

    <owl:NamedIndividual rdf:about="http://www.semanticweb.org/annag/ontologies/2024/1/ontoHorses#MaschioTedesco">
        <rdf:type rdf:resource="http://dbpedia.org/ontology/horse"/>
        <rdf:type rdf:resource="http://www.semanticweb.org/annag/ontologies/2024/1/ontoHorses#Cavallo"/>
        <rdf:type rdf:resource="http://www.semanticweb.org/annag/ontologies/2024/1/ontoHorses#CavalloASangueMisto"/>
        <rdf:type rdf:resource="http://www.semanticweb.org/annag/ontologies/2024/1/ontoHorses#CavalloAdulto"/>
        <rdf:type rdf:resource="http://www.semanticweb.org/annag/ontologies/2024/1/ontoHorses#CavalloDaSella"/>
        <rdf:type rdf:resource="http://www.semanticweb.org/annag/ontologies/2024/1/ontoHorses#CavalloMaschio"/>
        <rdf:type rdf:resource="http://www.semanticweb.org/annag/ontologies/2024/1/ontoHorses#CavalloPerCrossCountry"/>
        <rdf:type rdf:resource="http://www.semanticweb.org/annag/ontologies/2024/1/ontoHorses#CavalloSportivo"/>
        <price:hasPrice rdf:resource="http://www.semanticweb.org/annag/ontologies/2024/1/ontoHorses#15000Euro"/>
        <ontoHorses:adattoAlConseguimentoDi rdf:resource="http://www.semanticweb.org/annag/ontologies/2024/1/ontoHorses#brevetto"/>
        <ontoHorses:adattoAlConseguimentoDi rdf:resource="http://www.semanticweb.org/annag/ontologies/2024/1/ontoHorses#primoGrado"/>
        <ontoHorses:gareggiaNelleCategorieDiSalto rdf:resource="http://www.semanticweb.org/annag/ontologies/2024/1/ontoHorses#C115"/>
        <ontoHorses:haRazza rdf:resource="http://www.semanticweb.org/annag/ontologies/2024/1/ontoHorses#Holstein"/>
        <ontoHorses:vieneUtilizzatoPer rdf:resource="http://www.semanticweb.org/annag/ontologies/2024/1/ontoHorses#CrossCountry"/>
        <ontoHorses:vieneUtilizzatoPer rdf:resource="http://www.semanticweb.org/annag/ontologies/2024/1/ontoHorses#SaltoAdOstacoli"/>
        <ontoHorses:èAdattoPer rdf:resource="http://www.semanticweb.org/annag/ontologies/2024/1/ontoHorses#CavaliereEsperto"/>
        <ontoHorses:èAdattoPer rdf:resource="http://www.semanticweb.org/annag/ontologies/2024/1/ontoHorses#CavaliereIntermedio"/>
        <ontoHorses:èAdattoPer rdf:resource="http://www.semanticweb.org/annag/ontologies/2024/1/ontoHorses#CavalierePrincipiante"/>
        <ontoHorses:èPossedutoDa rdf:resource="http://www.semanticweb.org/annag/ontologies/2024/1/ontoHorses#paoloGrassi"/>
        <ontoHorses:èScuderizzatoIn rdf:resource="http://www.semanticweb.org/annag/ontologies/2024/1/ontoHorses#Italia"/>
        <ontoHorses:èScuderizzatoIn rdf:resource="http://www.semanticweb.org/annag/ontologies/2024/1/ontoHorses#Puglia"/>
        <ontoHorses:èScuderizzatoInCittàDi rdf:resource="http://www.semanticweb.org/annag/ontologies/2024/1/ontoHorses#taranto"/>
        <ontoHorses:altezzaGarrese rdf:datatype="http://www.w3.org/2001/XMLSchema#integer">168</ontoHorses:altezzaGarrese>
        <ontoHorses:eta rdf:datatype="http://www.w3.org/2001/XMLSchema#integer">16</ontoHorses:eta>
        <ontoHorses:haSesso>maschio</ontoHorses:haSesso>
        <ontoHorses:nomeCavallo>Luther Lucifer</ontoHorses:nomeCavallo>
        <schema:image rdf:resource="https://www.equirodi.it/images/annonces/xl/835574_1705591089.jpg"/>
        <rdfs:comment xml:lang="en">16 year old German male specimen for sale. It has vehicles up to category C115. Easy management. Suitable for everyone. Excellent for obtaining the patent.</rdfs:comment>
        <rdfs:comment xml:lang="it">Esemplare di maschio tedesco di 16 anni in vendita. Ha i mezzi fino alla categoria C115. Facile gestione. Adatto a tutti. Ottimo per il conseguimento del brevetto.</rdfs:comment>
        <rdfs:label xml:lang="en">German male</rdfs:label>
        <rdfs:label xml:lang="it">Maschio tedesco</rdfs:label>
    </owl:NamedIndividual>
    


    <!-- http://www.semanticweb.org/annag/ontologies/2024/1/ontoHorses#Murge -->

    <owl:NamedIndividual rdf:about="http://www.semanticweb.org/annag/ontologies/2024/1/ontoHorses#Murge">
        <rdf:type rdf:resource="http://schema.org/Place"/>
        <rdf:type rdf:resource="http://www.semanticweb.org/annag/ontologies/2024/1/ontoHorses#AreaGeografica"/>
        <partof:isPartOf rdf:resource="http://www.semanticweb.org/annag/ontologies/2024/1/ontoHorses#Italia"/>
        <schema:image rdf:resource="https://upload.wikimedia.org/wikipedia/commons/thumb/0/0a/Murge.jpg/1280px-Murge.jpg"/>
        <rdfs:comment xml:lang="it">Le Murge sono una subregione appulo-lucana piuttosto estesa, corrispondente a un altopiano carsico di origine tettonica e di forma quadrangolare situato tra la Puglia centrale e la Basilicata nord-orientale. Il territorio dell&apos;altopiano fa parte prevalentemente della città metropolitana di Bari e della provincia di Barletta-Andria-Trani e si estende a occidente fin nella provincia di Matera, in Basilicata; inoltre si prolunga verso sud nelle province di Taranto (Murge tarantine) e marginalmente Brindisi.</rdfs:comment>
        <rdfs:comment xml:lang="en">The Murge are a rather large Appulo-Lucanian subregion, corresponding to a karst plateau of tectonic origin and quadrangular in shape located between central Puglia and north-eastern Basilicata. The territory of the plateau is mainly part of the metropolitan city of Bari and the province of Barletta-Andria-Trani and extends westwards to the province of Matera, in Basilicata; it also extends southwards into the provinces of Taranto (Murge tarantine) and marginally Brindisi.</rdfs:comment>
        <rdfs:label xml:lang="en">Murge</rdfs:label>
        <rdfs:label xml:lang="it">Murge</rdfs:label>
    </owl:NamedIndividual>
    


    <!-- http://www.semanticweb.org/annag/ontologies/2024/1/ontoHorses#Murgese -->

    <owl:NamedIndividual rdf:about="http://www.semanticweb.org/annag/ontologies/2024/1/ontoHorses#Murgese">
        <rdf:type rdf:resource="http://www.semanticweb.org/annag/ontologies/2024/1/ontoHorses#RazzaASangueCaldo"/>
        <rdf:type rdf:resource="http://www.semanticweb.org/annag/ontologies/2024/1/ontoHorses#RazzaCavallo"/>
        <rdf:type rdf:resource="http://www.semanticweb.org/annag/ontologies/2024/1/ontoHorses#RazzaDaDressage"/>
        <rdf:type rdf:resource="http://www.semanticweb.org/annag/ontologies/2024/1/ontoHorses#RazzaDaLavoro"/>
        <rdf:type rdf:resource="http://www.semanticweb.org/annag/ontologies/2024/1/ontoHorses#RazzaDaSella"/>
        <rdf:type rdf:resource="http://www.semanticweb.org/annag/ontologies/2024/1/ontoHorses#RazzaSportiva"/>
        <rdf:type rdf:resource="http://www.semanticweb.org/annag/ontologies/2024/1/ontoHorses#RazzamMesomorfa"/>
        <ontoHorses:entitàWikidata rdf:resource="http://www.wikidata.org/entity/Q1953691"/>
        <ontoHorses:haClassificazioneMorfologica rdf:resource="http://www.semanticweb.org/annag/ontologies/2024/1/ontoHorses#mesomorfo"/>
        <ontoHorses:haIndole rdf:resource="http://www.semanticweb.org/annag/ontologies/2024/1/ontoHorses#sangueCaldo"/>
        <ontoHorses:haNazionalità rdf:resource="http://www.semanticweb.org/annag/ontologies/2024/1/ontoHorses#Italia"/>
        <ontoHorses:haRegioneDiOrigine rdf:resource="http://www.semanticweb.org/annag/ontologies/2024/1/ontoHorses#Murge"/>
        <ontoHorses:puòEssereImpiegataIn rdf:resource="http://www.semanticweb.org/annag/ontologies/2024/1/ontoHorses#Dressage"/>
        <ontoHorses:puòEssereImpiegataIn rdf:resource="http://www.semanticweb.org/annag/ontologies/2024/1/ontoHorses#TrainoCarrozze"/>
        <ontoHorses:altezzaMediaGarrese rdf:datatype="http://www.w3.org/2001/XMLSchema#integer">162</ontoHorses:altezzaMediaGarrese>
        <ontoHorses:haColoreMantello>morello</ontoHorses:haColoreMantello>
        <ontoHorses:pesoMedio rdf:datatype="http://www.w3.org/2001/XMLSchema#integer">500</ontoHorses:pesoMedio>
        <schema:image rdf:resource="https://www.animali.net/wp-content/uploads/2015/09/Il_Murgese.jpg"/>
        <rdfs:comment xml:lang="it">Il Murgese è una razza equina italiana che è originaria delle Murge, una regione geografica della Puglia e Basilicata, da cui ne deriva il nome</rdfs:comment>
        <rdfs:comment xml:lang="en">The Murgese is an Italian horse breed that originates from the Murge, a geographical region of Puglia and Basilicata, from which its name derives</rdfs:comment>
        <skos:exactMatch xml:lang="it">http://www.wikidata.org/entity/Q1953691</skos:exactMatch>
        <skos:prefLabel xml:lang="en">Murgese</skos:prefLabel>
        <skos:prefLabel xml:lang="it">Murgese</skos:prefLabel>
    </owl:NamedIndividual>
    


    <!-- http://www.semanticweb.org/annag/ontologies/2024/1/ontoHorses#Normandia -->

    <owl:NamedIndividual rdf:about="http://www.semanticweb.org/annag/ontologies/2024/1/ontoHorses#Normandia">
        <rdf:type rdf:resource="http://schema.org/Place"/>
        <rdf:type rdf:resource="http://www.semanticweb.org/annag/ontologies/2024/1/ontoHorses#AreaGeografica"/>
        <partof:isPartOf rdf:resource="http://www.semanticweb.org/annag/ontologies/2024/1/ontoHorses#Francia"/>
        <rdfs:comment xml:lang="it">La Normandia è una regione storica ed amministrativa della Francia.</rdfs:comment>
        <rdfs:comment xml:lang="en">Normandy is a historical and administrative region of France.</rdfs:comment>
        <rdfs:label xml:lang="it">Normandia</rdfs:label>
        <rdfs:label xml:lang="en">Normandy</rdfs:label>
    </owl:NamedIndividual>
    


    <!-- http://www.semanticweb.org/annag/ontologies/2024/1/ontoHorses#OlandeseASangueCaldo -->

    <owl:NamedIndividual rdf:about="http://www.semanticweb.org/annag/ontologies/2024/1/ontoHorses#OlandeseASangueCaldo">
        <rdf:type rdf:resource="http://www.semanticweb.org/annag/ontologies/2024/1/ontoHorses#RazzaASangueCaldo"/>
        <rdf:type rdf:resource="http://www.semanticweb.org/annag/ontologies/2024/1/ontoHorses#RazzaCavallo"/>
        <rdf:type rdf:resource="http://www.semanticweb.org/annag/ontologies/2024/1/ontoHorses#RazzaDaDressage"/>
        <rdf:type rdf:resource="http://www.semanticweb.org/annag/ontologies/2024/1/ontoHorses#RazzaDaSaltoOstacoli"/>
        <rdf:type rdf:resource="http://www.semanticweb.org/annag/ontologies/2024/1/ontoHorses#RazzaDaSella"/>
        <rdf:type rdf:resource="http://www.semanticweb.org/annag/ontologies/2024/1/ontoHorses#RazzaMesoDolicomorfa"/>
        <rdf:type rdf:resource="http://www.semanticweb.org/annag/ontologies/2024/1/ontoHorses#RazzaSportiva"/>
        <ontoHorses:entitàWikidata rdf:resource="http://www.wikidata.org/entity/Q1468737"/>
        <ontoHorses:haClassificazioneMorfologica rdf:resource="http://www.semanticweb.org/annag/ontologies/2024/1/ontoHorses#mesoDolicomorfo"/>
        <ontoHorses:haIndole rdf:resource="http://www.semanticweb.org/annag/ontologies/2024/1/ontoHorses#sangueCaldo"/>
        <ontoHorses:haNazionalità rdf:resource="http://www.semanticweb.org/annag/ontologies/2024/1/ontoHorses#PaesiBassi"/>
        <ontoHorses:puòEssereImpiegataIn rdf:resource="http://www.semanticweb.org/annag/ontologies/2024/1/ontoHorses#Dressage"/>
        <ontoHorses:puòEssereImpiegataIn rdf:resource="http://www.semanticweb.org/annag/ontologies/2024/1/ontoHorses#SaltoAdOstacoli"/>
        <ontoHorses:altezzaMediaGarrese rdf:datatype="http://www.w3.org/2001/XMLSchema#integer">165</ontoHorses:altezzaMediaGarrese>
        <ontoHorses:haColoreMantello>baio</ontoHorses:haColoreMantello>
        <ontoHorses:haColoreMantello>grigio</ontoHorses:haColoreMantello>
        <ontoHorses:haColoreMantello>morello</ontoHorses:haColoreMantello>
        <ontoHorses:haColoreMantello>pezzato</ontoHorses:haColoreMantello>
        <ontoHorses:haColoreMantello>sauro</ontoHorses:haColoreMantello>
        <ontoHorses:pesoMedio rdf:datatype="http://www.w3.org/2001/XMLSchema#integer">550</ontoHorses:pesoMedio>
        <schema:image rdf:resource="https://upload.wikimedia.org/wikipedia/commons/thumb/e/e3/Michael_Whitaker_and_Tackeray%2C_CSIO_Rome_2009.jpg/240px-Michael_Whitaker_and_Tackeray%2C_CSIO_Rome_2009.jpg"/>
        <rdfs:comment xml:lang="it">L&apos;Olandese a sangue caldo è una razza equina moderna di origini olandesi utilizzata per sport sebbene originariamente nasca come cavallo da tiro</rdfs:comment>
        <rdfs:comment xml:lang="en">The Dutch Warmblood is a modern equine breed of Dutch origins used for sport although it was originally born as a draft horse</rdfs:comment>
        <skos:exactMatch xml:lang="it">http://www.wikidata.org/entity/Q1468737</skos:exactMatch>
        <skos:prefLabel xml:lang="en">Dutch Warmblood</skos:prefLabel>
        <skos:prefLabel xml:lang="it">Olandese a sangue caldo</skos:prefLabel>
    </owl:NamedIndividual>
    


    <!-- http://www.semanticweb.org/annag/ontologies/2024/1/ontoHorses#Oldemburghese -->

    <owl:NamedIndividual rdf:about="http://www.semanticweb.org/annag/ontologies/2024/1/ontoHorses#Oldemburghese">
        <rdf:type rdf:resource="http://www.semanticweb.org/annag/ontologies/2024/1/ontoHorses#RazzaASangueCaldo"/>
        <rdf:type rdf:resource="http://www.semanticweb.org/annag/ontologies/2024/1/ontoHorses#RazzaCavallo"/>
        <rdf:type rdf:resource="http://www.semanticweb.org/annag/ontologies/2024/1/ontoHorses#RazzaDaDressage"/>
        <rdf:type rdf:resource="http://www.semanticweb.org/annag/ontologies/2024/1/ontoHorses#RazzaDaSaltoOstacoli"/>
        <rdf:type rdf:resource="http://www.semanticweb.org/annag/ontologies/2024/1/ontoHorses#RazzaDaSella"/>
        <rdf:type rdf:resource="http://www.semanticweb.org/annag/ontologies/2024/1/ontoHorses#RazzaSportiva"/>
        <rdf:type rdf:resource="http://www.semanticweb.org/annag/ontologies/2024/1/ontoHorses#RazzamMesomorfa"/>
        <ontoHorses:entitàWikidata rdf:resource="http://www.wikidata.org/entity/Q166777"/>
        <ontoHorses:haClassificazioneMorfologica rdf:resource="http://www.semanticweb.org/annag/ontologies/2024/1/ontoHorses#mesomorfo"/>
        <ontoHorses:haIndole rdf:resource="http://www.semanticweb.org/annag/ontologies/2024/1/ontoHorses#sangueCaldo"/>
        <ontoHorses:haNazionalità rdf:resource="http://www.semanticweb.org/annag/ontologies/2024/1/ontoHorses#Germania"/>
        <ontoHorses:puòEssereImpiegataIn rdf:resource="http://www.semanticweb.org/annag/ontologies/2024/1/ontoHorses#Dressage"/>
        <ontoHorses:puòEssereImpiegataIn rdf:resource="http://www.semanticweb.org/annag/ontologies/2024/1/ontoHorses#SaltoAdOstacoli"/>
        <ontoHorses:altezzaMediaGarrese rdf:datatype="http://www.w3.org/2001/XMLSchema#integer">170</ontoHorses:altezzaMediaGarrese>
        <ontoHorses:haColoreMantello>baio</ontoHorses:haColoreMantello>
        <ontoHorses:haColoreMantello>grigio</ontoHorses:haColoreMantello>
        <ontoHorses:haColoreMantello>morello</ontoHorses:haColoreMantello>
        <ontoHorses:haColoreMantello>sauro</ontoHorses:haColoreMantello>
        <ontoHorses:pesoMedio rdf:datatype="http://www.w3.org/2001/XMLSchema#integer">525</ontoHorses:pesoMedio>
        <schema:image rdf:resource="https://upload.wikimedia.org/wikipedia/commons/thumb/7/72/Bess2.jpg/240px-Bess2.jpg"/>
        <rdfs:comment xml:lang="it">L&apos;Oldemburghese è una razza di cavallo originaria della Germania. Molto tranquillo ma energico, è il più grosso dei cavalli a sangue caldo tedeschi.</rdfs:comment>
        <rdfs:comment xml:lang="en">The Oldenburger is a horse breed originating from Germany. Very calm but energetic, it is the largest of the German warmblood horses.</rdfs:comment>
        <skos:exactMatch xml:lang="it">http://www.wikidata.org/entity/Q166777</skos:exactMatch>
        <skos:prefLabel xml:lang="it">Oldemburghese</skos:prefLabel>
        <skos:prefLabel xml:lang="en">Oldenburg Horse</skos:prefLabel>
    </owl:NamedIndividual>
    


    <!-- http://www.semanticweb.org/annag/ontologies/2024/1/ontoHorses#PaesiBassi -->

    <owl:NamedIndividual rdf:about="http://www.semanticweb.org/annag/ontologies/2024/1/ontoHorses#PaesiBassi">
        <rdf:type rdf:resource="http://schema.org/Place"/>
        <rdf:type rdf:resource="http://www.semanticweb.org/annag/ontologies/2024/1/ontoHorses#AreaGeografica"/>
        <partof:hasPart rdf:resource="http://www.semanticweb.org/annag/ontologies/2024/1/ontoHorses#Frisia"/>
        <schema:image rdf:resource="https://upload.wikimedia.org/wikipedia/commons/thumb/2/20/Flag_of_the_Netherlands.svg/1280px-Flag_of_the_Netherlands.svg.png"/>
        <rdfs:comment xml:lang="it">I Paesi Bassi sono una delle quattro nazioni costitutive del Regno dei Paesi Bassi; si trovano principalmente in Europa ma comprendono anche i cosiddetti Paesi Bassi caraibici. Il nome Paesi Bassi è un riferimento alla sua bassa elevazione e alla sua topografia piatta, con solo il 50% circa del suo territorio che supera 1 metro sopra il livello del mare e quasi il 26% che scende sotto il livello del mare.</rdfs:comment>
        <rdfs:comment xml:lang="en">The Netherlands is one of the four constituent nations of the Kingdom of the Netherlands; they are found mainly in Europe but also include the so-called Caribbean Netherlands. The name Netherlands is a reference to its low elevation and flat topography, with only about 50% of its territory exceeding 1 meter above sea level and almost 26% falling below sea level.</rdfs:comment>
        <rdfs:label xml:lang="en">Netherlands</rdfs:label>
        <rdfs:label xml:lang="it">Paesi Bassi</rdfs:label>
    </owl:NamedIndividual>
    


    <!-- http://www.semanticweb.org/annag/ontologies/2024/1/ontoHorses#Perche -->

    <owl:NamedIndividual rdf:about="http://www.semanticweb.org/annag/ontologies/2024/1/ontoHorses#Perche">
        <rdf:type rdf:resource="http://schema.org/Place"/>
        <rdf:type rdf:resource="http://www.semanticweb.org/annag/ontologies/2024/1/ontoHorses#AreaGeografica"/>
        <partof:isPartOf rdf:resource="http://www.semanticweb.org/annag/ontologies/2024/1/ontoHorses#Francia"/>
        <rdfs:comment xml:lang="it">La contea del Perche è un territorio storico della Francia che costituisce una delle antiche province francesi.</rdfs:comment>
        <rdfs:comment xml:lang="en">The county of Perche is a historical territory of France which constitutes one of the ancient French provinces.</rdfs:comment>
        <rdfs:label xml:lang="it">Contea del Perche</rdfs:label>
        <rdfs:label xml:lang="en">Perche</rdfs:label>
    </owl:NamedIndividual>
    


    <!-- http://www.semanticweb.org/annag/ontologies/2024/1/ontoHorses#Percheron -->

    <owl:NamedIndividual rdf:about="http://www.semanticweb.org/annag/ontologies/2024/1/ontoHorses#Percheron">
        <rdf:type rdf:resource="http://www.semanticweb.org/annag/ontologies/2024/1/ontoHorses#RazzaASangueFreddo"/>
        <rdf:type rdf:resource="http://www.semanticweb.org/annag/ontologies/2024/1/ontoHorses#RazzaBrachimorfa"/>
        <rdf:type rdf:resource="http://www.semanticweb.org/annag/ontologies/2024/1/ontoHorses#RazzaCavallo"/>
        <rdf:type rdf:resource="http://www.semanticweb.org/annag/ontologies/2024/1/ontoHorses#RazzaDaLavoro"/>
        <rdf:type rdf:resource="http://www.semanticweb.org/annag/ontologies/2024/1/ontoHorses#RazzaDaTiroAgricolo"/>
        <ontoHorses:entitàWikidata rdf:resource="http://www.wikidata.org/entity/Q1232528"/>
        <ontoHorses:haClassificazioneMorfologica rdf:resource="http://www.semanticweb.org/annag/ontologies/2024/1/ontoHorses#brachimorfo"/>
        <ontoHorses:haIndole rdf:resource="http://www.semanticweb.org/annag/ontologies/2024/1/ontoHorses#sangueFreddo"/>
        <ontoHorses:haNazionalità rdf:resource="http://www.semanticweb.org/annag/ontologies/2024/1/ontoHorses#Francia"/>
        <ontoHorses:haRegioneDiOrigine rdf:resource="http://www.semanticweb.org/annag/ontologies/2024/1/ontoHorses#Perche"/>
        <ontoHorses:puòEssereImpiegataIn rdf:resource="http://www.semanticweb.org/annag/ontologies/2024/1/ontoHorses#TiroAgricolo"/>
        <ontoHorses:puòEssereImpiegataIn rdf:resource="http://www.semanticweb.org/annag/ontologies/2024/1/ontoHorses#TrainoCarrozze"/>
        <ontoHorses:altezzaMediaGarrese rdf:datatype="http://www.w3.org/2001/XMLSchema#integer">165</ontoHorses:altezzaMediaGarrese>
        <ontoHorses:haColoreMantello>grigio</ontoHorses:haColoreMantello>
        <ontoHorses:haColoreMantello>morello</ontoHorses:haColoreMantello>
        <ontoHorses:pesoMedio rdf:datatype="http://www.w3.org/2001/XMLSchema#integer">800</ontoHorses:pesoMedio>
        <schema:image rdf:resource="https://upload.wikimedia.org/wikipedia/commons/thumb/c/c1/Percheron_3_stehend_rechts.jpg/240px-Percheron_3_stehend_rechts.jpg"/>
        <rdfs:comment xml:lang="en">The Percheron is a French horse breed, originating from the province of Perche, in northern France, from which the breed takes its name. The Percheron is probably the best known and most widespread heavy breed in the world for agriculture and as a carriage horse</rdfs:comment>
        <rdfs:comment xml:lang="it">ll Percheron è una razza equina francese, originaria della provincia della Perche, nel nord della Francia, da cui prende nome la razza. Il Percheron è probabilmente la razza pesante più conosciuta e più diffusa del mondo per l’agricoltura e come cavallo da carrozza</rdfs:comment>
        <skos:exactMatch xml:lang="it">http://www.wikidata.org/entity/Q1232528</skos:exactMatch>
        <skos:prefLabel xml:lang="en">Percheron</skos:prefLabel>
        <skos:prefLabel xml:lang="it">Percheron</skos:prefLabel>
    </owl:NamedIndividual>
    


    <!-- http://www.semanticweb.org/annag/ontologies/2024/1/ontoHorses#Piemonte -->

    <owl:NamedIndividual rdf:about="http://www.semanticweb.org/annag/ontologies/2024/1/ontoHorses#Piemonte">
        <rdf:type rdf:resource="http://schema.org/Place"/>
        <rdf:type rdf:resource="http://www.semanticweb.org/annag/ontologies/2024/1/ontoHorses#AreaGeografica"/>
        <partof:hasPart rdf:resource="http://www.semanticweb.org/annag/ontologies/2024/1/ontoHorses#leini"/>
        <partof:hasPart rdf:resource="http://www.semanticweb.org/annag/ontologies/2024/1/ontoHorses#sanMauro"/>
        <partof:isPartOf rdf:resource="http://www.semanticweb.org/annag/ontologies/2024/1/ontoHorses#Italia"/>
        <rdfs:comment xml:lang="it">Il Piemonte è una regione a statuto ordinario di 4 252 581 abitanti dell&apos;Italia nord-occidentale, con capoluogo amministrativo – nonché capitale storica – la città di Torino.</rdfs:comment>
        <rdfs:comment xml:lang="en">Piedmont is a region with ordinary statute of 4,252,581 inhabitants in north-western Italy, with the administrative capital - as well as historical capital - the city of Turin.</rdfs:comment>
        <rdfs:label xml:lang="en">Piedmont</rdfs:label>
        <rdfs:label xml:lang="it">Piemonte</rdfs:label>
    </owl:NamedIndividual>
    


    <!-- http://www.semanticweb.org/annag/ontologies/2024/1/ontoHorses#Portogallo -->

    <owl:NamedIndividual rdf:about="http://www.semanticweb.org/annag/ontologies/2024/1/ontoHorses#Portogallo">
        <rdf:type rdf:resource="http://schema.org/Place"/>
        <rdf:type rdf:resource="http://www.semanticweb.org/annag/ontologies/2024/1/ontoHorses#AreaGeografica"/>
        <schema:image rdf:resource="https://upload.wikimedia.org/wikipedia/commons/thumb/5/5c/Flag_of_Portugal.svg/1280px-Flag_of_Portugal.svg.png"/>
        <rdfs:comment xml:lang="it">Il Portogallo è uno Stato membro dell&apos;Unione europea ed è collocato nella posizione più occidentale fra tutti gli Stati dell&apos;Europa continentale.</rdfs:comment>
        <rdfs:comment xml:lang="en">Portugal is a member state of the European Union and is located in the most western position among all the states of continental Europe.</rdfs:comment>
        <rdfs:label xml:lang="it">Portogallo</rdfs:label>
    </owl:NamedIndividual>
    


    <!-- http://www.semanticweb.org/annag/ontologies/2024/1/ontoHorses#Puglia -->

    <owl:NamedIndividual rdf:about="http://www.semanticweb.org/annag/ontologies/2024/1/ontoHorses#Puglia">
        <rdf:type rdf:resource="http://schema.org/Place"/>
        <rdf:type rdf:resource="http://www.semanticweb.org/annag/ontologies/2024/1/ontoHorses#AreaGeografica"/>
        <partof:hasPart rdf:resource="http://www.semanticweb.org/annag/ontologies/2024/1/ontoHorses#taranto"/>
        <partof:isPartOf rdf:resource="http://www.semanticweb.org/annag/ontologies/2024/1/ontoHorses#Italia"/>
        <rdfs:comment xml:lang="it">La Puglia è una regione italiana a statuto ordinario dell&apos;Italia meridionale, di 3 890 250 abitanti, con capoluogo Bari.</rdfs:comment>
        <rdfs:comment xml:lang="en">Puglia is an Italian region with ordinary statute in southern Italy, with 3,890,250 inhabitants, with Bari as its capital.</rdfs:comment>
        <rdfs:label xml:lang="en">Puglia</rdfs:label>
        <rdfs:label xml:lang="it">Puglia</rdfs:label>
    </owl:NamedIndividual>
    


    <!-- http://www.semanticweb.org/annag/ontologies/2024/1/ontoHorses#PuroSangueInglese -->

    <owl:NamedIndividual rdf:about="http://www.semanticweb.org/annag/ontologies/2024/1/ontoHorses#PuroSangueInglese">
        <rdf:type rdf:resource="http://www.semanticweb.org/annag/ontologies/2024/1/ontoHorses#RazzaASangueCaldo"/>
        <rdf:type rdf:resource="http://www.semanticweb.org/annag/ontologies/2024/1/ontoHorses#RazzaCavallo"/>
        <rdf:type rdf:resource="http://www.semanticweb.org/annag/ontologies/2024/1/ontoHorses#RazzaDaSaltoOstacoli"/>
        <rdf:type rdf:resource="http://www.semanticweb.org/annag/ontologies/2024/1/ontoHorses#RazzaDaSella"/>
        <rdf:type rdf:resource="http://www.semanticweb.org/annag/ontologies/2024/1/ontoHorses#RazzaDolicomorfa"/>
        <rdf:type rdf:resource="http://www.semanticweb.org/annag/ontologies/2024/1/ontoHorses#RazzaSportiva"/>
        <ontoHorses:entitàWikidata rdf:resource="http://www.wikidata.org/entity/Q210826"/>
        <ontoHorses:haClassificazioneMorfologica rdf:resource="http://www.semanticweb.org/annag/ontologies/2024/1/ontoHorses#dolicomorfo"/>
        <ontoHorses:haIndole rdf:resource="http://www.semanticweb.org/annag/ontologies/2024/1/ontoHorses#sangueCaldo"/>
        <ontoHorses:haNazionalità rdf:resource="http://www.semanticweb.org/annag/ontologies/2024/1/ontoHorses#RegnoUnito"/>
        <ontoHorses:puòEssereImpiegataIn rdf:resource="http://www.semanticweb.org/annag/ontologies/2024/1/ontoHorses#SaltoAdOstacoli"/>
        <ontoHorses:altezzaMediaGarrese rdf:datatype="http://www.w3.org/2001/XMLSchema#integer">160</ontoHorses:altezzaMediaGarrese>
        <ontoHorses:haColoreMantello>baio</ontoHorses:haColoreMantello>
        <ontoHorses:haColoreMantello>grigio</ontoHorses:haColoreMantello>
        <ontoHorses:haColoreMantello>morello</ontoHorses:haColoreMantello>
        <ontoHorses:haColoreMantello>roano</ontoHorses:haColoreMantello>
        <ontoHorses:haColoreMantello>sauro</ontoHorses:haColoreMantello>
        <ontoHorses:pesoMedio rdf:datatype="http://www.w3.org/2001/XMLSchema#integer">425</ontoHorses:pesoMedio>
        <schema:image rdf:resource="https://www.animali.net/wp-content/uploads/2012/12/puro-sangue-inglese.jpg"/>
        <rdfs:comment xml:lang="it">Il purosangue inglese è una razza equina originaria della Gran Bretagna e i  cavalli di tale razza sono ben noti per la loro agilità e velocità</rdfs:comment>
        <rdfs:comment xml:lang="en">The English Thoroughbred is a horse breed native to Great Britain and horses of this breed are well known for their agility and speed</rdfs:comment>
        <skos:exactMatch xml:lang="it">http://www.wikidata.org/entity/Q210826</skos:exactMatch>
        <skos:prefLabel xml:lang="it">Purosangue inglese</skos:prefLabel>
        <skos:prefLabel xml:lang="en">Thoroughbred</skos:prefLabel>
    </owl:NamedIndividual>
    


    <!-- http://www.semanticweb.org/annag/ontologies/2024/1/ontoHorses#RegioneBoullonnais -->

    <owl:NamedIndividual rdf:about="http://www.semanticweb.org/annag/ontologies/2024/1/ontoHorses#RegioneBoullonnais">
        <rdf:type rdf:resource="http://schema.org/Place"/>
        <rdf:type rdf:resource="http://www.semanticweb.org/annag/ontologies/2024/1/ontoHorses#AreaGeografica"/>
        <partof:isPartOf rdf:resource="http://www.semanticweb.org/annag/ontologies/2024/1/ontoHorses#Francia"/>
        <rdfs:comment xml:lang="en">Boulonnais is a natural coastal region in France, located on the English Channel coast in the Pas-de-Calais department.</rdfs:comment>
        <rdfs:comment xml:lang="it">Il Boulonnais è una regione naturale costiera francese, situata sul litorale della Manica nel dipartimento del Passo di Calais.</rdfs:comment>
        <rdfs:label xml:lang="en">Boulonnais Region</rdfs:label>
        <rdfs:label xml:lang="it">Regione del Boulonnais</rdfs:label>
    </owl:NamedIndividual>
    


    <!-- http://www.semanticweb.org/annag/ontologies/2024/1/ontoHorses#RegioneHannover -->

    <owl:NamedIndividual rdf:about="http://www.semanticweb.org/annag/ontologies/2024/1/ontoHorses#RegioneHannover">
        <rdf:type rdf:resource="http://schema.org/Place"/>
        <rdf:type rdf:resource="http://www.semanticweb.org/annag/ontologies/2024/1/ontoHorses#AreaGeografica"/>
        <partof:isPartOf rdf:resource="http://www.semanticweb.org/annag/ontologies/2024/1/ontoHorses#Germania"/>
        <rdfs:comment xml:lang="en">Hannover is a city in north-central Germany, capital of the federal state of Lower Saxony</rdfs:comment>
        <rdfs:comment xml:lang="it">Hannover è una città della Germania centro-settentrionale, capitale dello stato federato della Bassa Sassonia</rdfs:comment>
        <rdfs:label xml:lang="it">Hannover</rdfs:label>
        <rdfs:label xml:lang="en">Hanover</rdfs:label>
    </owl:NamedIndividual>
    


    <!-- http://www.semanticweb.org/annag/ontologies/2024/1/ontoHorses#RegnoUnito -->

    <owl:NamedIndividual rdf:about="http://www.semanticweb.org/annag/ontologies/2024/1/ontoHorses#RegnoUnito">
        <rdf:type rdf:resource="http://schema.org/Place"/>
        <rdf:type rdf:resource="http://www.semanticweb.org/annag/ontologies/2024/1/ontoHorses#AreaGeografica"/>
        <partof:hasPart rdf:resource="http://www.semanticweb.org/annag/ontologies/2024/1/ontoHorses#Scozia"/>
        <schema:image rdf:resource="https://upload.wikimedia.org/wikipedia/commons/thumb/a/a5/Flag_of_the_United_Kingdom_%281-2%29.svg/1920px-Flag_of_the_United_Kingdom_%281-2%29.svg.png"/>
        <rdfs:comment xml:lang="en">The United Kingdom, officially the United Kingdom of Great Britain and Northern Ireland, is an island country in Western Europe</rdfs:comment>
        <rdfs:comment xml:lang="it">ll Regno Unito, ufficialmente Regno Unito di Gran Bretagna e Irlanda del Nord è uno Stato insulare dell&apos;Europa occidentale</rdfs:comment>
        <rdfs:label xml:lang="it">Regno Unito</rdfs:label>
        <rdfs:label xml:lang="en">United Kingdom</rdfs:label>
    </owl:NamedIndividual>
    


    <!-- http://www.semanticweb.org/annag/ontologies/2024/1/ontoHorses#SaltoAdOstacoli -->

    <owl:NamedIndividual rdf:about="http://www.semanticweb.org/annag/ontologies/2024/1/ontoHorses#SaltoAdOstacoli">
        <rdf:type rdf:resource="http://dbpedia.org/ontology/horseRidingDiscipline"/>
        <rdf:type rdf:resource="http://www.semanticweb.org/annag/ontologies/2024/1/ontoHorses#Impiego"/>
        <rdf:type rdf:resource="http://www.semanticweb.org/annag/ontologies/2024/1/ontoHorses#Sella"/>
        <rdf:type rdf:resource="http://www.semanticweb.org/annag/ontologies/2024/1/ontoHorses#SportEquestre"/>
    </owl:NamedIndividual>
    


    <!-- http://www.semanticweb.org/annag/ontologies/2024/1/ontoHorses#Schleswig-Holstein -->

    <owl:NamedIndividual rdf:about="http://www.semanticweb.org/annag/ontologies/2024/1/ontoHorses#Schleswig-Holstein">
        <rdf:type rdf:resource="http://schema.org/Place"/>
        <rdf:type rdf:resource="http://www.semanticweb.org/annag/ontologies/2024/1/ontoHorses#AreaGeografica"/>
        <partof:isPartOf rdf:resource="http://www.semanticweb.org/annag/ontologies/2024/1/ontoHorses#Germania"/>
        <rdfs:comment xml:lang="it">Lo Schleswig-Holstein è uno dei sedici Stati federati della Germania, geograficamente il più settentrionale.</rdfs:comment>
        <rdfs:comment xml:lang="en">Schleswig-Holstein is one of the sixteen federal states of Germany, geographically the northernmost.</rdfs:comment>
        <rdfs:label xml:lang="en">Schleswig-Holstein</rdfs:label>
        <rdfs:label xml:lang="it">Schleswig-Holstein</rdfs:label>
    </owl:NamedIndividual>
    


    <!-- http://www.semanticweb.org/annag/ontologies/2024/1/ontoHorses#Scozia -->

    <owl:NamedIndividual rdf:about="http://www.semanticweb.org/annag/ontologies/2024/1/ontoHorses#Scozia">
        <rdf:type rdf:resource="http://schema.org/Place"/>
        <rdf:type rdf:resource="http://www.semanticweb.org/annag/ontologies/2024/1/ontoHorses#AreaGeografica"/>
        <partof:isPartOf rdf:resource="http://www.semanticweb.org/annag/ontologies/2024/1/ontoHorses#RegnoUnito"/>
        <rdfs:comment xml:lang="it">La Scozia è una nazione costitutiva del Regno Unito che è posta all&apos;estremità settentrionale dell&apos;isola di Gran Bretagna e ne occupa più di un terzo della superficie</rdfs:comment>
        <rdfs:comment xml:lang="en">Scotland is a constituent nation of the United Kingdom which is located at the northern tip of the island of Great Britain and occupies more than a third of its surface</rdfs:comment>
        <rdfs:label xml:lang="en">Scotland</rdfs:label>
        <rdfs:label xml:lang="it">Scozia</rdfs:label>
    </owl:NamedIndividual>
    


    <!-- http://www.semanticweb.org/annag/ontologies/2024/1/ontoHorses#SellaFrancese -->

    <owl:NamedIndividual rdf:about="http://www.semanticweb.org/annag/ontologies/2024/1/ontoHorses#SellaFrancese">
        <rdf:type rdf:resource="http://www.semanticweb.org/annag/ontologies/2024/1/ontoHorses#RazzaASangueCaldo"/>
        <rdf:type rdf:resource="http://www.semanticweb.org/annag/ontologies/2024/1/ontoHorses#RazzaCavallo"/>
        <rdf:type rdf:resource="http://www.semanticweb.org/annag/ontologies/2024/1/ontoHorses#RazzaDaEquiturismo"/>
        <rdf:type rdf:resource="http://www.semanticweb.org/annag/ontologies/2024/1/ontoHorses#RazzaDaSaltoOstacoli"/>
        <rdf:type rdf:resource="http://www.semanticweb.org/annag/ontologies/2024/1/ontoHorses#RazzaDaSella"/>
        <rdf:type rdf:resource="http://www.semanticweb.org/annag/ontologies/2024/1/ontoHorses#RazzaMesoDolicomorfa"/>
        <rdf:type rdf:resource="http://www.semanticweb.org/annag/ontologies/2024/1/ontoHorses#RazzaSportiva"/>
        <ontoHorses:entitàWikidata rdf:resource="http://www.wikidata.org/entity/Q1070901"/>
        <ontoHorses:haClassificazioneMorfologica rdf:resource="http://www.semanticweb.org/annag/ontologies/2024/1/ontoHorses#mesoDolicomorfo"/>
        <ontoHorses:haIndole rdf:resource="http://www.semanticweb.org/annag/ontologies/2024/1/ontoHorses#sangueCaldo"/>
        <ontoHorses:haNazionalità rdf:resource="http://www.semanticweb.org/annag/ontologies/2024/1/ontoHorses#Francia"/>
        <ontoHorses:haRegioneDiOrigine rdf:resource="http://www.semanticweb.org/annag/ontologies/2024/1/ontoHorses#Normandia"/>
        <ontoHorses:puòEssereImpiegataIn rdf:resource="http://www.semanticweb.org/annag/ontologies/2024/1/ontoHorses#Equiturismo"/>
        <ontoHorses:puòEssereImpiegataIn rdf:resource="http://www.semanticweb.org/annag/ontologies/2024/1/ontoHorses#SaltoAdOstacoli"/>
        <ontoHorses:altezzaMediaGarrese rdf:datatype="http://www.w3.org/2001/XMLSchema#integer">165</ontoHorses:altezzaMediaGarrese>
        <ontoHorses:haColoreMantello>baio</ontoHorses:haColoreMantello>
        <ontoHorses:haColoreMantello>grigio</ontoHorses:haColoreMantello>
        <ontoHorses:haColoreMantello>morello</ontoHorses:haColoreMantello>
        <ontoHorses:haColoreMantello>sauro</ontoHorses:haColoreMantello>
        <ontoHorses:pesoMedio rdf:datatype="http://www.w3.org/2001/XMLSchema#integer">525</ontoHorses:pesoMedio>
        <schema:image rdf:resource="https://upload.wikimedia.org/wikipedia/commons/thumb/5/5a/Cheval_selle.JPG/240px-Cheval_selle.JPG"/>
        <rdfs:comment xml:lang="it">Il Selle francese è una razza popolare di cavallo da sella di origine francese, utilizzato specialmente nelle gare di salto ostacoli e nel concorso completo</rdfs:comment>
        <rdfs:comment xml:lang="en">The French Selle is a popular breed of saddle horse of French origin, used especially in show jumping and eventing</rdfs:comment>
        <skos:exactMatch xml:lang="it">http://www.wikidata.org/entity/Q1070901</skos:exactMatch>
        <skos:prefLabel xml:lang="it">Sella Francese</skos:prefLabel>
        <skos:prefLabel xml:lang="en">Selle Français</skos:prefLabel>
    </owl:NamedIndividual>
    


    <!-- http://www.semanticweb.org/annag/ontologies/2024/1/ontoHorses#SellaItaliano -->

    <owl:NamedIndividual rdf:about="http://www.semanticweb.org/annag/ontologies/2024/1/ontoHorses#SellaItaliano">
        <rdf:type rdf:resource="http://www.semanticweb.org/annag/ontologies/2024/1/ontoHorses#RazzaASangueCaldo"/>
        <rdf:type rdf:resource="http://www.semanticweb.org/annag/ontologies/2024/1/ontoHorses#RazzaCavallo"/>
        <rdf:type rdf:resource="http://www.semanticweb.org/annag/ontologies/2024/1/ontoHorses#RazzaDaDressage"/>
        <rdf:type rdf:resource="http://www.semanticweb.org/annag/ontologies/2024/1/ontoHorses#RazzaDaSaltoOstacoli"/>
        <rdf:type rdf:resource="http://www.semanticweb.org/annag/ontologies/2024/1/ontoHorses#RazzaDaSella"/>
        <rdf:type rdf:resource="http://www.semanticweb.org/annag/ontologies/2024/1/ontoHorses#RazzaMesoDolicomorfa"/>
        <rdf:type rdf:resource="http://www.semanticweb.org/annag/ontologies/2024/1/ontoHorses#RazzaSportiva"/>
        <ontoHorses:entitàWikidata rdf:resource="http://www.wikidata.org/entity/Q428039"/>
        <ontoHorses:haClassificazioneMorfologica rdf:resource="http://www.semanticweb.org/annag/ontologies/2024/1/ontoHorses#mesoDolicomorfo"/>
        <ontoHorses:haIndole rdf:resource="http://www.semanticweb.org/annag/ontologies/2024/1/ontoHorses#sangueCaldo"/>
        <ontoHorses:haNazionalità rdf:resource="http://www.semanticweb.org/annag/ontologies/2024/1/ontoHorses#Italia"/>
        <ontoHorses:puòEssereImpiegataIn rdf:resource="http://www.semanticweb.org/annag/ontologies/2024/1/ontoHorses#Dressage"/>
        <ontoHorses:puòEssereImpiegataIn rdf:resource="http://www.semanticweb.org/annag/ontologies/2024/1/ontoHorses#SaltoAdOstacoli"/>
        <ontoHorses:altezzaMediaGarrese rdf:datatype="http://www.w3.org/2001/XMLSchema#integer">160</ontoHorses:altezzaMediaGarrese>
        <ontoHorses:haColoreMantello>baio</ontoHorses:haColoreMantello>
        <ontoHorses:haColoreMantello>morello</ontoHorses:haColoreMantello>
        <ontoHorses:haColoreMantello>sauro</ontoHorses:haColoreMantello>
        <ontoHorses:pesoMedio rdf:datatype="http://www.w3.org/2001/XMLSchema#integer">500</ontoHorses:pesoMedio>
        <schema:image rdf:resource="https://www.dothorse.it/wp-content/uploads/2014/07/sella-ita.jpg"/>
        <rdfs:comment xml:lang="it">Il sella italiano è una razza equina derivante prevalentemente da incroci del purosangue inglese, arabo, anglo-arabo. E&apos; un cavallo dall&apos;aspetto elegante e nobile con la robustezza tipica del purosangue inglese e la grande affidabilità delle razze italiche.</rdfs:comment>
        <rdfs:comment xml:lang="en">The Italian saddle is a horse breed deriving mainly from crosses of the English, Arabian and Anglo-Arab thoroughbreds. It is a horse with an elegant and noble appearance with the typical robustness of the English thoroughbred and the great reliability of the Italian breeds.</rdfs:comment>
        <skos:exactMatch xml:lang="it">http://www.wikidata.org/entity/Q428039</skos:exactMatch>
        <skos:prefLabel xml:lang="en">Sella Italiano</skos:prefLabel>
        <skos:prefLabel xml:lang="it">Sella Italiano</skos:prefLabel>
    </owl:NamedIndividual>
    


    <!-- http://www.semanticweb.org/annag/ontologies/2024/1/ontoHorses#Sicilia -->

    <owl:NamedIndividual rdf:about="http://www.semanticweb.org/annag/ontologies/2024/1/ontoHorses#Sicilia">
        <rdf:type rdf:resource="http://schema.org/Place"/>
        <rdf:type rdf:resource="http://www.semanticweb.org/annag/ontologies/2024/1/ontoHorses#AreaGeografica"/>
        <partof:hasPart rdf:resource="http://www.semanticweb.org/annag/ontologies/2024/1/ontoHorses#siracusa"/>
        <partof:isPartOf rdf:resource="http://www.semanticweb.org/annag/ontologies/2024/1/ontoHorses#Italia"/>
        <rdfs:comment xml:lang="it">La Sicilia è una regione italiana a statuto speciale di 4 791 993 abitanti, con capoluogo Palermo.</rdfs:comment>
        <rdfs:comment xml:lang="en">Sicily is an Italian region with a special statute of 4,791,993 inhabitants, with Palermo as its capital.</rdfs:comment>
        <rdfs:label xml:lang="it">Sicilia</rdfs:label>
        <rdfs:label xml:lang="en">Sicily</rdfs:label>
    </owl:NamedIndividual>
    


    <!-- http://www.semanticweb.org/annag/ontologies/2024/1/ontoHorses#Spagna -->

    <owl:NamedIndividual rdf:about="http://www.semanticweb.org/annag/ontologies/2024/1/ontoHorses#Spagna">
        <rdf:type rdf:resource="http://schema.org/Place"/>
        <rdf:type rdf:resource="http://www.semanticweb.org/annag/ontologies/2024/1/ontoHorses#AreaGeografica"/>
        <partof:hasPart rdf:resource="http://www.semanticweb.org/annag/ontologies/2024/1/ontoHorses#Andalusia"/>
        <schema:image rdf:resource="https://upload.wikimedia.org/wikipedia/commons/thumb/9/9a/Flag_of_Spain.svg/1280px-Flag_of_Spain.svg.png"/>
        <rdfs:comment xml:lang="it">La Spagna è uno Stato sovrano, membro dell&apos;Unione europea dal 1986 e si trova all&apos;estremità occidentale dell&apos;Europa occupando buona parte della superficie della penisola iberica.</rdfs:comment>
        <rdfs:comment xml:lang="en">Spain is a sovereign state, member of the European Union since 1986 and is located at the western end of Europe, occupying a large part of the surface of the Iberian peninsula.</rdfs:comment>
        <rdfs:label xml:lang="it">Spagna</rdfs:label>
        <rdfs:label xml:lang="en">Spain</rdfs:label>
    </owl:NamedIndividual>
    


    <!-- http://www.semanticweb.org/annag/ontologies/2024/1/ontoHorses#TiroAgricolo -->

    <owl:NamedIndividual rdf:about="http://www.semanticweb.org/annag/ontologies/2024/1/ontoHorses#TiroAgricolo">
        <rdf:type rdf:resource="http://www.semanticweb.org/annag/ontologies/2024/1/ontoHorses#Impiego"/>
        <rdf:type rdf:resource="http://www.semanticweb.org/annag/ontologies/2024/1/ontoHorses#Lavoro"/>
        <owl:differentFrom rdf:resource="http://www.semanticweb.org/annag/ontologies/2024/1/ontoHorses#TrainoCarrozze"/>
    </owl:NamedIndividual>
    


    <!-- http://www.semanticweb.org/annag/ontologies/2024/1/ontoHorses#TrainoCarrozze -->

    <owl:NamedIndividual rdf:about="http://www.semanticweb.org/annag/ontologies/2024/1/ontoHorses#TrainoCarrozze">
        <rdf:type rdf:resource="http://www.semanticweb.org/annag/ontologies/2024/1/ontoHorses#Impiego"/>
        <rdf:type rdf:resource="http://www.semanticweb.org/annag/ontologies/2024/1/ontoHorses#Lavoro"/>
    </owl:NamedIndividual>
    


    <!-- http://www.semanticweb.org/annag/ontologies/2024/1/ontoHorses#Trakehner -->

    <owl:NamedIndividual rdf:about="http://www.semanticweb.org/annag/ontologies/2024/1/ontoHorses#Trakehner">
        <rdf:type rdf:resource="http://www.semanticweb.org/annag/ontologies/2024/1/ontoHorses#RazzaASangueMisto"/>
        <rdf:type rdf:resource="http://www.semanticweb.org/annag/ontologies/2024/1/ontoHorses#RazzaCavallo"/>
        <rdf:type rdf:resource="http://www.semanticweb.org/annag/ontologies/2024/1/ontoHorses#RazzaDaDressage"/>
        <rdf:type rdf:resource="http://www.semanticweb.org/annag/ontologies/2024/1/ontoHorses#RazzaDaSaltoOstacoli"/>
        <rdf:type rdf:resource="http://www.semanticweb.org/annag/ontologies/2024/1/ontoHorses#RazzaDaSella"/>
        <rdf:type rdf:resource="http://www.semanticweb.org/annag/ontologies/2024/1/ontoHorses#RazzaMesoDolicomorfa"/>
        <rdf:type rdf:resource="http://www.semanticweb.org/annag/ontologies/2024/1/ontoHorses#RazzaSportiva"/>
        <ontoHorses:entitàWikidata rdf:resource="http://www.wikidata.org/entity/Q843585"/>
        <ontoHorses:haClassificazioneMorfologica rdf:resource="http://www.semanticweb.org/annag/ontologies/2024/1/ontoHorses#mesoDolicomorfo"/>
        <ontoHorses:haIndole rdf:resource="http://www.semanticweb.org/annag/ontologies/2024/1/ontoHorses#sangueMisto"/>
        <ontoHorses:haNazionalità rdf:resource="http://www.semanticweb.org/annag/ontologies/2024/1/ontoHorses#Germania"/>
        <ontoHorses:puòEssereImpiegataIn rdf:resource="http://www.semanticweb.org/annag/ontologies/2024/1/ontoHorses#Dressage"/>
        <ontoHorses:puòEssereImpiegataIn rdf:resource="http://www.semanticweb.org/annag/ontologies/2024/1/ontoHorses#SaltoAdOstacoli"/>
        <ontoHorses:altezzaMediaGarrese rdf:datatype="http://www.w3.org/2001/XMLSchema#integer">165</ontoHorses:altezzaMediaGarrese>
        <ontoHorses:haColoreMantello>baio</ontoHorses:haColoreMantello>
        <ontoHorses:haColoreMantello>crema</ontoHorses:haColoreMantello>
        <ontoHorses:haColoreMantello>grigio</ontoHorses:haColoreMantello>
        <ontoHorses:haColoreMantello>morello</ontoHorses:haColoreMantello>
        <ontoHorses:haColoreMantello>palomino</ontoHorses:haColoreMantello>
        <ontoHorses:haColoreMantello>roano</ontoHorses:haColoreMantello>
        <ontoHorses:haColoreMantello>sauro</ontoHorses:haColoreMantello>
        <ontoHorses:pesoMedio rdf:datatype="http://www.w3.org/2001/XMLSchema#integer">500</ontoHorses:pesoMedio>
        <schema:image rdf:resource="https://upload.wikimedia.org/wikipedia/commons/thumb/8/8b/Trakehner_Horse.jpg/240px-Trakehner_Horse.jpg"/>
        <rdfs:comment xml:lang="it">Il Trakehner è una razza di cavallo da sella e tiro leggero più allevati e amati al mondo, attualmente utilizzato negli sport equestri</rdfs:comment>
        <rdfs:comment xml:lang="en">The Trakehner is a breed of riding and light draft horse most bred and loved in the world, currently used in equestrian sports</rdfs:comment>
        <skos:exactMatch xml:lang="it">http://www.wikidata.org/entity/Q843585</skos:exactMatch>
        <skos:prefLabel xml:lang="en">Trakehner</skos:prefLabel>
        <skos:prefLabel xml:lang="it">Trakehner</skos:prefLabel>
    </owl:NamedIndividual>
    


    <!-- http://www.semanticweb.org/annag/ontologies/2024/1/ontoHorses#TrentinoAltoAdige -->

    <owl:NamedIndividual rdf:about="http://www.semanticweb.org/annag/ontologies/2024/1/ontoHorses#TrentinoAltoAdige">
        <rdf:type rdf:resource="http://schema.org/Place"/>
        <rdf:type rdf:resource="http://www.semanticweb.org/annag/ontologies/2024/1/ontoHorses#AreaGeografica"/>
        <partof:isPartOf rdf:resource="http://www.semanticweb.org/annag/ontologies/2024/1/ontoHorses#Italia"/>
        <rdfs:comment xml:lang="it">Il Trentino-Alto Adige  è una regione italiana a statuto speciale dell&apos;Italia Nord-orientale con capoluogo Trento.</rdfs:comment>
        <rdfs:comment xml:lang="en">Trentino-Alto Adige is an Italian region with a special statute in north-eastern Italy with Trento as its capital.</rdfs:comment>
        <rdfs:label xml:lang="en">Trentino-Alto Adige</rdfs:label>
        <rdfs:label xml:lang="it">Trentino-Alto Adige</rdfs:label>
    </owl:NamedIndividual>
    


    <!-- http://www.semanticweb.org/annag/ontologies/2024/1/ontoHorses#Vestfalia -->

    <owl:NamedIndividual rdf:about="http://www.semanticweb.org/annag/ontologies/2024/1/ontoHorses#Vestfalia">
        <rdf:type rdf:resource="http://schema.org/Place"/>
        <rdf:type rdf:resource="http://www.semanticweb.org/annag/ontologies/2024/1/ontoHorses#AreaGeografica"/>
        <partof:isPartOf rdf:resource="http://www.semanticweb.org/annag/ontologies/2024/1/ontoHorses#Germania"/>
        <rdfs:comment xml:lang="it">La Vestfalia è una regione della Germania, inclusa nei land della Renania Settentrionale-Vestfalia e Bassa Sassonia.</rdfs:comment>
        <rdfs:comment xml:lang="en">Westphalia is a region of Germany, included in the states of North Rhine-Westphalia and Lower Saxony.</rdfs:comment>
        <rdfs:label xml:lang="it">Vestfalia</rdfs:label>
        <rdfs:label xml:lang="en">Westphalia</rdfs:label>
    </owl:NamedIndividual>
    


    <!-- http://www.semanticweb.org/annag/ontologies/2024/1/ontoHorses#Westfalen -->

    <owl:NamedIndividual rdf:about="http://www.semanticweb.org/annag/ontologies/2024/1/ontoHorses#Westfalen">
        <rdf:type rdf:resource="http://www.semanticweb.org/annag/ontologies/2024/1/ontoHorses#RazzaASangueCaldo"/>
        <rdf:type rdf:resource="http://www.semanticweb.org/annag/ontologies/2024/1/ontoHorses#RazzaCavallo"/>
        <rdf:type rdf:resource="http://www.semanticweb.org/annag/ontologies/2024/1/ontoHorses#RazzaDaDressage"/>
        <rdf:type rdf:resource="http://www.semanticweb.org/annag/ontologies/2024/1/ontoHorses#RazzaDaSaltoOstacoli"/>
        <rdf:type rdf:resource="http://www.semanticweb.org/annag/ontologies/2024/1/ontoHorses#RazzaDaSella"/>
        <rdf:type rdf:resource="http://www.semanticweb.org/annag/ontologies/2024/1/ontoHorses#RazzaSportiva"/>
        <rdf:type rdf:resource="http://www.semanticweb.org/annag/ontologies/2024/1/ontoHorses#RazzamMesomorfa"/>
        <ontoHorses:entitàWikidata rdf:resource="http://www.wikidata.org/entity/Q195395"/>
        <ontoHorses:haClassificazioneMorfologica rdf:resource="http://www.semanticweb.org/annag/ontologies/2024/1/ontoHorses#mesomorfo"/>
        <ontoHorses:haIndole rdf:resource="http://www.semanticweb.org/annag/ontologies/2024/1/ontoHorses#sangueCaldo"/>
        <ontoHorses:haNazionalità rdf:resource="http://www.semanticweb.org/annag/ontologies/2024/1/ontoHorses#Germania"/>
        <ontoHorses:haRegioneDiOrigine rdf:resource="http://www.semanticweb.org/annag/ontologies/2024/1/ontoHorses#Vestfalia"/>
        <ontoHorses:puòEssereImpiegataIn rdf:resource="http://www.semanticweb.org/annag/ontologies/2024/1/ontoHorses#Dressage"/>
        <ontoHorses:puòEssereImpiegataIn rdf:resource="http://www.semanticweb.org/annag/ontologies/2024/1/ontoHorses#SaltoAdOstacoli"/>
        <ontoHorses:altezzaMediaGarrese rdf:datatype="http://www.w3.org/2001/XMLSchema#integer">165</ontoHorses:altezzaMediaGarrese>
        <ontoHorses:haColoreMantello>baio</ontoHorses:haColoreMantello>
        <ontoHorses:haColoreMantello>morello</ontoHorses:haColoreMantello>
        <ontoHorses:haColoreMantello>sauro</ontoHorses:haColoreMantello>
        <ontoHorses:pesoMedio rdf:datatype="http://www.w3.org/2001/XMLSchema#integer">500</ontoHorses:pesoMedio>
        <schema:image rdf:resource="https://upload.wikimedia.org/wikipedia/commons/thumb/9/9a/Avenger_-_Westphalian_horse.jpg/240px-Avenger_-_Westphalian_horse.jpg"/>
        <rdfs:comment xml:lang="it">Il Westfalen è  un’atletica e forte razza di cavalli tedesca da sport che ha ottenuto eccellenti risultati nel concorso di salto nel dressage.</rdfs:comment>
        <rdfs:comment xml:lang="en">The Westfalen is an athletic and strong German sport horse breed that has achieved excellent results in dressage jumping competition.</rdfs:comment>
        <skos:exactMatch xml:lang="it">http://www.wikidata.org/entity/Q195395</skos:exactMatch>
        <skos:prefLabel xml:lang="it">Westfalen</skos:prefLabel>
        <skos:prefLabel xml:lang="en">Westphalian horse</skos:prefLabel>
    </owl:NamedIndividual>
    


    <!-- http://www.semanticweb.org/annag/ontologies/2024/1/ontoHorses#bergamo -->

    <owl:NamedIndividual rdf:about="http://www.semanticweb.org/annag/ontologies/2024/1/ontoHorses#bergamo">
        <rdf:type rdf:resource="http://schema.org/Place"/>
        <rdf:type rdf:resource="http://www.semanticweb.org/annag/ontologies/2024/1/ontoHorses#AreaGeografica"/>
        <partof:isPartOf rdf:resource="http://www.semanticweb.org/annag/ontologies/2024/1/ontoHorses#Italia"/>
        <partof:isPartOf rdf:resource="http://www.semanticweb.org/annag/ontologies/2024/1/ontoHorses#Lombardia"/>
        <rdfs:comment xml:lang="en">Bergamo is an Italian municipality of 120,504 inhabitants[4], capital of the province of the same name in Lombardy. The town of Bergamo is divided into two distinct parts, the «Lower City» and the «Upper City»; the latter is located at a higher altitude and hosts the majority of the most significant monuments, while the Lower City has been made partly more modern by some urbanization interventions. The two portions of the town are separated by the Venetian walls, listed since 2017 among the world heritage sites protected by UNESCO.</rdfs:comment>
        <rdfs:comment xml:lang="it">Bergamo è un comune italiano di 120 504 abitanti[4], capoluogo dell&apos;omonima provincia in Lombardia. L&apos;abitato di Bergamo è suddiviso in due parti distinte, la «Città Bassa» e la «Città Alta»; quest&apos;ultima è posta in altitudine più elevata e ospita la maggioranza dei monumenti più significativi, mentre la Città Bassa è stata resa in parte più moderna da alcuni interventi di urbanizzazione. Le due porzioni dell&apos;abitato sono separate dalle mura venete, annoverate dal 2017 fra i patrimoni dell&apos;umanità tutelati dall&apos;UNESCO.</rdfs:comment>
        <rdfs:label xml:lang="en">Bergamo</rdfs:label>
        <rdfs:label xml:lang="it">Bergamo</rdfs:label>
    </owl:NamedIndividual>
    


    <!-- http://www.semanticweb.org/annag/ontologies/2024/1/ontoHorses#brachimorfo -->

    <owl:NamedIndividual rdf:about="http://www.semanticweb.org/annag/ontologies/2024/1/ontoHorses#brachimorfo">
        <rdf:type rdf:resource="http://www.semanticweb.org/annag/ontologies/2024/1/ontoHorses#Morfologia"/>
        <rdf:type rdf:resource="http://www.semanticweb.org/annag/ontologies/2024/1/ontoHorses#RazzaCavallo"/>
        <rdfs:comment xml:lang="it">Morfologia del cavallo caratterizzata da muscolatura molto sviluppata,  torace ampio, forme potenti, massicce e non molto lungo.</rdfs:comment>
        <rdfs:comment xml:lang="en">Morphology of the horse characterized by highly developed musculature, wide chest, powerful, massive shape and not very long.</rdfs:comment>
        <rdfs:label xml:lang="en">Brachimorphic morphology</rdfs:label>
        <rdfs:label xml:lang="it">brachimorfo</rdfs:label>
    </owl:NamedIndividual>
    


    <!-- http://www.semanticweb.org/annag/ontologies/2024/1/ontoHorses#brevetto -->

    <owl:NamedIndividual rdf:about="http://www.semanticweb.org/annag/ontologies/2024/1/ontoHorses#brevetto">
        <rdf:type rdf:resource="http://www.ontologydesignpatterns.org/cp/owl/bag.owl#Item"/>
        <rdf:type rdf:resource="http://www.ontologydesignpatterns.org/cp/owl/list.owl#ListItem"/>
        <rdf:type rdf:resource="http://www.semanticweb.org/annag/ontologies/2024/1/ontoHorses#Patente"/>
        <bag:itemOf rdf:resource="http://www.semanticweb.org/annag/ontologies/2024/1/ontoHorses#patenteAgonistica"/>
        <collectionentity:isMemberOf rdf:resource="http://www.semanticweb.org/annag/ontologies/2024/1/ontoHorses#patenteAgonistica"/>
        <sequence:precedes rdf:resource="http://www.semanticweb.org/annag/ontologies/2024/1/ontoHorses#primoGrado"/>
        <sequence:precedes rdf:resource="http://www.semanticweb.org/annag/ontologies/2024/1/ontoHorses#secondoGrado"/>
        <ontoHorses:vieneConseguitoDa rdf:resource="http://www.semanticweb.org/annag/ontologies/2024/1/ontoHorses#CavalierePrincipiante"/>
        <rdfs:comment xml:lang="en">Authorizes the practice of competitive equestrian sports based on the specific specialty of the license acquired by the rider. Thebrevetto authorizes participation in show jumping competitions of category C80 or higher</rdfs:comment>
        <rdfs:comment xml:lang="it">Autorizza all’esercizio della pratica sportiva agonistica degli sport equestri in funzione della specifica specialità del brevetto acquisito dal cavaliere. Il brevetto autorizza a partecipare a gare di salto ad ostacoli di categoria C80 o superiore</rdfs:comment>
        <rdfs:label xml:lang="en">brevetto</rdfs:label>
        <rdfs:label xml:lang="it">brevetto</rdfs:label>
    </owl:NamedIndividual>
    


    <!-- http://www.semanticweb.org/annag/ontologies/2024/1/ontoHorses#brunoGramaglia -->

    <owl:NamedIndividual rdf:about="http://www.semanticweb.org/annag/ontologies/2024/1/ontoHorses#brunoGramaglia">
        <rdf:type rdf:resource="http://www.semanticweb.org/annag/ontologies/2024/1/ontoHorses#Persona"/>
        <rdf:type rdf:resource="http://www.semanticweb.org/annag/ontologies/2024/1/ontoHorses#Proprietario"/>
        <rdf:type rdf:resource="http://xmlns.com/foaf/0.1/person"/>
        <ontoHorses:possiede rdf:resource="http://www.semanticweb.org/annag/ontologies/2024/1/ontoHorses#CastroneItaliano"/>
        <ontoHorses:possiede rdf:resource="http://www.semanticweb.org/annag/ontologies/2024/1/ontoHorses#MaschioAndaluso"/>
        <ontoHorses:possiede rdf:resource="http://www.semanticweb.org/annag/ontologies/2024/1/ontoHorses#MaschioPuroSangueInglese"/>
        <rdfs:comment xml:lang="it">Allevatore e commerciante di cavalli con sede a Leinì (To)</rdfs:comment>
        <rdfs:comment xml:lang="en">Horse breeder and trader based in Leinì (To)</rdfs:comment>
        <rdfs:label xml:lang="en">Bruno Gramaglia</rdfs:label>
        <rdfs:label xml:lang="it">Bruno Gramaglia</rdfs:label>
    </owl:NamedIndividual>
    


    <!-- http://www.semanticweb.org/annag/ontologies/2024/1/ontoHorses#claudioCavallo -->

    <owl:NamedIndividual rdf:about="http://www.semanticweb.org/annag/ontologies/2024/1/ontoHorses#claudioCavallo">
        <rdf:type rdf:resource="http://www.semanticweb.org/annag/ontologies/2024/1/ontoHorses#Persona"/>
        <rdf:type rdf:resource="http://www.semanticweb.org/annag/ontologies/2024/1/ontoHorses#Proprietario"/>
        <rdf:type rdf:resource="http://xmlns.com/foaf/0.1/person"/>
        <ontoHorses:possiede rdf:resource="http://www.semanticweb.org/annag/ontologies/2024/1/ontoHorses#CastroneAngloAraboFrancese"/>
        <ontoHorses:possiede rdf:resource="http://www.semanticweb.org/annag/ontologies/2024/1/ontoHorses#FemminaBretone"/>
        <ontoHorses:possiede rdf:resource="http://www.semanticweb.org/annag/ontologies/2024/1/ontoHorses#FemminaMaremmano"/>
        <rdfs:comment xml:lang="it">Allevatore e commerciante di cavalli con sede a Siracusa (SR)</rdfs:comment>
        <rdfs:comment xml:lang="en">Horse breeder and trader based in Syracuse (SR)</rdfs:comment>
        <rdfs:label xml:lang="en">Claudio Cavallo</rdfs:label>
        <rdfs:label xml:lang="it">Claudio Cavallo</rdfs:label>
    </owl:NamedIndividual>
    


    <!-- http://www.semanticweb.org/annag/ontologies/2024/1/ontoHorses#dolicomorfo -->

    <owl:NamedIndividual rdf:about="http://www.semanticweb.org/annag/ontologies/2024/1/ontoHorses#dolicomorfo">
        <rdf:type rdf:resource="http://www.semanticweb.org/annag/ontologies/2024/1/ontoHorses#Morfologia"/>
        <rdf:type rdf:resource="http://www.semanticweb.org/annag/ontologies/2024/1/ontoHorses#RazzaCavallo"/>
        <rdfs:comment xml:lang="it">Morfologia caratterizzata da  torace profondo, linee allungate e articolazioni con angoli molto aperti. La figura è agile, leggera e slanciata.</rdfs:comment>
        <rdfs:comment xml:lang="en">Morphology characterized by deep chest, elongated lines and joints with very open angles. The figure is agile, light and slender.</rdfs:comment>
        <rdfs:label xml:lang="it">dolicomorfo</rdfs:label>
        <rdfs:label xml:lang="en">dolicomorphic morphology</rdfs:label>
    </owl:NamedIndividual>
    


    <!-- http://www.semanticweb.org/annag/ontologies/2024/1/ontoHorses#francescoBertero -->

    <owl:NamedIndividual rdf:about="http://www.semanticweb.org/annag/ontologies/2024/1/ontoHorses#francescoBertero">
        <rdf:type rdf:resource="http://www.semanticweb.org/annag/ontologies/2024/1/ontoHorses#Persona"/>
        <rdf:type rdf:resource="http://www.semanticweb.org/annag/ontologies/2024/1/ontoHorses#Proprietario"/>
        <rdf:type rdf:resource="http://xmlns.com/foaf/0.1/person"/>
        <rdfs:comment xml:lang="it">Allevatore e commerciante di cavalli con sede a Bergamo (BG)</rdfs:comment>
        <rdfs:comment xml:lang="en">Horse breeder and trader based in Bergamo (BG)</rdfs:comment>
        <rdfs:label xml:lang="en">Francesco Bertero</rdfs:label>
        <rdfs:label xml:lang="it">Francesco Bertero</rdfs:label>
    </owl:NamedIndividual>
    


    <!-- http://www.semanticweb.org/annag/ontologies/2024/1/ontoHorses#gianlucaCamoletto -->

    <owl:NamedIndividual rdf:about="http://www.semanticweb.org/annag/ontologies/2024/1/ontoHorses#gianlucaCamoletto">
        <rdf:type rdf:resource="http://www.semanticweb.org/annag/ontologies/2024/1/ontoHorses#Persona"/>
        <rdf:type rdf:resource="http://www.semanticweb.org/annag/ontologies/2024/1/ontoHorses#Proprietario"/>
        <rdf:type rdf:resource="http://xmlns.com/foaf/0.1/person"/>
        <ontoHorses:possiede rdf:resource="http://www.semanticweb.org/annag/ontologies/2024/1/ontoHorses#CastroneFrancese"/>
        <ontoHorses:possiede rdf:resource="http://www.semanticweb.org/annag/ontologies/2024/1/ontoHorses#MaschioOlandese"/>
        <rdfs:comment xml:lang="it">Allevatore e commerciante di cavalli con sede in Leinì (TO)</rdfs:comment>
        <rdfs:comment xml:lang="en">Horse breeder and trader based in Leinì (TO)</rdfs:comment>
        <rdfs:label xml:lang="en">Gianluca Camoletto</rdfs:label>
        <rdfs:label xml:lang="it">Gianluca Camoletto</rdfs:label>
    </owl:NamedIndividual>
    


    <!-- http://www.semanticweb.org/annag/ontologies/2024/1/ontoHorses#leini -->

    <owl:NamedIndividual rdf:about="http://www.semanticweb.org/annag/ontologies/2024/1/ontoHorses#leini">
        <rdf:type rdf:resource="http://schema.org/Place"/>
        <rdf:type rdf:resource="http://www.semanticweb.org/annag/ontologies/2024/1/ontoHorses#AreaGeografica"/>
        <partof:isPartOf rdf:resource="http://www.semanticweb.org/annag/ontologies/2024/1/ontoHorses#Italia"/>
        <partof:isPartOf rdf:resource="http://www.semanticweb.org/annag/ontologies/2024/1/ontoHorses#Piemonte"/>
        <rdfs:comment xml:lang="en">Leini is an Italian municipality of 16,340 inhabitants in the metropolitan city of Turin in Piedmont.</rdfs:comment>
        <rdfs:comment xml:lang="it">Leini è un comune italiano di 16 340 abitanti della città metropolitana di Torino in Piemonte.</rdfs:comment>
        <rdfs:label xml:lang="en">Leinì</rdfs:label>
        <rdfs:label xml:lang="it">Leinì</rdfs:label>
    </owl:NamedIndividual>
    


    <!-- http://www.semanticweb.org/annag/ontologies/2024/1/ontoHorses#mesoBrachimorfo -->

    <owl:NamedIndividual rdf:about="http://www.semanticweb.org/annag/ontologies/2024/1/ontoHorses#mesoBrachimorfo">
        <rdf:type rdf:resource="http://www.semanticweb.org/annag/ontologies/2024/1/ontoHorses#Morfologia"/>
        <rdf:type rdf:resource="http://www.semanticweb.org/annag/ontologies/2024/1/ontoHorses#RazzaCavallo"/>
        <rdfs:comment xml:lang="it">Morfologia a metà strada tra quella dei cavalli da tiro e quella  dei cavalli da sella.</rdfs:comment>
        <rdfs:comment xml:lang="en">Morphology halfway between that of draft horses and that of riding horses.</rdfs:comment>
        <rdfs:label xml:lang="it">meso-brachimorfo</rdfs:label>
        <rdfs:label xml:lang="en">meso-brachimorphic morfology</rdfs:label>
    </owl:NamedIndividual>
    


    <!-- http://www.semanticweb.org/annag/ontologies/2024/1/ontoHorses#mesoDolicomorfo -->

    <owl:NamedIndividual rdf:about="http://www.semanticweb.org/annag/ontologies/2024/1/ontoHorses#mesoDolicomorfo">
        <rdf:type rdf:resource="http://www.semanticweb.org/annag/ontologies/2024/1/ontoHorses#Morfologia"/>
        <rdf:type rdf:resource="http://www.semanticweb.org/annag/ontologies/2024/1/ontoHorses#RazzaCavallo"/>
        <rdfs:comment xml:lang="it">Morfologia potente, forte ma contemporaneamente agile e nobile nel portamento.</rdfs:comment>
        <rdfs:comment xml:lang="en">Powerful morphology, strong but at the same time agile and noble in bearing.</rdfs:comment>
        <rdfs:label xml:lang="it">meso-dolicomorfo</rdfs:label>
        <rdfs:label xml:lang="en">meso-dolicomorphic morphology</rdfs:label>
    </owl:NamedIndividual>
    


    <!-- http://www.semanticweb.org/annag/ontologies/2024/1/ontoHorses#mesomorfo -->

    <owl:NamedIndividual rdf:about="http://www.semanticweb.org/annag/ontologies/2024/1/ontoHorses#mesomorfo">
        <rdf:type rdf:resource="http://www.semanticweb.org/annag/ontologies/2024/1/ontoHorses#Morfologia"/>
        <rdf:type rdf:resource="http://www.semanticweb.org/annag/ontologies/2024/1/ontoHorses#RazzaCavallo"/>
        <rdfs:comment xml:lang="it">Morfologia caratterizzata da una struttura fisica molto più leggera rispetto al brachimorfo, ma comunque potente e compatta.</rdfs:comment>
        <rdfs:comment xml:lang="en">Morphology characterized by a much lighter physical structure than the brachymorph, but still powerful and compact.</rdfs:comment>
        <rdfs:label xml:lang="en">Mesomorphic morfology</rdfs:label>
        <rdfs:label xml:lang="it">mesomorfo</rdfs:label>
    </owl:NamedIndividual>
    


    <!-- http://www.semanticweb.org/annag/ontologies/2024/1/ontoHorses#paoloGrassi -->

    <owl:NamedIndividual rdf:about="http://www.semanticweb.org/annag/ontologies/2024/1/ontoHorses#paoloGrassi">
        <rdf:type rdf:resource="http://www.semanticweb.org/annag/ontologies/2024/1/ontoHorses#Persona"/>
        <rdf:type rdf:resource="http://www.semanticweb.org/annag/ontologies/2024/1/ontoHorses#Proprietario"/>
        <rdf:type rdf:resource="http://xmlns.com/foaf/0.1/person"/>
        <ontoHorses:possiede rdf:resource="http://www.semanticweb.org/annag/ontologies/2024/1/ontoHorses#FemminaMurgese"/>
        <ontoHorses:possiede rdf:resource="http://www.semanticweb.org/annag/ontologies/2024/1/ontoHorses#MaschioTedesco"/>
        <rdfs:comment xml:lang="it">Allevatore e commerciante di cavalli con sede a Taranto (TA)</rdfs:comment>
        <rdfs:comment xml:lang="en">Horse breeder and trader based in Taranto (TA)</rdfs:comment>
        <rdfs:label xml:lang="en">Paolo Grassi</rdfs:label>
        <rdfs:label xml:lang="it">Paolo Grassi</rdfs:label>
    </owl:NamedIndividual>
    


    <!-- http://www.semanticweb.org/annag/ontologies/2024/1/ontoHorses#patenteAgonistica -->

    <owl:NamedIndividual rdf:about="http://www.semanticweb.org/annag/ontologies/2024/1/ontoHorses#patenteAgonistica">
        <rdf:type rdf:resource="http://www.ontologydesignpatterns.org/cp/owl/bag.owl#Bag"/>
        <rdf:type rdf:resource="http://www.ontologydesignpatterns.org/cp/owl/collectionentity.owl#Collection"/>
        <rdf:type rdf:resource="http://www.ontologydesignpatterns.org/cp/owl/list.owl#List"/>
        <rdf:type rdf:resource="http://www.semanticweb.org/annag/ontologies/2024/1/ontoHorses#CatalogoAutorizzazioniAMontareFise"/>
        <bag:hasItem rdf:resource="http://www.semanticweb.org/annag/ontologies/2024/1/ontoHorses#brevetto"/>
        <bag:hasItem rdf:resource="http://www.semanticweb.org/annag/ontologies/2024/1/ontoHorses#primoGrado"/>
        <bag:hasItem rdf:resource="http://www.semanticweb.org/annag/ontologies/2024/1/ontoHorses#secondoGrado"/>
        <collectionentity:hasMember rdf:resource="http://www.semanticweb.org/annag/ontologies/2024/1/ontoHorses#brevetto"/>
        <collectionentity:hasMember rdf:resource="http://www.semanticweb.org/annag/ontologies/2024/1/ontoHorses#primoGrado"/>
        <collectionentity:hasMember rdf:resource="http://www.semanticweb.org/annag/ontologies/2024/1/ontoHorses#secondoGrado"/>
        <sequence:follows rdf:resource="http://www.semanticweb.org/annag/ontologies/2024/1/ontoHorses#patenteNonAgonistica"/>
        <rdfs:comment xml:lang="en">License that enables the practice of competitive sports</rdfs:comment>
        <rdfs:comment xml:lang="it">Patente che abilita all&apos;esercizio della pratica sportiva agonistica</rdfs:comment>
        <rdfs:label xml:lang="en">Competitive license</rdfs:label>
        <rdfs:label xml:lang="it">Patente agonistica</rdfs:label>
    </owl:NamedIndividual>
    


    <!-- http://www.semanticweb.org/annag/ontologies/2024/1/ontoHorses#patenteLudicaA -->

    <owl:NamedIndividual rdf:about="http://www.semanticweb.org/annag/ontologies/2024/1/ontoHorses#patenteLudicaA">
        <rdf:type rdf:resource="http://www.ontologydesignpatterns.org/cp/owl/bag.owl#Item"/>
        <rdf:type rdf:resource="http://www.ontologydesignpatterns.org/cp/owl/list.owl#ListItem"/>
        <rdf:type rdf:resource="http://www.semanticweb.org/annag/ontologies/2024/1/ontoHorses#Patente"/>
        <bag:itemOf rdf:resource="http://www.semanticweb.org/annag/ontologies/2024/1/ontoHorses#patenteNonAgonistica"/>
        <collectionentity:isMemberOf rdf:resource="http://www.semanticweb.org/annag/ontologies/2024/1/ontoHorses#patenteNonAgonistica"/>
        <ontoHorses:vieneConseguitoDa rdf:resource="http://www.semanticweb.org/annag/ontologies/2024/1/ontoHorses#CavalierePrincipiante"/>
        <rdfs:comment xml:lang="en">Authorizes the practice of recreational and training equestrian sports in any discipline.</rdfs:comment>
        <rdfs:comment xml:lang="it">Autorizza all’esercizio della pratica sportiva ludico-addestrativa degli sport equestri in qualsiasi disciplina.</rdfs:comment>
        <rdfs:label xml:lang="en">Patente ludica A</rdfs:label>
        <rdfs:label xml:lang="it">Patente ludica A</rdfs:label>
    </owl:NamedIndividual>
    


    <!-- http://www.semanticweb.org/annag/ontologies/2024/1/ontoHorses#patenteNonAgonistica -->

    <owl:NamedIndividual rdf:about="http://www.semanticweb.org/annag/ontologies/2024/1/ontoHorses#patenteNonAgonistica">
        <rdf:type rdf:resource="http://www.ontologydesignpatterns.org/cp/owl/bag.owl#Bag"/>
        <rdf:type rdf:resource="http://www.ontologydesignpatterns.org/cp/owl/collectionentity.owl#Collection"/>
        <rdf:type rdf:resource="http://www.ontologydesignpatterns.org/cp/owl/list.owl#List"/>
        <rdf:type rdf:resource="http://www.semanticweb.org/annag/ontologies/2024/1/ontoHorses#CatalogoAutorizzazioniAMontareFise"/>
        <bag:hasItem rdf:resource="http://www.semanticweb.org/annag/ontologies/2024/1/ontoHorses#patenteLudicaA"/>
        <collectionentity:hasMember rdf:resource="http://www.semanticweb.org/annag/ontologies/2024/1/ontoHorses#patenteLudicaA"/>
        <sequence:precedes rdf:resource="http://www.semanticweb.org/annag/ontologies/2024/1/ontoHorses#patenteAgonistica"/>
        <rdfs:comment xml:lang="en">Authorizes the practice of recreational and training equestrian sports and social integration activities through sport</rdfs:comment>
        <rdfs:comment xml:lang="it">Autorizza all&apos;esercizio della pratica sportiva equestre ludico-addestrativa e alle attività di integrazione sociale attraverso lo sport</rdfs:comment>
        <rdfs:label xml:lang="en">Not competitive licence</rdfs:label>
        <rdfs:label xml:lang="it">Patente non agonistica</rdfs:label>
    </owl:NamedIndividual>
    


    <!-- http://www.semanticweb.org/annag/ontologies/2024/1/ontoHorses#primoGrado -->

    <owl:NamedIndividual rdf:about="http://www.semanticweb.org/annag/ontologies/2024/1/ontoHorses#primoGrado">
        <rdf:type rdf:resource="http://www.ontologydesignpatterns.org/cp/owl/bag.owl#Item"/>
        <rdf:type rdf:resource="http://www.ontologydesignpatterns.org/cp/owl/list.owl#ListItem"/>
        <rdf:type rdf:resource="http://www.semanticweb.org/annag/ontologies/2024/1/ontoHorses#Patente"/>
        <bag:itemOf rdf:resource="http://www.semanticweb.org/annag/ontologies/2024/1/ontoHorses#patenteAgonistica"/>
        <collectionentity:isMemberOf rdf:resource="http://www.semanticweb.org/annag/ontologies/2024/1/ontoHorses#patenteAgonistica"/>
        <sequence:follows rdf:resource="http://www.semanticweb.org/annag/ontologies/2024/1/ontoHorses#brevetto"/>
        <sequence:precedes rdf:resource="http://www.semanticweb.org/annag/ontologies/2024/1/ontoHorses#secondoGrado"/>
        <ontoHorses:vieneConseguitoDa rdf:resource="http://www.semanticweb.org/annag/ontologies/2024/1/ontoHorses#CavaliereEsperto"/>
        <ontoHorses:vieneConseguitoDa rdf:resource="http://www.semanticweb.org/annag/ontologies/2024/1/ontoHorses#CavaliereIntermedio"/>
        <rdfs:comment xml:lang="en">Authorizes the practice of competitive equestrian sports based on the specific specialty of the license acquired by the rider. The 1° grado authorizes participation in show jumping competitions of category C115 or higher</rdfs:comment>
        <rdfs:comment xml:lang="it">Autorizza all’esercizio della pratica sportiva agonistica degli sport equestri in funzione della specifica specialità del brevetto acquisito dal cavaliere. Il 1° grado autorizza a partecipare a gare di salto ad ostacoli di categoria C115 o superiore</rdfs:comment>
        <rdfs:label xml:lang="en">1° grado</rdfs:label>
        <rdfs:label xml:lang="it">1° grado</rdfs:label>
    </owl:NamedIndividual>
    


    <!-- http://www.semanticweb.org/annag/ontologies/2024/1/ontoHorses#sanMauro -->

    <owl:NamedIndividual rdf:about="http://www.semanticweb.org/annag/ontologies/2024/1/ontoHorses#sanMauro">
        <rdf:type rdf:resource="http://schema.org/Place"/>
        <rdf:type rdf:resource="http://www.semanticweb.org/annag/ontologies/2024/1/ontoHorses#AreaGeografica"/>
        <partof:isPartOf rdf:resource="http://www.semanticweb.org/annag/ontologies/2024/1/ontoHorses#Italia"/>
        <partof:isPartOf rdf:resource="http://www.semanticweb.org/annag/ontologies/2024/1/ontoHorses#Piemonte"/>
        <rdfs:comment xml:lang="en">San Mauro Torinese is an Italian municipality of 18,922 inhabitants in the metropolitan city of Turin, in Piedmont.</rdfs:comment>
        <rdfs:comment xml:lang="it">San Mauro Torinese è un comune italiano di 18.922 abitanti della città metropolitana di Torino, in Piemonte.</rdfs:comment>
        <rdfs:label xml:lang="en">San Mauro Torinese</rdfs:label>
        <rdfs:label xml:lang="it">San Mauro Torinese</rdfs:label>
    </owl:NamedIndividual>
    


    <!-- http://www.semanticweb.org/annag/ontologies/2024/1/ontoHorses#sangueCaldo -->

    <owl:NamedIndividual rdf:about="http://www.semanticweb.org/annag/ontologies/2024/1/ontoHorses#sangueCaldo">
        <rdf:type rdf:resource="http://www.semanticweb.org/annag/ontologies/2024/1/ontoHorses#Indole"/>
        <rdfs:comment xml:lang="it">E&apos; una categoria di razze di cavalli, classificate sulla base del temperamento, generalmente molto reattive adatte all&apos;impiego nelle attività sportive equestri</rdfs:comment>
        <rdfs:comment xml:lang="en">It is a category of horses, classified on the basis of temperament, generally suitable for use in equestrian sporting activities</rdfs:comment>
        <rdfs:label xml:lang="it">sangue caldo</rdfs:label>
        <rdfs:label xml:lang="en">warm blooded horses</rdfs:label>
    </owl:NamedIndividual>
    


    <!-- http://www.semanticweb.org/annag/ontologies/2024/1/ontoHorses#sangueFreddo -->

    <owl:NamedIndividual rdf:about="http://www.semanticweb.org/annag/ontologies/2024/1/ontoHorses#sangueFreddo">
        <rdf:type rdf:resource="http://www.semanticweb.org/annag/ontologies/2024/1/ontoHorses#Indole"/>
        <rdfs:comment xml:lang="it">E&apos; una categoria di razze di cavalli, classificate sulla base del temperamento, che derivano da linee di sangue di razze di cavalli da lavoro. Sono razze di cavalli molto docili e tranquilli. Necessitano maggiore impegno nell’addestramento e sollecitazioni nel lavoro.</rdfs:comment>
        <rdfs:comment xml:lang="en">It is a category of horses, classified on the basis of temperament, which derive from bloodlines of working horses. They are very docile and calm horses. They require greater commitment to training and stress at work.</rdfs:comment>
        <rdfs:label xml:lang="en">cold blood</rdfs:label>
        <rdfs:label xml:lang="it">sangue freddo</rdfs:label>
    </owl:NamedIndividual>
    


    <!-- http://www.semanticweb.org/annag/ontologies/2024/1/ontoHorses#sangueMisto -->

    <owl:NamedIndividual rdf:about="http://www.semanticweb.org/annag/ontologies/2024/1/ontoHorses#sangueMisto">
        <rdf:type rdf:resource="http://www.semanticweb.org/annag/ontologies/2024/1/ontoHorses#Indole"/>
        <rdfs:comment xml:lang="it">E&apos; una categoria di razze di cavalli, classificate sulla base del temperamento, che presentano caratteristiche ibride tra le razze a sangue caldo e quelle a sangue freddo</rdfs:comment>
        <rdfs:comment xml:lang="en">It is a category of horse breeds, classified on the basis of temperament, which present hybrid characteristics between warm-blooded and cold-blooded breeds.</rdfs:comment>
        <rdfs:label xml:lang="en">mixed blood</rdfs:label>
        <rdfs:label xml:lang="it">sangue misto</rdfs:label>
    </owl:NamedIndividual>
    


    <!-- http://www.semanticweb.org/annag/ontologies/2024/1/ontoHorses#secondoGrado -->

    <owl:NamedIndividual rdf:about="http://www.semanticweb.org/annag/ontologies/2024/1/ontoHorses#secondoGrado">
        <rdf:type rdf:resource="http://www.ontologydesignpatterns.org/cp/owl/bag.owl#Item"/>
        <rdf:type rdf:resource="http://www.ontologydesignpatterns.org/cp/owl/list.owl#ListItem"/>
        <rdf:type rdf:resource="http://www.semanticweb.org/annag/ontologies/2024/1/ontoHorses#Patente"/>
        <bag:itemOf rdf:resource="http://www.semanticweb.org/annag/ontologies/2024/1/ontoHorses#patenteAgonistica"/>
        <collectionentity:isMemberOf rdf:resource="http://www.semanticweb.org/annag/ontologies/2024/1/ontoHorses#patenteAgonistica"/>
        <sequence:follows rdf:resource="http://www.semanticweb.org/annag/ontologies/2024/1/ontoHorses#brevetto"/>
        <sequence:follows rdf:resource="http://www.semanticweb.org/annag/ontologies/2024/1/ontoHorses#primoGrado"/>
        <ontoHorses:vieneConseguitoDa rdf:resource="http://www.semanticweb.org/annag/ontologies/2024/1/ontoHorses#CavaliereMoltoEsperto"/>
        <rdfs:comment xml:lang="en">Authorizes the practice of competitive equestrian sports based on the specific specialty of the license acquired by the rider. The 2° grado authorizes participation in show jumping competitions of category C135 or higher</rdfs:comment>
        <rdfs:comment xml:lang="it">Autorizza all’esercizio della pratica sportiva agonistica degli sport equestri in funzione della specifica specialità del brevetto acquisito dal cavaliere. Il 2° grado autorizza a partecipare a gare di salto ad ostacoli di categoria C135 o superiore</rdfs:comment>
        <rdfs:label xml:lang="en">2° grado</rdfs:label>
        <rdfs:label xml:lang="it">2° grado</rdfs:label>
    </owl:NamedIndividual>
    


    <!-- http://www.semanticweb.org/annag/ontologies/2024/1/ontoHorses#siracusa -->

    <owl:NamedIndividual rdf:about="http://www.semanticweb.org/annag/ontologies/2024/1/ontoHorses#siracusa">
        <rdf:type rdf:resource="http://schema.org/Place"/>
        <rdf:type rdf:resource="http://www.semanticweb.org/annag/ontologies/2024/1/ontoHorses#AreaGeografica"/>
        <partof:isPartOf rdf:resource="http://www.semanticweb.org/annag/ontologies/2024/1/ontoHorses#Italia"/>
        <partof:isPartOf rdf:resource="http://www.semanticweb.org/annag/ontologies/2024/1/ontoHorses#Sicilia"/>
        <rdfs:comment xml:lang="it">Siracusa è un comune italiano di 115 681 abitanti, capoluogo del libero consorzio comunale omonimo, in Sicilia.</rdfs:comment>
        <rdfs:comment xml:lang="en">Syracuse is an Italian municipality of 115,681 inhabitants, capital of the free municipal consortium of the same name, in Sicily.</rdfs:comment>
        <rdfs:label xml:lang="it">Siracusa</rdfs:label>
        <rdfs:label xml:lang="en">Syracuse</rdfs:label>
    </owl:NamedIndividual>
    


    <!-- http://www.semanticweb.org/annag/ontologies/2024/1/ontoHorses#taranto -->

    <owl:NamedIndividual rdf:about="http://www.semanticweb.org/annag/ontologies/2024/1/ontoHorses#taranto">
        <rdf:type rdf:resource="http://schema.org/Place"/>
        <rdf:type rdf:resource="http://www.semanticweb.org/annag/ontologies/2024/1/ontoHorses#AreaGeografica"/>
        <partof:isPartOf rdf:resource="http://www.semanticweb.org/annag/ontologies/2024/1/ontoHorses#Italia"/>
        <partof:isPartOf rdf:resource="http://www.semanticweb.org/annag/ontologies/2024/1/ontoHorses#Puglia"/>
        <rdfs:comment xml:lang="en">Taranto is an Italian municipality of 186,798 inhabitants, capital of the province of the same name, in Puglia.</rdfs:comment>
        <rdfs:comment xml:lang="it">Taranto è un comune italiano di 186 798 abitanti, capoluogo dell&apos;omonima provincia, in Puglia.</rdfs:comment>
        <rdfs:label xml:lang="en">Taranto</rdfs:label>
        <rdfs:label xml:lang="it">Taranto</rdfs:label>
    </owl:NamedIndividual>
    


    <!-- http://www.semanticweb.org/annag/ontologies/2024/1/ontoHorses#12000Euro -->

    <owl:NamedIndividual rdf:about="http://www.semanticweb.org/annag/ontologies/2024/1/ontoHorses#12000Euro">
        <rdf:type rdf:resource="http://www.ontologydesignpatterns.org/cp/owl/price.owl#Price"/>
        <price:hasCurrency rdf:resource="http://www.semanticweb.org/annag/ontologies/2024/1/ontoHorses#Euro"/>
        <price:isPriceOf rdf:resource="http://www.semanticweb.org/annag/ontologies/2024/1/ontoHorses#CastroneItaliano"/>
        <price:hasValue rdf:datatype="http://www.w3.org/2001/XMLSchema#float">12000.0</price:hasValue>
        <rdfs:comment xml:lang="it">12000 Euro</rdfs:comment>
        <rdfs:label xml:lang="it">12000 Euro</rdfs:label>
    </owl:NamedIndividual>
    


    <!-- http://www.semanticweb.org/annag/ontologies/2024/1/ontoHorses#15000Euro -->

    <owl:NamedIndividual rdf:about="http://www.semanticweb.org/annag/ontologies/2024/1/ontoHorses#15000Euro">
        <rdf:type rdf:resource="http://www.ontologydesignpatterns.org/cp/owl/price.owl#Price"/>
        <price:hasCurrency rdf:resource="http://www.semanticweb.org/annag/ontologies/2024/1/ontoHorses#Euro"/>
        <price:isPriceOf rdf:resource="http://www.semanticweb.org/annag/ontologies/2024/1/ontoHorses#CastroneAngloAraboFrancese"/>
        <price:isPriceOf rdf:resource="http://www.semanticweb.org/annag/ontologies/2024/1/ontoHorses#MaschioTedesco"/>
        <price:hasValue rdf:datatype="http://www.w3.org/2001/XMLSchema#float">15000.0</price:hasValue>
        <rdfs:comment xml:lang="it">15000 Euro</rdfs:comment>
        <rdfs:label xml:lang="it">15000 Euro</rdfs:label>
    </owl:NamedIndividual>
    


    <!-- http://www.semanticweb.org/annag/ontologies/2024/1/ontoHorses#18000Euro -->

    <owl:NamedIndividual rdf:about="http://www.semanticweb.org/annag/ontologies/2024/1/ontoHorses#18000Euro">
        <rdf:type rdf:resource="http://www.ontologydesignpatterns.org/cp/owl/price.owl#Price"/>
        <price:hasCurrency rdf:resource="http://www.semanticweb.org/annag/ontologies/2024/1/ontoHorses#Euro"/>
        <price:isPriceOf rdf:resource="http://www.semanticweb.org/annag/ontologies/2024/1/ontoHorses#CastroneFrancese"/>
        <price:hasValue rdf:datatype="http://www.w3.org/2001/XMLSchema#float">18000.0</price:hasValue>
        <rdfs:comment xml:lang="it">18000 Euro</rdfs:comment>
        <rdfs:label xml:lang="it">18000 Euro</rdfs:label>
    </owl:NamedIndividual>
    


    <!-- http://www.semanticweb.org/annag/ontologies/2024/1/ontoHorses#20000Euro -->

    <owl:NamedIndividual rdf:about="http://www.semanticweb.org/annag/ontologies/2024/1/ontoHorses#20000Euro">
        <rdf:type rdf:resource="http://www.ontologydesignpatterns.org/cp/owl/price.owl#Price"/>
        <price:hasCurrency rdf:resource="http://www.semanticweb.org/annag/ontologies/2024/1/ontoHorses#Euro"/>
        <price:isPriceOf rdf:resource="http://www.semanticweb.org/annag/ontologies/2024/1/ontoHorses#MaschioPuroSangueInglese"/>
        <price:hasValue rdf:datatype="http://www.w3.org/2001/XMLSchema#float">20000.0</price:hasValue>
        <rdfs:comment xml:lang="it">20000 Euro</rdfs:comment>
        <rdfs:label xml:lang="it">20000 Euro</rdfs:label>
    </owl:NamedIndividual>
    


    <!-- http://www.semanticweb.org/annag/ontologies/2024/1/ontoHorses#2500Euro -->

    <owl:NamedIndividual rdf:about="http://www.semanticweb.org/annag/ontologies/2024/1/ontoHorses#2500Euro">
        <rdf:type rdf:resource="http://www.ontologydesignpatterns.org/cp/owl/price.owl#Price"/>
        <price:hasCurrency rdf:resource="http://www.semanticweb.org/annag/ontologies/2024/1/ontoHorses#Euro"/>
        <price:isPriceOf rdf:resource="http://www.semanticweb.org/annag/ontologies/2024/1/ontoHorses#FemminaBretone"/>
        <price:hasValue rdf:datatype="http://www.w3.org/2001/XMLSchema#float">2500.0</price:hasValue>
        <rdfs:comment xml:lang="it">2500 Euro</rdfs:comment>
        <rdfs:label xml:lang="it">2500 Euro</rdfs:label>
    </owl:NamedIndividual>
    


    <!-- http://www.semanticweb.org/annag/ontologies/2024/1/ontoHorses#35000Euro -->

    <owl:NamedIndividual rdf:about="http://www.semanticweb.org/annag/ontologies/2024/1/ontoHorses#35000Euro">
        <rdf:type rdf:resource="http://www.ontologydesignpatterns.org/cp/owl/price.owl#Price"/>
        <price:hasCurrency rdf:resource="http://www.semanticweb.org/annag/ontologies/2024/1/ontoHorses#Euro"/>
        <price:isPriceOf rdf:resource="http://www.semanticweb.org/annag/ontologies/2024/1/ontoHorses#MaschioOlandese"/>
        <price:hasValue rdf:datatype="http://www.w3.org/2001/XMLSchema#float">35000.0</price:hasValue>
        <rdfs:comment xml:lang="it">35000 Euro</rdfs:comment>
        <rdfs:label xml:lang="it">35000 Euro</rdfs:label>
    </owl:NamedIndividual>
    


    <!-- http://www.semanticweb.org/annag/ontologies/2024/1/ontoHorses#4800Euro -->

    <owl:NamedIndividual rdf:about="http://www.semanticweb.org/annag/ontologies/2024/1/ontoHorses#4800Euro">
        <rdf:type rdf:resource="http://www.ontologydesignpatterns.org/cp/owl/price.owl#Price"/>
        <price:hasCurrency rdf:resource="http://www.semanticweb.org/annag/ontologies/2024/1/ontoHorses#Euro"/>
        <price:isPriceOf rdf:resource="http://www.semanticweb.org/annag/ontologies/2024/1/ontoHorses#FemminaMurgese"/>
        <price:hasValue rdf:datatype="http://www.w3.org/2001/XMLSchema#float">4800.0</price:hasValue>
        <rdfs:comment xml:lang="it">4800 Euro</rdfs:comment>
        <rdfs:label xml:lang="it">4800 Euro</rdfs:label>
    </owl:NamedIndividual>
    


    <!-- http://www.semanticweb.org/annag/ontologies/2024/1/ontoHorses#5000Euro -->

    <owl:NamedIndividual rdf:about="http://www.semanticweb.org/annag/ontologies/2024/1/ontoHorses#5000Euro">
        <rdf:type rdf:resource="http://www.ontologydesignpatterns.org/cp/owl/price.owl#Price"/>
        <price:hasCurrency rdf:resource="http://www.semanticweb.org/annag/ontologies/2024/1/ontoHorses#Euro"/>
        <price:isPriceOf rdf:resource="http://www.semanticweb.org/annag/ontologies/2024/1/ontoHorses#FemminaMaremmano"/>
        <price:hasValue rdf:datatype="http://www.w3.org/2001/XMLSchema#float">5000.0</price:hasValue>
        <rdfs:comment xml:lang="it">5000 Euro</rdfs:comment>
        <rdfs:label xml:lang="it">5000 Euro</rdfs:label>
    </owl:NamedIndividual>
    


    <!-- http://www.semanticweb.org/annag/ontologies/2024/1/ontoHorses#7000Euro -->

    <owl:NamedIndividual rdf:about="http://www.semanticweb.org/annag/ontologies/2024/1/ontoHorses#7000Euro">
        <rdf:type rdf:resource="http://www.ontologydesignpatterns.org/cp/owl/price.owl#Price"/>
        <price:hasCurrency rdf:resource="http://www.semanticweb.org/annag/ontologies/2024/1/ontoHorses#Euro"/>
        <price:isPriceOf rdf:resource="http://www.semanticweb.org/annag/ontologies/2024/1/ontoHorses#MaschioAndaluso"/>
        <price:hasValue rdf:datatype="http://www.w3.org/2001/XMLSchema#float">7000.0</price:hasValue>
        <rdfs:comment xml:lang="it">7000 Euro</rdfs:comment>
        <rdfs:label xml:lang="it">7000 Euro</rdfs:label>
    </owl:NamedIndividual>
    


    <!-- http://www.wikidata.org/entity/Q1070901 -->

    <owl:NamedIndividual rdf:about="http://www.wikidata.org/entity/Q1070901"/>
    


    <!-- http://www.wikidata.org/entity/Q1232528 -->

    <owl:NamedIndividual rdf:about="http://www.wikidata.org/entity/Q1232528"/>
    


    <!-- http://www.wikidata.org/entity/Q1468737 -->

    <owl:NamedIndividual rdf:about="http://www.wikidata.org/entity/Q1468737"/>
    


    <!-- http://www.wikidata.org/entity/Q1501738 -->

    <owl:NamedIndividual rdf:about="http://www.wikidata.org/entity/Q1501738"/>
    


    <!-- http://www.wikidata.org/entity/Q1665430 -->

    <owl:NamedIndividual rdf:about="http://www.wikidata.org/entity/Q1665430"/>
    


    <!-- http://www.wikidata.org/entity/Q166777 -->

    <owl:NamedIndividual rdf:about="http://www.wikidata.org/entity/Q166777"/>
    


    <!-- http://www.wikidata.org/entity/Q1684175 -->

    <owl:NamedIndividual rdf:about="http://www.wikidata.org/entity/Q1684175"/>
    


    <!-- http://www.wikidata.org/entity/Q1894708 -->

    <owl:NamedIndividual rdf:about="http://www.wikidata.org/entity/Q1894708"/>
    


    <!-- http://www.wikidata.org/entity/Q1953691 -->

    <owl:NamedIndividual rdf:about="http://www.wikidata.org/entity/Q1953691"/>
    


    <!-- http://www.wikidata.org/entity/Q195395 -->

    <owl:NamedIndividual rdf:about="http://www.wikidata.org/entity/Q195395"/>
    


    <!-- http://www.wikidata.org/entity/Q210826 -->

    <owl:NamedIndividual rdf:about="http://www.wikidata.org/entity/Q210826"/>
    


    <!-- http://www.wikidata.org/entity/Q217671 -->

    <owl:NamedIndividual rdf:about="http://www.wikidata.org/entity/Q217671"/>
    


    <!-- http://www.wikidata.org/entity/Q3617386 -->

    <owl:NamedIndividual rdf:about="http://www.wikidata.org/entity/Q3617386"/>
    


    <!-- http://www.wikidata.org/entity/Q3620866 -->

    <owl:NamedIndividual rdf:about="http://www.wikidata.org/entity/Q3620866"/>
    


    <!-- http://www.wikidata.org/entity/Q388952 -->

    <owl:NamedIndividual rdf:about="http://www.wikidata.org/entity/Q388952"/>
    


    <!-- http://www.wikidata.org/entity/Q428039 -->

    <owl:NamedIndividual rdf:about="http://www.wikidata.org/entity/Q428039"/>
    


    <!-- http://www.wikidata.org/entity/Q489798 -->

    <owl:NamedIndividual rdf:about="http://www.wikidata.org/entity/Q489798"/>
    


    <!-- http://www.wikidata.org/entity/Q514553 -->

    <owl:NamedIndividual rdf:about="http://www.wikidata.org/entity/Q514553"/>
    


    <!-- http://www.wikidata.org/entity/Q571149 -->

    <owl:NamedIndividual rdf:about="http://www.wikidata.org/entity/Q571149"/>
    


    <!-- http://www.wikidata.org/entity/Q588252 -->

    <owl:NamedIndividual rdf:about="http://www.wikidata.org/entity/Q588252"/>
    


    <!-- http://www.wikidata.org/entity/Q638976 -->

    <owl:NamedIndividual rdf:about="http://www.wikidata.org/entity/Q638976"/>
    


    <!-- http://www.wikidata.org/entity/Q7029480 -->

    <owl:NamedIndividual rdf:about="http://www.wikidata.org/entity/Q7029480"/>
    


    <!-- http://www.wikidata.org/entity/Q843585 -->

    <owl:NamedIndividual rdf:about="http://www.wikidata.org/entity/Q843585"/>
    


    <!-- http://www.wikidata.org/entity/Q844058 -->

    <owl:NamedIndividual rdf:about="http://www.wikidata.org/entity/Q844058"/>
    


    <!-- http://www.wikidata.org/entity/Q896476 -->

    <owl:NamedIndividual rdf:about="http://www.wikidata.org/entity/Q896476"/>
    


    <!-- http://www.wikidata.org/entity/Q937595 -->

    <owl:NamedIndividual rdf:about="http://www.wikidata.org/entity/Q937595"/>
    


    <!-- 
    ///////////////////////////////////////////////////////////////////////////////////////
    //
    // Annotations
    //
    ///////////////////////////////////////////////////////////////////////////////////////
     -->

    <rdf:Description rdf:about="http://www.ontologydesignpatterns.org/cp/owl/price.owl#hasValue">
        <rdfs:isDefinedBy rdf:resource="http://www.ontologydesignpatterns.org/cp/owl/price.owl"/>
        <rdfs:label xml:lang="en">has value</rdfs:label>
    </rdf:Description>
    <rdf:Description rdf:about="http://www.ontologydesignpatterns.org/schemas/cpannotationschema.owl#hasUnitTest">
        <rdfs:comment>This property can be used to annotate a unit test (e.g. in the form of a SPARQL query) to be launched to evaluate an ontology against a requirement-based task.</rdfs:comment>
    </rdf:Description>
    <rdf:Description rdf:about="http://www.ontologydesignpatterns.org/schemas/cpannotationschema.owl#isCloneOf">
        <rdfs:comment>This annotation property is used for referring a cloned ontology entity to its cloning source.</rdfs:comment>
    </rdf:Description>
    <rdf:Description rdf:about="http://www.semanticweb.org/annag/ontologies/2024/1/ontoHorses#AltaScuola">
        <schema:image rdf:resource="https://www.sef-italia.it/wp-content/uploads/2020/02/Schermata-2020-02-05-alle-14.52.05-768x712.png"/>
        <rdfs:comment xml:lang="it">E&apos; uno sport equestre simile al Dressage che ha per scopo lo sviluppo armonioso dell&apos;organismo e dei mezzi del cavallo</rdfs:comment>
        <rdfs:comment xml:lang="en">It is an equestrian sport similar to Dressage which has as its aim the harmonious development of the horse&apos;s organism and means</rdfs:comment>
        <rdfs:label xml:lang="it">Alta Scuola</rdfs:label>
        <rdfs:label xml:lang="en">Spanish riding school</rdfs:label>
    </rdf:Description>
    <rdf:Description rdf:about="http://www.semanticweb.org/annag/ontologies/2024/1/ontoHorses#CrossCountry">
        <rdfs:comment xml:lang="en">Cross-country is an Olympic equestrian sport, which consists of a speed test on varied terrain, and the overcoming of various types of fixed obstacles.</rdfs:comment>
        <rdfs:comment xml:lang="it">Il cross-country è uno sport equestre olimpico, che consiste in una prova di velocità su terreno vario, e nel superamento di vari tipi di ostacoli fissi.</rdfs:comment>
        <rdfs:label xml:lang="en">Cross-country</rdfs:label>
        <rdfs:label xml:lang="it">Cross-country</rdfs:label>
    </rdf:Description>
    <rdf:Description rdf:about="http://www.semanticweb.org/annag/ontologies/2024/1/ontoHorses#Dressage">
        <rdfs:comment xml:lang="en">Dressage is an Olympic equestrian discipline which is also called a training competition, as the horse and rider perform predominantly geometric movements on a rectangular field, measuring 20x40 meters for low level competitions and 20x60 in medium/high level ones.</rdfs:comment>
        <rdfs:comment xml:lang="it">Il Dressage è una disciplina equestre olimpionica che viene anche chiamata gara di addestramento, in quanto cavallo e cavaliere eseguono movimenti prevalentemente geometrici su un campo di forma rettangolare, di dimensioni 20x40 metri per le gare di basso livello e 20x60 in quelle di livello medio/alto.</rdfs:comment>
        <rdfs:label xml:lang="en">Dressage</rdfs:label>
        <rdfs:label xml:lang="it">Dressage</rdfs:label>
    </rdf:Description>
    <rdf:Description rdf:about="http://www.semanticweb.org/annag/ontologies/2024/1/ontoHorses#Endurance">
        <rdfs:comment xml:lang="en">Endurance is one of the most popular equestrian sports in the world. The competitions consist of endurance races on routes of various nature and a mileage that varies from 30 to 160 km depending on the categories.</rdfs:comment>
        <rdfs:comment xml:lang="it">L&apos;Endurance è uno degli sport equestri di maggior diffusione al mondo. Le competizioni consistono in corse di resistenza su percorsi di varia natura ed un chilometraggio che varia dai 30 ai 160 km a seconda delle categorie.</rdfs:comment>
        <rdfs:label xml:lang="en">Endurance</rdfs:label>
        <rdfs:label xml:lang="it">Endurance</rdfs:label>
    </rdf:Description>
    <rdf:Description rdf:about="http://www.semanticweb.org/annag/ontologies/2024/1/ontoHorses#Equiturismo">
        <rdfs:comment xml:lang="en">Equestrian tourism is a practice of horse riding which consists in the use of the horse for the pleasure of riding in places far from civilization, for example the countryside, woods, hills or mountains.</rdfs:comment>
        <rdfs:comment xml:lang="it">L&apos;equiturismo è una pratica dell&apos;equitazione che consiste nell&apos;uso del cavallo per il piacere di cavalcare in luoghi lontani dalla civiltà, ad esempio i campagna, boschi, collina o montagna.</rdfs:comment>
        <rdfs:label xml:lang="it">Equiturismo</rdfs:label>
        <rdfs:label xml:lang="en">Trail riding</rdfs:label>
    </rdf:Description>
    <rdf:Description rdf:about="http://www.semanticweb.org/annag/ontologies/2024/1/ontoHorses#Eventing">
        <rdfs:comment xml:lang="en">Full riding is a discipline that originates from the training of soldiers to face the difficulties of the campaign. At the same time they had to demonstrate perfect dressage training and also complete a show jumping course. The event trials are called &quot;three day events&quot; in the Anglo-Saxon world precisely because the three trials are spread over three days. Undoubtedly the most spectacular test is the countryside one, the cross country, during which the pairs have to face challenging natural obstacles such as trunks, ditches, uphill and downhill jumps, combinations and lakes.</rdfs:comment>
        <rdfs:comment xml:lang="it">Il completo di equitazione è una disciplina che ha origine dall&apos;addestramento dei militari per affrontare le difficoltà della campagna. Allo stesso tempo dovevano dimostrare un perfetto addestramento in dressage e superare anche un percorso di salto ostacoli. Le prove di completo sono chiamate nel mondo anglosassone &quot;three day event&quot; proprio perchè le tre prove sono distribuite su tre giornate. Indubbiamente la prova più spettacolare è quella di campagna, il cross country, durante la quale i binomi devono affrontare impegnativi ostacoli naturali come tronchi, fossi, salti in salita e discesa, combinazioni e laghetti.</rdfs:comment>
        <rdfs:label xml:lang="it">Eventing</rdfs:label>
    </rdf:Description>
    <rdf:Description rdf:about="http://www.semanticweb.org/annag/ontologies/2024/1/ontoHorses#SaltoAdOstacoli">
        <rdfs:comment xml:lang="it">Il salto ostacoli è un termine che identifica una disciplina dell&apos;equitazione, la quale vede impegnato il binomio uomo-cavallo, nell&apos;interpretazione e risoluzione di un percorso ad ostacoli. L&apos;altezza degli ostacoli, la difficoltà del percorso e il numero di ostacoli da superare dipende dalla categoria alla quale si partecipa e dalla preparazione atletica di cavallo e cavaliere. L&apos;altezza degli ostacoli varia dai 40 cm a 1,60 m  con categorie intermedie di 60, 70, 80, 90, 100, 105, 110, 115, 120, 125,130, 135, 140,145, 150, 160. Il numero di ostacoli varia da 8 a 13 con eventuali combinazioni di più ostacoli dette gabbie.</rdfs:comment>
        <rdfs:comment xml:lang="en">Show jumping is a term that identifies a discipline of horse riding, which involves the man-horse duo in the interpretation and resolution of an obstacle course. The height of the obstacles, the difficulty of the route and the number of obstacles to overcome depends on the category in which you participate and the athletic preparation of the horse and rider. The height of the obstacles varies from 40 cm to 1.60 m with intermediate categories of 60, 70, 80, 90, 100, 105, 110, 115, 120, 125,130, 135, 140,145, 150, 160. The number of obstacles varies from 8 to 13 with possible combinations of multiple obstacles called cages.</rdfs:comment>
        <rdfs:label xml:lang="it">Salto Ostacoli</rdfs:label>
        <rdfs:label xml:lang="en">Show jumping</rdfs:label>
    </rdf:Description>
    <rdf:Description rdf:about="http://www.semanticweb.org/annag/ontologies/2024/1/ontoHorses#TiroAgricolo">
        <rdfs:comment xml:lang="en">Use of the horse for agricultural work</rdfs:comment>
        <rdfs:comment xml:lang="it">Utilizzo del cavallo per lavori in campo agricolo</rdfs:comment>
        <rdfs:label xml:lang="it">Tiro agricolo</rdfs:label>
        <rdfs:label xml:lang="en">agricultural draft</rdfs:label>
    </rdf:Description>
    <rdf:Description rdf:about="http://www.semanticweb.org/annag/ontologies/2024/1/ontoHorses#TrainoCarrozze">
        <rdfs:comment xml:lang="en">Using the horse to pull carriages for the transport of goods or people</rdfs:comment>
        <rdfs:comment xml:lang="it">Utilizzo del cavallo per trainare carrozze per il trasporto di merci o persone</rdfs:comment>
        <rdfs:label xml:lang="en">Towing carriages</rdfs:label>
        <rdfs:label xml:lang="it">Traino carrozze</rdfs:label>
    </rdf:Description>
    


    <!-- 
    ///////////////////////////////////////////////////////////////////////////////////////
    //
    // General axioms
    //
    ///////////////////////////////////////////////////////////////////////////////////////
     -->

    <rdf:Description>
        <rdf:type rdf:resource="http://www.w3.org/2002/07/owl#AllDisjointClasses"/>
        <owl:members rdf:parseType="Collection">
            <rdf:Description rdf:about="http://www.semanticweb.org/annag/ontologies/2024/1/ontoHorses#CavalloAdulto"/>
            <rdf:Description rdf:about="http://www.semanticweb.org/annag/ontologies/2024/1/ontoHorses#CavalloAnziano"/>
            <rdf:Description rdf:about="http://www.semanticweb.org/annag/ontologies/2024/1/ontoHorses#Puledro"/>
        </owl:members>
    </rdf:Description>
    <rdf:Description>
        <rdf:type rdf:resource="http://www.w3.org/2002/07/owl#AllDisjointClasses"/>
        <owl:members rdf:parseType="Collection">
            <rdf:Description rdf:about="http://www.semanticweb.org/annag/ontologies/2024/1/ontoHorses#RazzaASangueCaldo"/>
            <rdf:Description rdf:about="http://www.semanticweb.org/annag/ontologies/2024/1/ontoHorses#RazzaASangueFreddo"/>
            <rdf:Description rdf:about="http://www.semanticweb.org/annag/ontologies/2024/1/ontoHorses#RazzaASangueMisto"/>
        </owl:members>
    </rdf:Description>
    <rdf:Description>
        <rdf:type rdf:resource="http://www.w3.org/2002/07/owl#AllDifferent"/>
        <owl:distinctMembers rdf:parseType="Collection">
            <rdf:Description rdf:about="http://www.semanticweb.org/annag/ontologies/2024/1/ontoHorses#AltaScuola"/>
            <rdf:Description rdf:about="http://www.semanticweb.org/annag/ontologies/2024/1/ontoHorses#CrossCountry"/>
            <rdf:Description rdf:about="http://www.semanticweb.org/annag/ontologies/2024/1/ontoHorses#Dressage"/>
            <rdf:Description rdf:about="http://www.semanticweb.org/annag/ontologies/2024/1/ontoHorses#Endurance"/>
            <rdf:Description rdf:about="http://www.semanticweb.org/annag/ontologies/2024/1/ontoHorses#Eventing"/>
            <rdf:Description rdf:about="http://www.semanticweb.org/annag/ontologies/2024/1/ontoHorses#SaltoAdOstacoli"/>
        </owl:distinctMembers>
    </rdf:Description>
    <rdf:Description>
        <rdf:type rdf:resource="http://www.w3.org/2002/07/owl#AllDifferent"/>
        <owl:distinctMembers rdf:parseType="Collection">
            <rdf:Description rdf:about="http://www.semanticweb.org/annag/ontologies/2024/1/ontoHorses#Andalusia"/>
            <rdf:Description rdf:about="http://www.semanticweb.org/annag/ontologies/2024/1/ontoHorses#AppenninoToscoEmiliano"/>
            <rdf:Description rdf:about="http://www.semanticweb.org/annag/ontologies/2024/1/ontoHorses#Ardenne"/>
            <rdf:Description rdf:about="http://www.semanticweb.org/annag/ontologies/2024/1/ontoHorses#Belgio"/>
            <rdf:Description rdf:about="http://www.semanticweb.org/annag/ontologies/2024/1/ontoHorses#Bretagna"/>
            <rdf:Description rdf:about="http://www.semanticweb.org/annag/ontologies/2024/1/ontoHorses#Danimarca"/>
            <rdf:Description rdf:about="http://www.semanticweb.org/annag/ontologies/2024/1/ontoHorses#Francia"/>
            <rdf:Description rdf:about="http://www.semanticweb.org/annag/ontologies/2024/1/ontoHorses#Frisia"/>
            <rdf:Description rdf:about="http://www.semanticweb.org/annag/ontologies/2024/1/ontoHorses#Germania"/>
            <rdf:Description rdf:about="http://www.semanticweb.org/annag/ontologies/2024/1/ontoHorses#Irlanda"/>
            <rdf:Description rdf:about="http://www.semanticweb.org/annag/ontologies/2024/1/ontoHorses#Jutland"/>
            <rdf:Description rdf:about="http://www.semanticweb.org/annag/ontologies/2024/1/ontoHorses#Lombardia"/>
            <rdf:Description rdf:about="http://www.semanticweb.org/annag/ontologies/2024/1/ontoHorses#Lusitano"/>
            <rdf:Description rdf:about="http://www.semanticweb.org/annag/ontologies/2024/1/ontoHorses#Maremma"/>
            <rdf:Description rdf:about="http://www.semanticweb.org/annag/ontologies/2024/1/ontoHorses#Murge"/>
            <rdf:Description rdf:about="http://www.semanticweb.org/annag/ontologies/2024/1/ontoHorses#Normandia"/>
            <rdf:Description rdf:about="http://www.semanticweb.org/annag/ontologies/2024/1/ontoHorses#PaesiBassi"/>
            <rdf:Description rdf:about="http://www.semanticweb.org/annag/ontologies/2024/1/ontoHorses#Perche"/>
            <rdf:Description rdf:about="http://www.semanticweb.org/annag/ontologies/2024/1/ontoHorses#Piemonte"/>
            <rdf:Description rdf:about="http://www.semanticweb.org/annag/ontologies/2024/1/ontoHorses#Portogallo"/>
            <rdf:Description rdf:about="http://www.semanticweb.org/annag/ontologies/2024/1/ontoHorses#Puglia"/>
            <rdf:Description rdf:about="http://www.semanticweb.org/annag/ontologies/2024/1/ontoHorses#RegioneBoullonnais"/>
            <rdf:Description rdf:about="http://www.semanticweb.org/annag/ontologies/2024/1/ontoHorses#RegioneHannover"/>
            <rdf:Description rdf:about="http://www.semanticweb.org/annag/ontologies/2024/1/ontoHorses#RegnoUnito"/>
            <rdf:Description rdf:about="http://www.semanticweb.org/annag/ontologies/2024/1/ontoHorses#Schleswig-Holstein"/>
            <rdf:Description rdf:about="http://www.semanticweb.org/annag/ontologies/2024/1/ontoHorses#Scozia"/>
            <rdf:Description rdf:about="http://www.semanticweb.org/annag/ontologies/2024/1/ontoHorses#Sicilia"/>
            <rdf:Description rdf:about="http://www.semanticweb.org/annag/ontologies/2024/1/ontoHorses#Spagna"/>
            <rdf:Description rdf:about="http://www.semanticweb.org/annag/ontologies/2024/1/ontoHorses#Trakehner"/>
            <rdf:Description rdf:about="http://www.semanticweb.org/annag/ontologies/2024/1/ontoHorses#TrentinoAltoAdige"/>
            <rdf:Description rdf:about="http://www.semanticweb.org/annag/ontologies/2024/1/ontoHorses#Vestfalia"/>
            <rdf:Description rdf:about="http://www.semanticweb.org/annag/ontologies/2024/1/ontoHorses#bergamo"/>
            <rdf:Description rdf:about="http://www.semanticweb.org/annag/ontologies/2024/1/ontoHorses#leini"/>
            <rdf:Description rdf:about="http://www.semanticweb.org/annag/ontologies/2024/1/ontoHorses#sanMauro"/>
            <rdf:Description rdf:about="http://www.semanticweb.org/annag/ontologies/2024/1/ontoHorses#siracusa"/>
            <rdf:Description rdf:about="http://www.semanticweb.org/annag/ontologies/2024/1/ontoHorses#taranto"/>
        </owl:distinctMembers>
    </rdf:Description>
    <rdf:Description>
        <rdf:type rdf:resource="http://www.w3.org/2002/07/owl#AllDifferent"/>
        <owl:distinctMembers rdf:parseType="Collection">
            <rdf:Description rdf:about="http://www.semanticweb.org/annag/ontologies/2024/1/ontoHorses#Andaluso"/>
            <rdf:Description rdf:about="http://www.semanticweb.org/annag/ontologies/2024/1/ontoHorses#AngloAraboFrancese"/>
            <rdf:Description rdf:about="http://www.semanticweb.org/annag/ontologies/2024/1/ontoHorses#AngloAraboSpagnolo"/>
            <rdf:Description rdf:about="http://www.semanticweb.org/annag/ontologies/2024/1/ontoHorses#Appenninico"/>
            <rdf:Description rdf:about="http://www.semanticweb.org/annag/ontologies/2024/1/ontoHorses#Ardennese"/>
            <rdf:Description rdf:about="http://www.semanticweb.org/annag/ontologies/2024/1/ontoHorses#BelgaDaTiro"/>
            <rdf:Description rdf:about="http://www.semanticweb.org/annag/ontologies/2024/1/ontoHorses#Boulonnais"/>
            <rdf:Description rdf:about="http://www.semanticweb.org/annag/ontologies/2024/1/ontoHorses#Bretone"/>
            <rdf:Description rdf:about="http://www.semanticweb.org/annag/ontologies/2024/1/ontoHorses#CavalloDelloJutland"/>
            <rdf:Description rdf:about="http://www.semanticweb.org/annag/ontologies/2024/1/ontoHorses#Clydesdale"/>
            <rdf:Description rdf:about="http://www.semanticweb.org/annag/ontologies/2024/1/ontoHorses#Frisone"/>
            <rdf:Description rdf:about="http://www.semanticweb.org/annag/ontologies/2024/1/ontoHorses#Hannover"/>
            <rdf:Description rdf:about="http://www.semanticweb.org/annag/ontologies/2024/1/ontoHorses#Holstein"/>
            <rdf:Description rdf:about="http://www.semanticweb.org/annag/ontologies/2024/1/ontoHorses#IrishSportHorse"/>
            <rdf:Description rdf:about="http://www.semanticweb.org/annag/ontologies/2024/1/ontoHorses#Lipizzano"/>
            <rdf:Description rdf:about="http://www.semanticweb.org/annag/ontologies/2024/1/ontoHorses#Lusitano"/>
            <rdf:Description rdf:about="http://www.semanticweb.org/annag/ontologies/2024/1/ontoHorses#Maremmano"/>
            <rdf:Description rdf:about="http://www.semanticweb.org/annag/ontologies/2024/1/ontoHorses#Murgese"/>
            <rdf:Description rdf:about="http://www.semanticweb.org/annag/ontologies/2024/1/ontoHorses#OlandeseASangueCaldo"/>
            <rdf:Description rdf:about="http://www.semanticweb.org/annag/ontologies/2024/1/ontoHorses#Oldemburghese"/>
            <rdf:Description rdf:about="http://www.semanticweb.org/annag/ontologies/2024/1/ontoHorses#Percheron"/>
            <rdf:Description rdf:about="http://www.semanticweb.org/annag/ontologies/2024/1/ontoHorses#PuroSangueInglese"/>
            <rdf:Description rdf:about="http://www.semanticweb.org/annag/ontologies/2024/1/ontoHorses#SellaFrancese"/>
            <rdf:Description rdf:about="http://www.semanticweb.org/annag/ontologies/2024/1/ontoHorses#SellaItaliano"/>
            <rdf:Description rdf:about="http://www.semanticweb.org/annag/ontologies/2024/1/ontoHorses#Trakehner"/>
            <rdf:Description rdf:about="http://www.semanticweb.org/annag/ontologies/2024/1/ontoHorses#Westfalen"/>
        </owl:distinctMembers>
    </rdf:Description>
    <rdf:Description>
        <rdf:type rdf:resource="http://www.w3.org/2002/07/owl#AllDifferent"/>
        <owl:distinctMembers rdf:parseType="Collection">
            <rdf:Description rdf:about="http://www.semanticweb.org/annag/ontologies/2024/1/ontoHorses#C100"/>
            <rdf:Description rdf:about="http://www.semanticweb.org/annag/ontologies/2024/1/ontoHorses#C105"/>
            <rdf:Description rdf:about="http://www.semanticweb.org/annag/ontologies/2024/1/ontoHorses#C110"/>
            <rdf:Description rdf:about="http://www.semanticweb.org/annag/ontologies/2024/1/ontoHorses#C115"/>
            <rdf:Description rdf:about="http://www.semanticweb.org/annag/ontologies/2024/1/ontoHorses#C120"/>
            <rdf:Description rdf:about="http://www.semanticweb.org/annag/ontologies/2024/1/ontoHorses#C125"/>
            <rdf:Description rdf:about="http://www.semanticweb.org/annag/ontologies/2024/1/ontoHorses#C130"/>
            <rdf:Description rdf:about="http://www.semanticweb.org/annag/ontologies/2024/1/ontoHorses#C135"/>
            <rdf:Description rdf:about="http://www.semanticweb.org/annag/ontologies/2024/1/ontoHorses#C80"/>
            <rdf:Description rdf:about="http://www.semanticweb.org/annag/ontologies/2024/1/ontoHorses#C90"/>
        </owl:distinctMembers>
    </rdf:Description>
    <rdf:Description>
        <rdf:type rdf:resource="http://www.w3.org/2002/07/owl#AllDifferent"/>
        <owl:distinctMembers rdf:parseType="Collection">
            <rdf:Description rdf:about="http://www.semanticweb.org/annag/ontologies/2024/1/ontoHorses#CavaliereEsperto"/>
            <rdf:Description rdf:about="http://www.semanticweb.org/annag/ontologies/2024/1/ontoHorses#CavaliereIntermedio"/>
            <rdf:Description rdf:about="http://www.semanticweb.org/annag/ontologies/2024/1/ontoHorses#CavaliereMoltoEsperto"/>
            <rdf:Description rdf:about="http://www.semanticweb.org/annag/ontologies/2024/1/ontoHorses#CavalierePrincipiante"/>
        </owl:distinctMembers>
    </rdf:Description>
    <rdf:Description>
        <rdf:type rdf:resource="http://www.w3.org/2002/07/owl#AllDifferent"/>
        <owl:distinctMembers rdf:parseType="Collection">
            <rdf:Description rdf:about="http://www.semanticweb.org/annag/ontologies/2024/1/ontoHorses#D"/>
            <rdf:Description rdf:about="http://www.semanticweb.org/annag/ontologies/2024/1/ontoHorses#E"/>
            <rdf:Description rdf:about="http://www.semanticweb.org/annag/ontologies/2024/1/ontoHorses#F"/>
            <rdf:Description rdf:about="http://www.semanticweb.org/annag/ontologies/2024/1/ontoHorses#M"/>
        </owl:distinctMembers>
    </rdf:Description>
    <rdf:Description>
        <rdf:type rdf:resource="http://www.w3.org/2002/07/owl#AllDifferent"/>
        <owl:distinctMembers rdf:parseType="Collection">
            <rdf:Description rdf:about="http://www.semanticweb.org/annag/ontologies/2024/1/ontoHorses#brachimorfo"/>
            <rdf:Description rdf:about="http://www.semanticweb.org/annag/ontologies/2024/1/ontoHorses#dolicomorfo"/>
            <rdf:Description rdf:about="http://www.semanticweb.org/annag/ontologies/2024/1/ontoHorses#mesoBrachimorfo"/>
            <rdf:Description rdf:about="http://www.semanticweb.org/annag/ontologies/2024/1/ontoHorses#mesoDolicomorfo"/>
            <rdf:Description rdf:about="http://www.semanticweb.org/annag/ontologies/2024/1/ontoHorses#mesomorfo"/>
        </owl:distinctMembers>
    </rdf:Description>
    <rdf:Description>
        <rdf:type rdf:resource="http://www.w3.org/2002/07/owl#AllDifferent"/>
        <owl:distinctMembers rdf:parseType="Collection">
            <rdf:Description rdf:about="http://www.semanticweb.org/annag/ontologies/2024/1/ontoHorses#brevetto"/>
            <rdf:Description rdf:about="http://www.semanticweb.org/annag/ontologies/2024/1/ontoHorses#patenteLudicaA"/>
            <rdf:Description rdf:about="http://www.semanticweb.org/annag/ontologies/2024/1/ontoHorses#primoGrado"/>
            <rdf:Description rdf:about="http://www.semanticweb.org/annag/ontologies/2024/1/ontoHorses#secondoGrado"/>
        </owl:distinctMembers>
    </rdf:Description>
    <rdf:Description>
        <rdf:type rdf:resource="http://www.w3.org/2002/07/owl#AllDifferent"/>
        <owl:distinctMembers rdf:parseType="Collection">
            <rdf:Description rdf:about="http://www.semanticweb.org/annag/ontologies/2024/1/ontoHorses#brunoGramaglia"/>
            <rdf:Description rdf:about="http://www.semanticweb.org/annag/ontologies/2024/1/ontoHorses#claudioCavallo"/>
            <rdf:Description rdf:about="http://www.semanticweb.org/annag/ontologies/2024/1/ontoHorses#francescoBertero"/>
            <rdf:Description rdf:about="http://www.semanticweb.org/annag/ontologies/2024/1/ontoHorses#gianlucaCamoletto"/>
            <rdf:Description rdf:about="http://www.semanticweb.org/annag/ontologies/2024/1/ontoHorses#paoloGrassi"/>
        </owl:distinctMembers>
    </rdf:Description>
    <rdf:Description>
        <rdf:type rdf:resource="http://www.w3.org/2002/07/owl#AllDifferent"/>
        <owl:distinctMembers rdf:parseType="Collection">
            <rdf:Description rdf:about="http://www.semanticweb.org/annag/ontologies/2024/1/ontoHorses#sangueCaldo"/>
            <rdf:Description rdf:about="http://www.semanticweb.org/annag/ontologies/2024/1/ontoHorses#sangueFreddo"/>
            <rdf:Description rdf:about="http://www.semanticweb.org/annag/ontologies/2024/1/ontoHorses#sangueMisto"/>
        </owl:distinctMembers>
    </rdf:Description>
    <rdf:Description>
        <rdf:type rdf:resource="http://www.w3.org/2002/07/owl#AllDifferent"/>
        <owl:distinctMembers rdf:parseType="Collection">
            <rdf:Description rdf:about="http://www.semanticweb.org/annag/ontologies/2024/1/ontoHorses#12000Euro"/>
            <rdf:Description rdf:about="http://www.semanticweb.org/annag/ontologies/2024/1/ontoHorses#15000Euro"/>
            <rdf:Description rdf:about="http://www.semanticweb.org/annag/ontologies/2024/1/ontoHorses#18000Euro"/>
            <rdf:Description rdf:about="http://www.semanticweb.org/annag/ontologies/2024/1/ontoHorses#20000Euro"/>
            <rdf:Description rdf:about="http://www.semanticweb.org/annag/ontologies/2024/1/ontoHorses#2500Euro"/>
            <rdf:Description rdf:about="http://www.semanticweb.org/annag/ontologies/2024/1/ontoHorses#35000Euro"/>
            <rdf:Description rdf:about="http://www.semanticweb.org/annag/ontologies/2024/1/ontoHorses#4800Euro"/>
            <rdf:Description rdf:about="http://www.semanticweb.org/annag/ontologies/2024/1/ontoHorses#5000Euro"/>
            <rdf:Description rdf:about="http://www.semanticweb.org/annag/ontologies/2024/1/ontoHorses#7000Euro"/>
        </owl:distinctMembers>
    </rdf:Description>
    <rdf:Description>
        <rdf:type rdf:resource="http://www.w3.org/2002/07/owl#AllDifferent"/>
        <owl:distinctMembers rdf:parseType="Collection">
            <rdf:Description rdf:about="http://www.wikidata.org/entity/Q1070901"/>
            <rdf:Description rdf:about="http://www.wikidata.org/entity/Q1232528"/>
            <rdf:Description rdf:about="http://www.wikidata.org/entity/Q1468737"/>
            <rdf:Description rdf:about="http://www.wikidata.org/entity/Q1501738"/>
            <rdf:Description rdf:about="http://www.wikidata.org/entity/Q1665430"/>
            <rdf:Description rdf:about="http://www.wikidata.org/entity/Q166777"/>
            <rdf:Description rdf:about="http://www.wikidata.org/entity/Q1684175"/>
            <rdf:Description rdf:about="http://www.wikidata.org/entity/Q1894708"/>
            <rdf:Description rdf:about="http://www.wikidata.org/entity/Q1953691"/>
            <rdf:Description rdf:about="http://www.wikidata.org/entity/Q195395"/>
            <rdf:Description rdf:about="http://www.wikidata.org/entity/Q210826"/>
            <rdf:Description rdf:about="http://www.wikidata.org/entity/Q217671"/>
            <rdf:Description rdf:about="http://www.wikidata.org/entity/Q3617386"/>
            <rdf:Description rdf:about="http://www.wikidata.org/entity/Q3620866"/>
            <rdf:Description rdf:about="http://www.wikidata.org/entity/Q388952"/>
            <rdf:Description rdf:about="http://www.wikidata.org/entity/Q428039"/>
            <rdf:Description rdf:about="http://www.wikidata.org/entity/Q489798"/>
            <rdf:Description rdf:about="http://www.wikidata.org/entity/Q514553"/>
            <rdf:Description rdf:about="http://www.wikidata.org/entity/Q571149"/>
            <rdf:Description rdf:about="http://www.wikidata.org/entity/Q588252"/>
            <rdf:Description rdf:about="http://www.wikidata.org/entity/Q638976"/>
            <rdf:Description rdf:about="http://www.wikidata.org/entity/Q7029480"/>
            <rdf:Description rdf:about="http://www.wikidata.org/entity/Q843585"/>
            <rdf:Description rdf:about="http://www.wikidata.org/entity/Q844058"/>
            <rdf:Description rdf:about="http://www.wikidata.org/entity/Q896476"/>
            <rdf:Description rdf:about="http://www.wikidata.org/entity/Q937595"/>
        </owl:distinctMembers>
    </rdf:Description>
</rdf:RDF>



<!-- Generated by the OWL API (version 4.5.26.2023-07-17T20:34:13Z) https://github.com/owlcs/owlapi -->

